@prefix : <http://purl.org/iow/Glossary#> .
@prefix dc: <http://purl.org/dc/elements/1.1/> .
@prefix dct: <http://purl.org/dc/terms/> .
@prefix fn: <http://www.w3.org/2005/xpath-functions#> .
@prefix grddl: <http://www.w3.org/2003/g/data-view#> .
@prefix owl: <http://www.w3.org/2002/07/owl#> .
@prefix rdf: <http://www.w3.org/1999/02/22-rdf-syntax-ns#> .
@prefix rdfs: <http://www.w3.org/2000/01/rdf-schema#> .
@prefix sesame: <http://www.openrdf.org/schema/sesame#> .
@prefix skos: <http://www.w3.org/2004/02/skos/core#> .
@prefix skosxl: <http://www.w3.org/2008/05/skos-xl#> .
@prefix xsd: <http://www.w3.org/2001/XMLSchema#> .

<http://www.w3.org/1999/02/22-rdf-syntax-ns#> a owl:Ontology;
  dc:description "This is the RDF Schema for the RDF vocabulary terms in the RDF Namespace, defined in RDF 1.1 Concepts.";
  dc:title "The RDF Concepts Vocabulary (RDF)";
  rdfs:seeAlso <http://www.w3.org/2000/01/rdf-schema-more> .

rdf:HTML a rdfs:Datatype;
  rdfs:comment "The datatype of RDF literals storing fragments of HTML content";
  rdfs:isDefinedBy <http://www.w3.org/1999/02/22-rdf-syntax-ns#>;
  rdfs:label "HTML";
  rdfs:seeAlso <http://www.w3.org/TR/rdf11-concepts/#section-html>;
  rdfs:subClassOf rdfs:Literal .

rdf:langString a rdfs:Datatype;
  rdfs:comment "The datatype of language-tagged string values";
  rdfs:isDefinedBy <http://www.w3.org/1999/02/22-rdf-syntax-ns#>;
  rdfs:label "langString";
  rdfs:seeAlso <http://www.w3.org/TR/rdf11-concepts/#section-Graph-Literal>;
  rdfs:subClassOf rdfs:Literal .

rdf:PlainLiteral a rdfs:Datatype;
  rdfs:comment "The class of plain (i.e. untyped) literal values, as used in RIF and OWL 2";
  rdfs:isDefinedBy <http://www.w3.org/1999/02/22-rdf-syntax-ns#>;
  rdfs:label "PlainLiteral";
  rdfs:seeAlso <http://www.w3.org/TR/rdf-plain-literal/>;
  rdfs:subClassOf rdfs:Literal .

rdf:type a rdf:Property;
  rdfs:comment "The subject is an instance of a class.";
  rdfs:domain rdfs:Resource;
  rdfs:isDefinedBy <http://www.w3.org/1999/02/22-rdf-syntax-ns#>;
  rdfs:label "type";
  rdfs:range rdfs:Class .

rdf:Property a rdfs:Class;
  rdfs:comment "The class of RDF properties.";
  rdfs:isDefinedBy <http://www.w3.org/1999/02/22-rdf-syntax-ns#>;
  rdfs:label "Property";
  rdfs:subClassOf rdfs:Resource .

rdf:Statement a rdfs:Class;
  rdfs:comment "The class of RDF statements.";
  rdfs:isDefinedBy <http://www.w3.org/1999/02/22-rdf-syntax-ns#>;
  rdfs:label "Statement";
  rdfs:subClassOf rdfs:Resource .

rdf:subject a rdf:Property;
  rdfs:comment "The subject of the subject RDF statement.";
  rdfs:domain rdf:Statement;
  rdfs:isDefinedBy <http://www.w3.org/1999/02/22-rdf-syntax-ns#>;
  rdfs:label "subject";
  rdfs:range rdfs:Resource .

rdf:predicate a rdf:Property;
  rdfs:comment "The predicate of the subject RDF statement.";
  rdfs:domain rdf:Statement;
  rdfs:isDefinedBy <http://www.w3.org/1999/02/22-rdf-syntax-ns#>;
  rdfs:label "predicate";
  rdfs:range rdfs:Resource .

rdf:object a rdf:Property;
  rdfs:comment "The object of the subject RDF statement.";
  rdfs:domain rdf:Statement;
  rdfs:isDefinedBy <http://www.w3.org/1999/02/22-rdf-syntax-ns#>;
  rdfs:label "object";
  rdfs:range rdfs:Resource .

rdf:Bag a rdfs:Class;
  rdfs:comment "The class of unordered containers.";
  rdfs:isDefinedBy <http://www.w3.org/1999/02/22-rdf-syntax-ns#>;
  rdfs:label "Bag";
  rdfs:subClassOf rdfs:Container .

rdf:Seq a rdfs:Class;
  rdfs:comment "The class of ordered containers.";
  rdfs:isDefinedBy <http://www.w3.org/1999/02/22-rdf-syntax-ns#>;
  rdfs:label "Seq";
  rdfs:subClassOf rdfs:Container .

rdf:Alt a rdfs:Class;
  rdfs:comment "The class of containers of alternatives.";
  rdfs:isDefinedBy <http://www.w3.org/1999/02/22-rdf-syntax-ns#>;
  rdfs:label "Alt";
  rdfs:subClassOf rdfs:Container .

rdf:value a rdf:Property;
  rdfs:comment "Idiomatic property used for structured values.";
  rdfs:domain rdfs:Resource;
  rdfs:isDefinedBy <http://www.w3.org/1999/02/22-rdf-syntax-ns#>;
  rdfs:label "value";
  rdfs:range rdfs:Resource .

rdf:List a rdfs:Class;
  rdfs:comment "The class of RDF Lists.";
  rdfs:isDefinedBy <http://www.w3.org/1999/02/22-rdf-syntax-ns#>;
  rdfs:label "List";
  rdfs:subClassOf rdfs:Resource .

rdf:nil a rdf:List;
  rdfs:comment "The empty list, with no items in it. If the rest of a list is nil then the list has no more items in it.";
  rdfs:isDefinedBy <http://www.w3.org/1999/02/22-rdf-syntax-ns#>;
  rdfs:label "nil" .

rdf:first a rdf:Property;
  rdfs:comment "The first item in the subject RDF list.";
  rdfs:domain rdf:List;
  rdfs:isDefinedBy <http://www.w3.org/1999/02/22-rdf-syntax-ns#>;
  rdfs:label "first";
  rdfs:range rdfs:Resource .

rdf:rest a rdf:Property;
  rdfs:comment "The rest of the subject RDF list after the first item.";
  rdfs:domain rdf:List;
  rdfs:isDefinedBy <http://www.w3.org/1999/02/22-rdf-syntax-ns#>;
  rdfs:label "rest";
  rdfs:range rdf:List .

rdf:XMLLiteral a rdfs:Datatype;
  rdfs:comment "The datatype of XML literal values.";
  rdfs:isDefinedBy <http://www.w3.org/1999/02/22-rdf-syntax-ns#>;
  rdfs:label "XMLLiteral";
  rdfs:subClassOf rdfs:Literal .

<http://www.w3.org/2008/05/skos-xl> a owl:Ontology;
  dct:contributor "Participants in W3C's Semantic Web Deployment Working Group.";
  dct:creator "Alistair Miles", "Sean Bechhofer";
  dct:description "An RDF vocabulary extending SKOS and allowing the description and linking of lexical entities."@en;
  dct:title "SKOS XL Vocabulary"@en;
  rdfs:seeAlso <http://www.w3.org/2008/05/skos>;
  owl:imports <http://www.w3.org/2004/02/skos/core> .

skosxl:Label a owl:Class;
  rdfs:isDefinedBy <http://www.w3.org/2008/05/skos-xl>;
  rdfs:label "Label"@en;
  rdfs:subClassOf _:node1dm3rmd0px1 .

_:node1dm3rmd0px1 a owl:Restriction;
  owl:cardinality "1"^^xsd:nonNegativeInteger;
  owl:onProperty skosxl:literalForm .

skosxl:Label owl:disjointWith skos:Collection, skos:Concept, skos:ConceptScheme;
  skos:definition "A special class of lexical entities."@en .

skosxl:literalForm a rdf:Property, owl:DatatypeProperty;
  rdfs:comment "If two instances of the class skosxl:Label have the same literal form, they are not necessarily the same resource."@en,
    "The range of skosxl:literalForm is the class of RDF plain literals."@en;
  rdfs:domain skosxl:Label;
  rdfs:isDefinedBy <http://www.w3.org/2008/05/skos-xl>;
  rdfs:label "literal form"@en;
  skos:definition "The property skosxl:literalForm is used to give the literal form of an skosxl:Label."@en .

skosxl:prefLabel a rdf:Property, owl:ObjectProperty;
  rdfs:comment "If C skosxl:prefLabel L and L skosxl:literalForm V, then X skos:prefLabel V."@en;
  rdfs:isDefinedBy <http://www.w3.org/2008/05/skos-xl>;
  rdfs:label "preferred label"@en;
  rdfs:range skosxl:Label;
  rdfs:seeAlso skos:prefLabel;
  skos:definition "The property skosxl:prefLabel is used to associate an skosxl:Label with a skos:Concept. The property is analogous to skos:prefLabel."@en .

skosxl:altLabel a rdf:Property, owl:ObjectProperty;
  rdfs:comment "If C skosxl:altLabel L and L skosxl:literalForm V, then X skos:altLabel V."@en;
  rdfs:isDefinedBy <http://www.w3.org/2008/05/skos-xl>;
  rdfs:label "alternative label"@en;
  rdfs:range skosxl:Label;
  rdfs:seeAlso skos:altLabel;
  skos:definition "The property skosxl:altLabel is used to associate an skosxl:Label with a skos:Concept. The property is analogous to skos:altLabel."@en .

skosxl:hiddenLabel a rdf:Property, owl:ObjectProperty;
  rdfs:comment "If C skosxl:hiddenLabel L and L skosxl:literalForm V, then C skos:hiddenLabel V."@en;
  rdfs:isDefinedBy <http://www.w3.org/2008/05/skos-xl>;
  rdfs:label "hidden label"@en;
  rdfs:range skosxl:Label;
  rdfs:seeAlso skos:hiddenLabel;
  skos:definition "The property skosxl:hiddenLabel is used to associate an skosxl:Label with a skos:Concept. The property is analogous to skos:hiddenLabel."@en .

skosxl:labelRelation a rdf:Property, owl:ObjectProperty, owl:SymmetricProperty;
  rdfs:domain skosxl:Label;
  rdfs:isDefinedBy <http://www.w3.org/2008/05/skos-xl>;
  rdfs:label "label relation"@en;
  rdfs:range skosxl:Label;
  skos:definition "The property skosxl:labelRelation is used for representing binary ('direct') relations between instances of the class skosxl:Label."@en;
  skos:scopeNote "skosxl:labelRelation is not intended to be used directly, but rather as the basis for a design pattern which can be refined for more specific labeling scenarios."@en .

<http://www.w3.org/2002/07/owl> a owl:Ontology;
  dc:title "The OWL 2 Schema vocabulary (OWL 2)";
  rdfs:comment """
  This ontology partially describes the built-in classes and
  properties that together form the basis of the RDF/XML syntax of OWL 2.
  The content of this ontology is based on Tables 6.1 and 6.2
  in Section 6.4 of the OWL 2 RDF-Based Semantics specification,
  available at http://www.w3.org/TR/owl2-rdf-based-semantics/.
  Please note that those tables do not include the different annotations
  (labels, comments and rdfs:isDefinedBy links) used in this file.
  Also note that the descriptions provided in this ontology do not
  provide a complete and correct formal description of either the syntax
  or the semantics of the introduced terms (please see the OWL 2
  recommendations for the complete and normative specifications).
  Furthermore, the information provided by this ontology may be
  misleading if not used with care. This ontology SHOULD NOT be imported
  into OWL ontologies. Importing this file into an OWL 2 DL ontology
  will cause it to become an OWL 2 Full ontology and may have other,
  unexpected, consequences.
   """;
  rdfs:isDefinedBy <http://www.w3.org/TR/owl2-mapping-to-rdf/>, <http://www.w3.org/TR/owl2-rdf-based-semantics/>,
    <http://www.w3.org/TR/owl2-syntax/>;
  rdfs:seeAlso <http://www.w3.org/TR/owl2-rdf-based-semantics/#table-axiomatic-classes>,
    <http://www.w3.org/TR/owl2-rdf-based-semantics/#table-axiomatic-properties>;
  owl:imports <http://www.w3.org/2000/01/rdf-schema>;
  owl:versionIRI <http://www.w3.org/2002/07/owl>;
  owl:versionInfo "$Date: 2009/11/15 10:54:12 $";
  grddl:namespaceTransformation <http://dev.w3.org/cvsweb/2009/owl-grddl/owx2rdf.xsl> .

owl:AllDifferent a rdfs:Class;
  rdfs:comment "The class of collections of pairwise different individuals.";
  rdfs:isDefinedBy <http://www.w3.org/2002/07/owl#>;
  rdfs:label "AllDifferent";
  rdfs:subClassOf rdfs:Resource .

owl:AllDisjointClasses a rdfs:Class;
  rdfs:comment "The class of collections of pairwise disjoint classes.";
  rdfs:isDefinedBy <http://www.w3.org/2002/07/owl#>;
  rdfs:label "AllDisjointClasses";
  rdfs:subClassOf rdfs:Resource .

owl:AllDisjointProperties a rdfs:Class;
  rdfs:comment "The class of collections of pairwise disjoint properties.";
  rdfs:isDefinedBy <http://www.w3.org/2002/07/owl#>;
  rdfs:label "AllDisjointProperties";
  rdfs:subClassOf rdfs:Resource .

owl:Annotation a rdfs:Class;
  rdfs:comment "The class of annotated annotations for which the RDF serialization consists of an annotated subject, predicate and object.";
  rdfs:isDefinedBy <http://www.w3.org/2002/07/owl#>;
  rdfs:label "Annotation";
  rdfs:subClassOf rdfs:Resource .

owl:AnnotationProperty a rdfs:Class;
  rdfs:comment "The class of annotation properties.";
  rdfs:isDefinedBy <http://www.w3.org/2002/07/owl#>;
  rdfs:label "AnnotationProperty";
  rdfs:subClassOf rdf:Property .

owl:AsymmetricProperty a rdfs:Class;
  rdfs:comment "The class of asymmetric properties.";
  rdfs:isDefinedBy <http://www.w3.org/2002/07/owl#>;
  rdfs:label "AsymmetricProperty";
  rdfs:subClassOf owl:ObjectProperty .

owl:Axiom a rdfs:Class;
  rdfs:comment "The class of annotated axioms for which the RDF serialization consists of an annotated subject, predicate and object.";
  rdfs:isDefinedBy <http://www.w3.org/2002/07/owl#>;
  rdfs:label "Axiom";
  rdfs:subClassOf rdfs:Resource .

owl:Class a rdfs:Class;
  rdfs:comment "The class of OWL classes.";
  rdfs:isDefinedBy <http://www.w3.org/2002/07/owl#>;
  rdfs:label "Class";
  rdfs:subClassOf rdfs:Class .

owl:DataRange a rdfs:Class;
  rdfs:comment "The class of OWL data ranges, which are special kinds of datatypes. Note: The use of the IRI owl:DataRange has been deprecated as of OWL 2. The IRI rdfs:Datatype SHOULD be used instead.";
  rdfs:isDefinedBy <http://www.w3.org/2002/07/owl#>;
  rdfs:label "DataRange";
  rdfs:subClassOf rdfs:Datatype .

owl:DatatypeProperty a rdfs:Class;
  rdfs:comment "The class of data properties.";
  rdfs:isDefinedBy <http://www.w3.org/2002/07/owl#>;
  rdfs:label "DatatypeProperty";
  rdfs:subClassOf rdf:Property .

owl:DeprecatedClass a rdfs:Class;
  rdfs:comment "The class of deprecated classes.";
  rdfs:isDefinedBy <http://www.w3.org/2002/07/owl#>;
  rdfs:label "DeprecatedClass";
  rdfs:subClassOf rdfs:Class .

owl:DeprecatedProperty a rdfs:Class;
  rdfs:comment "The class of deprecated properties.";
  rdfs:isDefinedBy <http://www.w3.org/2002/07/owl#>;
  rdfs:label "DeprecatedProperty";
  rdfs:subClassOf rdf:Property .

owl:FunctionalProperty a rdfs:Class;
  rdfs:comment "The class of functional properties.";
  rdfs:isDefinedBy <http://www.w3.org/2002/07/owl#>;
  rdfs:label "FunctionalProperty";
  rdfs:subClassOf rdf:Property .

owl:InverseFunctionalProperty a rdfs:Class;
  rdfs:comment "The class of inverse-functional properties.";
  rdfs:isDefinedBy <http://www.w3.org/2002/07/owl#>;
  rdfs:label "InverseFunctionalProperty";
  rdfs:subClassOf owl:ObjectProperty .

owl:IrreflexiveProperty a rdfs:Class;
  rdfs:comment "The class of irreflexive properties.";
  rdfs:isDefinedBy <http://www.w3.org/2002/07/owl#>;
  rdfs:label "IrreflexiveProperty";
  rdfs:subClassOf owl:ObjectProperty .

owl:NamedIndividual a rdfs:Class;
  rdfs:comment "The class of named individuals.";
  rdfs:isDefinedBy <http://www.w3.org/2002/07/owl#>;
  rdfs:label "NamedIndividual";
  rdfs:subClassOf owl:Thing .

owl:NegativePropertyAssertion a rdfs:Class;
  rdfs:comment "The class of negative property assertions.";
  rdfs:isDefinedBy <http://www.w3.org/2002/07/owl#>;
  rdfs:label "NegativePropertyAssertion";
  rdfs:subClassOf rdfs:Resource .

owl:Nothing a owl:Class;
  rdfs:comment "This is the empty class.";
  rdfs:isDefinedBy <http://www.w3.org/2002/07/owl#>;
  rdfs:label "Nothing";
  rdfs:subClassOf owl:Thing .

owl:ObjectProperty a rdfs:Class;
  rdfs:comment "The class of object properties.";
  rdfs:isDefinedBy <http://www.w3.org/2002/07/owl#>;
  rdfs:label "ObjectProperty";
  rdfs:subClassOf rdf:Property .

owl:Ontology a rdfs:Class;
  rdfs:comment "The class of ontologies.";
  rdfs:isDefinedBy <http://www.w3.org/2002/07/owl#>;
  rdfs:label "Ontology";
  rdfs:subClassOf rdfs:Resource .

owl:OntologyProperty a rdfs:Class;
  rdfs:comment "The class of ontology properties.";
  rdfs:isDefinedBy <http://www.w3.org/2002/07/owl#>;
  rdfs:label "OntologyProperty";
  rdfs:subClassOf rdf:Property .

owl:ReflexiveProperty a rdfs:Class;
  rdfs:comment "The class of reflexive properties.";
  rdfs:isDefinedBy <http://www.w3.org/2002/07/owl#>;
  rdfs:label "ReflexiveProperty";
  rdfs:subClassOf owl:ObjectProperty .

owl:Restriction a rdfs:Class;
  rdfs:comment "The class of property restrictions.";
  rdfs:isDefinedBy <http://www.w3.org/2002/07/owl#>;
  rdfs:label "Restriction";
  rdfs:subClassOf owl:Class .

owl:SymmetricProperty a rdfs:Class;
  rdfs:comment "The class of symmetric properties.";
  rdfs:isDefinedBy <http://www.w3.org/2002/07/owl#>;
  rdfs:label "SymmetricProperty";
  rdfs:subClassOf owl:ObjectProperty .

owl:Thing a owl:Class;
  rdfs:comment "The class of OWL individuals.";
  rdfs:isDefinedBy <http://www.w3.org/2002/07/owl#>;
  rdfs:label "Thing" .

owl:TransitiveProperty a rdfs:Class;
  rdfs:comment "The class of transitive properties.";
  rdfs:isDefinedBy <http://www.w3.org/2002/07/owl#>;
  rdfs:label "TransitiveProperty";
  rdfs:subClassOf owl:ObjectProperty .

owl:allValuesFrom a rdf:Property;
  rdfs:comment "The property that determines the class that a universal property restriction refers to.";
  rdfs:domain owl:Restriction;
  rdfs:isDefinedBy <http://www.w3.org/2002/07/owl#>;
  rdfs:label "allValuesFrom";
  rdfs:range rdfs:Class .

owl:annotatedProperty a rdf:Property;
  rdfs:comment "The property that determines the predicate of an annotated axiom or annotated annotation.";
  rdfs:domain rdfs:Resource;
  rdfs:isDefinedBy <http://www.w3.org/2002/07/owl#>;
  rdfs:label "annotatedProperty";
  rdfs:range rdfs:Resource .

owl:annotatedSource a rdf:Property;
  rdfs:comment "The property that determines the subject of an annotated axiom or annotated annotation.";
  rdfs:domain rdfs:Resource;
  rdfs:isDefinedBy <http://www.w3.org/2002/07/owl#>;
  rdfs:label "annotatedSource";
  rdfs:range rdfs:Resource .

owl:annotatedTarget a rdf:Property;
  rdfs:comment "The property that determines the object of an annotated axiom or annotated annotation.";
  rdfs:domain rdfs:Resource;
  rdfs:isDefinedBy <http://www.w3.org/2002/07/owl#>;
  rdfs:label "annotatedTarget";
  rdfs:range rdfs:Resource .

owl:assertionProperty a rdf:Property;
  rdfs:comment "The property that determines the predicate of a negative property assertion.";
  rdfs:domain owl:NegativePropertyAssertion;
  rdfs:isDefinedBy <http://www.w3.org/2002/07/owl#>;
  rdfs:label "assertionProperty";
  rdfs:range rdf:Property .

owl:backwardCompatibleWith a owl:AnnotationProperty, owl:OntologyProperty;
  rdfs:comment "The annotation property that indicates that a given ontology is backward compatible with another ontology.";
  rdfs:domain owl:Ontology;
  rdfs:isDefinedBy <http://www.w3.org/2002/07/owl#>;
  rdfs:label "backwardCompatibleWith";
  rdfs:range owl:Ontology .

owl:bottomDataProperty a owl:DatatypeProperty;
  rdfs:comment "The data property that does not relate any individual to any data value.";
  rdfs:domain owl:Thing;
  rdfs:isDefinedBy <http://www.w3.org/2002/07/owl#>;
  rdfs:label "bottomDataProperty";
  rdfs:range rdfs:Literal .

owl:bottomObjectProperty a owl:ObjectProperty;
  rdfs:comment "The object property that does not relate any two individuals.";
  rdfs:domain owl:Thing;
  rdfs:isDefinedBy <http://www.w3.org/2002/07/owl#>;
  rdfs:label "bottomObjectProperty";
  rdfs:range owl:Thing .

owl:cardinality a rdf:Property;
  rdfs:comment "The property that determines the cardinality of an exact cardinality restriction.";
  rdfs:domain owl:Restriction;
  rdfs:isDefinedBy <http://www.w3.org/2002/07/owl#>;
  rdfs:label "cardinality";
  rdfs:range xsd:nonNegativeInteger .

owl:complementOf a rdf:Property;
  rdfs:comment "The property that determines that a given class is the complement of another class.";
  rdfs:domain owl:Class;
  rdfs:isDefinedBy <http://www.w3.org/2002/07/owl#>;
  rdfs:label "complementOf";
  rdfs:range owl:Class .

owl:datatypeComplementOf a rdf:Property;
  rdfs:comment "The property that determines that a given data range is the complement of another data range with respect to the data domain.";
  rdfs:domain rdfs:Datatype;
  rdfs:isDefinedBy <http://www.w3.org/2002/07/owl#>;
  rdfs:label "datatypeComplementOf";
  rdfs:range rdfs:Datatype .

owl:deprecated a owl:AnnotationProperty;
  rdfs:comment "The annotation property that indicates that a given entity has been deprecated.";
  rdfs:domain rdfs:Resource;
  rdfs:isDefinedBy <http://www.w3.org/2002/07/owl#>;
  rdfs:label "deprecated";
  rdfs:range rdfs:Resource .

owl:differentFrom a rdf:Property;
  rdfs:comment "The property that determines that two given individuals are different.";
  rdfs:domain owl:Thing;
  rdfs:isDefinedBy <http://www.w3.org/2002/07/owl#>;
  rdfs:label "differentFrom";
  rdfs:range owl:Thing .

owl:disjointUnionOf a rdf:Property;
  rdfs:comment "The property that determines that a given class is equivalent to the disjoint union of a collection of other classes.";
  rdfs:domain owl:Class;
  rdfs:isDefinedBy <http://www.w3.org/2002/07/owl#>;
  rdfs:label "disjointUnionOf";
  rdfs:range rdf:List .

owl:disjointWith a rdf:Property;
  rdfs:comment "The property that determines that two given classes are disjoint.";
  rdfs:domain owl:Class;
  rdfs:isDefinedBy <http://www.w3.org/2002/07/owl#>;
  rdfs:label "disjointWith";
  rdfs:range owl:Class .

owl:distinctMembers a rdf:Property;
  rdfs:comment "The property that determines the collection of pairwise different individuals in a owl:AllDifferent axiom.";
  rdfs:domain owl:AllDifferent;
  rdfs:isDefinedBy <http://www.w3.org/2002/07/owl#>;
  rdfs:label "distinctMembers";
  rdfs:range rdf:List .

owl:equivalentClass a rdf:Property;
  rdfs:comment "The property that determines that two given classes are equivalent, and that is used to specify datatype definitions.";
  rdfs:domain rdfs:Class;
  rdfs:isDefinedBy <http://www.w3.org/2002/07/owl#>;
  rdfs:label "equivalentClass";
  rdfs:range rdfs:Class .

owl:equivalentProperty a rdf:Property;
  rdfs:comment "The property that determines that two given properties are equivalent.";
  rdfs:domain rdf:Property;
  rdfs:isDefinedBy <http://www.w3.org/2002/07/owl#>;
  rdfs:label "equivalentProperty";
  rdfs:range rdf:Property .

owl:hasKey a rdf:Property;
  rdfs:comment "The property that determines the collection of properties that jointly build a key.";
  rdfs:domain owl:Class;
  rdfs:isDefinedBy <http://www.w3.org/2002/07/owl#>;
  rdfs:label "hasKey";
  rdfs:range rdf:List .

owl:hasSelf a rdf:Property;
  rdfs:comment "The property that determines the property that a self restriction refers to.";
  rdfs:domain owl:Restriction;
  rdfs:isDefinedBy <http://www.w3.org/2002/07/owl#>;
  rdfs:label "hasSelf";
  rdfs:range rdfs:Resource .

owl:hasValue a rdf:Property;
  rdfs:comment "The property that determines the individual that a has-value restriction refers to.";
  rdfs:domain owl:Restriction;
  rdfs:isDefinedBy <http://www.w3.org/2002/07/owl#>;
  rdfs:label "hasValue";
  rdfs:range rdfs:Resource .

owl:imports a owl:OntologyProperty;
  rdfs:comment "The property that is used for importing other ontologies into a given ontology.";
  rdfs:domain owl:Ontology;
  rdfs:isDefinedBy <http://www.w3.org/2002/07/owl#>;
  rdfs:label "imports";
  rdfs:range owl:Ontology .

owl:incompatibleWith a owl:AnnotationProperty, owl:OntologyProperty;
  rdfs:comment "The annotation property that indicates that a given ontology is incompatible with another ontology.";
  rdfs:domain owl:Ontology;
  rdfs:isDefinedBy <http://www.w3.org/2002/07/owl#>;
  rdfs:label "incompatibleWith";
  rdfs:range owl:Ontology .

owl:intersectionOf a rdf:Property;
  rdfs:comment "The property that determines the collection of classes or data ranges that build an intersection.";
  rdfs:domain rdfs:Class;
  rdfs:isDefinedBy <http://www.w3.org/2002/07/owl#>;
  rdfs:label "intersectionOf";
  rdfs:range rdf:List .

owl:inverseOf a rdf:Property;
  rdfs:comment "The property that determines that two given properties are inverse.";
  rdfs:domain owl:ObjectProperty;
  rdfs:isDefinedBy <http://www.w3.org/2002/07/owl#>;
  rdfs:label "inverseOf";
  rdfs:range owl:ObjectProperty .

owl:maxCardinality a rdf:Property;
  rdfs:comment "The property that determines the cardinality of a maximum cardinality restriction.";
  rdfs:domain owl:Restriction;
  rdfs:isDefinedBy <http://www.w3.org/2002/07/owl#>;
  rdfs:label "maxCardinality";
  rdfs:range xsd:nonNegativeInteger .

owl:maxQualifiedCardinality a rdf:Property;
  rdfs:comment "The property that determines the cardinality of a maximum qualified cardinality restriction.";
  rdfs:domain owl:Restriction;
  rdfs:isDefinedBy <http://www.w3.org/2002/07/owl#>;
  rdfs:label "maxQualifiedCardinality";
  rdfs:range xsd:nonNegativeInteger .

owl:members a rdf:Property;
  rdfs:comment "The property that determines the collection of members in either a owl:AllDifferent, owl:AllDisjointClasses or owl:AllDisjointProperties axiom.";
  rdfs:domain rdfs:Resource;
  rdfs:isDefinedBy <http://www.w3.org/2002/07/owl#>;
  rdfs:label "members";
  rdfs:range rdf:List .

owl:minCardinality a rdf:Property;
  rdfs:comment "The property that determines the cardinality of a minimum cardinality restriction.";
  rdfs:domain owl:Restriction;
  rdfs:isDefinedBy <http://www.w3.org/2002/07/owl#>;
  rdfs:label "minCardinality";
  rdfs:range xsd:nonNegativeInteger .

owl:minQualifiedCardinality a rdf:Property;
  rdfs:comment "The property that determines the cardinality of a minimum qualified cardinality restriction.";
  rdfs:domain owl:Restriction;
  rdfs:isDefinedBy <http://www.w3.org/2002/07/owl#>;
  rdfs:label "minQualifiedCardinality";
  rdfs:range xsd:nonNegativeInteger .

owl:onClass a rdf:Property;
  rdfs:comment "The property that determines the class that a qualified object cardinality restriction refers to.";
  rdfs:domain owl:Restriction;
  rdfs:isDefinedBy <http://www.w3.org/2002/07/owl#>;
  rdfs:label "onClass";
  rdfs:range owl:Class .

owl:onDataRange a rdf:Property;
  rdfs:comment "The property that determines the data range that a qualified data cardinality restriction refers to.";
  rdfs:domain owl:Restriction;
  rdfs:isDefinedBy <http://www.w3.org/2002/07/owl#>;
  rdfs:label "onDataRange";
  rdfs:range rdfs:Datatype .

owl:onDatatype a rdf:Property;
  rdfs:comment "The property that determines the datatype that a datatype restriction refers to.";
  rdfs:domain rdfs:Datatype;
  rdfs:isDefinedBy <http://www.w3.org/2002/07/owl#>;
  rdfs:label "onDatatype";
  rdfs:range rdfs:Datatype .

owl:oneOf a rdf:Property;
  rdfs:comment "The property that determines the collection of individuals or data values that build an enumeration.";
  rdfs:domain rdfs:Class;
  rdfs:isDefinedBy <http://www.w3.org/2002/07/owl#>;
  rdfs:label "oneOf";
  rdfs:range rdf:List .

owl:onProperties a rdf:Property;
  rdfs:comment "The property that determines the n-tuple of properties that a property restriction on an n-ary data range refers to.";
  rdfs:domain owl:Restriction;
  rdfs:isDefinedBy <http://www.w3.org/2002/07/owl#>;
  rdfs:label "onProperties";
  rdfs:range rdf:List .

owl:onProperty a rdf:Property;
  rdfs:comment "The property that determines the property that a property restriction refers to.";
  rdfs:domain owl:Restriction;
  rdfs:isDefinedBy <http://www.w3.org/2002/07/owl#>;
  rdfs:label "onProperty";
  rdfs:range rdf:Property .

owl:priorVersion a owl:AnnotationProperty, owl:OntologyProperty;
  rdfs:comment "The annotation property that indicates the predecessor ontology of a given ontology.";
  rdfs:domain owl:Ontology;
  rdfs:isDefinedBy <http://www.w3.org/2002/07/owl#>;
  rdfs:label "priorVersion";
  rdfs:range owl:Ontology .

owl:propertyChainAxiom a rdf:Property;
  rdfs:comment "The property that determines the n-tuple of properties that build a sub property chain of a given property.";
  rdfs:domain owl:ObjectProperty;
  rdfs:isDefinedBy <http://www.w3.org/2002/07/owl#>;
  rdfs:label "propertyChainAxiom";
  rdfs:range rdf:List .

owl:propertyDisjointWith a rdf:Property;
  rdfs:comment "The property that determines that two given properties are disjoint.";
  rdfs:domain rdf:Property;
  rdfs:isDefinedBy <http://www.w3.org/2002/07/owl#>;
  rdfs:label "propertyDisjointWith";
  rdfs:range rdf:Property .

owl:qualifiedCardinality a rdf:Property;
  rdfs:comment "The property that determines the cardinality of an exact qualified cardinality restriction.";
  rdfs:domain owl:Restriction;
  rdfs:isDefinedBy <http://www.w3.org/2002/07/owl#>;
  rdfs:label "qualifiedCardinality";
  rdfs:range xsd:nonNegativeInteger .

owl:sameAs a rdf:Property;
  rdfs:comment "The property that determines that two given individuals are equal.";
  rdfs:domain owl:Thing;
  rdfs:isDefinedBy <http://www.w3.org/2002/07/owl#>;
  rdfs:label "sameAs";
  rdfs:range owl:Thing .

owl:someValuesFrom a rdf:Property;
  rdfs:comment "The property that determines the class that an existential property restriction refers to.";
  rdfs:domain owl:Restriction;
  rdfs:isDefinedBy <http://www.w3.org/2002/07/owl#>;
  rdfs:label "someValuesFrom";
  rdfs:range rdfs:Class .

owl:sourceIndividual a rdf:Property;
  rdfs:comment "The property that determines the subject of a negative property assertion.";
  rdfs:domain owl:NegativePropertyAssertion;
  rdfs:isDefinedBy <http://www.w3.org/2002/07/owl#>;
  rdfs:label "sourceIndividual";
  rdfs:range owl:Thing .

owl:targetIndividual a rdf:Property;
  rdfs:comment "The property that determines the object of a negative object property assertion.";
  rdfs:domain owl:NegativePropertyAssertion;
  rdfs:isDefinedBy <http://www.w3.org/2002/07/owl#>;
  rdfs:label "targetIndividual";
  rdfs:range owl:Thing .

owl:targetValue a rdf:Property;
  rdfs:comment "The property that determines the value of a negative data property assertion.";
  rdfs:domain owl:NegativePropertyAssertion;
  rdfs:isDefinedBy <http://www.w3.org/2002/07/owl#>;
  rdfs:label "targetValue";
  rdfs:range rdfs:Literal .

owl:topDataProperty a owl:DatatypeProperty;
  rdfs:comment "The data property that relates every individual to every data value.";
  rdfs:domain owl:Thing;
  rdfs:isDefinedBy <http://www.w3.org/2002/07/owl#>;
  rdfs:label "topDataProperty";
  rdfs:range rdfs:Literal .

owl:topObjectProperty a owl:ObjectProperty;
  rdfs:comment "The object property that relates every two individuals.";
  rdfs:domain owl:Thing;
  rdfs:isDefinedBy <http://www.w3.org/2002/07/owl#>;
  rdfs:label "topObjectProperty";
  rdfs:range owl:Thing .

owl:unionOf a rdf:Property;
  rdfs:comment "The property that determines the collection of classes or data ranges that build a union.";
  rdfs:domain rdfs:Class;
  rdfs:isDefinedBy <http://www.w3.org/2002/07/owl#>;
  rdfs:label "unionOf";
  rdfs:range rdf:List .

owl:versionInfo a owl:AnnotationProperty;
  rdfs:comment "The annotation property that provides version information for an ontology or another OWL construct.";
  rdfs:domain rdfs:Resource;
  rdfs:isDefinedBy <http://www.w3.org/2002/07/owl#>;
  rdfs:label "versionInfo";
  rdfs:range rdfs:Resource .

owl:versionIRI a owl:OntologyProperty;
  rdfs:comment "The property that identifies the version IRI of an ontology.";
  rdfs:domain owl:Ontology;
  rdfs:isDefinedBy <http://www.w3.org/2002/07/owl#>;
  rdfs:label "versionIRI";
  rdfs:range owl:Ontology .

owl:withRestrictions a rdf:Property;
  rdfs:comment "The property that determines the collection of facet-value pairs that define a datatype restriction.";
  rdfs:domain rdfs:Datatype;
  rdfs:isDefinedBy <http://www.w3.org/2002/07/owl#>;
  rdfs:label "withRestrictions";
  rdfs:range rdf:List .

<http://www.w3.org/2000/01/rdf-schema#> a owl:Ontology;
  dc:title "The RDF Schema vocabulary (RDFS)";
  rdfs:seeAlso <http://www.w3.org/2000/01/rdf-schema-more> .

rdfs:Resource a rdfs:Class;
  rdfs:comment "The class resource, everything.";
  rdfs:isDefinedBy <http://www.w3.org/2000/01/rdf-schema#>;
  rdfs:label "Resource" .

rdfs:Class a rdfs:Class;
  rdfs:comment "The class of classes.";
  rdfs:isDefinedBy <http://www.w3.org/2000/01/rdf-schema#>;
  rdfs:label "Class";
  rdfs:subClassOf rdfs:Resource .

rdfs:subClassOf a rdf:Property;
  rdfs:comment "The subject is a subclass of a class.";
  rdfs:domain rdfs:Class;
  rdfs:isDefinedBy <http://www.w3.org/2000/01/rdf-schema#>;
  rdfs:label "subClassOf";
  rdfs:range rdfs:Class .

rdfs:subPropertyOf a rdf:Property;
  rdfs:comment "The subject is a subproperty of a property.";
  rdfs:domain rdf:Property;
  rdfs:isDefinedBy <http://www.w3.org/2000/01/rdf-schema#>;
  rdfs:label "subPropertyOf";
  rdfs:range rdf:Property .

rdfs:comment a rdf:Property;
  rdfs:comment "A description of the subject resource.";
  rdfs:domain rdfs:Resource;
  rdfs:isDefinedBy <http://www.w3.org/2000/01/rdf-schema#>;
  rdfs:label "comment";
  rdfs:range rdfs:Literal .

rdfs:label a rdf:Property;
  rdfs:comment "A human-readable name for the subject.";
  rdfs:domain rdfs:Resource;
  rdfs:isDefinedBy <http://www.w3.org/2000/01/rdf-schema#>;
  rdfs:label "label";
  rdfs:range rdfs:Literal .

rdfs:domain a rdf:Property;
  rdfs:comment "A domain of the subject property.";
  rdfs:domain rdf:Property;
  rdfs:isDefinedBy <http://www.w3.org/2000/01/rdf-schema#>;
  rdfs:label "domain";
  rdfs:range rdfs:Class .

rdfs:range a rdf:Property;
  rdfs:comment "A range of the subject property.";
  rdfs:domain rdf:Property;
  rdfs:isDefinedBy <http://www.w3.org/2000/01/rdf-schema#>;
  rdfs:label "range";
  rdfs:range rdfs:Class .

rdfs:seeAlso a rdf:Property;
  rdfs:comment "Further information about the subject resource.";
  rdfs:domain rdfs:Resource;
  rdfs:isDefinedBy <http://www.w3.org/2000/01/rdf-schema#>;
  rdfs:label "seeAlso";
  rdfs:range rdfs:Resource .

rdfs:isDefinedBy a rdf:Property;
  rdfs:comment "The defininition of the subject resource.";
  rdfs:domain rdfs:Resource;
  rdfs:isDefinedBy <http://www.w3.org/2000/01/rdf-schema#>;
  rdfs:label "isDefinedBy";
  rdfs:range rdfs:Resource;
  rdfs:subPropertyOf rdfs:seeAlso .

rdfs:Literal a rdfs:Class;
  rdfs:comment "The class of literal values, eg. textual strings and integers.";
  rdfs:isDefinedBy <http://www.w3.org/2000/01/rdf-schema#>;
  rdfs:label "Literal";
  rdfs:subClassOf rdfs:Resource .

rdfs:Container a rdfs:Class;
  rdfs:comment "The class of RDF containers.";
  rdfs:isDefinedBy <http://www.w3.org/2000/01/rdf-schema#>;
  rdfs:label "Container";
  rdfs:subClassOf rdfs:Resource .

rdfs:ContainerMembershipProperty a rdfs:Class;
  rdfs:comment """The class of container membership properties, rdf:_1, rdf:_2, ...,
                    all of which are sub-properties of 'member'.""";
  rdfs:isDefinedBy <http://www.w3.org/2000/01/rdf-schema#>;
  rdfs:label "ContainerMembershipProperty";
  rdfs:subClassOf rdf:Property .

rdfs:member a rdf:Property;
  rdfs:comment "A member of the subject resource.";
  rdfs:domain rdfs:Resource;
  rdfs:isDefinedBy <http://www.w3.org/2000/01/rdf-schema#>;
  rdfs:label "member";
  rdfs:range rdfs:Resource .

rdfs:Datatype a rdfs:Class;
  rdfs:comment "The class of RDF datatypes.";
  rdfs:isDefinedBy <http://www.w3.org/2000/01/rdf-schema#>;
  rdfs:label "Datatype";
  rdfs:subClassOf rdfs:Class .

<http://www.w3.org/2004/02/skos/core> a owl:Ontology;
  dct:contributor "Dave Beckett", "Nikki Rogers", "Participants in W3C's Semantic Web Deployment Working Group.";
  dct:creator "Alistair Miles", "Sean Bechhofer";
  dct:description "An RDF vocabulary for describing the basic structure and content of concept schemes such as thesauri, classification schemes, subject heading lists, taxonomies, 'folksonomies', other types of controlled vocabulary, and also concept schemes embedded in glossaries and terminologies."@en;
  dct:title "SKOS Vocabulary"@en;
  rdfs:seeAlso <http://www.w3.org/TR/skos-reference/> .

skos:Concept a owl:Class;
  rdfs:isDefinedBy <http://www.w3.org/2004/02/skos/core>;
  rdfs:label "Concept"@en;
  skos:definition "An idea or notion; a unit of thought."@en .

skos:ConceptScheme a owl:Class;
  rdfs:isDefinedBy <http://www.w3.org/2004/02/skos/core>;
  rdfs:label "Concept Scheme"@en;
  owl:disjointWith skos:Concept;
  skos:definition "A set of concepts, optionally including statements about semantic relationships between those concepts."@en;
  skos:example "Thesauri, classification schemes, subject heading lists, taxonomies, 'folksonomies', and other types of controlled vocabulary are all examples of concept schemes. Concept schemes are also embedded in glossaries and terminologies."@en;
  skos:scopeNote "A concept scheme may be defined to include concepts from different sources."@en .

skos:Collection a owl:Class;
  rdfs:isDefinedBy <http://www.w3.org/2004/02/skos/core>;
  rdfs:label "Collection"@en;
  owl:disjointWith skos:Concept, skos:ConceptScheme;
  skos:definition "A meaningful collection of concepts."@en;
  skos:scopeNote "Labelled collections can be used where you would like a set of concepts to be displayed under a 'node label' in the hierarchy."@en .

skos:OrderedCollection a owl:Class;
  rdfs:isDefinedBy <http://www.w3.org/2004/02/skos/core>;
  rdfs:label "Ordered Collection"@en;
  rdfs:subClassOf skos:Collection;
  skos:definition "An ordered collection of concepts, where both the grouping and the ordering are meaningful."@en;
  skos:scopeNote "Ordered collections can be used where you would like a set of concepts to be displayed in a specific order, and optionally under a 'node label'."@en .

skos:inScheme a rdf:Property, owl:ObjectProperty;
  rdfs:isDefinedBy <http://www.w3.org/2004/02/skos/core>;
  rdfs:label "is in scheme"@en;
  rdfs:range skos:ConceptScheme;
  skos:definition "Relates a resource (for example a concept) to a concept scheme in which it is included."@en;
  skos:scopeNote "A concept may be a member of more than one concept scheme."@en .

skos:hasTopConcept a rdf:Property, owl:ObjectProperty;
  rdfs:domain skos:ConceptScheme;
  rdfs:isDefinedBy <http://www.w3.org/2004/02/skos/core>;
  rdfs:label "has top concept"@en;
  rdfs:range skos:Concept;
  owl:inverseOf skos:topConceptOf;
  skos:definition "Relates, by convention, a concept scheme to a concept which is topmost in the broader/narrower concept hierarchies for that scheme, providing an entry point to these hierarchies."@en .

skos:topConceptOf a rdf:Property, owl:ObjectProperty;
  rdfs:domain skos:Concept;
  rdfs:isDefinedBy <http://www.w3.org/2004/02/skos/core>;
  rdfs:label "is top concept in scheme"@en;
  rdfs:range skos:ConceptScheme;
  rdfs:subPropertyOf skos:inScheme;
  owl:inverseOf skos:hasTopConcept;
  skos:definition "Relates a concept to the concept scheme that it is a top level concept of."@en .

skos:prefLabel a rdf:Property, owl:AnnotationProperty;
  rdfs:comment "A resource has no more than one value of skos:prefLabel per language tag, and no more than one value of skos:prefLabel without language tag."@en,
    "The range of skos:prefLabel is the class of RDF plain literals."@en, """skos:prefLabel, skos:altLabel and skos:hiddenLabel are pairwise
      disjoint properties."""@en;
  rdfs:isDefinedBy <http://www.w3.org/2004/02/skos/core>;
  rdfs:label "preferred label"@en;
  rdfs:subPropertyOf rdfs:label;
  skos:definition "The preferred lexical label for a resource, in a given language."@en .

skos:altLabel a rdf:Property, owl:AnnotationProperty;
  rdfs:comment "The range of skos:altLabel is the class of RDF plain literals."@en,
    "skos:prefLabel, skos:altLabel and skos:hiddenLabel are pairwise disjoint properties."@en;
  rdfs:isDefinedBy <http://www.w3.org/2004/02/skos/core>;
  rdfs:label "alternative label"@en;
  rdfs:subPropertyOf rdfs:label;
  skos:definition "An alternative lexical label for a resource."@en;
  skos:example "Acronyms, abbreviations, spelling variants, and irregular plural/singular forms may be included among the alternative labels for a concept. Mis-spelled terms are normally included as hidden labels (see skos:hiddenLabel)."@en .

skos:hiddenLabel a rdf:Property, owl:AnnotationProperty;
  rdfs:comment "The range of skos:hiddenLabel is the class of RDF plain literals."@en,
    "skos:prefLabel, skos:altLabel and skos:hiddenLabel are pairwise disjoint properties."@en;
  rdfs:isDefinedBy <http://www.w3.org/2004/02/skos/core>;
  rdfs:label "hidden label"@en;
  rdfs:subPropertyOf rdfs:label;
  skos:definition "A lexical label for a resource that should be hidden when generating visual displays of the resource, but should still be accessible to free text search operations."@en .

skos:notation a rdf:Property, owl:DatatypeProperty;
  rdfs:isDefinedBy <http://www.w3.org/2004/02/skos/core>;
  rdfs:label "notation"@en;
  skos:definition "A notation, also known as classification code, is a string of characters such as \"T58.5\" or \"303.4833\" used to uniquely identify a concept within the scope of a given concept scheme."@en;
  skos:scopeNote "By convention, skos:notation is used with a typed literal in the object position of the triple."@en .

skos:note a rdf:Property, owl:AnnotationProperty;
  rdfs:isDefinedBy <http://www.w3.org/2004/02/skos/core>;
  rdfs:label "note"@en;
  skos:definition "A general note, for any purpose."@en;
  skos:scopeNote "This property may be used directly, or as a super-property for more specific note types."@en .

skos:changeNote a rdf:Property, owl:AnnotationProperty;
  rdfs:isDefinedBy <http://www.w3.org/2004/02/skos/core>;
  rdfs:label "change note"@en;
  rdfs:subPropertyOf skos:note;
  skos:definition "A note about a modification to a concept."@en .

skos:definition a rdf:Property, owl:AnnotationProperty;
  rdfs:isDefinedBy <http://www.w3.org/2004/02/skos/core>;
  rdfs:label "definition"@en;
  rdfs:subPropertyOf skos:note;
  skos:definition "A statement or formal explanation of the meaning of a concept."@en .

skos:editorialNote a rdf:Property, owl:AnnotationProperty;
  rdfs:isDefinedBy <http://www.w3.org/2004/02/skos/core>;
  rdfs:label "editorial note"@en;
  rdfs:subPropertyOf skos:note;
  skos:definition "A note for an editor, translator or maintainer of the vocabulary."@en .

skos:example a rdf:Property, owl:AnnotationProperty;
  rdfs:isDefinedBy <http://www.w3.org/2004/02/skos/core>;
  rdfs:label "example"@en;
  rdfs:subPropertyOf skos:note;
  skos:definition "An example of the use of a concept."@en .

skos:historyNote a rdf:Property, owl:AnnotationProperty;
  rdfs:isDefinedBy <http://www.w3.org/2004/02/skos/core>;
  rdfs:label "history note"@en;
  rdfs:subPropertyOf skos:note;
  skos:definition "A note about the past state/use/meaning of a concept."@en .

skos:scopeNote a rdf:Property, owl:AnnotationProperty;
  rdfs:isDefinedBy <http://www.w3.org/2004/02/skos/core>;
  rdfs:label "scope note"@en;
  rdfs:subPropertyOf skos:note;
  skos:definition "A note that helps to clarify the meaning and/or the use of a concept."@en .

skos:semanticRelation a rdf:Property, owl:ObjectProperty;
  rdfs:domain skos:Concept;
  rdfs:isDefinedBy <http://www.w3.org/2004/02/skos/core>;
  rdfs:label "is in semantic relation with"@en;
  rdfs:range skos:Concept;
  skos:definition "Links a concept to a concept related by meaning."@en;
  skos:scopeNote "This property should not be used directly, but as a super-property for all properties denoting a relationship of meaning between concepts."@en .

skos:broader a rdf:Property, owl:ObjectProperty;
  rdfs:comment "Broader concepts are typically rendered as parents in a concept hierarchy (tree)."@en;
  rdfs:isDefinedBy <http://www.w3.org/2004/02/skos/core>;
  rdfs:label "has broader"@en;
  rdfs:subPropertyOf skos:broaderTransitive;
  owl:inverseOf skos:narrower;
  skos:definition "Relates a concept to a concept that is more general in meaning."@en;
  skos:scopeNote "By convention, skos:broader is only used to assert an immediate (i.e. direct) hierarchical link between two conceptual resources."@en .

skos:narrower a rdf:Property, owl:ObjectProperty;
  rdfs:comment "Narrower concepts are typically rendered as children in a concept hierarchy (tree)."@en;
  rdfs:isDefinedBy <http://www.w3.org/2004/02/skos/core>;
  rdfs:label "has narrower"@en;
  rdfs:subPropertyOf skos:narrowerTransitive;
  owl:inverseOf skos:broader;
  skos:definition "Relates a concept to a concept that is more specific in meaning."@en;
  skos:scopeNote "By convention, skos:broader is only used to assert an immediate (i.e. direct) hierarchical link between two conceptual resources."@en .

skos:related a rdf:Property, owl:ObjectProperty, owl:SymmetricProperty;
  rdfs:comment "skos:related is disjoint with skos:broaderTransitive"@en;
  rdfs:isDefinedBy <http://www.w3.org/2004/02/skos/core>;
  rdfs:label "has related"@en;
  rdfs:subPropertyOf skos:semanticRelation;
  skos:definition "Relates a concept to a concept with which there is an associative semantic relationship."@en .

skos:broaderTransitive a rdf:Property, owl:ObjectProperty, owl:TransitiveProperty;
  rdfs:isDefinedBy <http://www.w3.org/2004/02/skos/core>;
  rdfs:label "has broader transitive"@en;
  rdfs:subPropertyOf skos:semanticRelation;
  owl:inverseOf skos:narrowerTransitive;
  skos:definition "skos:broaderTransitive is a transitive superproperty of skos:broader.";
  skos:scopeNote "By convention, skos:broaderTransitive is not used to make assertions. Rather, the properties can be used to draw inferences about the transitive closure of the hierarchical relation, which is useful e.g. when implementing a simple query expansion algorithm in a search application."@en .

skos:narrowerTransitive a rdf:Property, owl:ObjectProperty, owl:TransitiveProperty;
  rdfs:isDefinedBy <http://www.w3.org/2004/02/skos/core>;
  rdfs:label "has narrower transitive"@en;
  rdfs:subPropertyOf skos:semanticRelation;
  owl:inverseOf skos:broaderTransitive;
  skos:definition "skos:narrowerTransitive is a transitive superproperty of skos:narrower.";
  skos:scopeNote "By convention, skos:narrowerTransitive is not used to make assertions. Rather, the properties can be used to draw inferences about the transitive closure of the hierarchical relation, which is useful e.g. when implementing a simple query expansion algorithm in a search application."@en .

skos:member a rdf:Property, owl:ObjectProperty;
  rdfs:domain skos:Collection;
  rdfs:isDefinedBy <http://www.w3.org/2004/02/skos/core>;
  rdfs:label "has member"@en;
  rdfs:range _:node1dm3rmd0px2 .

_:node1dm3rmd0px2 a owl:Class;
  owl:unionOf _:node1dm3rmd0px3 .

_:node1dm3rmd0px3 rdf:first skos:Concept;
  rdf:rest _:node1dm3rmd0px4 .

_:node1dm3rmd0px4 rdf:first skos:Collection;
  rdf:rest rdf:nil .

skos:member skos:definition "Relates a collection to one of its members."@en .

skos:memberList a rdf:Property, owl:FunctionalProperty, owl:ObjectProperty;
  rdfs:comment """For any resource, every item in the list given as the value of the
      skos:memberList property is also a value of the skos:member property."""@en;
  rdfs:domain skos:OrderedCollection;
  rdfs:isDefinedBy <http://www.w3.org/2004/02/skos/core>;
  rdfs:label "has member list"@en;
  rdfs:range rdf:List;
  skos:definition "Relates an ordered collection to the RDF list containing its members."@en .

skos:mappingRelation a rdf:Property, owl:ObjectProperty;
  rdfs:comment "These concept mapping relations mirror semantic relations, and the data model defined below is similar (with the exception of skos:exactMatch) to the data model defined for semantic relations. A distinct vocabulary is provided for concept mapping relations, to provide a convenient way to differentiate links within a concept scheme from links between concept schemes. However, this pattern of usage is not a formal requirement of the SKOS data model, and relies on informal definitions of best practice."@en;
  rdfs:isDefinedBy <http://www.w3.org/2004/02/skos/core>;
  rdfs:label "is in mapping relation with"@en;
  rdfs:subPropertyOf skos:semanticRelation;
  skos:definition "Relates two concepts coming, by convention, from different schemes, and that have comparable meanings"@en .

skos:broadMatch a rdf:Property, owl:ObjectProperty;
  rdfs:isDefinedBy <http://www.w3.org/2004/02/skos/core>;
  rdfs:label "has broader match"@en;
  rdfs:subPropertyOf skos:broader, skos:mappingRelation;
  owl:inverseOf skos:narrowMatch;
  skos:definition "skos:broadMatch is used to state a hierarchical mapping link between two conceptual resources in different concept schemes."@en .

skos:narrowMatch a rdf:Property, owl:ObjectProperty;
  rdfs:isDefinedBy <http://www.w3.org/2004/02/skos/core>;
  rdfs:label "has narrower match"@en;
  rdfs:subPropertyOf skos:mappingRelation, skos:narrower;
  owl:inverseOf skos:broadMatch;
  skos:definition "skos:narrowMatch is used to state a hierarchical mapping link between two conceptual resources in different concept schemes."@en .

skos:relatedMatch a rdf:Property, owl:ObjectProperty, owl:SymmetricProperty;
  rdfs:isDefinedBy <http://www.w3.org/2004/02/skos/core>;
  rdfs:label "has related match"@en;
  rdfs:subPropertyOf skos:mappingRelation, skos:related;
  skos:definition "skos:relatedMatch is used to state an associative mapping link between two conceptual resources in different concept schemes."@en .

skos:exactMatch a rdf:Property, owl:ObjectProperty, owl:SymmetricProperty, owl:TransitiveProperty;
  rdfs:comment "skos:exactMatch is disjoint with each of the properties skos:broadMatch and skos:relatedMatch."@en;
  rdfs:isDefinedBy <http://www.w3.org/2004/02/skos/core>;
  rdfs:label "has exact match"@en;
  rdfs:subPropertyOf skos:closeMatch;
  skos:definition "skos:exactMatch is used to link two concepts, indicating a high degree of confidence that the concepts can be used interchangeably across a wide range of information retrieval applications. skos:exactMatch is a transitive property, and is a sub-property of skos:closeMatch."@en .

skos:closeMatch a rdf:Property, owl:ObjectProperty, owl:SymmetricProperty;
  rdfs:isDefinedBy <http://www.w3.org/2004/02/skos/core>;
  rdfs:label "has close match"@en;
  rdfs:subPropertyOf skos:mappingRelation;
  skos:definition "skos:closeMatch is used to link two concepts that are sufficiently similar that they can be used interchangeably in some information retrieval applications. In order to avoid the possibility of \"compound errors\" when combining mappings across more than two concept schemes, skos:closeMatch is not declared to be a transitive property."@en .

:c_c397370b skos:topConceptOf :epa-abg .

<http://www.w3.org/1999/02/22-rdf-syntax-ns#> a owl:Ontology;
  dc:description "This is the RDF Schema for the RDF vocabulary terms in the RDF Namespace, defined in RDF 1.1 Concepts.";
  dc:title "The RDF Concepts Vocabulary (RDF)";
  rdfs:seeAlso <http://www.w3.org/2000/01/rdf-schema-more> .

rdf:HTML a rdfs:Datatype;
  rdfs:comment "The datatype of RDF literals storing fragments of HTML content";
  rdfs:isDefinedBy <http://www.w3.org/1999/02/22-rdf-syntax-ns#>;
  rdfs:label "HTML";
  rdfs:seeAlso <http://www.w3.org/TR/rdf11-concepts/#section-html>;
  rdfs:subClassOf rdfs:Literal .

rdf:langString a rdfs:Datatype;
  rdfs:comment "The datatype of language-tagged string values";
  rdfs:isDefinedBy <http://www.w3.org/1999/02/22-rdf-syntax-ns#>;
  rdfs:label "langString";
  rdfs:seeAlso <http://www.w3.org/TR/rdf11-concepts/#section-Graph-Literal>;
  rdfs:subClassOf rdfs:Literal .

rdf:PlainLiteral a rdfs:Datatype;
  rdfs:comment "The class of plain (i.e. untyped) literal values, as used in RIF and OWL 2";
  rdfs:isDefinedBy <http://www.w3.org/1999/02/22-rdf-syntax-ns#>;
  rdfs:label "PlainLiteral";
  rdfs:seeAlso <http://www.w3.org/TR/rdf-plain-literal/>;
  rdfs:subClassOf rdfs:Literal .

rdf:type a rdf:Property;
  rdfs:comment "The subject is an instance of a class.";
  rdfs:domain rdfs:Resource;
  rdfs:isDefinedBy <http://www.w3.org/1999/02/22-rdf-syntax-ns#>;
  rdfs:label "type";
  rdfs:range rdfs:Class .

rdf:Property a rdfs:Class;
  rdfs:comment "The class of RDF properties.";
  rdfs:isDefinedBy <http://www.w3.org/1999/02/22-rdf-syntax-ns#>;
  rdfs:label "Property";
  rdfs:subClassOf rdfs:Resource .

rdf:Statement a rdfs:Class;
  rdfs:comment "The class of RDF statements.";
  rdfs:isDefinedBy <http://www.w3.org/1999/02/22-rdf-syntax-ns#>;
  rdfs:label "Statement";
  rdfs:subClassOf rdfs:Resource .

rdf:subject a rdf:Property;
  rdfs:comment "The subject of the subject RDF statement.";
  rdfs:domain rdf:Statement;
  rdfs:isDefinedBy <http://www.w3.org/1999/02/22-rdf-syntax-ns#>;
  rdfs:label "subject";
  rdfs:range rdfs:Resource .

rdf:predicate a rdf:Property;
  rdfs:comment "The predicate of the subject RDF statement.";
  rdfs:domain rdf:Statement;
  rdfs:isDefinedBy <http://www.w3.org/1999/02/22-rdf-syntax-ns#>;
  rdfs:label "predicate";
  rdfs:range rdfs:Resource .

rdf:object a rdf:Property;
  rdfs:comment "The object of the subject RDF statement.";
  rdfs:domain rdf:Statement;
  rdfs:isDefinedBy <http://www.w3.org/1999/02/22-rdf-syntax-ns#>;
  rdfs:label "object";
  rdfs:range rdfs:Resource .

rdf:Bag a rdfs:Class;
  rdfs:comment "The class of unordered containers.";
  rdfs:isDefinedBy <http://www.w3.org/1999/02/22-rdf-syntax-ns#>;
  rdfs:label "Bag";
  rdfs:subClassOf rdfs:Container .

rdf:Seq a rdfs:Class;
  rdfs:comment "The class of ordered containers.";
  rdfs:isDefinedBy <http://www.w3.org/1999/02/22-rdf-syntax-ns#>;
  rdfs:label "Seq";
  rdfs:subClassOf rdfs:Container .

rdf:Alt a rdfs:Class;
  rdfs:comment "The class of containers of alternatives.";
  rdfs:isDefinedBy <http://www.w3.org/1999/02/22-rdf-syntax-ns#>;
  rdfs:label "Alt";
  rdfs:subClassOf rdfs:Container .

rdf:value a rdf:Property;
  rdfs:comment "Idiomatic property used for structured values.";
  rdfs:domain rdfs:Resource;
  rdfs:isDefinedBy <http://www.w3.org/1999/02/22-rdf-syntax-ns#>;
  rdfs:label "value";
  rdfs:range rdfs:Resource .

rdf:List a rdfs:Class;
  rdfs:comment "The class of RDF Lists.";
  rdfs:isDefinedBy <http://www.w3.org/1999/02/22-rdf-syntax-ns#>;
  rdfs:label "List";
  rdfs:subClassOf rdfs:Resource .

rdf:nil a rdf:List;
  rdfs:comment "The empty list, with no items in it. If the rest of a list is nil then the list has no more items in it.";
  rdfs:isDefinedBy <http://www.w3.org/1999/02/22-rdf-syntax-ns#>;
  rdfs:label "nil" .

rdf:first a rdf:Property;
  rdfs:comment "The first item in the subject RDF list.";
  rdfs:domain rdf:List;
  rdfs:isDefinedBy <http://www.w3.org/1999/02/22-rdf-syntax-ns#>;
  rdfs:label "first";
  rdfs:range rdfs:Resource .

rdf:rest a rdf:Property;
  rdfs:comment "The rest of the subject RDF list after the first item.";
  rdfs:domain rdf:List;
  rdfs:isDefinedBy <http://www.w3.org/1999/02/22-rdf-syntax-ns#>;
  rdfs:label "rest";
  rdfs:range rdf:List .

rdf:XMLLiteral a rdfs:Datatype;
  rdfs:comment "The datatype of XML literal values.";
  rdfs:isDefinedBy <http://www.w3.org/1999/02/22-rdf-syntax-ns#>;
  rdfs:label "XMLLiteral";
  rdfs:subClassOf rdfs:Literal .

<http://www.w3.org/2002/07/owl> a owl:Ontology;
  dc:title "The OWL 2 Schema vocabulary (OWL 2)";
  rdfs:comment """
  This ontology partially describes the built-in classes and
  properties that together form the basis of the RDF/XML syntax of OWL 2.
  The content of this ontology is based on Tables 6.1 and 6.2
  in Section 6.4 of the OWL 2 RDF-Based Semantics specification,
  available at http://www.w3.org/TR/owl2-rdf-based-semantics/.
  Please note that those tables do not include the different annotations
  (labels, comments and rdfs:isDefinedBy links) used in this file.
  Also note that the descriptions provided in this ontology do not
  provide a complete and correct formal description of either the syntax
  or the semantics of the introduced terms (please see the OWL 2
  recommendations for the complete and normative specifications).
  Furthermore, the information provided by this ontology may be
  misleading if not used with care. This ontology SHOULD NOT be imported
  into OWL ontologies. Importing this file into an OWL 2 DL ontology
  will cause it to become an OWL 2 Full ontology and may have other,
  unexpected, consequences.
   """;
  rdfs:isDefinedBy <http://www.w3.org/TR/owl2-mapping-to-rdf/>, <http://www.w3.org/TR/owl2-rdf-based-semantics/>,
    <http://www.w3.org/TR/owl2-syntax/>;
  rdfs:seeAlso <http://www.w3.org/TR/owl2-rdf-based-semantics/#table-axiomatic-classes>,
    <http://www.w3.org/TR/owl2-rdf-based-semantics/#table-axiomatic-properties>;
  owl:imports <http://www.w3.org/2000/01/rdf-schema>;
  owl:versionIRI <http://www.w3.org/2002/07/owl>;
  owl:versionInfo "$Date: 2009/11/15 10:54:12 $";
  grddl:namespaceTransformation <http://dev.w3.org/cvsweb/2009/owl-grddl/owx2rdf.xsl> .

owl:AllDifferent a rdfs:Class;
  rdfs:comment "The class of collections of pairwise different individuals.";
  rdfs:isDefinedBy <http://www.w3.org/2002/07/owl#>;
  rdfs:label "AllDifferent";
  rdfs:subClassOf rdfs:Resource .

owl:AllDisjointClasses a rdfs:Class;
  rdfs:comment "The class of collections of pairwise disjoint classes.";
  rdfs:isDefinedBy <http://www.w3.org/2002/07/owl#>;
  rdfs:label "AllDisjointClasses";
  rdfs:subClassOf rdfs:Resource .

owl:AllDisjointProperties a rdfs:Class;
  rdfs:comment "The class of collections of pairwise disjoint properties.";
  rdfs:isDefinedBy <http://www.w3.org/2002/07/owl#>;
  rdfs:label "AllDisjointProperties";
  rdfs:subClassOf rdfs:Resource .

owl:Annotation a rdfs:Class;
  rdfs:comment "The class of annotated annotations for which the RDF serialization consists of an annotated subject, predicate and object.";
  rdfs:isDefinedBy <http://www.w3.org/2002/07/owl#>;
  rdfs:label "Annotation";
  rdfs:subClassOf rdfs:Resource .

owl:AnnotationProperty a rdfs:Class;
  rdfs:comment "The class of annotation properties.";
  rdfs:isDefinedBy <http://www.w3.org/2002/07/owl#>;
  rdfs:label "AnnotationProperty";
  rdfs:subClassOf rdf:Property .

owl:AsymmetricProperty a rdfs:Class;
  rdfs:comment "The class of asymmetric properties.";
  rdfs:isDefinedBy <http://www.w3.org/2002/07/owl#>;
  rdfs:label "AsymmetricProperty";
  rdfs:subClassOf owl:ObjectProperty .

owl:Axiom a rdfs:Class;
  rdfs:comment "The class of annotated axioms for which the RDF serialization consists of an annotated subject, predicate and object.";
  rdfs:isDefinedBy <http://www.w3.org/2002/07/owl#>;
  rdfs:label "Axiom";
  rdfs:subClassOf rdfs:Resource .

owl:Class a rdfs:Class;
  rdfs:comment "The class of OWL classes.";
  rdfs:isDefinedBy <http://www.w3.org/2002/07/owl#>;
  rdfs:label "Class";
  rdfs:subClassOf rdfs:Class .

owl:DataRange a rdfs:Class;
  rdfs:comment "The class of OWL data ranges, which are special kinds of datatypes. Note: The use of the IRI owl:DataRange has been deprecated as of OWL 2. The IRI rdfs:Datatype SHOULD be used instead.";
  rdfs:isDefinedBy <http://www.w3.org/2002/07/owl#>;
  rdfs:label "DataRange";
  rdfs:subClassOf rdfs:Datatype .

owl:DatatypeProperty a rdfs:Class;
  rdfs:comment "The class of data properties.";
  rdfs:isDefinedBy <http://www.w3.org/2002/07/owl#>;
  rdfs:label "DatatypeProperty";
  rdfs:subClassOf rdf:Property .

owl:DeprecatedClass a rdfs:Class;
  rdfs:comment "The class of deprecated classes.";
  rdfs:isDefinedBy <http://www.w3.org/2002/07/owl#>;
  rdfs:label "DeprecatedClass";
  rdfs:subClassOf rdfs:Class .

owl:DeprecatedProperty a rdfs:Class;
  rdfs:comment "The class of deprecated properties.";
  rdfs:isDefinedBy <http://www.w3.org/2002/07/owl#>;
  rdfs:label "DeprecatedProperty";
  rdfs:subClassOf rdf:Property .

owl:FunctionalProperty a rdfs:Class;
  rdfs:comment "The class of functional properties.";
  rdfs:isDefinedBy <http://www.w3.org/2002/07/owl#>;
  rdfs:label "FunctionalProperty";
  rdfs:subClassOf rdf:Property .

owl:InverseFunctionalProperty a rdfs:Class;
  rdfs:comment "The class of inverse-functional properties.";
  rdfs:isDefinedBy <http://www.w3.org/2002/07/owl#>;
  rdfs:label "InverseFunctionalProperty";
  rdfs:subClassOf owl:ObjectProperty .

owl:IrreflexiveProperty a rdfs:Class;
  rdfs:comment "The class of irreflexive properties.";
  rdfs:isDefinedBy <http://www.w3.org/2002/07/owl#>;
  rdfs:label "IrreflexiveProperty";
  rdfs:subClassOf owl:ObjectProperty .

owl:NamedIndividual a rdfs:Class;
  rdfs:comment "The class of named individuals.";
  rdfs:isDefinedBy <http://www.w3.org/2002/07/owl#>;
  rdfs:label "NamedIndividual";
  rdfs:subClassOf owl:Thing .

owl:NegativePropertyAssertion a rdfs:Class;
  rdfs:comment "The class of negative property assertions.";
  rdfs:isDefinedBy <http://www.w3.org/2002/07/owl#>;
  rdfs:label "NegativePropertyAssertion";
  rdfs:subClassOf rdfs:Resource .

owl:Nothing a owl:Class;
  rdfs:comment "This is the empty class.";
  rdfs:isDefinedBy <http://www.w3.org/2002/07/owl#>;
  rdfs:label "Nothing";
  rdfs:subClassOf owl:Thing .

owl:ObjectProperty a rdfs:Class;
  rdfs:comment "The class of object properties.";
  rdfs:isDefinedBy <http://www.w3.org/2002/07/owl#>;
  rdfs:label "ObjectProperty";
  rdfs:subClassOf rdf:Property .

owl:Ontology a rdfs:Class;
  rdfs:comment "The class of ontologies.";
  rdfs:isDefinedBy <http://www.w3.org/2002/07/owl#>;
  rdfs:label "Ontology";
  rdfs:subClassOf rdfs:Resource .

owl:OntologyProperty a rdfs:Class;
  rdfs:comment "The class of ontology properties.";
  rdfs:isDefinedBy <http://www.w3.org/2002/07/owl#>;
  rdfs:label "OntologyProperty";
  rdfs:subClassOf rdf:Property .

owl:ReflexiveProperty a rdfs:Class;
  rdfs:comment "The class of reflexive properties.";
  rdfs:isDefinedBy <http://www.w3.org/2002/07/owl#>;
  rdfs:label "ReflexiveProperty";
  rdfs:subClassOf owl:ObjectProperty .

owl:Restriction a rdfs:Class;
  rdfs:comment "The class of property restrictions.";
  rdfs:isDefinedBy <http://www.w3.org/2002/07/owl#>;
  rdfs:label "Restriction";
  rdfs:subClassOf owl:Class .

owl:SymmetricProperty a rdfs:Class;
  rdfs:comment "The class of symmetric properties.";
  rdfs:isDefinedBy <http://www.w3.org/2002/07/owl#>;
  rdfs:label "SymmetricProperty";
  rdfs:subClassOf owl:ObjectProperty .

owl:Thing a owl:Class;
  rdfs:comment "The class of OWL individuals.";
  rdfs:isDefinedBy <http://www.w3.org/2002/07/owl#>;
  rdfs:label "Thing" .

owl:TransitiveProperty a rdfs:Class;
  rdfs:comment "The class of transitive properties.";
  rdfs:isDefinedBy <http://www.w3.org/2002/07/owl#>;
  rdfs:label "TransitiveProperty";
  rdfs:subClassOf owl:ObjectProperty .

owl:allValuesFrom a rdf:Property;
  rdfs:comment "The property that determines the class that a universal property restriction refers to.";
  rdfs:domain owl:Restriction;
  rdfs:isDefinedBy <http://www.w3.org/2002/07/owl#>;
  rdfs:label "allValuesFrom";
  rdfs:range rdfs:Class .

owl:annotatedProperty a rdf:Property;
  rdfs:comment "The property that determines the predicate of an annotated axiom or annotated annotation.";
  rdfs:domain rdfs:Resource;
  rdfs:isDefinedBy <http://www.w3.org/2002/07/owl#>;
  rdfs:label "annotatedProperty";
  rdfs:range rdfs:Resource .

owl:annotatedSource a rdf:Property;
  rdfs:comment "The property that determines the subject of an annotated axiom or annotated annotation.";
  rdfs:domain rdfs:Resource;
  rdfs:isDefinedBy <http://www.w3.org/2002/07/owl#>;
  rdfs:label "annotatedSource";
  rdfs:range rdfs:Resource .

owl:annotatedTarget a rdf:Property;
  rdfs:comment "The property that determines the object of an annotated axiom or annotated annotation.";
  rdfs:domain rdfs:Resource;
  rdfs:isDefinedBy <http://www.w3.org/2002/07/owl#>;
  rdfs:label "annotatedTarget";
  rdfs:range rdfs:Resource .

owl:assertionProperty a rdf:Property;
  rdfs:comment "The property that determines the predicate of a negative property assertion.";
  rdfs:domain owl:NegativePropertyAssertion;
  rdfs:isDefinedBy <http://www.w3.org/2002/07/owl#>;
  rdfs:label "assertionProperty";
  rdfs:range rdf:Property .

owl:backwardCompatibleWith a owl:AnnotationProperty, owl:OntologyProperty;
  rdfs:comment "The annotation property that indicates that a given ontology is backward compatible with another ontology.";
  rdfs:domain owl:Ontology;
  rdfs:isDefinedBy <http://www.w3.org/2002/07/owl#>;
  rdfs:label "backwardCompatibleWith";
  rdfs:range owl:Ontology .

owl:bottomDataProperty a owl:DatatypeProperty;
  rdfs:comment "The data property that does not relate any individual to any data value.";
  rdfs:domain owl:Thing;
  rdfs:isDefinedBy <http://www.w3.org/2002/07/owl#>;
  rdfs:label "bottomDataProperty";
  rdfs:range rdfs:Literal .

owl:bottomObjectProperty a owl:ObjectProperty;
  rdfs:comment "The object property that does not relate any two individuals.";
  rdfs:domain owl:Thing;
  rdfs:isDefinedBy <http://www.w3.org/2002/07/owl#>;
  rdfs:label "bottomObjectProperty";
  rdfs:range owl:Thing .

owl:cardinality a rdf:Property;
  rdfs:comment "The property that determines the cardinality of an exact cardinality restriction.";
  rdfs:domain owl:Restriction;
  rdfs:isDefinedBy <http://www.w3.org/2002/07/owl#>;
  rdfs:label "cardinality";
  rdfs:range xsd:nonNegativeInteger .

owl:complementOf a rdf:Property;
  rdfs:comment "The property that determines that a given class is the complement of another class.";
  rdfs:domain owl:Class;
  rdfs:isDefinedBy <http://www.w3.org/2002/07/owl#>;
  rdfs:label "complementOf";
  rdfs:range owl:Class .

owl:datatypeComplementOf a rdf:Property;
  rdfs:comment "The property that determines that a given data range is the complement of another data range with respect to the data domain.";
  rdfs:domain rdfs:Datatype;
  rdfs:isDefinedBy <http://www.w3.org/2002/07/owl#>;
  rdfs:label "datatypeComplementOf";
  rdfs:range rdfs:Datatype .

owl:deprecated a owl:AnnotationProperty;
  rdfs:comment "The annotation property that indicates that a given entity has been deprecated.";
  rdfs:domain rdfs:Resource;
  rdfs:isDefinedBy <http://www.w3.org/2002/07/owl#>;
  rdfs:label "deprecated";
  rdfs:range rdfs:Resource .

owl:differentFrom a rdf:Property;
  rdfs:comment "The property that determines that two given individuals are different.";
  rdfs:domain owl:Thing;
  rdfs:isDefinedBy <http://www.w3.org/2002/07/owl#>;
  rdfs:label "differentFrom";
  rdfs:range owl:Thing .

owl:disjointUnionOf a rdf:Property;
  rdfs:comment "The property that determines that a given class is equivalent to the disjoint union of a collection of other classes.";
  rdfs:domain owl:Class;
  rdfs:isDefinedBy <http://www.w3.org/2002/07/owl#>;
  rdfs:label "disjointUnionOf";
  rdfs:range rdf:List .

owl:disjointWith a rdf:Property;
  rdfs:comment "The property that determines that two given classes are disjoint.";
  rdfs:domain owl:Class;
  rdfs:isDefinedBy <http://www.w3.org/2002/07/owl#>;
  rdfs:label "disjointWith";
  rdfs:range owl:Class .

owl:distinctMembers a rdf:Property;
  rdfs:comment "The property that determines the collection of pairwise different individuals in a owl:AllDifferent axiom.";
  rdfs:domain owl:AllDifferent;
  rdfs:isDefinedBy <http://www.w3.org/2002/07/owl#>;
  rdfs:label "distinctMembers";
  rdfs:range rdf:List .

owl:equivalentClass a rdf:Property;
  rdfs:comment "The property that determines that two given classes are equivalent, and that is used to specify datatype definitions.";
  rdfs:domain rdfs:Class;
  rdfs:isDefinedBy <http://www.w3.org/2002/07/owl#>;
  rdfs:label "equivalentClass";
  rdfs:range rdfs:Class .

owl:equivalentProperty a rdf:Property;
  rdfs:comment "The property that determines that two given properties are equivalent.";
  rdfs:domain rdf:Property;
  rdfs:isDefinedBy <http://www.w3.org/2002/07/owl#>;
  rdfs:label "equivalentProperty";
  rdfs:range rdf:Property .

owl:hasKey a rdf:Property;
  rdfs:comment "The property that determines the collection of properties that jointly build a key.";
  rdfs:domain owl:Class;
  rdfs:isDefinedBy <http://www.w3.org/2002/07/owl#>;
  rdfs:label "hasKey";
  rdfs:range rdf:List .

owl:hasSelf a rdf:Property;
  rdfs:comment "The property that determines the property that a self restriction refers to.";
  rdfs:domain owl:Restriction;
  rdfs:isDefinedBy <http://www.w3.org/2002/07/owl#>;
  rdfs:label "hasSelf";
  rdfs:range rdfs:Resource .

owl:hasValue a rdf:Property;
  rdfs:comment "The property that determines the individual that a has-value restriction refers to.";
  rdfs:domain owl:Restriction;
  rdfs:isDefinedBy <http://www.w3.org/2002/07/owl#>;
  rdfs:label "hasValue";
  rdfs:range rdfs:Resource .

owl:imports a owl:OntologyProperty;
  rdfs:comment "The property that is used for importing other ontologies into a given ontology.";
  rdfs:domain owl:Ontology;
  rdfs:isDefinedBy <http://www.w3.org/2002/07/owl#>;
  rdfs:label "imports";
  rdfs:range owl:Ontology .

owl:incompatibleWith a owl:AnnotationProperty, owl:OntologyProperty;
  rdfs:comment "The annotation property that indicates that a given ontology is incompatible with another ontology.";
  rdfs:domain owl:Ontology;
  rdfs:isDefinedBy <http://www.w3.org/2002/07/owl#>;
  rdfs:label "incompatibleWith";
  rdfs:range owl:Ontology .

owl:intersectionOf a rdf:Property;
  rdfs:comment "The property that determines the collection of classes or data ranges that build an intersection.";
  rdfs:domain rdfs:Class;
  rdfs:isDefinedBy <http://www.w3.org/2002/07/owl#>;
  rdfs:label "intersectionOf";
  rdfs:range rdf:List .

owl:inverseOf a rdf:Property;
  rdfs:comment "The property that determines that two given properties are inverse.";
  rdfs:domain owl:ObjectProperty;
  rdfs:isDefinedBy <http://www.w3.org/2002/07/owl#>;
  rdfs:label "inverseOf";
  rdfs:range owl:ObjectProperty .

owl:maxCardinality a rdf:Property;
  rdfs:comment "The property that determines the cardinality of a maximum cardinality restriction.";
  rdfs:domain owl:Restriction;
  rdfs:isDefinedBy <http://www.w3.org/2002/07/owl#>;
  rdfs:label "maxCardinality";
  rdfs:range xsd:nonNegativeInteger .

owl:maxQualifiedCardinality a rdf:Property;
  rdfs:comment "The property that determines the cardinality of a maximum qualified cardinality restriction.";
  rdfs:domain owl:Restriction;
  rdfs:isDefinedBy <http://www.w3.org/2002/07/owl#>;
  rdfs:label "maxQualifiedCardinality";
  rdfs:range xsd:nonNegativeInteger .

owl:members a rdf:Property;
  rdfs:comment "The property that determines the collection of members in either a owl:AllDifferent, owl:AllDisjointClasses or owl:AllDisjointProperties axiom.";
  rdfs:domain rdfs:Resource;
  rdfs:isDefinedBy <http://www.w3.org/2002/07/owl#>;
  rdfs:label "members";
  rdfs:range rdf:List .

owl:minCardinality a rdf:Property;
  rdfs:comment "The property that determines the cardinality of a minimum cardinality restriction.";
  rdfs:domain owl:Restriction;
  rdfs:isDefinedBy <http://www.w3.org/2002/07/owl#>;
  rdfs:label "minCardinality";
  rdfs:range xsd:nonNegativeInteger .

owl:minQualifiedCardinality a rdf:Property;
  rdfs:comment "The property that determines the cardinality of a minimum qualified cardinality restriction.";
  rdfs:domain owl:Restriction;
  rdfs:isDefinedBy <http://www.w3.org/2002/07/owl#>;
  rdfs:label "minQualifiedCardinality";
  rdfs:range xsd:nonNegativeInteger .

owl:onClass a rdf:Property;
  rdfs:comment "The property that determines the class that a qualified object cardinality restriction refers to.";
  rdfs:domain owl:Restriction;
  rdfs:isDefinedBy <http://www.w3.org/2002/07/owl#>;
  rdfs:label "onClass";
  rdfs:range owl:Class .

owl:onDataRange a rdf:Property;
  rdfs:comment "The property that determines the data range that a qualified data cardinality restriction refers to.";
  rdfs:domain owl:Restriction;
  rdfs:isDefinedBy <http://www.w3.org/2002/07/owl#>;
  rdfs:label "onDataRange";
  rdfs:range rdfs:Datatype .

owl:onDatatype a rdf:Property;
  rdfs:comment "The property that determines the datatype that a datatype restriction refers to.";
  rdfs:domain rdfs:Datatype;
  rdfs:isDefinedBy <http://www.w3.org/2002/07/owl#>;
  rdfs:label "onDatatype";
  rdfs:range rdfs:Datatype .

owl:oneOf a rdf:Property;
  rdfs:comment "The property that determines the collection of individuals or data values that build an enumeration.";
  rdfs:domain rdfs:Class;
  rdfs:isDefinedBy <http://www.w3.org/2002/07/owl#>;
  rdfs:label "oneOf";
  rdfs:range rdf:List .

owl:onProperties a rdf:Property;
  rdfs:comment "The property that determines the n-tuple of properties that a property restriction on an n-ary data range refers to.";
  rdfs:domain owl:Restriction;
  rdfs:isDefinedBy <http://www.w3.org/2002/07/owl#>;
  rdfs:label "onProperties";
  rdfs:range rdf:List .

owl:onProperty a rdf:Property;
  rdfs:comment "The property that determines the property that a property restriction refers to.";
  rdfs:domain owl:Restriction;
  rdfs:isDefinedBy <http://www.w3.org/2002/07/owl#>;
  rdfs:label "onProperty";
  rdfs:range rdf:Property .

owl:priorVersion a owl:AnnotationProperty, owl:OntologyProperty;
  rdfs:comment "The annotation property that indicates the predecessor ontology of a given ontology.";
  rdfs:domain owl:Ontology;
  rdfs:isDefinedBy <http://www.w3.org/2002/07/owl#>;
  rdfs:label "priorVersion";
  rdfs:range owl:Ontology .

owl:propertyChainAxiom a rdf:Property;
  rdfs:comment "The property that determines the n-tuple of properties that build a sub property chain of a given property.";
  rdfs:domain owl:ObjectProperty;
  rdfs:isDefinedBy <http://www.w3.org/2002/07/owl#>;
  rdfs:label "propertyChainAxiom";
  rdfs:range rdf:List .

owl:propertyDisjointWith a rdf:Property;
  rdfs:comment "The property that determines that two given properties are disjoint.";
  rdfs:domain rdf:Property;
  rdfs:isDefinedBy <http://www.w3.org/2002/07/owl#>;
  rdfs:label "propertyDisjointWith";
  rdfs:range rdf:Property .

owl:qualifiedCardinality a rdf:Property;
  rdfs:comment "The property that determines the cardinality of an exact qualified cardinality restriction.";
  rdfs:domain owl:Restriction;
  rdfs:isDefinedBy <http://www.w3.org/2002/07/owl#>;
  rdfs:label "qualifiedCardinality";
  rdfs:range xsd:nonNegativeInteger .

owl:sameAs a rdf:Property;
  rdfs:comment "The property that determines that two given individuals are equal.";
  rdfs:domain owl:Thing;
  rdfs:isDefinedBy <http://www.w3.org/2002/07/owl#>;
  rdfs:label "sameAs";
  rdfs:range owl:Thing .

owl:someValuesFrom a rdf:Property;
  rdfs:comment "The property that determines the class that an existential property restriction refers to.";
  rdfs:domain owl:Restriction;
  rdfs:isDefinedBy <http://www.w3.org/2002/07/owl#>;
  rdfs:label "someValuesFrom";
  rdfs:range rdfs:Class .

owl:sourceIndividual a rdf:Property;
  rdfs:comment "The property that determines the subject of a negative property assertion.";
  rdfs:domain owl:NegativePropertyAssertion;
  rdfs:isDefinedBy <http://www.w3.org/2002/07/owl#>;
  rdfs:label "sourceIndividual";
  rdfs:range owl:Thing .

owl:targetIndividual a rdf:Property;
  rdfs:comment "The property that determines the object of a negative object property assertion.";
  rdfs:domain owl:NegativePropertyAssertion;
  rdfs:isDefinedBy <http://www.w3.org/2002/07/owl#>;
  rdfs:label "targetIndividual";
  rdfs:range owl:Thing .

owl:targetValue a rdf:Property;
  rdfs:comment "The property that determines the value of a negative data property assertion.";
  rdfs:domain owl:NegativePropertyAssertion;
  rdfs:isDefinedBy <http://www.w3.org/2002/07/owl#>;
  rdfs:label "targetValue";
  rdfs:range rdfs:Literal .

owl:topDataProperty a owl:DatatypeProperty;
  rdfs:comment "The data property that relates every individual to every data value.";
  rdfs:domain owl:Thing;
  rdfs:isDefinedBy <http://www.w3.org/2002/07/owl#>;
  rdfs:label "topDataProperty";
  rdfs:range rdfs:Literal .

owl:topObjectProperty a owl:ObjectProperty;
  rdfs:comment "The object property that relates every two individuals.";
  rdfs:domain owl:Thing;
  rdfs:isDefinedBy <http://www.w3.org/2002/07/owl#>;
  rdfs:label "topObjectProperty";
  rdfs:range owl:Thing .

owl:unionOf a rdf:Property;
  rdfs:comment "The property that determines the collection of classes or data ranges that build a union.";
  rdfs:domain rdfs:Class;
  rdfs:isDefinedBy <http://www.w3.org/2002/07/owl#>;
  rdfs:label "unionOf";
  rdfs:range rdf:List .

owl:versionInfo a owl:AnnotationProperty;
  rdfs:comment "The annotation property that provides version information for an ontology or another OWL construct.";
  rdfs:domain rdfs:Resource;
  rdfs:isDefinedBy <http://www.w3.org/2002/07/owl#>;
  rdfs:label "versionInfo";
  rdfs:range rdfs:Resource .

owl:versionIRI a owl:OntologyProperty;
  rdfs:comment "The property that identifies the version IRI of an ontology.";
  rdfs:domain owl:Ontology;
  rdfs:isDefinedBy <http://www.w3.org/2002/07/owl#>;
  rdfs:label "versionIRI";
  rdfs:range owl:Ontology .

owl:withRestrictions a rdf:Property;
  rdfs:comment "The property that determines the collection of facet-value pairs that define a datatype restriction.";
  rdfs:domain rdfs:Datatype;
  rdfs:isDefinedBy <http://www.w3.org/2002/07/owl#>;
  rdfs:label "withRestrictions";
  rdfs:range rdf:List .

<http://www.w3.org/2000/01/rdf-schema#> a owl:Ontology;
  dc:title "The RDF Schema vocabulary (RDFS)";
  rdfs:seeAlso <http://www.w3.org/2000/01/rdf-schema-more> .

rdfs:Resource a rdfs:Class;
  rdfs:comment "The class resource, everything.";
  rdfs:isDefinedBy <http://www.w3.org/2000/01/rdf-schema#>;
  rdfs:label "Resource" .

rdfs:Class a rdfs:Class;
  rdfs:comment "The class of classes.";
  rdfs:isDefinedBy <http://www.w3.org/2000/01/rdf-schema#>;
  rdfs:label "Class";
  rdfs:subClassOf rdfs:Resource .

rdfs:subClassOf a rdf:Property;
  rdfs:comment "The subject is a subclass of a class.";
  rdfs:domain rdfs:Class;
  rdfs:isDefinedBy <http://www.w3.org/2000/01/rdf-schema#>;
  rdfs:label "subClassOf";
  rdfs:range rdfs:Class .

rdfs:subPropertyOf a rdf:Property;
  rdfs:comment "The subject is a subproperty of a property.";
  rdfs:domain rdf:Property;
  rdfs:isDefinedBy <http://www.w3.org/2000/01/rdf-schema#>;
  rdfs:label "subPropertyOf";
  rdfs:range rdf:Property .

rdfs:comment a rdf:Property;
  rdfs:comment "A description of the subject resource.";
  rdfs:domain rdfs:Resource;
  rdfs:isDefinedBy <http://www.w3.org/2000/01/rdf-schema#>;
  rdfs:label "comment";
  rdfs:range rdfs:Literal .

rdfs:label a rdf:Property;
  rdfs:comment "A human-readable name for the subject.";
  rdfs:domain rdfs:Resource;
  rdfs:isDefinedBy <http://www.w3.org/2000/01/rdf-schema#>;
  rdfs:label "label";
  rdfs:range rdfs:Literal .

rdfs:domain a rdf:Property;
  rdfs:comment "A domain of the subject property.";
  rdfs:domain rdf:Property;
  rdfs:isDefinedBy <http://www.w3.org/2000/01/rdf-schema#>;
  rdfs:label "domain";
  rdfs:range rdfs:Class .

rdfs:range a rdf:Property;
  rdfs:comment "A range of the subject property.";
  rdfs:domain rdf:Property;
  rdfs:isDefinedBy <http://www.w3.org/2000/01/rdf-schema#>;
  rdfs:label "range";
  rdfs:range rdfs:Class .

rdfs:seeAlso a rdf:Property;
  rdfs:comment "Further information about the subject resource.";
  rdfs:domain rdfs:Resource;
  rdfs:isDefinedBy <http://www.w3.org/2000/01/rdf-schema#>;
  rdfs:label "seeAlso";
  rdfs:range rdfs:Resource .

rdfs:isDefinedBy a rdf:Property;
  rdfs:comment "The defininition of the subject resource.";
  rdfs:domain rdfs:Resource;
  rdfs:isDefinedBy <http://www.w3.org/2000/01/rdf-schema#>;
  rdfs:label "isDefinedBy";
  rdfs:range rdfs:Resource;
  rdfs:subPropertyOf rdfs:seeAlso .

rdfs:Literal a rdfs:Class;
  rdfs:comment "The class of literal values, eg. textual strings and integers.";
  rdfs:isDefinedBy <http://www.w3.org/2000/01/rdf-schema#>;
  rdfs:label "Literal";
  rdfs:subClassOf rdfs:Resource .

rdfs:Container a rdfs:Class;
  rdfs:comment "The class of RDF containers.";
  rdfs:isDefinedBy <http://www.w3.org/2000/01/rdf-schema#>;
  rdfs:label "Container";
  rdfs:subClassOf rdfs:Resource .

rdfs:ContainerMembershipProperty a rdfs:Class;
  rdfs:comment """The class of container membership properties, rdf:_1, rdf:_2, ...,
                    all of which are sub-properties of 'member'.""";
  rdfs:isDefinedBy <http://www.w3.org/2000/01/rdf-schema#>;
  rdfs:label "ContainerMembershipProperty";
  rdfs:subClassOf rdf:Property .

rdfs:member a rdf:Property;
  rdfs:comment "A member of the subject resource.";
  rdfs:domain rdfs:Resource;
  rdfs:isDefinedBy <http://www.w3.org/2000/01/rdf-schema#>;
  rdfs:label "member";
  rdfs:range rdfs:Resource .

rdfs:Datatype a rdfs:Class;
  rdfs:comment "The class of RDF datatypes.";
  rdfs:isDefinedBy <http://www.w3.org/2000/01/rdf-schema#>;
  rdfs:label "Datatype";
  rdfs:subClassOf rdfs:Class .

<http://www.w3.org/2004/02/skos/core> a owl:Ontology;
  dct:contributor "Dave Beckett", "Nikki Rogers", "Participants in W3C's Semantic Web Deployment Working Group.";
  dct:creator "Alistair Miles", "Sean Bechhofer";
  dct:description "An RDF vocabulary for describing the basic structure and content of concept schemes such as thesauri, classification schemes, subject heading lists, taxonomies, 'folksonomies', other types of controlled vocabulary, and also concept schemes embedded in glossaries and terminologies."@en;
  dct:title "SKOS Vocabulary"@en;
  rdfs:seeAlso <http://www.w3.org/TR/skos-reference/> .

skos:Concept a owl:Class;
  rdfs:isDefinedBy <http://www.w3.org/2004/02/skos/core>;
  rdfs:label "Concept"@en;
  skos:definition "An idea or notion; a unit of thought."@en .

skos:ConceptScheme a owl:Class;
  rdfs:isDefinedBy <http://www.w3.org/2004/02/skos/core>;
  rdfs:label "Concept Scheme"@en;
  owl:disjointWith skos:Concept;
  skos:definition "A set of concepts, optionally including statements about semantic relationships between those concepts."@en;
  skos:example "Thesauri, classification schemes, subject heading lists, taxonomies, 'folksonomies', and other types of controlled vocabulary are all examples of concept schemes. Concept schemes are also embedded in glossaries and terminologies."@en;
  skos:scopeNote "A concept scheme may be defined to include concepts from different sources."@en .

skos:Collection a owl:Class;
  rdfs:isDefinedBy <http://www.w3.org/2004/02/skos/core>;
  rdfs:label "Collection"@en;
  owl:disjointWith skos:Concept, skos:ConceptScheme;
  skos:definition "A meaningful collection of concepts."@en;
  skos:scopeNote "Labelled collections can be used where you would like a set of concepts to be displayed under a 'node label' in the hierarchy."@en .

skos:OrderedCollection a owl:Class;
  rdfs:isDefinedBy <http://www.w3.org/2004/02/skos/core>;
  rdfs:label "Ordered Collection"@en;
  rdfs:subClassOf skos:Collection;
  skos:definition "An ordered collection of concepts, where both the grouping and the ordering are meaningful."@en;
  skos:scopeNote "Ordered collections can be used where you would like a set of concepts to be displayed in a specific order, and optionally under a 'node label'."@en .

skos:inScheme a rdf:Property, owl:ObjectProperty;
  rdfs:isDefinedBy <http://www.w3.org/2004/02/skos/core>;
  rdfs:label "is in scheme"@en;
  rdfs:range skos:ConceptScheme;
  skos:definition "Relates a resource (for example a concept) to a concept scheme in which it is included."@en;
  skos:scopeNote "A concept may be a member of more than one concept scheme."@en .

skos:hasTopConcept a rdf:Property, owl:ObjectProperty;
  rdfs:domain skos:ConceptScheme;
  rdfs:isDefinedBy <http://www.w3.org/2004/02/skos/core>;
  rdfs:label "has top concept"@en;
  rdfs:range skos:Concept;
  owl:inverseOf skos:topConceptOf;
  skos:definition "Relates, by convention, a concept scheme to a concept which is topmost in the broader/narrower concept hierarchies for that scheme, providing an entry point to these hierarchies."@en .

skos:topConceptOf a rdf:Property, owl:ObjectProperty;
  rdfs:domain skos:Concept;
  rdfs:isDefinedBy <http://www.w3.org/2004/02/skos/core>;
  rdfs:label "is top concept in scheme"@en;
  rdfs:range skos:ConceptScheme;
  rdfs:subPropertyOf skos:inScheme;
  owl:inverseOf skos:hasTopConcept;
  skos:definition "Relates a concept to the concept scheme that it is a top level concept of."@en .

skos:prefLabel a rdf:Property, owl:AnnotationProperty;
  rdfs:comment "A resource has no more than one value of skos:prefLabel per language tag, and no more than one value of skos:prefLabel without language tag."@en,
    "The range of skos:prefLabel is the class of RDF plain literals."@en, """skos:prefLabel, skos:altLabel and skos:hiddenLabel are pairwise
      disjoint properties."""@en;
  rdfs:isDefinedBy <http://www.w3.org/2004/02/skos/core>;
  rdfs:label "preferred label"@en;
  rdfs:subPropertyOf rdfs:label;
  skos:definition "The preferred lexical label for a resource, in a given language."@en .

skos:altLabel a rdf:Property, owl:AnnotationProperty;
  rdfs:comment "The range of skos:altLabel is the class of RDF plain literals."@en,
    "skos:prefLabel, skos:altLabel and skos:hiddenLabel are pairwise disjoint properties."@en;
  rdfs:isDefinedBy <http://www.w3.org/2004/02/skos/core>;
  rdfs:label "alternative label"@en;
  rdfs:subPropertyOf rdfs:label;
  skos:definition "An alternative lexical label for a resource."@en;
  skos:example "Acronyms, abbreviations, spelling variants, and irregular plural/singular forms may be included among the alternative labels for a concept. Mis-spelled terms are normally included as hidden labels (see skos:hiddenLabel)."@en .

skos:hiddenLabel a rdf:Property, owl:AnnotationProperty;
  rdfs:comment "The range of skos:hiddenLabel is the class of RDF plain literals."@en,
    "skos:prefLabel, skos:altLabel and skos:hiddenLabel are pairwise disjoint properties."@en;
  rdfs:isDefinedBy <http://www.w3.org/2004/02/skos/core>;
  rdfs:label "hidden label"@en;
  rdfs:subPropertyOf rdfs:label;
  skos:definition "A lexical label for a resource that should be hidden when generating visual displays of the resource, but should still be accessible to free text search operations."@en .

skos:notation a rdf:Property, owl:DatatypeProperty;
  rdfs:isDefinedBy <http://www.w3.org/2004/02/skos/core>;
  rdfs:label "notation"@en;
  skos:definition "A notation, also known as classification code, is a string of characters such as \"T58.5\" or \"303.4833\" used to uniquely identify a concept within the scope of a given concept scheme."@en;
  skos:scopeNote "By convention, skos:notation is used with a typed literal in the object position of the triple."@en .

skos:note a rdf:Property, owl:AnnotationProperty;
  rdfs:isDefinedBy <http://www.w3.org/2004/02/skos/core>;
  rdfs:label "note"@en;
  skos:definition "A general note, for any purpose."@en;
  skos:scopeNote "This property may be used directly, or as a super-property for more specific note types."@en .

skos:changeNote a rdf:Property, owl:AnnotationProperty;
  rdfs:isDefinedBy <http://www.w3.org/2004/02/skos/core>;
  rdfs:label "change note"@en;
  rdfs:subPropertyOf skos:note;
  skos:definition "A note about a modification to a concept."@en .

skos:definition a rdf:Property, owl:AnnotationProperty;
  rdfs:isDefinedBy <http://www.w3.org/2004/02/skos/core>;
  rdfs:label "definition"@en;
  rdfs:subPropertyOf skos:note;
  skos:definition "A statement or formal explanation of the meaning of a concept."@en .

skos:editorialNote a rdf:Property, owl:AnnotationProperty;
  rdfs:isDefinedBy <http://www.w3.org/2004/02/skos/core>;
  rdfs:label "editorial note"@en;
  rdfs:subPropertyOf skos:note;
  skos:definition "A note for an editor, translator or maintainer of the vocabulary."@en .

skos:example a rdf:Property, owl:AnnotationProperty;
  rdfs:isDefinedBy <http://www.w3.org/2004/02/skos/core>;
  rdfs:label "example"@en;
  rdfs:subPropertyOf skos:note;
  skos:definition "An example of the use of a concept."@en .

skos:historyNote a rdf:Property, owl:AnnotationProperty;
  rdfs:isDefinedBy <http://www.w3.org/2004/02/skos/core>;
  rdfs:label "history note"@en;
  rdfs:subPropertyOf skos:note;
  skos:definition "A note about the past state/use/meaning of a concept."@en .

skos:scopeNote a rdf:Property, owl:AnnotationProperty;
  rdfs:isDefinedBy <http://www.w3.org/2004/02/skos/core>;
  rdfs:label "scope note"@en;
  rdfs:subPropertyOf skos:note;
  skos:definition "A note that helps to clarify the meaning and/or the use of a concept."@en .

skos:semanticRelation a rdf:Property, owl:ObjectProperty;
  rdfs:domain skos:Concept;
  rdfs:isDefinedBy <http://www.w3.org/2004/02/skos/core>;
  rdfs:label "is in semantic relation with"@en;
  rdfs:range skos:Concept;
  skos:definition "Links a concept to a concept related by meaning."@en;
  skos:scopeNote "This property should not be used directly, but as a super-property for all properties denoting a relationship of meaning between concepts."@en .

skos:broader a rdf:Property, owl:ObjectProperty;
  rdfs:comment "Broader concepts are typically rendered as parents in a concept hierarchy (tree)."@en;
  rdfs:isDefinedBy <http://www.w3.org/2004/02/skos/core>;
  rdfs:label "has broader"@en;
  rdfs:subPropertyOf skos:broaderTransitive;
  owl:inverseOf skos:narrower;
  skos:definition "Relates a concept to a concept that is more general in meaning."@en;
  skos:scopeNote "By convention, skos:broader is only used to assert an immediate (i.e. direct) hierarchical link between two conceptual resources."@en .

skos:narrower a rdf:Property, owl:ObjectProperty;
  rdfs:comment "Narrower concepts are typically rendered as children in a concept hierarchy (tree)."@en;
  rdfs:isDefinedBy <http://www.w3.org/2004/02/skos/core>;
  rdfs:label "has narrower"@en;
  rdfs:subPropertyOf skos:narrowerTransitive;
  owl:inverseOf skos:broader;
  skos:definition "Relates a concept to a concept that is more specific in meaning."@en;
  skos:scopeNote "By convention, skos:broader is only used to assert an immediate (i.e. direct) hierarchical link between two conceptual resources."@en .

skos:related a rdf:Property, owl:ObjectProperty, owl:SymmetricProperty;
  rdfs:comment "skos:related is disjoint with skos:broaderTransitive"@en;
  rdfs:isDefinedBy <http://www.w3.org/2004/02/skos/core>;
  rdfs:label "has related"@en;
  rdfs:subPropertyOf skos:semanticRelation;
  skos:definition "Relates a concept to a concept with which there is an associative semantic relationship."@en .

skos:broaderTransitive a rdf:Property, owl:ObjectProperty, owl:TransitiveProperty;
  rdfs:isDefinedBy <http://www.w3.org/2004/02/skos/core>;
  rdfs:label "has broader transitive"@en;
  rdfs:subPropertyOf skos:semanticRelation;
  owl:inverseOf skos:narrowerTransitive;
  skos:definition "skos:broaderTransitive is a transitive superproperty of skos:broader.";
  skos:scopeNote "By convention, skos:broaderTransitive is not used to make assertions. Rather, the properties can be used to draw inferences about the transitive closure of the hierarchical relation, which is useful e.g. when implementing a simple query expansion algorithm in a search application."@en .

skos:narrowerTransitive a rdf:Property, owl:ObjectProperty, owl:TransitiveProperty;
  rdfs:isDefinedBy <http://www.w3.org/2004/02/skos/core>;
  rdfs:label "has narrower transitive"@en;
  rdfs:subPropertyOf skos:semanticRelation;
  owl:inverseOf skos:broaderTransitive;
  skos:definition "skos:narrowerTransitive is a transitive superproperty of skos:narrower.";
  skos:scopeNote "By convention, skos:narrowerTransitive is not used to make assertions. Rather, the properties can be used to draw inferences about the transitive closure of the hierarchical relation, which is useful e.g. when implementing a simple query expansion algorithm in a search application."@en .

skos:member a rdf:Property, owl:ObjectProperty;
  rdfs:domain skos:Collection;
  rdfs:isDefinedBy <http://www.w3.org/2004/02/skos/core>;
  rdfs:label "has member"@en;
  rdfs:range _:node1dm3s2690x1 .

_:node1dm3s2690x1 a owl:Class;
  owl:unionOf _:node1dm3s2690x2 .

_:node1dm3s2690x2 rdf:first skos:Concept;
  rdf:rest _:node1dm3s2690x3 .

_:node1dm3s2690x3 rdf:first skos:Collection;
  rdf:rest rdf:nil .

skos:member skos:definition "Relates a collection to one of its members."@en .

skos:memberList a rdf:Property, owl:FunctionalProperty, owl:ObjectProperty;
  rdfs:comment """For any resource, every item in the list given as the value of the
      skos:memberList property is also a value of the skos:member property."""@en;
  rdfs:domain skos:OrderedCollection;
  rdfs:isDefinedBy <http://www.w3.org/2004/02/skos/core>;
  rdfs:label "has member list"@en;
  rdfs:range rdf:List;
  skos:definition "Relates an ordered collection to the RDF list containing its members."@en .

skos:mappingRelation a rdf:Property, owl:ObjectProperty;
  rdfs:comment "These concept mapping relations mirror semantic relations, and the data model defined below is similar (with the exception of skos:exactMatch) to the data model defined for semantic relations. A distinct vocabulary is provided for concept mapping relations, to provide a convenient way to differentiate links within a concept scheme from links between concept schemes. However, this pattern of usage is not a formal requirement of the SKOS data model, and relies on informal definitions of best practice."@en;
  rdfs:isDefinedBy <http://www.w3.org/2004/02/skos/core>;
  rdfs:label "is in mapping relation with"@en;
  rdfs:subPropertyOf skos:semanticRelation;
  skos:definition "Relates two concepts coming, by convention, from different schemes, and that have comparable meanings"@en .

skos:broadMatch a rdf:Property, owl:ObjectProperty;
  rdfs:isDefinedBy <http://www.w3.org/2004/02/skos/core>;
  rdfs:label "has broader match"@en;
  rdfs:subPropertyOf skos:broader, skos:mappingRelation;
  owl:inverseOf skos:narrowMatch;
  skos:definition "skos:broadMatch is used to state a hierarchical mapping link between two conceptual resources in different concept schemes."@en .

skos:narrowMatch a rdf:Property, owl:ObjectProperty;
  rdfs:isDefinedBy <http://www.w3.org/2004/02/skos/core>;
  rdfs:label "has narrower match"@en;
  rdfs:subPropertyOf skos:mappingRelation, skos:narrower;
  owl:inverseOf skos:broadMatch;
  skos:definition "skos:narrowMatch is used to state a hierarchical mapping link between two conceptual resources in different concept schemes."@en .

skos:relatedMatch a rdf:Property, owl:ObjectProperty, owl:SymmetricProperty;
  rdfs:isDefinedBy <http://www.w3.org/2004/02/skos/core>;
  rdfs:label "has related match"@en;
  rdfs:subPropertyOf skos:mappingRelation, skos:related;
  skos:definition "skos:relatedMatch is used to state an associative mapping link between two conceptual resources in different concept schemes."@en .

skos:exactMatch a rdf:Property, owl:ObjectProperty, owl:SymmetricProperty, owl:TransitiveProperty;
  rdfs:comment "skos:exactMatch is disjoint with each of the properties skos:broadMatch and skos:relatedMatch."@en;
  rdfs:isDefinedBy <http://www.w3.org/2004/02/skos/core>;
  rdfs:label "has exact match"@en;
  rdfs:subPropertyOf skos:closeMatch;
  skos:definition "skos:exactMatch is used to link two concepts, indicating a high degree of confidence that the concepts can be used interchangeably across a wide range of information retrieval applications. skos:exactMatch is a transitive property, and is a sub-property of skos:closeMatch."@en .

skos:closeMatch a rdf:Property, owl:ObjectProperty, owl:SymmetricProperty;
  rdfs:isDefinedBy <http://www.w3.org/2004/02/skos/core>;
  rdfs:label "has close match"@en;
  rdfs:subPropertyOf skos:mappingRelation;
  skos:definition "skos:closeMatch is used to link two concepts that are sufficiently similar that they can be used interchangeably in some information retrieval applications. In order to avoid the possibility of \"compound errors\" when combining mappings across more than two concept schemes, skos:closeMatch is not declared to be a transitive property."@en .

:AL a skos:Concept .

<http://purl.org/iow/Glossary#> a owl:Ontology .

:Units dct:created "2019-09-18T19:59:11.407Z"^^xsd:dateTime;
  skos:inScheme :glos;
  skosxl:prefLabel :xl_en_9a48cf9b .

:Data a :Themes, skos:Concept .

:xl_en_b750a869 a skosxl:Label;
  dct:created "2019-09-16T16:34:42.863Z"^^xsd:dateTime;
  skosxl:literalForm "Organizations"@en .

:Organizations a owl:Class;
  dct:created "2019-09-16T16:08:23.725Z"^^xsd:dateTime;
  dct:modified "2019-09-16T16:34:42.863Z"^^xsd:dateTime;
  rdfs:subClassOf skos:Concept;
  skosxl:prefLabel :xl_en_b750a869 .

:Geospatial a skos:Concept;
  dct:created "2019-09-18T19:59:28.909Z"^^xsd:dateTime;
  skos:inScheme :glos;
  skosxl:prefLabel :xl_en_ffa0c1bf .

:c_8e256c3d skos:topConceptOf :epa-abg .

:c_3a974a14 skos:topConceptOf :epa-abg .

:xl_en_0437695c a skosxl:Label;
  dct:created "2019-09-16T14:47:31.864Z"^^xsd:dateTime;
  skosxl:literalForm "Term (Class)"@en .

:xl_en_9bdacb85 a skosxl:Label;
  dct:created "2019-09-16T14:44:43.356Z"^^xsd:dateTime;
  skosxl:literalForm "Organization (Class)"@en .

:xl_en_e695f7c9 a skosxl:Label;
  dct:created "2019-09-16T14:45:59.597Z"^^xsd:dateTime;
  skosxl:literalForm "Vocabulary (Class)"@en .

:USGS dct:modified "2019-09-18T18:01:13.100Z"^^xsd:dateTime .

:Themes a rdfs:Class, owl:Class;
  dct:created "2019-09-16T16:25:36.454Z"^^xsd:dateTime;
  rdfs:subClassOf skos:Concept .

:xl_en_820c2844 a skosxl:Label;
  dct:created "2019-09-16T16:29:34.981Z"^^xsd:dateTime;
  skosxl:literalForm "Theme"@en .

:Theme a skos:Concept;
  dct:created "2019-09-16T16:29:34.981Z"^^xsd:dateTime;
  skos:topConceptOf :glos;
  skosxl:prefLabel :xl_en_820c2844 .

:Organization a skos:Concept;
  dct:created "2019-09-16T16:29:03.323Z"^^xsd:dateTime;
  skosxl:prefLabel :xl_en_7d8b9e30 .

:Water_Use a :Themes, skos:Concept;
  dct:modified "2019-09-18T20:09:43.369Z"^^xsd:dateTime;
  skos:broader :Theme;
  skos:inScheme :glos;
  skosxl:literalForm "Water Use" .

:c_d0fa72e2 skos:topConceptOf :epa-abg .

:c_5d4cbc0a skos:topConceptOf :epa-abg .

:c_35edc6f7 skos:topConceptOf :epa-abg .

:c_75b4a3a0 skos:topConceptOf :epa-abg .

:c_bd7d9638 skos:topConceptOf :epa-abg .

:c_8def1e2e skos:topConceptOf :epa-abg .

:Infrastructure skos:inScheme :glos;
  skosxl:literalForm "Infrastructure" .

:xl_en_ffa0c1bf a skosxl:Label;
  dct:created "2019-09-18T19:59:28.909Z"^^xsd:dateTime;
  skosxl:literalForm "Geospatial"@en .

:xl_en_7d8b9e30 a skosxl:Label;
  dct:created "2019-09-16T16:29:03.323Z"^^xsd:dateTime;
  skosxl:literalForm "Organization"@en .

:Water_Quality a :Themes, skos:Concept;
  dct:modified "2019-09-18T20:09:20.085Z"^^xsd:dateTime;
  skos:broader :Theme;
  skos:inScheme :glos;
  skosxl:literalForm "Water Quality" .

:Ecology a :Themes, skos:Concept;
  dct:modified "2019-09-18T20:06:58.494Z"^^xsd:dateTime;
  skos:broader :Theme;
  skos:inScheme :glos;
  skosxl:literalForm "Ecology" .

:Hydrology a :Themes, skos:Concept;
  dct:modified "2019-09-18T20:07:09.741Z"^^xsd:dateTime;
  skos:broader :Theme;
  skos:inScheme :glos .

:c_f98834e6 skos:topConceptOf :epa-abg .

:c_17f6d6d9 skos:topConceptOf :epa-abg .

:c_37656125 skos:topConceptOf :epa-abg .

:c_56a11087 skos:topConceptOf :epa-abg .

:c_1da88ee3 skos:topConceptOf :epa-abg .

:c_24c2a3d7 skos:topConceptOf :epa-abg .

:xl_en_9a48cf9b a skosxl:Label;
  dct:created "2019-09-18T19:59:11.407Z"^^xsd:dateTime;
  skosxl:literalForm "Units"@en .

:c_79a78368 skos:topConceptOf :epa-abg .

:c_61777e73 skos:topConceptOf :epa-abg .

:c_fb2cf0cd skos:topConceptOf :epa-abg .

:c_c1291eab skos:topConceptOf :epa-abg .

:c_24cc3016 skos:topConceptOf :epa-abg .

:c_21006d83 skos:topConceptOf :epa-abg .

:c_5810681a skos:topConceptOf :epa-abg .

:Beneficial_Use a :Themes, skos:Concept;
  dct:created "2019-09-26T17:45:03.954Z"^^xsd:dateTime;
  dct:modified "2019-09-26T17:45:40.037Z"^^xsd:dateTime;
  skos:broader :Water_Use;
  skos:inScheme :glos;
  skosxl:prefLabel :xl_en_fc31e317 .

:usgs-wut a skos:ConceptScheme;
  skos:definition "The following terms have been used in one or more of the <a href=\"/science/mission-areas/water-resources/science/water-use-united-states?qt-science_center_objects=3#qt-science_center_objects\" target=\"_blank\">water-use publications</a>. The <a href=\"/mission-areas/water-resources/science/changes-water-use-categories?qt-science_center_objects=0#qt-science_center_objects\" target=\"_blank\">comparison of water-use categories over the history of these reports</a> may also help clarify the use of some of the terms.";
  skos:scopeNote :USGS .

:c_f5b5ce44 dct:modified "2019-10-01T18:57:12.009Z"^^xsd:dateTime;
  skos:related :c_d428b229 .

:Vocabularies a owl:Class;
  dct:created "2019-09-16T16:08:31.437Z"^^xsd:dateTime;
  rdfs:subClassOf skos:Concept .

:c_b176fb27 skos:topConceptOf :epa-abg .

:c_62d17e1d skos:topConceptOf :epa-abg .

:c_13cbbc62 skos:topConceptOf :epa-abg .

:c_651b42f6 dct:modified "2019-10-01T18:58:41.120Z"^^xsd:dateTime;
  skos:related :c_cf4d74ad .

:c_bc61313f dct:modified "2019-10-01T18:59:01.997Z"^^xsd:dateTime;
  skos:related :c_cf4d74ad .

:c_631994db dct:modified "2019-10-01T19:05:04.165Z"^^xsd:dateTime;
  skos:exactMatch :c_50848288 .

:Terms a owl:Class;
  dct:created "2019-09-16T16:10:08.087Z"^^xsd:dateTime;
  dct:modified "2019-09-16T16:24:08.763Z"^^xsd:dateTime;
  rdfs:subClassOf skos:Concept .

:c_b519ac68 skos:topConceptOf :epa-abg .

:c_cfba7d50 skos:topConceptOf :epa-abg .

:c_334faf2c skos:topConceptOf :epa-abg .

:c_8d3599bf skos:topConceptOf :epa-abg .

:c_b47d3731 skos:topConceptOf :epa-abg .

:c_5b685993 skos:topConceptOf :epa-abg .

:xl_en_fc31e317 a skosxl:Label;
  skosxl:literalForm "Beneficial Use"@en .

:Data dct:modified "2019-10-02T03:11:57.441Z"^^xsd:dateTime;
  skos:broader :Theme;
  skos:inScheme :glos;
  skosxl:prefLabel :xl_en_e481b456 .

:xl_en_e481b456 skosxl:literalForm "Data"@en .

:c_9929c59d skos:topConceptOf :epa-abg .

:c_dd843071 skos:topConceptOf :epa-abg .

:c_fceba1d7 skos:topConceptOf :epa-abg .

:c_bf04de70 skos:topConceptOf :epa-abg .

:c_ecad58cf skos:topConceptOf :epa-abg .

:c_9180b163 dct:modified "2019-10-01T19:05:34.861Z"^^xsd:dateTime;
  skos:related :c_f5b5ce44 .

:xl_en_9c1894ee a skosxl:Label;
  dct:created "2019-09-18T20:04:48.787Z"^^xsd:dateTime .

:Utilities skosxl:literalForm "Utilities (Water, Wastewater, Stormwater)" .

:xl_en_9cd64803 a skosxl:Label;
  dct:created "2019-09-18T20:05:15.293Z"^^xsd:dateTime;
  skosxl:literalForm "Data Sources"@en .

:Data_Sources a skos:Concept;
  dct:created "2019-09-18T20:05:15.293Z"^^xsd:dateTime;
  skos:broader :Data;
  skos:inScheme :glos;
  skosxl:prefLabel :xl_en_9cd64803 .

:c_d4c2baf8 dct:modified "2019-10-01T18:54:25.746Z"^^xsd:dateTime .

:xl_en_c0a86bab a skosxl:Label;
  dct:created "2019-09-18T20:06:58.494Z"^^xsd:dateTime;
  dct:modified "2019-10-02T03:13:40.518Z"^^xsd:dateTime;
  skosxl:literalForm "Environment and Ecology"@en .

:c_d2921141 skos:topConceptOf :epa-abg .

:Variables a skos:Concept;
  dct:created "2019-09-18T19:59:01.049Z"^^xsd:dateTime;
  skos:broader :Data;
  skos:inScheme :glos;
  skosxl:prefLabel :xl_en_16c04f2d .

:Units a skos:Concept;
  skos:broader :Data .

:Nonprofit a skos:Concept;
  dct:created "2019-09-16T18:57:47.921Z"^^xsd:dateTime;
  dct:modified "2019-09-18T18:01:13.100Z"^^xsd:dateTime;
  skos:broader :Organization;
  skos:inScheme :glos;
  skosxl:prefLabel :xl_en_f08196ef .

:c_4f14be71 skos:topConceptOf :epa-abg .

:c_c578ab81 skos:topConceptOf :epa-abg .

:c_fe1af19f skos:topConceptOf :epa-abg .

:c_5ddc6dcc skos:topConceptOf :epa-abg .

:c_a050c59f skos:topConceptOf :epa-abg .

:xl_en_16c04f2d a skosxl:Label;
  dct:created "2019-09-18T19:59:01.049Z"^^xsd:dateTime;
  skosxl:literalForm "Variables"@en .

:State_Government a skos:Concept;
  dct:created "2019-09-16T18:57:56.712Z"^^xsd:dateTime;
  dct:modified "2019-09-18T18:01:13.100Z"^^xsd:dateTime;
  skos:broader :Organization;
  skos:inScheme :glos;
  skosxl:prefLabel :xl_en_faef1fb0 .

:Infrastructure a :Themes, skos:Concept;
  dct:modified "2019-09-18T20:07:33.146Z"^^xsd:dateTime;
  skos:broader :Theme;
  skosxl:prefLabel :xl_en_3e2a20c6 .

:xl_en_f08196ef a skosxl:Label;
  dct:created "2019-09-16T18:57:47.921Z"^^xsd:dateTime;
  skosxl:literalForm "Nonprofit"@en .

:Federal_Government a skos:Concept;
  dct:created "2019-09-16T18:58:21.831Z"^^xsd:dateTime;
  dct:modified "2019-09-18T18:01:13.100Z"^^xsd:dateTime;
  skos:broader :Organization;
  skos:inScheme :glos;
  skosxl:prefLabel :xl_en_5d6a86de .

:xl_en_faef1fb0 a skosxl:Label;
  dct:created "2019-09-16T18:57:56.712Z"^^xsd:dateTime;
  dct:modified "2019-09-16T18:59:10.550Z"^^xsd:dateTime;
  skosxl:literalForm "State Government"@en .

:xl_en_5d6a86de a skosxl:Label;
  dct:created "2019-09-16T18:58:21.831Z"^^xsd:dateTime;
  skosxl:literalForm "Federal Government"@en .

:Private a skos:Concept;
  dct:created "2019-09-16T18:59:29.192Z"^^xsd:dateTime;
  dct:modified "2019-09-18T18:01:13.100Z"^^xsd:dateTime;
  skos:broader :Organization;
  skos:inScheme :glos;
  skosxl:prefLabel :xl_en_85806933 .

:xl_en_85806933 a skosxl:Label;
  dct:created "2019-09-16T18:59:29.192Z"^^xsd:dateTime;
  skosxl:literalForm "Private"@en .

:USGS a :Organizations, skos:Concept;
  dct:created "2019-09-16T19:19:39.152Z"^^xsd:dateTime;
  rdfs:isDefinedBy "https://www.usgs.gov/"^^rdf:HTML;
  skos:broader :Federal_Government;
  skos:inScheme :glos;
  skosxl:altLabel :xl_en_9eb3fdcd;
  skosxl:prefLabel :xl_en_a7f6496b .

:xl_en_a7f6496b a skosxl:Label;
  dct:created "2019-09-16T19:19:39.152Z"^^xsd:dateTime;
  skosxl:literalForm "United States Geological Survey"@en .

:Organization dct:modified "2019-09-18T18:01:13.100Z"^^xsd:dateTime;
  skos:inScheme :glos;
  skos:topConceptOf :glos .

:xl_en_9eb3fdcd a skosxl:Label;
  dct:created "2019-09-16T19:20:39.761Z"^^xsd:dateTime;
  skosxl:literalForm "USGS"@en .

:xl_en_22e0d72c a skosxl:Label;
  dct:created "2019-09-18T17:58:08.726Z"^^xsd:dateTime;
  skosxl:literalForm "Glossary"@en .

:glos a skos:ConceptScheme;
  dct:created "2019-09-18T17:58:08.726Z"^^xsd:dateTime;
  skosxl:prefLabel :xl_en_22e0d72c .

:usgs-wut dct:created "2019-09-18T18:00:15.429Z"^^xsd:dateTime;
  rdfs:isDefinedBy "https://www.usgs.gov/mission-areas/water-resources/science/water-use-terminology?qt-science_center_objects=0#qt-science_center_objects"^^rdf:HTML;
  skos:note "https://www.usgs.gov/mission-areas/water-resources/science/water-use-terminology?qt-science_center_objects=0#qt-science_center_objects"^^rdf:HTML;
  skosxl:prefLabel :xl_en_569bfac4 .

:xl_en_569bfac4 a skosxl:Label;
  dct:created "2019-09-18T18:00:15.429Z"^^xsd:dateTime;
  skosxl:literalForm "USGS Water Use Terminology"@en .

:Theme dct:modified "2019-09-18T18:01:13.100Z"^^xsd:dateTime;
  skos:inScheme :glos .

:Geospatial skos:broader :Data .

:Ecology skosxl:prefLabel :xl_en_c0a86bab .

:Hydrology skosxl:prefLabel :xl_en_2f731054 .

:xl_en_2f731054 a skosxl:Label;
  dct:created "2019-09-18T20:07:09.741Z"^^xsd:dateTime;
  skosxl:literalForm "Hydrology"@en .

:c_74745111 skos:topConceptOf :epa-abg .

:c_871c0928 skos:topConceptOf :epa-abg .

:c_d3a88eef skos:topConceptOf :epa-abg .

:c_91d53bd4 dct:modified "2019-10-01T17:49:23.918Z"^^xsd:dateTime;
  skos:exactMatch :c_a6ee839e .

:xl_en_3e2a20c6 a skosxl:Label;
  dct:created "2019-09-18T20:07:33.146Z"^^xsd:dateTime;
  skosxl:literalForm "Infrastructure"@en .

:c_afee82d5 skos:topConceptOf :epa-abg .

:c_92f02cd4 skos:topConceptOf :epa-abg .

:c_eecca9b8 skos:topConceptOf :epa-abg .

:c_88319145 skos:topConceptOf :epa-abg .

:c_1ff194d9 dct:modified "2019-10-01T19:07:02.439Z"^^xsd:dateTime;
  skos:related :c_5cc31c7e, :c_5e095931 .

:c_1c3d1b27 dct:modified "2019-10-01T18:53:37.124Z"^^xsd:dateTime;
  skos:related :c_333fbc4c .

:c_d4c2baf8 skos:related :c_a17e96f1 .

:xl_en_e481b456 a skosxl:Label;
  dct:created "2019-09-18T20:08:35.972Z"^^xsd:dateTime;
  dct:modified "2019-10-02T03:10:23.439Z"^^xsd:dateTime .

:c_62d4bfb6 skos:topConceptOf :epa-abg .

:Utilities a :Themes, skos:Concept;
  dct:modified "2019-10-02T05:09:39.967Z"^^xsd:dateTime;
  skos:broader :Theme;
  skos:inScheme :glos;
  skosxl:prefLabel :xl_en_9c1894ee .

:Water_Quality skosxl:prefLabel :xl_en_a0c8c04c .

:xl_en_a0c8c04c a skosxl:Label;
  dct:created "2019-09-18T20:09:20.085Z"^^xsd:dateTime;
  skosxl:literalForm "Water Quality"@en .

:xl_en_9c1894ee skosxl:literalForm "Utilities (Water, Wastewater, Stormwater)"@en .

:Water_Use skosxl:prefLabel :xl_en_a575652a .

:xl_en_a575652a a skosxl:Label;
  dct:created "2019-09-18T20:09:43.369Z"^^xsd:dateTime;
  skosxl:literalForm "Water Use"@en .

:EPA a :Organizations, skos:Concept;
  dct:created "2019-09-18T21:34:05.518Z"^^xsd:dateTime;
  dct:modified "2019-09-19T05:25:45.681Z"^^xsd:dateTime;
  skos:broader :Federal_Government;
  skos:definition "An independent federal agency, created in 1970, that sets and enforces rules and standards that protect the environment and control pollution."@en;
  skos:inScheme :glos;
  skos:note "https://www.epa.gov"^^rdf:HTML;
  skosxl:altLabel :xl_en_66d3b2f9;
  skosxl:prefLabel :xl_en_81bf407b .

:xl_en_81bf407b a skosxl:Label;
  dct:created "2019-09-18T21:34:05.518Z"^^xsd:dateTime;
  skosxl:literalForm "Environmental Protection Agency"@en .

:xl_en_66d3b2f9 a skosxl:Label;
  dct:created "2019-09-18T21:42:23.211Z"^^xsd:dateTime;
  skosxl:literalForm "EPA"@en .

:epa-abg a skos:ConceptScheme;
  dct:created "2019-09-18T22:05:57.724Z"^^xsd:dateTime;
  dct:modified "2019-09-18T22:34:56.535Z"^^xsd:dateTime;
  skos:definition "A glossary of terms used for aquatic biodiversity "@en;
  skos:note "https://ofmpub.epa.gov/sor_internet/registry/termreg/searchandretrieve/glossariesandkeywordlists/search.do?details&glossaryName=Aquatic+Biodiversity+Glossary"^^rdf:HTML;
  skos:scopeNote :EPA;
  skosxl:prefLabel :xl_en_4a969c94 .

:xl_en_4a969c94 a skosxl:Label;
  dct:created "2019-09-18T22:05:57.724Z"^^xsd:dateTime;
  skosxl:literalForm "EPA Aquatic Biodiversity Glossary"@en .

:c_ced4b01e a :Terms;
  skos:broader :Ecology, :Water_Quality;
  skos:definition "Response by an animal that enables it to tolerate a change in a single factor (e.g. temperature) in its environment. "@en;
  skos:inScheme :epa-abg;
  skosxl:prefLabel :xl_en_23c2af31 .

:xl_en_23c2af31 a skosxl:Label;
  skosxl:literalForm "Acclimation"@en .

:c_28a146be a :Terms;
  skos:broader :Ecology, :Water_Quality;
  skos:definition "A complex chemical and atmospheric phenomenon that occurs when emissions of sulfur and nitrogen compounds and other substances are transformed by chemical processes in the atmosphere, often far from the original sources, and then deposited on earth in either wet or dry form. The wet forms, popularly called \"acid rain\", can fall as rain, snow, or fog. The dry forms are acidic gases or particulates. "@en;
  skos:inScheme :epa-abg;
  skosxl:prefLabel :xl_en_9cab5dcc .

:xl_en_9cab5dcc a skosxl:Label;
  skosxl:literalForm "Acid Deposition"@en .

:c_12032ab6 a :Terms;
  skos:broader :Ecology, :Water_Quality;
  skos:definition "Drainage of water from areas that have been mined for coal of other mineral ores. The water has a low pH because of its contact with sulfur-bearing material and is harmful to aquatic organisms. "@en;
  skos:inScheme :epa-abg;
  skosxl:prefLabel :xl_en_f3b94ed2 .

:xl_en_f3b94ed2 a skosxl:Label;
  skosxl:literalForm "Acid Mine Drainage"@en .

:c_d2baf0fd a :Terms;
  skos:broader :Ecology, :Water_Quality;
  skos:definition "Adjustments made by animals in respect of their environments. The adjustments may occur by natural selection, as individuals with favorable genetically acquired traits breed more prolifically than those lacking these traits (genotypic adaptation), or they may involve non-genetic changes in individuals, such as physiological modification (e.g. acclimatization) or behavioral changes (phenotypic adaptation). "@en;
  skos:inScheme :epa-abg;
  skosxl:prefLabel :xl_en_10a059cf .

:xl_en_10a059cf a skosxl:Label;
  skosxl:literalForm "Adaptation"@en .

:c_5a1e1954 a :Terms;
  skos:broader :Ecology, :Water_Quality;
  skos:definition "Any treatment of sewage that goes beyond the secondary or biological water treatment stage and includes the removal of nutrients such as phosphorus and nitrogen and a high percentage of suspended solids. "@en;
  skos:inScheme :epa-abg;
  skosxl:prefLabel :xl_en_367b20f1 .

:xl_en_367b20f1 a skosxl:Label;
  skosxl:literalForm "Advanced Wastewater Treatment"@en .

:c_2f897ccc a :Terms;
  skos:broader :Ecology, :Water_Quality;
  skos:definition "Life or processes that can occur only in the presence of oxygen. "@en;
  skos:inScheme :epa-abg;
  skosxl:prefLabel :xl_en_a161e5b0 .

:xl_en_a161e5b0 a skosxl:Label;
  skosxl:literalForm "Aerobic"@en .

:c_ee107987 a :Terms;
  skos:broader :Ecology, :Water_Quality;
  skos:definition "The liquid and solid wastes from all types of farming, including runoff from pesticides, fertilizers and feedlots; erosion and dust from plowing, animal manure and carcasses and crop residues and debris. "@en;
  skos:inScheme :epa-abg;
  skosxl:prefLabel :xl_en_5477325d .

:xl_en_5477325d a skosxl:Label;
  skosxl:literalForm "Agricultural Pollution"@en .

:c_3d964577 a :Terms;
  skos:broader :Ecology, :Water_Quality;
  skos:definition "Simple rootless plants that grow in sunlit waters in proportion to the amount of available nutrients. They can affect water quality adversely by lowering the dissolved oxygen in the water. They are food for fish and small aquatic animals. "@en;
  skos:inScheme :epa-abg;
  skosxl:prefLabel :xl_en_3cb53d78 .

:xl_en_3cb53d78 a skosxl:Label;
  skosxl:literalForm "Algae"@en .

:c_773b7b6c a :Terms;
  skos:broader :Ecology, :Water_Quality;
  skos:definition "An episode of excessive nutrient content in a river, stream or lake, which causes a proliferation of living algae. The end result is a depletion of much needed oxygen in the water. Excessive algae blooms can lead to the death of the fish and aquatic organisms of the given waterbody through oxygen deprivation called a \"fish kill\". "@en;
  skos:inScheme :epa-abg;
  skosxl:prefLabel :xl_en_2135cdae .

:xl_en_2135cdae a skosxl:Label;
  skosxl:literalForm "Algal Bloom"@en .

:c_48ea95f3 a :Terms;
  skos:broader :Ecology, :Water_Quality;
  skos:definition "The condition of water or soil that contains a sufficient amount of alkali substance to raise the pH above 7.0. "@en;
  skos:inScheme :epa-abg;
  skosxl:prefLabel :xl_en_2df4e481 .

:xl_en_2df4e481 a skosxl:Label;
  skosxl:literalForm "Alkaline"@en .

:c_99baa24b a :Terms;
  skos:broader :Ecology, :Water_Quality;
  skos:definition "The capacity of water to neutralize acids. "@en;
  skos:inScheme :epa-abg;
  skosxl:prefLabel :xl_en_0e12db7e .

:xl_en_0e12db7e a skosxl:Label;
  skosxl:literalForm "Alkalinity"@en .

:c_53de4e31 a :Terms;
  skos:broader :Ecology, :Water_Quality;
  skos:definition "Life or processes that occur in the absence of oxygen. "@en;
  skos:inScheme :epa-abg;
  skosxl:prefLabel :xl_en_59547980 .

:xl_en_59547980 a skosxl:Label;
  skosxl:literalForm "Anaerobic"@en .

:c_06bb3cf2 a :Terms;
  skos:broader :Ecology, :Water_Quality;
  skos:definition "An organism group of interacting populations in a given waterbody, for example, fish assemblage or a benthic macroinvertebrate assemblage. "@en;
  skos:inScheme :epa-abg;
  skosxl:prefLabel :xl_en_cd64569a .

:xl_en_cd64569a a skosxl:Label;
  skosxl:literalForm "Aquatic Assemblage"@en .

:c_0d6ff9cd a :Terms;
  skos:broader :Ecology, :Water_Quality;
  skos:definition "Collective term describing the organisms living in or depending on the aquatic environment. "@en;
  skos:inScheme :epa-abg;
  skosxl:prefLabel :xl_en_65b59140 .

:xl_en_65b59140 a skosxl:Label;
  skosxl:literalForm "Aquatic Biota"@en .

:c_f33909f1 a :Terms;
  skos:broader :Ecology, :Water_Quality;
  skos:definition "Association of interacting assemblages in a given waterbody, the biotic component of an ecosystem. "@en;
  skos:inScheme :epa-abg;
  skosxl:prefLabel :xl_en_631fce70 .

:xl_en_631fce70 a skosxl:Label;
  skosxl:literalForm "Aquatic Community"@en .

:c_0a03c69e a :Terms;
  skos:broader :Ecology, :Water_Quality;
  skos:definition "A beneficial use designation in which the waterbody provides suitable habitat for survival and reproduction of desirable fish, shellfish, and other aquatic organisms. "@en;
  skos:inScheme :epa-abg;
  skosxl:prefLabel :xl_en_1fc7b31e .

:xl_en_1fc7b31e a skosxl:Label;
  skosxl:literalForm "Aquatic Life Use"@en .

:c_3a50aaaf a :Terms;
  skos:broader :Ecology, :Water_Quality;
  skos:definition "Plants that grow in water either floating on the surface, growing up from the bottom of the body of water or growing under the surface of the water. "@en;
  skos:inScheme :epa-abg;
  skosxl:prefLabel :xl_en_1114757a .

:xl_en_1114757a a skosxl:Label;
  skosxl:literalForm "Aquatic Plants"@en .

:c_5f11be9d a :Terms;
  skos:broader :Ecology, :Water_Quality;
  skos:definition "An underground bed or stratum of earth, gravel or porous stone that contains water. "@en;
  skos:inScheme :epa-abg;
  skosxl:prefLabel :xl_en_77bf27d0 .

:xl_en_77bf27d0 a skosxl:Label;
  skosxl:literalForm "Aquifer"@en .

:c_f563ac9c a :Terms;
  skos:broader :Ecology, :Water_Quality;
  skos:definition "A measurable component of a biological system. "@en;
  skos:inScheme :epa-abg;
  skosxl:prefLabel :xl_en_90147493 .

:xl_en_90147493 a skosxl:Label;
  skosxl:literalForm "Attribute"@en .

:c_dfdea833 a :Terms;
  skos:broader :Ecology, :Water_Quality;
  skos:definition "Single-celled microorganisms that lack chlorophyll. Some bacteria are capable of causing human, animal or plant diseases, others are essential in pollution control because they break down organic matter in the air and water. "@en;
  skos:inScheme :epa-abg;
  skosxl:prefLabel :xl_en_fe837a8c .

:xl_en_fe837a8c a skosxl:Label;
  skosxl:literalForm "Bacteria"@en .

:c_ccce6454 a :Terms;
  skos:broader :Ecology, :Water_Quality;
  skos:definition "rm: Benthos "@en;
  skos:inScheme :epa-abg;
  skosxl:prefLabel :xl_en_c8f52fc1 .

:xl_en_c8f52fc1 a skosxl:Label;
  skosxl:literalForm "Benthic Marcroinvertebrates"@en .

:c_5d486d0b a :Terms;
  skos:broader :Ecology, :Water_Quality;
  skos:definition "The bottom of a body of water. This region supports the benthos, a type of life that not only lives upon, but also contributes to the character of the bottom. "@en;
  skos:inScheme :epa-abg;
  skosxl:prefLabel :xl_en_cc47c46e .

:xl_en_cc47c46e a skosxl:Label;
  skosxl:literalForm "Benthic Region"@en .

:c_9c396253 a :Terms;
  skos:broader :Ecology, :Water_Quality;
  skos:definition "The name used to describe the plants and animals (without backbones) living in the streambed or benthic zone, a size large enough to be seen by the unaided eye, and which can be retained by a U.S. Standard No. 30 sieve (28 openings/inch, 0.595-mm openings). Also referred to as bentic macroinvertebrates, infauna, or macrobenthos. "@en;
  skos:inScheme :epa-abg;
  skosxl:prefLabel :xl_en_0caf1978 .

:xl_en_0caf1978 a skosxl:Label;
  skosxl:literalForm "Benthos"@en .

:c_817edf3c a :Terms;
  skos:broader :Ecology, :Water_Quality;
  skos:definition """Methods that have been determined to be the most effective, practical means of preventing or reducing pollution from nonpoint sources. 
Acronym: BMP """@en;
  skos:inScheme :epa-abg;
  skosxl:altLabel :xl_en_5708b360;
  skosxl:prefLabel :xl_en_afe9df53 .

:xl_en_afe9df53 a skosxl:Label;
  skosxl:literalForm "Best Management Practice"@en .

:xl_en_5708b360 a skosxl:Label;
  skosxl:literalForm "BMP"@en .

:c_d1f703d0 a :Terms;
  skos:broader :Ecology, :Water_Quality;
  skos:definition "Substances that increase in concentration in living organisms as they take in contaminated air, water, or food because the substances are very slowly metabolized or excreted. "@en;
  skos:inScheme :epa-abg;
  skosxl:prefLabel :xl_en_6618e9dd .

:xl_en_6618e9dd a skosxl:Label;
  skosxl:literalForm "Bioaccumulants"@en .

:c_ac554243 a :Terms;
  skos:broader :Ecology, :Water_Quality;
  skos:definition "Evaluation of the biological condition of a waterbody using biological surveys and other direct measurements of resident biota in surface waters. "@en;
  skos:inScheme :epa-abg;
  skosxl:prefLabel :xl_en_eea5c064 .

:xl_en_eea5c064 a skosxl:Label;
  skosxl:literalForm "Bioassessments"@en .

:c_d0a5258b a :Terms;
  skos:broader :Ecology, :Water_Quality;
  skos:definition "Degree to which chemicals can be taken up by organisms. "@en;
  skos:inScheme :epa-abg;
  skosxl:prefLabel :xl_en_65ab53c2 .

:xl_en_65ab53c2 a skosxl:Label;
  skosxl:literalForm "Bioavailability"@en .

:c_c5fe43e8 a :Terms;
  skos:broader :Ecology, :Water_Quality;
  skos:definition """A measure of the amount of oxygen consumed in the biological processes that break down organic matter in water. The greater the BOD, the greater the degree of pollution. 
Acronym: BOD """@en;
  skos:inScheme :epa-abg;
  skosxl:altLabel :xl_en_cca67e04;
  skosxl:prefLabel :xl_en_44b51c79 .

:xl_en_44b51c79 a skosxl:Label;
  skosxl:literalForm "Biochemical Oxygen Demand"@en .

:xl_en_cca67e04 a skosxl:Label;
  skosxl:literalForm "BOD"@en .

:c_178eed3e a :Terms;
  skos:broader :Ecology, :Water_Quality;
  skos:definition "The accumulation of a chemical in tissues of an organism (such as a fish) to levels greater than in the surrounding medium in which the organism lives. "@en;
  skos:inScheme :epa-abg;
  skosxl:prefLabel :xl_en_b4298e43 .

:xl_en_b4298e43 a skosxl:Label;
  skosxl:literalForm "Bioconcentration"@en .

:c_b79034fb a :Terms;
  skos:broader :Ecology, :Water_Quality;
  skos:definition "Narrative or numeric expressions that describe the biological condition (structure and function) of aquatic communities inhabiting waters of a designated aquatic life use. Biocriteria are based on the numbers and kinds of organisms present and are regulatory-based biological measurements. "@en;
  skos:inScheme :epa-abg;
  skosxl:prefLabel :xl_en_1b28dce1 .

:xl_en_1b28dce1 a skosxl:Label;
  skosxl:literalForm "Biocriteria"@en .

:c_2508ee26 a :Terms;
  skos:broader :Ecology, :Water_Quality;
  skos:definition "Capable of decomposing rapidly under natural conditions. "@en;
  skos:inScheme :epa-abg;
  skosxl:prefLabel :xl_en_6246cac9 .

:xl_en_6246cac9 a skosxl:Label;
  skosxl:literalForm "Biodegradable"@en .

:c_60251af7 a :Terms;
  skos:broader :Ecology, :Water_Quality;
  skos:definition "Refers to the variety and variability among living organisms and the ecological complexes in which they occur. Diversity can be defined as the number of different items and their relative frequencies. For biological diversity, these items are organized at many levels, ranging from complete ecosystems to the biochemical structures that are the molecular basis of heredity. Thus, the term encompasses different ecosystem, species, and genes. "@en;
  skos:inScheme :epa-abg;
  skosxl:prefLabel :xl_en_fad55066 .

:xl_en_fad55066 a skosxl:Label;
  skosxl:literalForm "Biodiversity"@en .

:c_681f119a a :Terms;
  skos:broader :Ecology, :Water_Quality;
  skos:definition "Preferred Term: Bioassessments "@en;
  skos:inScheme :epa-abg;
  skosxl:prefLabel :xl_en_cca019dd .

:xl_en_cca019dd a skosxl:Label;
  skosxl:literalForm "Biological Assessments"@en .

:c_def1eb08 a :Terms;
  skos:broader :Ecology, :Water_Quality;
  skos:definition "Preferred Term: Biocriteria "@en;
  skos:inScheme :epa-abg;
  skosxl:prefLabel :xl_en_6764e7d3 .

:xl_en_6764e7d3 a skosxl:Label;
  skosxl:literalForm "Biological Criteria"@en .

:c_a2bba777 a :Terms;
  skos:broader :Ecology, :Water_Quality;
  skos:definition "The ability of an aquatic ecosystem to support and maintain a balanced, adaptive community of organisms having a species composition, diversity, and functional organization comparable to that of natural habitats within a region. "@en;
  skos:inScheme :epa-abg;
  skosxl:prefLabel :xl_en_092c7fd6 .

:xl_en_092c7fd6 a skosxl:Label;
  skosxl:literalForm "Biological Integrity"@en .

:c_9481cd83 a :Terms;
  skos:broader :Ecology, :Water_Quality;
  skos:definition "Refers to the process whereby certain substances such as pesticides or heavy metals move up the food chain, work their way into rivers or lakes, and are eaten by aquatic organisms such as fish, which in turn are eaten by large birds, animals or humans. The substances become concentrated in tissues or internal organs as they move up the chain. "@en;
  skos:inScheme :epa-abg;
  skosxl:prefLabel :xl_en_d3d467a3 .

:xl_en_d3d467a3 a skosxl:Label;
  skosxl:literalForm "Biological Magnification"@en .

:c_1b17940f a :Terms;
  skos:broader :Ecology, :Water_Quality;
  skos:definition "Preferred Term: Biomonitoring "@en;
  skos:inScheme :epa-abg;
  skosxl:prefLabel :xl_en_4f18aced .

:xl_en_4f18aced a skosxl:Label;
  skosxl:literalForm "Biological Monitoring"@en .

:c_87daa77c a :Terms;
  skos:broader :Ecology, :Water_Quality;
  skos:definition "Preferred Term: Biosurvey "@en;
  skos:inScheme :epa-abg;
  skosxl:prefLabel :xl_en_2daf08b0 .

:xl_en_2daf08b0 a skosxl:Label;
  skosxl:literalForm "Biological Survey"@en .

:c_990217f6 a :Terms;
  skos:broader :Ecology, :Water_Quality;
  skos:definition "Entire community of living organisms in a single major ecological area. "@en;
  skos:inScheme :epa-abg;
  skosxl:prefLabel :xl_en_37440d6b .

:xl_en_37440d6b a skosxl:Label;
  skosxl:literalForm "Biome"@en .

:c_40c2a3c5 a :Terms;
  skos:broader :Ecology, :Water_Quality;
  skos:definition "Use of a biological entity as a detector and its response as a measure to determine environmental conditions. Toxicity tests and ambient biological surveys are common biological monitoring methods. "@en;
  skos:inScheme :epa-abg;
  skosxl:prefLabel :xl_en_49dee873 .

:xl_en_49dee873 a skosxl:Label;
  skosxl:literalForm "Biomonitoring"@en .

:c_6bf2dc94 a :Terms;
  skos:broader :Ecology, :Water_Quality;
  skos:definition "Any geographical region characterized by a distinctive flora and fauna. "@en;
  skos:inScheme :epa-abg;
  skosxl:prefLabel :xl_en_98a6157e .

:xl_en_98a6157e a skosxl:Label;
  skosxl:literalForm "Bioregion"@en .

:c_a2ee4156 a :Terms;
  skos:broader :Ecology, :Water_Quality;
  skos:definition "Collecting, processing, and analyzing a representative portion of the resident aquatic community to determine its structural and/or functional characteristics. "@en;
  skos:inScheme :epa-abg;
  skosxl:prefLabel :xl_en_8dce1727 .

:xl_en_8dce1727 a skosxl:Label;
  skosxl:literalForm "Biosurvey"@en .

:c_4f154be7 a :Terms;
  skos:broader :Ecology, :Water_Quality;
  skos:definition "The animal and plant life of a given region. "@en;
  skos:inScheme :epa-abg;
  skosxl:prefLabel :xl_en_149c6592 .

:xl_en_149c6592 a skosxl:Label;
  skosxl:literalForm "Biota"@en .

:c_edc84aa8 a :Terms;
  skos:broader :Ecology, :Water_Quality;
  skos:definition "A naturally occurring assemblage of plants and animals that live in the same environment and are mutually sustaining and interdependent. "@en;
  skos:inScheme :epa-abg;
  skosxl:prefLabel :xl_en_a3b2a854 .

:xl_en_a3b2a854 a skosxl:Label;
  skosxl:literalForm "Biotic Community"@en .

:c_c4ce4107 a :Terms;
  skos:broader :Ecology, :Water_Quality;
  skos:definition "A proliferation of algae and/or higher aquatic plants in a body of water; often related to pollution, especially when pollutants accelerate growth. "@en;
  skos:inScheme :epa-abg;
  skosxl:prefLabel :xl_en_32170b8e .

:xl_en_32170b8e a skosxl:Label;
  skosxl:literalForm "Bloom (Algal)"@en .

:c_10b9fb11 a :Terms;
  skos:broader :Ecology, :Water_Quality;
  skos:definition "A type of wetland that accumulates appreciable peat deposits. Bogs depend primarily on precipitation for their water source, and are usually acidic and rich in plant residue with a conspicuous mat of living green moss. "@en;
  skos:inScheme :epa-abg;
  skosxl:prefLabel :xl_en_a2f04a12 .

:xl_en_a2f04a12 a skosxl:Label;
  skosxl:literalForm "Bog"@en .

:c_74d63618 a :Terms;
  skos:broader :Ecology, :Water_Quality;
  skos:definition "Mixed fresh and salt water. "@en;
  skos:inScheme :epa-abg;
  skosxl:prefLabel :xl_en_27b55ee9 .

:xl_en_27b55ee9 a skosxl:Label;
  skosxl:literalForm "Brackish"@en .

:c_ec689587 a :Terms;
  skos:broader :Ecology, :Water_Quality;
  skos:definition "A solution or liquid whose chemical makeup neutralizes acids or bases without a great change in pH. "@en;
  skos:inScheme :epa-abg;
  skosxl:prefLabel :xl_en_3f69f59b .

:xl_en_3f69f59b a skosxl:Label;
  skosxl:literalForm "Buffer"@en .

:c_e2f415cb a :Terms;
  skos:broader :Ecology, :Water_Quality;
  skos:definition "Strips of grass or other erosion-resisting vegetation between or below cultivated strips or fields. "@en;
  skos:inScheme :epa-abg;
  skosxl:prefLabel :xl_en_306522cd .

:xl_en_306522cd a skosxl:Label;
  skosxl:literalForm "Buffer Strips"@en .

:c_da4f8325 a :Terms;
  skos:broader :Ecology, :Water_Quality;
  skos:definition "A stream or riverbed. "@en;
  skos:inScheme :epa-abg;
  skosxl:prefLabel :xl_en_c0a1dfdc .

:xl_en_c0a1dfdc a skosxl:Label;
  skosxl:literalForm "Channel"@en .

:c_1c3eebed a :Terms;
  skos:broader :Ecology, :Water_Quality;
  skos:definition "The straightening and deepening of streams to permit water to move faster, to reduce flooding or to drain marshy acreage for farming. However, channelization reduces the organic waste assimilation capacity of the stream and may disturb fish breeding and destroy the stream's natural beauty. "@en;
  skos:inScheme :epa-abg;
  skosxl:prefLabel :xl_en_71edc7ab .

:xl_en_71edc7ab a skosxl:Label;
  skosxl:literalForm "Channelization"@en .

:c_2d5a5a40 a :Terms;
  skos:broader :Ecology, :Water_Quality;
  skos:definition "A chemical mixture or compound found in the chloroplasts of plant cells and gives plants their green color. Plants use chlorophyll to convert the energy of sunlight to food in the process known as photosynthesis. "@en;
  skos:inScheme :epa-abg;
  skosxl:prefLabel :xl_en_0692ee33 .

:xl_en_0692ee33 a skosxl:Label;
  skosxl:literalForm "Chlorophyll"@en .

:c_bc8e39e5 a :Terms;
  skos:broader :Ecology, :Water_Quality;
  skos:definition """An act passed by the U.S. Congress to control water pollution (formerly referred to as the Federal Water Pollution Control Act of 1972). Public Law 92-500, as amended. 33 U.S.C. 1251 et seq. 
Acronym: CWA """@en;
  skos:inScheme :epa-abg;
  skosxl:altLabel :xl_en_e633d4f6;
  skosxl:prefLabel :xl_en_6ce1cd7d .

:xl_en_6ce1cd7d a skosxl:Label;
  skosxl:literalForm "Clean Water Act"@en .

:xl_en_e633d4f6 a skosxl:Label;
  skosxl:literalForm "CWA"@en .

:c_4a50fa88 a :Terms;
  skos:broader :Ecology, :Water_Quality;
  skos:definition "Annual report to Congress from EPA that identifies those waters for which existing controls are not sufficiently stringent to achieve applicable water quality standards. "@en;
  skos:inScheme :epa-abg;
  skosxl:prefLabel :xl_en_ffbd281d .

:xl_en_ffbd281d a skosxl:Label;
  skosxl:literalForm "Clean Water Act Section 303(d)"@en .

:c_bd5b34d7 a :Terms;
  skos:broader :Ecology, :Water_Quality;
  skos:definition "Biennial reporting requires description of the quality of the Nation's surface waters, evaluation of progress made in maintaining and restoring water quality, and description of the extent of remaining problems by using biological data to make aquatic life use support decisions. "@en;
  skos:inScheme :epa-abg;
  skosxl:prefLabel :xl_en_63cc37d5 .

:xl_en_63cc37d5 a skosxl:Label;
  skosxl:literalForm "Clean Water Act Section 305(b)"@en .

:c_9f076510 a :Terms;
  skos:broader :Ecology, :Water_Quality;
  skos:definition "Microorganisms found in the intestinal tract of humans and animals. Their presence in water indicates fecal pollution and potentially adverse contamination by pathogens. "@en;
  skos:inScheme :epa-abg;
  skosxl:prefLabel :xl_en_ab1b45b5 .

:xl_en_ab1b45b5 a skosxl:Label;
  skosxl:literalForm "Coliform Organism"@en .

:c_40ca3850 a :Terms;
  skos:broader :Ecology, :Water_Quality;
  skos:definition "Pipes used to collect and carry wastewater from individual sources to an interceptor sewer that will carry it to a treatment facility. "@en;
  skos:inScheme :epa-abg;
  skosxl:prefLabel :xl_en_3a537438 .

:xl_en_3a537438 a skosxl:Label;
  skosxl:literalForm "Collector Sewers"@en .

:c_95dd9832 a :Terms;
  skos:broader :Ecology, :Water_Quality;
  skos:definition "Discharge of a mixture of storm water and domestic waste when the flow capacity of a sewer system is exceeded during rainstorms. "@en;
  skos:inScheme :epa-abg;
  skosxl:prefLabel :xl_en_4fdc5ce9 .

:xl_en_4fdc5ce9 a skosxl:Label;
  skosxl:literalForm "Combined Sewer Overflows"@en .

:c_18db2546 a :Terms;
  skos:broader :Ecology, :Water_Quality;
  skos:definition "A sewer system that carries both sewage and storm-water runoff. Normally, its entire flow goes to a waste treatment plant, but during a heavy storm, the volume of water may be so great as to cause overflows of untreated mixtures of storm water and sewage into receiving waters. Storm-water runoff may also carry toxic chemicals from industrial areas or streets into the sewer system. "@en;
  skos:inScheme :epa-abg;
  skosxl:prefLabel :xl_en_be56b9ed .

:xl_en_be56b9ed a skosxl:Label;
  skosxl:literalForm "Combined Sewers"@en .

:c_a2353449 a :Terms;
  skos:broader :Ecology, :Water_Quality;
  skos:definition "In ecology, a group of interacting populations in time and space. Sometimes, a particular subgrouping may be specified, such as the fish community in a lake or the soil arthropod community in a forest. "@en;
  skos:inScheme :epa-abg;
  skosxl:prefLabel :xl_en_a88c13d1 .

:xl_en_a88c13d1 a skosxl:Label;
  skosxl:literalForm "Community"@en .

:c_c88fb39c a :Terms;
  skos:broader :Ecology, :Water_Quality;
  skos:definition "A heterotrophic organism in a food chain that ingests other organisms or organic matter. "@en;
  skos:inScheme :epa-abg;
  skosxl:prefLabel :xl_en_9d06195e .

:xl_en_9d06195e a skosxl:Label;
  skosxl:literalForm "Consumer"@en .

:c_58e5c7cb a :Terms;
  skos:broader :Ecology, :Water_Quality;
  skos:definition "Statements of the conditions presumed to support or protect the designated use or uses of a waterbody. Criteria may be narrative or numeric. "@en;
  skos:inScheme :epa-abg;
  skosxl:prefLabel :xl_en_b19f4571 .

:xl_en_b19f4571 a skosxl:Label;
  skosxl:literalForm "Criteria"@en .

:c_0c2cf147 a :Terms;
  skos:broader :Ecology, :Water_Quality;
  skos:definition "Acceleration by man of the natural aging process of bodies of water. "@en;
  skos:inScheme :epa-abg;
  skosxl:prefLabel :xl_en_76db6070 .

:xl_en_76db6070 a skosxl:Label;
  skosxl:literalForm "Cultural Eutrophication"@en .

:c_9a9b73b9 a :Terms;
  skos:broader :Ecology, :Water_Quality;
  skos:definition "The segment of a stream, river, or other waterbody that moves with a velocity much greater than the average of the rest of the water. "@en;
  skos:inScheme :epa-abg;
  skosxl:prefLabel :xl_en_a16799b9 .

:xl_en_a16799b9 a skosxl:Label;
  skosxl:literalForm "Current"@en .

:c_3fac87b5 a :Terms;
  skos:broader :Ecology, :Water_Quality;
  skos:definition "Regulation of the size of a population by mechanisms that are themselves controlled by the size of that population (e.g. the availability of resources) and whose effectiveness increases as population size increases. "@en;
  skos:inScheme :epa-abg;
  skosxl:prefLabel :xl_en_16a2fcca .

:xl_en_16a2fcca a skosxl:Label;
  skosxl:literalForm "Density-Dependence"@en .

:c_f7336870 a :Terms;
  skos:broader :Ecology, :Water_Quality;
  skos:definition "Classification specified in water quality standards for each waterbody or segment describing the level of protection from perturbation afforded by the regulatory programs. The designated aquatic life uses established by the state or authorized tribes set forth the goals for restoration and/or baseline conditions for maintenance and prevention from future degradation of the aquatic life in specific waterbodies. "@en;
  skos:inScheme :epa-abg;
  skosxl:prefLabel :xl_en_cee097b7 .

:xl_en_cee097b7 a skosxl:Label;
  skosxl:literalForm "Designated Use"@en .

:c_47a36070 a :Terms;
  skos:broader :Ecology, :Water_Quality;
  skos:definition "Loose fragments, particles, or grains formed by the disintegration of rocks. "@en;
  skos:inScheme :epa-abg;
  skosxl:prefLabel :xl_en_a213ff23 .

:xl_en_a213ff23 a skosxl:Label;
  skosxl:literalForm "Detritus"@en .

:c_ad1766fd a :Terms;
  skos:broader :Ecology, :Water_Quality;
  skos:definition "Microscopic algae with cell walls made of silicon and have two separating halves. "@en;
  skos:inScheme :epa-abg;
  skosxl:prefLabel :xl_en_8f18b051 .

:xl_en_8f18b051 a skosxl:Label;
  skosxl:literalForm "Diatom"@en .

:c_e3340e37 a :Terms;
  skos:broader :Ecology, :Water_Quality;
  skos:definition """The oxygen dissolved in water or sewage. Adequately dissolved oxygen is necessary for the life of fish and other aquatic organisms and for the prevention of offensive odors. 
Acronym: DO """@en;
  skos:inScheme :epa-abg;
  skosxl:altLabel :xl_en_3695d037;
  skosxl:prefLabel :xl_en_36b18f33 .

:xl_en_36b18f33 a skosxl:Label;
  skosxl:literalForm "Dissolved Oxygen"@en .

:xl_en_3695d037 a skosxl:Label;
  skosxl:literalForm "DO"@en .

:c_71390156 a :Terms;
  skos:broader :Ecology, :Water_Quality;
  skos:definition "A method for deepening streams, swamps or coastal waters by scraping and removing solids from the bottom. The resulting mud is usually deposited in marshes in a process called filling. Dredging and filling can disturb natural ecological cycles. For example, dredging can destroy oyster beds and other aquatic life; filling can destroy the feeding and breeding grounds for many fish species. "@en;
  skos:inScheme :epa-abg;
  skosxl:prefLabel :xl_en_667a992f .

:xl_en_667a992f a skosxl:Label;
  skosxl:literalForm "Dredging"@en .

:c_35665364 a :Terms;
  skos:broader :Ecology, :Water_Quality;
  skos:definition "The condition of an unimpaired ecosystem as measured by combined chemical, physical (including physical habitat), and biological attributes. "@en;
  skos:inScheme :epa-abg;
  skosxl:prefLabel :xl_en_824ea7d0 .

:xl_en_824ea7d0 a skosxl:Label;
  skosxl:literalForm "Ecological Integrity"@en .

:c_c78898ec a :Terms;
  skos:broader :Ecology, :Water_Quality;
  skos:definition "The interrelationships of living things to one another and to their environment or the study of such interrelationships. "@en;
  skos:inScheme :epa-abg;
  skosxl:prefLabel :xl_en_03c29a90 .

:xl_en_03c29a90 a skosxl:Label;
  skosxl:literalForm "Ecology"@en .

:c_1d6ffa67 a :Terms;
  skos:broader :Ecology, :Water_Quality;
  skos:definition "A relatively homogeneous ecological area defined by similarity of climate, landform, soil, potential natural vegetation, hydrology, or other ecologically relevant variables. "@en;
  skos:inScheme :epa-abg;
  skosxl:prefLabel :xl_en_1d009a73 .

:xl_en_1d009a73 a skosxl:Label;
  skosxl:literalForm "Ecoregion"@en .

:c_0274cc14 a :Terms;
  skos:broader :Ecology, :Water_Quality;
  skos:definition "Preferred Term: Regionalization "@en;
  skos:inScheme :epa-abg;
  skosxl:prefLabel :xl_en_ef527f76 .

:xl_en_ef527f76 a skosxl:Label;
  skosxl:literalForm "Ecoregionalization"@en .

:c_11b47abe a :Terms;
  skos:broader :Ecology, :Water_Quality;
  skos:definition "The interacting system of a biological community and its non-living environment. "@en;
  skos:inScheme :epa-abg;
  skosxl:prefLabel :xl_en_741c901a .

:xl_en_741c901a a skosxl:Label;
  skosxl:literalForm "Ecosystem"@en .

:c_8071067c a :Terms;
  skos:broader :Ecology, :Water_Quality;
  skos:definition "A discharge of pollutants into the environment, partially or completely treated or in its natural state. Generally used in regard to discharges into waters. "@en;
  skos:inScheme :epa-abg;
  skosxl:prefLabel :xl_en_01f6ec7d .

:xl_en_01f6ec7d a skosxl:Label;
  skosxl:literalForm "Effluent"@en .

:c_2d43db08 a :Terms;
  skos:broader :Ecology, :Water_Quality;
  skos:definition "A discharge of pollutants into the environment, partially or completely treated or in its natural state. Generally used in regard to discharges into the air. "@en;
  skos:inScheme :epa-abg;
  skosxl:prefLabel :xl_en_e654841e .

:xl_en_e654841e a skosxl:Label;
  skosxl:literalForm "Emission"@en .

:c_36b2800e a :Terms;
  skos:broader :Ecology, :Water_Quality;
  skos:definition "The addition of nitrogen, phosphorus and carbon compounds or other nutrients into a lake or other waterway that greatly increases the growth potential for algae and other aquatic plants. Most frequently, enrichment results from the inflow of sewage effluent or from agricultural runoff. "@en;
  skos:inScheme :epa-abg;
  skosxl:prefLabel :xl_en_7b3f3333 .

:xl_en_7b3f3333 a skosxl:Label;
  skosxl:literalForm "Enrichment"@en .

:c_044ab9ac a :Terms;
  skos:broader :Ecology, :Water_Quality;
  skos:definition "The sum of all external conditions and influences affecting the life, development and, ultimately, the survival of an organism. "@en;
  skos:inScheme :epa-abg;
  skosxl:prefLabel :xl_en_cd05ac8e .

:xl_en_cd05ac8e a skosxl:Label;
  skosxl:literalForm "Environment"@en .

:c_f4d62c40 a :Terms;
  skos:broader :Ecology, :Water_Quality;
  skos:definition "The wearing away of the land surface by wind or water. Erosion occurs naturally from weather or runoff but is often intensified by man's land-clearing practices. "@en;
  skos:inScheme :epa-abg;
  skosxl:prefLabel :xl_en_973f6103 .

:xl_en_973f6103 a skosxl:Label;
  skosxl:literalForm "Erosion"@en .

:c_0e833719 a :Terms;
  skos:broader :Ecology, :Water_Quality;
  skos:definition "Areas where the fresh water meets salt water. For example, bays, mouths of rivers, salt marshes and lagoons. Estuaries are delicate ecosystems; they serve as nurseries, spawning and feeding grounds for a large group of marine life and provide shelter and food for birds and wildlife. "@en;
  skos:inScheme :epa-abg;
  skosxl:prefLabel :xl_en_bdc3fe9b .

:xl_en_bdc3fe9b a skosxl:Label;
  skosxl:literalForm "Estuaries"@en .

:c_278b73ec a :Terms;
  skos:broader :Ecology, :Water_Quality;
  skos:definition "Shallow lakes weed-choked at the edges and very rich in nutrients. The water is characterized by large amounts of algae, low water transparency and low dissolved oxygen. "@en;
  skos:inScheme :epa-abg;
  skosxl:prefLabel :xl_en_5cf9b41d .

:xl_en_5cf9b41d a skosxl:Label;
  skosxl:literalForm "Eutrophic Lakes"@en .

:c_2fd5bb59 a :Terms;
  skos:broader :Ecology, :Water_Quality;
  skos:definition "The normally slow aging process by which a lake evolves into a bog or marsh and ultimately assumes a completely terrestrial state and disappears. During eutrophication the lake becomes so rich in nutritive compounds, especially nitrogen and phosphorus, that algae and other microscopic plant life become superabundant, thereby \"choking\" the lade, and causing it eventually to dry up. Eutrophication may be accelerated by human activities. "@en;
  skos:inScheme :epa-abg;
  skosxl:prefLabel :xl_en_64ba27ce .

:xl_en_64ba27ce a skosxl:Label;
  skosxl:literalForm "Eutrophication"@en .

:c_06e09c9b a :Terms;
  skos:broader :Ecology, :Water_Quality;
  skos:definition "The changing of a substance from a liquid to a gas; evaporation generally occurs when the molecules of a liquid are broken apart by heat. In the water cycle, water evaporates from land, plants and waterbodies and enters the atmosphere as water vapor. "@en;
  skos:inScheme :epa-abg;
  skosxl:prefLabel :xl_en_82dc55af .

:xl_en_82dc55af a skosxl:Label;
  skosxl:literalForm "Evaporation"@en .

:c_91457516 a :Terms;
  skos:broader :Ecology, :Water_Quality;
  skos:definition "A group of organisms common to the intestinal tracts of man and of animals. The presence of fecal Coliform bacteria in water is an indicator of pollution and of potentially dangerous bacterial contamination. "@en;
  skos:inScheme :epa-abg;
  skosxl:prefLabel :xl_en_5481f452 .

:xl_en_5481f452 a skosxl:Label;
  skosxl:literalForm "Fecal Coliform Bacteria"@en .

:c_fc45de6f a :Terms;
  skos:broader :Ecology, :Water_Quality;
  skos:definition "Slender and or threadlike. Filamentous is a term used to describe the slender, sometimes transparent stems of algae. "@en;
  skos:inScheme :epa-abg;
  skosxl:prefLabel :xl_en_03215a80 .

:xl_en_03215a80 a skosxl:Label;
  skosxl:literalForm "Filamentous"@en .

:c_29e7234c a :Terms;
  skos:broader :Ecology, :Water_Quality;
  skos:definition "When aquatic life within a river, lake, or stream dies in a mass extinction. "@en;
  skos:inScheme :epa-abg;
  skosxl:prefLabel :xl_en_dfd89c8d .

:xl_en_dfd89c8d a skosxl:Label;
  skosxl:literalForm "Fish Kill"@en .

:c_baa4c68e a :Terms;
  skos:broader :Ecology, :Water_Quality;
  skos:definition "A strip of relatively level land bordering a stream or river subject to flooding. Floodplain build up over time by deposits of sediment carried in flood waters. "@en;
  skos:inScheme :epa-abg;
  skosxl:prefLabel :xl_en_c8736d5d .

:xl_en_c8736d5d a skosxl:Label;
  skosxl:literalForm "Floodplain"@en .

:c_2baef830 a :Terms;
  skos:broader :Ecology, :Water_Quality;
  skos:definition "Small, often microscopic plants without chlorophyll. Some fungi infect and cause disease in plants or animals; other fungi are useful in stabilizing sewage or in breaking down wastes for compost. "@en;
  skos:inScheme :epa-abg;
  skosxl:prefLabel :xl_en_bd7d60cb .

:xl_en_bd7d60cb a skosxl:Label;
  skosxl:literalForm "Fungi"@en .

:c_71153440 a :Terms;
  skos:broader :Ecology, :Water_Quality;
  skos:definition "Those species of fish sought by sports fisherman (trout, bass, salmon, etc). Game fish are usually more sensitive to environmental changes and water quality degradation than \"rough\" fish. "@en;
  skos:inScheme :epa-abg;
  skosxl:prefLabel :xl_en_92e47647 .

:xl_en_92e47647 a skosxl:Label;
  skosxl:literalForm "Game Fish"@en .

:c_7b00a71a a :Terms;
  skos:broader :Ecology, :Water_Quality;
  skos:definition "The supply of freshwater under the earth's surface in an aquifer or soil that forms the natural reservoir for man's use. "@en;
  skos:inScheme :epa-abg;
  skosxl:prefLabel :xl_en_4f7652a1 .

:xl_en_4f7652a1 a skosxl:Label;
  skosxl:literalForm "Groundwater"@en .

:c_0fcdf7be a :Terms;
  skos:broader :Ecology, :Water_Quality;
  skos:definition "Groundwater that is discharged into a stream channel as spring or seepage water. "@en;
  skos:inScheme :epa-abg;
  skosxl:prefLabel :xl_en_bce84d40 .

:xl_en_bce84d40 a skosxl:Label;
  skosxl:literalForm "Groundwater Runoff"@en .

:c_4996f7cf a :Terms;
  skos:broader :Ecology, :Water_Quality;
  skos:definition "A place where the physical and biological elements of ecosystems provide a suitable environment including the food, cover, and space resources needed for plant and animal livelihood. "@en;
  skos:inScheme :epa-abg;
  skosxl:prefLabel :xl_en_1db0af1e .

:xl_en_1db0af1e a skosxl:Label;
  skosxl:literalForm "Habitat"@en .

:c_76da11b5 a :Terms;
  skos:broader :Ecology, :Water_Quality;
  skos:definition "Data sets from previous studies, which can range from handwritten field notes to published journal articles. "@en;
  skos:inScheme :epa-abg;
  skosxl:prefLabel :xl_en_c3a9e7d4 .

:xl_en_c3a9e7d4 a skosxl:Label;
  skosxl:literalForm "Historical Data"@en .

:c_8709c7ed a :Terms;
  skos:broader :Ecology, :Water_Quality;
  skos:definition "The movement of water in all of its phases (gas, liquid, solid) from the Earth to the atmosphere and back to the Earth. "@en;
  skos:inScheme :epa-abg;
  skosxl:prefLabel :xl_en_0b97a685 .

:xl_en_0b97a685 a skosxl:Label;
  skosxl:literalForm "Hydrologic Cycle"@en .

:c_f12f6680 a :Terms;
  skos:broader :Ecology, :Water_Quality;
  skos:definition "The science dealing with the properties, distribution and circulation of water and snow. "@en;
  skos:inScheme :epa-abg;
  skosxl:prefLabel :xl_en_66a0fb3b .

:xl_en_66a0fb3b a skosxl:Label;
  skosxl:literalForm "Hydrology"@en .

:c_34dd7e7e a :Terms;
  skos:broader :Ecology, :Water_Quality;
  skos:definition "Vegetation that only grows in water or substrate that is at least periodically deficient in oxygen during a growing season as the result of excessive water content. Hydrophytes have poorly developed root systems and weak stems; they rely upon the water for support. "@en;
  skos:inScheme :epa-abg;
  skosxl:prefLabel :xl_en_96ebadf1 .

:xl_en_96ebadf1 a skosxl:Label;
  skosxl:literalForm "Hydrophytic Vegetation"@en .

:c_b3984ed0 a :Terms;
  skos:broader :Ecology, :Water_Quality;
  skos:definition "change in the chemical, physical (including habitat) or biological quality or condition of a waterbody caused by external sources. "@en;
  skos:inScheme :epa-abg;
  skosxl:prefLabel :xl_en_80e8da2e .

:xl_en_80e8da2e a skosxl:Label;
  skosxl:literalForm "Impact"@en .

:c_27833921 a :Terms;
  skos:broader :Ecology, :Water_Quality;
  skos:definition "Detrimental effect on the biological integrity of a waterbody caused by an impact that prevents attainment of the designated use. "@en;
  skos:inScheme :epa-abg;
  skosxl:prefLabel :xl_en_5fd9c608 .

:xl_en_5fd9c608 a skosxl:Label;
  skosxl:literalForm "Impairment"@en .

:c_8cac60a2 a :Terms;
  skos:broader :Ecology, :Water_Quality;
  skos:definition "A body of water, such as a pond, confined by a dam, dike, floodgate or other barrier. "@en;
  skos:inScheme :epa-abg;
  skosxl:prefLabel :xl_en_d46c34d9 .

:xl_en_d46c34d9 a skosxl:Label;
  skosxl:literalForm "Impoundment"@en .

:c_86af95fd a :Terms;
  skos:broader :Ecology, :Water_Quality;
  skos:definition """An integrative expression of site condition across multiple metrics. An index of biological integrity is often composed of at least seven metrics. The plural form is either indices or indexes. 
Acronym: IBI """@en;
  skos:inScheme :epa-abg;
  skosxl:altLabel :xl_en_851b68a4;
  skosxl:prefLabel :xl_en_62c6b911 .

:xl_en_62c6b911 a skosxl:Label;
  skosxl:literalForm "Index of Biological Integrity"@en .

:xl_en_851b68a4 a skosxl:Label;
  skosxl:literalForm "IBI"@en .

:c_97f17ef2 a :Terms;
  skos:broader :Ecology, :Water_Quality;
  skos:definition "The flow of a fluid into a substance through pores or small openings. Commonly used to in hydrology to denote the flow of water into soil material. "@en;
  skos:inScheme :epa-abg;
  skosxl:prefLabel :xl_en_d960ea1a .

:xl_en_d960ea1a a skosxl:Label;
  skosxl:literalForm "Infiltration"@en .

:c_7a79bc61 a :Terms;
  skos:broader :Ecology, :Water_Quality;
  skos:definition "Applying water or wastewater to land areas to supply the water and nutrient needs of plants. "@en;
  skos:inScheme :epa-abg;
  skosxl:prefLabel :xl_en_2c2388ec .

:xl_en_2c2388ec a skosxl:Label;
  skosxl:literalForm "Irrigation"@en .

:c_74ad006c a :Terms;
  skos:broader :Ecology, :Water_Quality;
  skos:definition "Surface and subsurface water that leaves the field following application of irrigation water. "@en;
  skos:inScheme :epa-abg;
  skosxl:prefLabel :xl_en_2311bc65 .

:xl_en_2311bc65 a skosxl:Label;
  skosxl:literalForm "Irrigation Return Flow"@en .

:c_baa72ff1 a :Terms;
  skos:broader :Ecology, :Water_Quality;
  skos:definition "A shallow pond where sunlight, bacterial action, and oxygen work to purify wastewater; also used for storage of wastewater or spent nuclear fuel rods. Shallow body of water, often separated from the sea by coral reefs or sandbars. "@en;
  skos:inScheme :epa-abg;
  skosxl:prefLabel :xl_en_0239d3fb .

:xl_en_0239d3fb a skosxl:Label;
  skosxl:literalForm "Lagoon"@en .

:c_756e2d70 a :Terms;
  skos:broader :Ecology, :Water_Quality;
  skos:definition "The study of the physical, chemical, meteorological and biological aspects of fresh waters. "@en;
  skos:inScheme :epa-abg;
  skosxl:prefLabel :xl_en_f73e5146 .

:xl_en_f73e5146 a skosxl:Label;
  skosxl:literalForm "Limnology"@en .

:c_8c62431e a :Terms;
  skos:broader :Ecology, :Water_Quality;
  skos:definition "Of, relating to, or existing on a shore. "@en;
  skos:inScheme :epa-abg;
  skosxl:prefLabel :xl_en_73e0a826 .

:xl_en_73e0a826 a skosxl:Label;
  skosxl:literalForm "Littoral"@en .

:c_0c0ff1cc a :Terms;
  skos:broader :Ecology, :Water_Quality;
  skos:definition "Animals without backbones of a size large enough to be seen by the unaided eye and which can be retained by a U.S. Standard No. 30 sieve (28 meshes per inch, 0.595 mm openings). "@en;
  skos:inScheme :epa-abg;
  skosxl:prefLabel :xl_en_f7815615 .

:xl_en_f7815615 a skosxl:Label;
  skosxl:literalForm "Macroinvertebrates"@en .

:c_8df339dc a :Terms;
  skos:broader :Ecology, :Water_Quality;
  skos:definition "A type of wetland that does not accumulate appreciable peat deposits and is dominated by herbaceous vegetation. Marshes may be either fresh or saltwater, tidal or non-tidal. "@en;
  skos:inScheme :epa-abg;
  skosxl:prefLabel :xl_en_9cf3897c .

:xl_en_9cf3897c a skosxl:Label;
  skosxl:literalForm "Marsh"@en .

:c_c9d2869c a :Terms;
  skos:broader :Ecology, :Water_Quality;
  skos:definition "Reservoirs and lakes that contain moderate quantities of nutrients and are moderately productive in terms of aquatic animal and plant life. "@en;
  skos:inScheme :epa-abg;
  skosxl:prefLabel :xl_en_ba37a55f .

:xl_en_ba37a55f a skosxl:Label;
  skosxl:literalForm "Mesotrophic"@en .

:c_aaffcb42 a :Terms;
  skos:broader :Ecology, :Water_Quality;
  skos:definition "The middle layer of a thermally stratified lake or reservoir. In this layer there is a rapid decrease in temperature with depth. Also called thermocline. "@en;
  skos:inScheme :epa-abg;
  skosxl:prefLabel :xl_en_9d66e537 .

:xl_en_9d66e537 a skosxl:Label;
  skosxl:literalForm "Metalimnion"@en .

:c_06c154fe a :Terms;
  skos:broader :Ecology, :Water_Quality;
  skos:definition "A calculated term or enumeration representing some aspect of biological assemblage, function, or other measurable aspect and is a characteristic of the biota that changes in some predictable way with increased human influence. A multimetric approach involves combinations of metrics to provide an integrative assessment of the status of aquatic resources. "@en;
  skos:inScheme :epa-abg;
  skosxl:prefLabel :xl_en_a79ed6cf .

:xl_en_a79ed6cf a skosxl:Label;
  skosxl:literalForm "Metric"@en .

:c_0f5bbd8a a :Terms;
  skos:broader :Ecology, :Water_Quality;
  skos:definition "Animals without backbones that are not large enough to be seen by the unaided eye; they will not be retained by a U.S. Standard No. 30 sieve (28 meshes per inch, 0.595 mm openings). "@en;
  skos:inScheme :epa-abg;
  skosxl:prefLabel :xl_en_a6930a5c .

:xl_en_a6930a5c a skosxl:Label;
  skosxl:literalForm "Microinvertebrates"@en .

:c_525e18f0 a :Terms;
  skos:broader :Ecology, :Water_Quality;
  skos:definition "Sites or conditions with slight anthropogenic perturbation relative to the overall region of the study. "@en;
  skos:inScheme :epa-abg;
  skosxl:prefLabel :xl_en_ad8c4d54 .

:xl_en_ad8c4d54 a skosxl:Label;
  skosxl:literalForm "Minimally Impaired"@en .

:c_3bb891cf a :Terms;
  skos:broader :Ecology, :Water_Quality;
  skos:definition "Measures taken to reduce adverse impacts on the environment. "@en;
  skos:inScheme :epa-abg;
  skosxl:prefLabel :xl_en_a3da488a .

:xl_en_a3da488a a skosxl:Label;
  skosxl:literalForm "Mitigation"@en .

:c_07861457 a :Terms;
  skos:broader :Ecology, :Water_Quality;
  skos:definition "Lakes and reservoirs which are relatively deep, do not freeze over during the winter months, and undergo a single stratification and mixing cycle during the year (usually in the fall). "@en;
  skos:inScheme :epa-abg;
  skosxl:prefLabel :xl_en_e959a47c .

:xl_en_e959a47c a skosxl:Label;
  skosxl:literalForm "Monomictic"@en .

:c_d0fa72e2 a :Terms;
  skos:broader :Ecology, :Water_Quality;
  skos:definition "Analysis techniques using several measurable characteristics of a biological assemblage. "@en;
  skos:inScheme :epa-abg;
  skosxl:prefLabel :xl_en_6d6231a3 .

:xl_en_6d6231a3 a skosxl:Label;
  skosxl:literalForm "Multimetric"@en .

:c_5d4cbc0a a :Terms;
  skos:broader :Ecology, :Water_Quality;
  skos:definition "Statistical methods (e.g. ordination or discriminant analysis) for analyzing physical and biological community data using multiple variables. "@en;
  skos:inScheme :epa-abg;
  skosxl:prefLabel :xl_en_708c2530 .

:xl_en_708c2530 a skosxl:Label;
  skosxl:literalForm "Multivariate Community Analysis"@en .

:c_79a78368 a :Terms;
  skos:broader :Ecology, :Water_Quality;
  skos:definition "Discharge of effluent from waste water treatment plants, which receive waste water from households, commercial establishments, and industries in the coastal drainage basin. Combined sewer/separate storm overflows are included in this category. "@en;
  skos:inScheme :epa-abg;
  skosxl:prefLabel :xl_en_def9d9b9 .

:xl_en_def9d9b9 a skosxl:Label;
  skosxl:literalForm "Municipal Discharge"@en .

:c_61777e73 a :Terms;
  skos:broader :Ecology, :Water_Quality;
  skos:definition "Wastes (mostly liquid) originating from a community; may be composed of domestic wastewaters and/or industrial discharges. "@en;
  skos:inScheme :epa-abg;
  skosxl:prefLabel :xl_en_a8f5c1a4 .

:xl_en_a8f5c1a4 a skosxl:Label;
  skosxl:literalForm "Municipal Sewage"@en .

:c_fb2cf0cd a :Terms;
  skos:broader :Ecology, :Water_Quality;
  skos:definition "General statements of attainable or attained conditions of biological integrity and water quality for a given designated aquatic life use. "@en;
  skos:inScheme :epa-abg;
  skosxl:prefLabel :xl_en_9460394e .

:xl_en_9460394e a skosxl:Label;
  skosxl:literalForm "Narrative Biological Criteria"@en .

:c_c1291eab a :Terms;
  skos:broader :Ecology, :Water_Quality;
  skos:definition """A provision of the Clean Water Act which prohibits discharge of pollutants into waters of the United States unless a special permit is issued by EPA, a state, or, where delegated, a tribal government on an Indian reservation. 
Acronym: NPDES """@en;
  skos:inScheme :epa-abg;
  skosxl:altLabel :xl_en_b9574cb3;
  skosxl:prefLabel :xl_en_e8c1b90b .

:xl_en_e8c1b90b a skosxl:Label;
  skosxl:literalForm "National Pollutant Discharge Elimination System"@en .

:xl_en_b9574cb3 a skosxl:Label;
  skosxl:literalForm "NPDES"@en .

:c_ff73992f a :Terms;
  skos:broader :Ecology, :Water_Quality;
  skos:definition "Traditionally, waters sufficiently deep and wide for navigation by all, or specified vessels; such waters in the United States come under federal jurisdiction and are protected by certain provisions of the Clean Water Act. "@en;
  skos:inScheme :epa-abg;
  skosxl:prefLabel :xl_en_00f3bd87 .

:xl_en_00f3bd87 a skosxl:Label;
  skosxl:literalForm "Navigable Waters"@en .

:c_24cc3016 a :Terms;
  skos:broader :Ecology, :Water_Quality;
  skos:definition "Decreasing the acidity or alkalinity of a substance by adding alkaline or acidic materials, respectively. "@en;
  skos:inScheme :epa-abg;
  skosxl:prefLabel :xl_en_76496dd4 .

:xl_en_76496dd4 a skosxl:Label;
  skosxl:literalForm "Neutralization"@en .

:c_21006d83 a :Terms;
  skos:broader :Ecology, :Water_Quality;
  skos:definition "Plant nutrient and inorganic fertilizer that enters water supply sources from septic systems, animal feed lots, agricultural fertilizers, manure, industrial waste waters, sanitary landfills and garbage dumps. "@en;
  skos:inScheme :epa-abg;
  skosxl:prefLabel :xl_en_88e9a098 .

:xl_en_88e9a098 a skosxl:Label;
  skosxl:literalForm "Nitrate"@en .

:c_5810681a a :Terms;
  skos:broader :Ecology, :Water_Quality;
  skos:definition "The process whereby ammonia in wastewater is oxidized to nitrite and then to nitrate by bacterial or chemical reactions. "@en;
  skos:inScheme :epa-abg;
  skosxl:prefLabel :xl_en_22c8ecb3 .

:xl_en_22c8ecb3 a skosxl:Label;
  skosxl:literalForm "Nitrification"@en .

:c_afee82d5 a :Terms;
  skos:broader :Ecology, :Water_Quality;
  skos:definition "Animal or vegetable residues that contain significant amounts of nitrogen. "@en;
  skos:inScheme :epa-abg;
  skosxl:prefLabel :xl_en_d892b0cc .

:xl_en_d892b0cc a skosxl:Label;
  skosxl:literalForm "Nitrogenous Wastes"@en .

:c_92f02cd4 a :Terms;
  skos:broader :Ecology, :Water_Quality;
  skos:definition "Diffuse pollution sources (i.e., without a single point of origin or not introduced into a receiving stream from a specific outlet). The pollutants are generally carried off the land by storm water. Common nonpoint sources are agriculture, forestry, urban, mining, construction, dams, channels, land disposal, saltwater intrusion, and city streets. "@en;
  skos:inScheme :epa-abg;
  skosxl:prefLabel :xl_en_2d462015 .

:xl_en_2d462015 a skosxl:Label;
  skosxl:literalForm "Non-Point Source"@en .

:c_eecca9b8 a :Terms;
  skos:broader :Ecology, :Water_Quality;
  skos:definition "Pollution that occurs when rainfall, snowmelt, or irrigation runs over land or through the ground, picks up pollutants, and deposits them into rivers, lakes, and coastal waters or introduces them into ground water. "@en;
  skos:inScheme :epa-abg;
  skosxl:prefLabel :xl_en_fe2facc0 .

:xl_en_fe2facc0 a skosxl:Label;
  skosxl:literalForm "Non-Point Source Pollution"@en .

:c_88319145 a :Terms;
  skos:broader :Ecology, :Water_Quality;
  skos:definition "Numerical indices that describe expected attainable community attributes for different designated aquatic life uses. "@en;
  skos:inScheme :epa-abg;
  skosxl:prefLabel :xl_en_0e1c58ba .

:xl_en_0e1c58ba a skosxl:Label;
  skosxl:literalForm "Numeric Biocriteria"@en .

:c_62d4bfb6 a :Terms;
  skos:broader :Ecology, :Water_Quality;
  skos:definition "Contamination of water resources by excessive inputs of nutrients. In surface waters, excess algal production is a major concern. "@en;
  skos:inScheme :epa-abg;
  skosxl:prefLabel :xl_en_f049f37d .

:xl_en_f049f37d a skosxl:Label;
  skosxl:literalForm "Nutrient Pollution"@en .

:c_8e256c3d a :Terms;
  skos:broader :Ecology, :Water_Quality;
  skos:definition "Any substance assimilated by living things that promotes growth. Elements or compounds essential as raw materials for organism growth and development; for example, carbon, oxygen, nitrogen and phosphorus. The term is generally applied to nitrogen and phosphorus in wastewater. "@en;
  skos:inScheme :epa-abg;
  skosxl:prefLabel :xl_en_2c268422 .

:xl_en_2c268422 a skosxl:Label;
  skosxl:literalForm "Nutrients"@en .

:c_3a974a14 a :Terms;
  skos:broader :Ecology, :Water_Quality;
  skos:definition "Deep lakes that have a low supply of nutrients and thus contain little organic matter. Such lakes are characterized by high water transparency and high dissolved oxygen. "@en;
  skos:inScheme :epa-abg;
  skosxl:prefLabel :xl_en_b453753d .

:xl_en_b453753d a skosxl:Label;
  skosxl:literalForm "Oligotrophic Lakes"@en .

:c_b176fb27 a :Terms;
  skos:broader :Ecology, :Water_Quality;
  skos:definition "Animal or plant-produced substances containing mainly carbon, hydrogen, nitrogen, and oxygen. "@en;
  skos:inScheme :epa-abg;
  skosxl:prefLabel :xl_en_98f0aec9 .

:xl_en_98f0aec9 a skosxl:Label;
  skosxl:literalForm "Organic Chemicals/Compounds"@en .

:c_62d17e1d a :Terms;
  skos:broader :Ecology, :Water_Quality;
  skos:definition "Carbonaceous waste contained in plant or animal matter and originating from domestic or industrial sources. "@en;
  skos:inScheme :epa-abg;
  skosxl:prefLabel :xl_en_f706764f .

:xl_en_f706764f a skosxl:Label;
  skosxl:literalForm "Organic Matter"@en .

:c_13cbbc62 a :Terms;
  skos:broader :Ecology, :Water_Quality;
  skos:definition "Any living thing. All organisms are comprised of one or more cells, eat, and reproduce. "@en;
  skos:inScheme :epa-abg;
  skosxl:prefLabel :xl_en_c030d2fe .

:xl_en_c030d2fe a skosxl:Label;
  skosxl:literalForm "Organism"@en .

:c_b519ac68 a :Terms;
  skos:broader :Ecology, :Water_Quality;
  skos:definition "Finely divided solid or liquid particles in the air or in an emission. Particulates include dust, smoke, fumes, mist, spray and fog. "@en;
  skos:inScheme :epa-abg;
  skosxl:prefLabel :xl_en_960128f9 .

:xl_en_960128f9 a skosxl:Label;
  skosxl:literalForm "Particulates"@en .

:c_cfba7d50 a :Terms;
  skos:broader :Ecology, :Water_Quality;
  skos:definition "Partially decomposed organic material. "@en;
  skos:inScheme :epa-abg;
  skosxl:prefLabel :xl_en_15fbb039 .

:xl_en_15fbb039 a skosxl:Label;
  skosxl:literalForm "Peat"@en .

:c_334faf2c a :Terms;
  skos:broader :Ecology, :Water_Quality;
  skos:definition "The passage of liquids, powders or small particles through a porous substance. Water percolates through soil in the water cycle. "@en;
  skos:inScheme :epa-abg;
  skosxl:prefLabel :xl_en_67fb7e25 .

:xl_en_67fb7e25 a skosxl:Label;
  skosxl:literalForm "Percolation"@en .

:c_8d3599bf a :Terms;
  skos:broader :Ecology, :Water_Quality;
  skos:definition "Sessile organisms that live attached to the surface projecting from the bottom in a freshwater aquatic environment. "@en;
  skos:inScheme :epa-abg;
  skosxl:prefLabel :xl_en_37b53734 .

:xl_en_37b53734 a skosxl:Label;
  skosxl:literalForm "Periphyton"@en .

:c_b47d3731 a :Terms;
  skos:broader :Ecology, :Water_Quality;
  skos:definition "An agent used to control pests. This includes insecticides for use against harmful insects; herbicides for weed control; fungicides for control of plant diseases; rodenticides for killing rats, mice, etc.; and germicides used in disinfectant products, algaecides, slimicides, etc. Some pesticides can contaminate water, air or soil and accumulate in man, animals and the environment, particularly if they are misused. Certain of these chemicals have been shown to interfere with the reproductive processes of predatory birds and possibly other animals. "@en;
  skos:inScheme :epa-abg;
  skosxl:prefLabel :xl_en_1eee309d .

:xl_en_1eee309d a skosxl:Label;
  skosxl:literalForm "Pesticide"@en .

:c_5b685993 a :Terms;
  skos:broader :Ecology, :Water_Quality;
  skos:definition "A measure of the acidity pr alkalinity of a material, liquid or solid. pH is represented on a scale of 0 to 14 with 7 representing a neutral state, 0 representing the most acid and 14, the most alkaline. "@en;
  skos:inScheme :epa-abg;
  skosxl:prefLabel :xl_en_0ff32f04 .

:xl_en_0ff32f04 a skosxl:Label;
  skosxl:literalForm "pH"@en .

:c_062b396a a :Terms;
  skos:broader :Ecology, :Water_Quality;
  skos:definition "Very tiny, often microscopic, plants found in fresh and saltwater. Phytoplankton drift near the surface of the water where there is plenty of sunlight for growth. Phytoplankton form the basis for all food chains. "@en;
  skos:inScheme :epa-abg;
  skosxl:prefLabel :xl_en_5eb5541c .

:xl_en_5eb5541c a skosxl:Label;
  skosxl:literalForm "Phytoplankton"@en .

:c_dd843071 a :Terms;
  skos:broader :Ecology, :Water_Quality;
  skos:definition "The floating or weakly swimming plant and animal life in a body of water, often microscopic in size. "@en;
  skos:inScheme :epa-abg;
  skosxl:prefLabel :xl_en_2a6532b3 .

:xl_en_2a6532b3 a skosxl:Label;
  skosxl:literalForm "Plankton"@en .

:c_fceba1d7 a :Terms;
  skos:broader :Ecology, :Water_Quality;
  skos:definition "Origin of a pollutant discharge from a discrete conveyance typically thought of as an effluent from the end of a pipe. "@en;
  skos:inScheme :epa-abg;
  skosxl:prefLabel :xl_en_829b240a .

:xl_en_829b240a a skosxl:Label;
  skosxl:literalForm "Point Source"@en .

:c_bf04de70 a :Terms;
  skos:broader :Ecology, :Water_Quality;
  skos:definition "Any introduced gas, liquid or solid that makes a resource unfit for a specific purpose. "@en;
  skos:inScheme :epa-abg;
  skosxl:prefLabel :xl_en_03b2d45e .

:xl_en_03b2d45e a skosxl:Label;
  skosxl:literalForm "Pollutant"@en .

:c_ecad58cf a :Terms;
  skos:broader :Ecology, :Water_Quality;
  skos:definition "The presence of matter or energy whose nature, location or quantity produces undesired environmental effects. "@en;
  skos:inScheme :epa-abg;
  skosxl:prefLabel :xl_en_33eb2ee5 .

:xl_en_33eb2ee5 a skosxl:Label;
  skosxl:literalForm "Pollution"@en .

:c_4f14be71 a :Terms;
  skos:broader :Ecology, :Water_Quality;
  skos:definition "Aggregate of individuals of a biological species that are geographically isolated from other members of the species and are actually or potentially interbreeding. "@en;
  skos:inScheme :epa-abg;
  skosxl:prefLabel :xl_en_c51e0180 .

:xl_en_c51e0180 a skosxl:Label;
  skosxl:literalForm "Population"@en .

:c_c578ab81 a :Terms;
  skos:broader :Ecology, :Water_Quality;
  skos:definition "Water suitable for drinking or cooking purposes from both health and aesthetic considerations. "@en;
  skos:inScheme :epa-abg;
  skosxl:prefLabel :xl_en_c43a72e7 .

:xl_en_c43a72e7 a skosxl:Label;
  skosxl:literalForm "Potable Water"@en .

:c_fe1af19f a :Terms;
  skos:broader :Ecology, :Water_Quality;
  skos:definition "Water droplets or ice particles in the form of rain or snow, condensed from atmospheric water vapor. "@en;
  skos:inScheme :epa-abg;
  skosxl:prefLabel :xl_en_373c899c .

:xl_en_373c899c a skosxl:Label;
  skosxl:literalForm "Precipitation"@en .

:c_5ddc6dcc a :Terms;
  skos:broader :Ecology, :Water_Quality;
  skos:definition "The act or practice of capturing another creature (prey) as a means for securing food. "@en;
  skos:inScheme :epa-abg;
  skosxl:prefLabel :xl_en_173a92bd .

:xl_en_173a92bd a skosxl:Label;
  skosxl:literalForm "Predation"@en .

:c_a050c59f a :Terms;
  skos:broader :Ecology, :Water_Quality;
  skos:definition "#VALUE!"@en;
  skos:inScheme :epa-abg;
  skosxl:prefLabel :xl_en_0dd25bf0 .

:xl_en_0dd25bf0 a skosxl:Label;
  skosxl:literalForm "Primary Treatment"@en .

:c_0419e86c a :Terms;
  skos:broader :Ecology, :Water_Quality;
  skos:definition "Untreated domestic or commercial waste water. "@en;
  skos:inScheme :epa-abg;
  skosxl:prefLabel :xl_en_da64abfb .

:xl_en_da64abfb a skosxl:Label;
  skosxl:literalForm "Raw Sewage"@en .

:c_35edc6f7 a :Terms;
  skos:broader :Ecology, :Water_Quality;
  skos:definition "Rivers, lakes, oceans or other bodies that receive treated or untreated waste waters. "@en;
  skos:inScheme :epa-abg;
  skosxl:prefLabel :xl_en_a52f26ad .

:xl_en_a52f26ad a skosxl:Label;
  skosxl:literalForm "Receiving Waters"@en .

:c_276979f7 a :Terms;
  skos:broader :Ecology, :Water_Quality;
  skos:definition "Set of selected measurements or conditions of unimpaired or minimally impaired waterbodies characteristic of a waterbody type in a region. "@en;
  skos:inScheme :epa-abg;
  skosxl:prefLabel :xl_en_073adcf0 .

:xl_en_073adcf0 a skosxl:Label;
  skosxl:literalForm "Reference Condition"@en .

:c_75b4a3a0 a :Terms;
  skos:broader :Ecology, :Water_Quality;
  skos:definition "Specific locality on a waterbody which is unimpaired or minimally impaired and is representative of the expected biological integrity of other localities on the same waterbody or nearby waterbodies. "@en;
  skos:inScheme :epa-abg;
  skosxl:prefLabel :xl_en_80fa1e68 .

:xl_en_80fa1e68 a skosxl:Label;
  skosxl:literalForm "Reference Site"@en .

:c_bd7d9638 a :Terms;
  skos:broader :Ecology, :Water_Quality;
  skos:definition "Procedure for subdividing a geographic area into regions of relative homogeneity in ecological systems or in relationship between organisms and their environment. "@en;
  skos:inScheme :epa-abg;
  skosxl:prefLabel :xl_en_05a2685e .

:xl_en_05a2685e a skosxl:Label;
  skosxl:literalForm "Regionalization"@en .

:c_8def1e2e a :Terms;
  skos:broader :Ecology, :Water_Quality;
  skos:definition "A pond, lake, tank or basin, natural or man-made, used for the storage, regulation and control of water. "@en;
  skos:inScheme :epa-abg;
  skosxl:prefLabel :xl_en_38a5f2be .

:xl_en_38a5f2be a skosxl:Label;
  skosxl:literalForm "Reservoir"@en .

:c_f98834e6 a :Terms;
  skos:broader :Ecology, :Water_Quality;
  skos:definition "A rocky shoal or sandbar lying just below the surface of a waterway. The choppy water created by such sand bars and shoals is also referred to as a riffle. "@en;
  skos:inScheme :epa-abg;
  skosxl:prefLabel :xl_en_aacef294 .

:xl_en_aacef294 a skosxl:Label;
  skosxl:literalForm "Riffle"@en .

:c_17f6d6d9 a :Terms;
  skos:broader :Ecology, :Water_Quality;
  skos:definition "Entitlement of a land owner to certain uses of water on or bordering his property, including the right to prevent diversion or misuse of upstream waters. Generally a matter of state law. "@en;
  skos:inScheme :epa-abg;
  skosxl:prefLabel :xl_en_bac965bb .

:xl_en_bac965bb a skosxl:Label;
  skosxl:literalForm "Riparian Rights"@en .

:c_37656125 a :Terms;
  skos:broader :Ecology, :Water_Quality;
  skos:definition "Those fish species considered to be of poor fighting quality when taken on tackle or of poor eating quality (gar, suckers, etc.). Most rough fish are more tolerant of widely changing environmental conditions than are game fish. "@en;
  skos:inScheme :epa-abg;
  skosxl:prefLabel :xl_en_20de8ed8 .

:xl_en_20de8ed8 a skosxl:Label;
  skosxl:literalForm "Rough Fish"@en .

:c_56a11087 a :Terms;
  skos:broader :Ecology, :Water_Quality;
  skos:definition "The portion of rainfall, melted snow or irrigation water that flows across ground surface and eventually is returned to streams. Runoff can pick up pollutants from the air or the land and carry them to the receiving waters. "@en;
  skos:inScheme :epa-abg;
  skosxl:prefLabel :xl_en_420a1983 .

:xl_en_420a1983 a skosxl:Label;
  skosxl:literalForm "Runoff"@en .

:c_007145c9 a :Terms;
  skos:broader :Ecology, :Water_Quality;
  skos:definition "The degree of salt in water. "@en;
  skos:inScheme :epa-abg;
  skosxl:prefLabel :xl_en_1297823a .

:xl_en_1297823a a skosxl:Label;
  skosxl:literalForm "Salinity"@en .

:c_1da88ee3 a :Terms;
  skos:broader :Ecology, :Water_Quality;
  skos:definition "#VALUE!"@en;
  skos:inScheme :epa-abg;
  skosxl:prefLabel :xl_en_2293c161 .

:xl_en_2293c161 a skosxl:Label;
  skosxl:literalForm "Secondary Treatment"@en .

:c_24c2a3d7 a :Terms;
  skos:broader :Ecology, :Water_Quality;
  skos:definition "Plants of the family Cyperacae that resemble grasses, but have solid stems. "@en;
  skos:inScheme :epa-abg;
  skosxl:prefLabel :xl_en_89a2fd76 .

:xl_en_89a2fd76 a skosxl:Label;
  skosxl:literalForm "Sedges"@en .

:c_9929c59d a :Terms;
  skos:broader :Ecology, :Water_Quality;
  skos:definition "Letting solids settle out of wastewater by gravity during treatment. "@en;
  skos:inScheme :epa-abg;
  skosxl:prefLabel :xl_en_36908ade .

:xl_en_36908ade a skosxl:Label;
  skosxl:literalForm "Sedimentation"@en .

:c_d2921141 a :Terms;
  skos:broader :Ecology, :Water_Quality;
  skos:definition "Wastewater tanks in which floating wastes are skimmed off and settled solids are removed for disposal. "@en;
  skos:inScheme :epa-abg;
  skosxl:prefLabel :xl_en_3f0df980 .

:xl_en_3f0df980 a skosxl:Label;
  skosxl:literalForm "Sedimentation Tanks"@en .

:c_74745111 a :Terms;
  skos:broader :Ecology, :Water_Quality;
  skos:definition "Soil, sand, and minerals washed from land into water, usually after rain. They pile up in reservoirs, rivers and harbors, destroying fish and wildlife habitat, and clouding the water so that sunlight cannot reach aquatic plants. Careless farming, mining, and building activities will expose sediment materials, allowing them to wash off the land after rainfall. "@en;
  skos:inScheme :epa-abg;
  skosxl:prefLabel :xl_en_a8473cd9 .

:xl_en_a8473cd9 a skosxl:Label;
  skosxl:literalForm "Sediments"@en .

:c_871c0928 a :Terms;
  skos:broader :Ecology, :Water_Quality;
  skos:definition "Water that flows through the soil. "@en;
  skos:inScheme :epa-abg;
  skosxl:prefLabel :xl_en_d451dd95 .

:xl_en_d451dd95 a skosxl:Label;
  skosxl:literalForm "Seepage"@en .

:c_d3a88eef a :Terms;
  skos:broader :Ecology, :Water_Quality;
  skos:definition "The total of organic waste and waste water generated by residential and commercial establishments. "@en;
  skos:inScheme :epa-abg;
  skosxl:prefLabel :xl_en_42411174 .

:xl_en_42411174 a skosxl:Label;
  skosxl:literalForm "Sewage"@en .

:c_c397370b a :Terms;
  skos:broader :Ecology, :Water_Quality;
  skos:definition "Finely divided particles of soil or rock. Often carried in cloudy suspension in water and eventually deposited as sediment. "@en;
  skos:inScheme :epa-abg;
  skosxl:prefLabel :xl_en_db500002 .

:xl_en_db500002 a skosxl:Label;
  skosxl:literalForm "Silt"@en .

:c_2b934ca8 a :Terms;
  skos:broader :Ecology, :Water_Quality;
  skos:definition "An aquifer that supplies 50 percent or more of the drinking water of an area. "@en;
  skos:inScheme :epa-abg;
  skosxl:prefLabel :xl_en_8f934cf6 .

:xl_en_8f934cf6 a skosxl:Label;
  skosxl:literalForm "Sole Source Aquifer"@en .

:c_2ff144c8 a :Terms;
  skos:broader :Ecology, :Water_Quality;
  skos:definition "A reproductively isolated aggregate of interbreeding organisms. "@en;
  skos:inScheme :epa-abg;
  skosxl:prefLabel :xl_en_ff4155fd .

:xl_en_ff4155fd a skosxl:Label;
  skosxl:literalForm "Species"@en .

:c_db1de5cc a :Terms;
  skos:broader :Ecology, :Water_Quality;
  skos:definition "The process by which warm temperatures melt winter snow and ice. Because various forms of acid deposition may have been stored in the frozen water, the melt can result in abnormally large amounts of acidity entering streams and rivers, sometimes causing fish kills. "@en;
  skos:inScheme :epa-abg;
  skosxl:prefLabel :xl_en_8826c82c .

:xl_en_8826c82c a skosxl:Label;
  skosxl:literalForm "Spring Melt/Thaw"@en .

:c_271b7032 a :Terms;
  skos:broader :Ecology, :Water_Quality;
  skos:definition "Separating into layers. "@en;
  skos:inScheme :epa-abg;
  skosxl:prefLabel :xl_en_0ceb7ca4 .

:xl_en_0ceb7ca4 a skosxl:Label;
  skosxl:literalForm "Stratification"@en .

:c_3394f41e a :Terms;
  skos:broader :Ecology, :Water_Quality;
  skos:definition "The channel through which a natural stream or river runs or once ran through. "@en;
  skos:inScheme :epa-abg;
  skosxl:prefLabel :xl_en_30ce28b8 .

:xl_en_30ce28b8 a skosxl:Label;
  skosxl:literalForm "Streambed"@en .

:c_c29e378a a :Terms;
  skos:broader :Ecology, :Water_Quality;
  skos:definition "physical and biological factors that adversely affect aquatic organisms. "@en;
  skos:inScheme :epa-abg;
  skosxl:prefLabel :xl_en_f0458ff5 .

:xl_en_f0458ff5 a skosxl:Label;
  skosxl:literalForm "Stressors"@en .

:c_84e77ccd a :Terms;
  skos:broader :Ecology, :Water_Quality;
  skos:definition "Precipitation, snow melt, or irrigation in excess of what can infiltrate the soil surface and be stored in small surface depressions; a major transporter of nonpoint source pollutants. "@en;
  skos:inScheme :epa-abg;
  skosxl:prefLabel :xl_en_0c3cb97d .

:xl_en_0c3cb97d a skosxl:Label;
  skosxl:literalForm "Surface Runoff"@en .

:c_64990663 a :Terms;
  skos:broader :Ecology, :Water_Quality;
  skos:definition "All water naturally open to the atmosphere (rivers, lakes, reservoirs, ponds, streams, impoundments, seas, estuaries, etc.) and all springs, wells, or other collectors directly influenced by surface water. "@en;
  skos:inScheme :epa-abg;
  skosxl:prefLabel :xl_en_a60a3cf4 .

:xl_en_a60a3cf4 a skosxl:Label;
  skosxl:literalForm "Surface Water"@en .

:c_7e8fb6ba a :Terms;
  skos:broader :Ecology, :Water_Quality;
  skos:definition "Small particles of solid pollutants that float on the surface of, or are suspended in, sewage or other liquids. They resist removal by conventional means. "@en;
  skos:inScheme :epa-abg;
  skosxl:prefLabel :xl_en_c676dcd9 .

:xl_en_c676dcd9 a skosxl:Label;
  skosxl:literalForm "Suspended Solids"@en .

:c_d54bff58 a :Terms;
  skos:broader :Ecology, :Water_Quality;
  skos:definition "a grouping of organisms given a formal taxonomic name such as species, genus, family, etc. "@en;
  skos:inScheme :epa-abg;
  skosxl:prefLabel :xl_en_f6b696c4 .

:xl_en_f6b696c4 a skosxl:Label;
  skosxl:literalForm "Taxa"@en .

:c_09460d77 a :Terms;
  skos:broader :Ecology, :Water_Quality;
  skos:definition "Preferred Term: Metalimnion "@en;
  skos:inScheme :epa-abg;
  skosxl:prefLabel :xl_en_3b3b282e .

:xl_en_3b3b282e a skosxl:Label;
  skosxl:literalForm "Thermocline"@en .

:c_a709c1ee a :Terms;
  skos:broader :Ecology, :Water_Quality;
  skos:definition "Plowing, seedbed preparation, and cultivation practices. "@en;
  skos:inScheme :epa-abg;
  skosxl:prefLabel :xl_en_a2519c8d .

:xl_en_a2519c8d a skosxl:Label;
  skosxl:literalForm "Tillage"@en .

:c_2d97a8c4 a :Terms;
  skos:broader :Ecology, :Water_Quality;
  skos:definition "The physical features of a surface area including relative elevations and the position of natural and man-made features. "@en;
  skos:inScheme :epa-abg;
  skosxl:prefLabel :xl_en_a1f6dbf8 .

:xl_en_a1f6dbf8 a skosxl:Label;
  skosxl:literalForm "Topography"@en .

:c_1769f129 a :Terms;
  skos:broader :Ecology, :Water_Quality;
  skos:definition """Calculation of the maximum amount of a pollutant that a waterbody can receive and still meet water quality standards and an allocation of that amount to the pollutant's source. 
Acronym: TMDL """@en;
  skos:inScheme :epa-abg;
  skosxl:altLabel :xl_en_db9d4e05;
  skosxl:prefLabel :xl_en_6ccaf363 .

:xl_en_6ccaf363 a skosxl:Label;
  skosxl:literalForm "Total Maximum Daily Loads"@en .

:xl_en_db9d4e05 a skosxl:Label;
  skosxl:literalForm "TMDL"@en .

:c_9da283c9 a :Terms;
  skos:broader :Ecology, :Water_Quality;
  skos:definition "A method of monitoring particulate matter by total weight. "@en;
  skos:inScheme :epa-abg;
  skosxl:prefLabel :xl_en_76996df5 .

:xl_en_76996df5 a skosxl:Label;
  skosxl:literalForm "Total Suspended Particles"@en .

:c_67b80a28 a :Terms;
  skos:broader :Ecology, :Water_Quality;
  skos:definition """A measure of the suspended solids in wastewater, effluent, or water bodies, determined by tests for total suspended nonfilterable solids. 
Acronym: TSS """@en;
  skos:inScheme :epa-abg;
  skosxl:altLabel :xl_en_fd41f663;
  skosxl:prefLabel :xl_en_678bbc2c .

:xl_en_678bbc2c a skosxl:Label;
  skosxl:literalForm "Total Suspended Solids"@en .

:xl_en_fd41f663 a skosxl:Label;
  skosxl:literalForm "TSS"@en .

:c_51ac3765 a :Terms;
  skos:broader :Ecology, :Water_Quality;
  skos:definition "Materials that cause death, disease, or birth defects in organisms that ingest or absorb them. The quantities and exposures necessary to cause these effects can vary widely. "@en;
  skos:inScheme :epa-abg;
  skosxl:prefLabel :xl_en_701669d3 .

:xl_en_701669d3 a skosxl:Label;
  skosxl:literalForm "Toxic Pollutants"@en .

:c_35819cc0 a :Terms;
  skos:broader :Ecology, :Water_Quality;
  skos:definition "The quality or degree of being poisonous or harmful to plant or animal life. "@en;
  skos:inScheme :epa-abg;
  skosxl:prefLabel :xl_en_9e112e6d .

:xl_en_9e112e6d a skosxl:Label;
  skosxl:literalForm "Toxicity"@en .

:c_074149dd a :Terms;
  skos:broader :Ecology, :Water_Quality;
  skos:definition "The loss of water vapor by plants through tiny holes in their leaves called stomata. According to Environment Canada, an actively growing plant may transpire as much as ten times the amount of water it can hold at once within a twenty-four hour period. "@en;
  skos:inScheme :epa-abg;
  skosxl:prefLabel :xl_en_48644c98 .

:xl_en_48644c98 a skosxl:Label;
  skosxl:literalForm "Transpiration"@en .

:c_9ee7e4e6 a :Terms;
  skos:broader :Ecology, :Water_Quality;
  skos:definition "A stream or other body of water, surface or underground, which intermittently contributes its water in small quantities to another larger stream or body of water. "@en;
  skos:inScheme :epa-abg;
  skosxl:prefLabel :xl_en_b0fb0208 .

:xl_en_b0fb0208 a skosxl:Label;
  skosxl:literalForm "Tributary"@en .

:c_1a1186ee a :Terms;
  skos:broader :Ecology, :Water_Quality;
  skos:definition "Available phosphate content and subsequent biological productivity. "@en;
  skos:inScheme :epa-abg;
  skosxl:prefLabel :xl_en_2dba9d19 .

:xl_en_2dba9d19 a skosxl:Label;
  skosxl:literalForm "Trophic Status"@en .

:c_ba09dc70 a :Terms;
  skos:broader :Ecology, :Water_Quality;
  skos:definition "Storm water from city streets and adjacent domestic or commercial properties that carries pollutants of various kinds into the sewer systems and receiving waters. "@en;
  skos:inScheme :epa-abg;
  skosxl:prefLabel :xl_en_0afe1ccc .

:xl_en_0afe1ccc a skosxl:Label;
  skosxl:literalForm "Urban Runoff"@en .

:c_4d16deb7 a :Terms;
  skos:broader :Ecology, :Water_Quality;
  skos:definition """Analysis that describes factors limiting designated use of waterbodies. 
Acronym: UAA """@en;
  skos:inScheme :epa-abg;
  skosxl:altLabel :xl_en_66aab3ee;
  skosxl:prefLabel :xl_en_298ae236 .

:xl_en_298ae236 a skosxl:Label;
  skosxl:literalForm "Use Attainability Analysis"@en .

:xl_en_66aab3ee a skosxl:Label;
  skosxl:literalForm "UAA"@en .

:c_29198b40 a :Terms;
  skos:broader :Ecology, :Water_Quality;
  skos:definition "Water carrying wastes from homes, businesses and industries that is a mixture of water and dissolved or suspended solids. "@en;
  skos:inScheme :epa-abg;
  skosxl:prefLabel :xl_en_80fb1844 .

:xl_en_80fb1844 a skosxl:Label;
  skosxl:literalForm "Waste Water"@en .

:c_cb7d7def a :Terms;
  skos:broader :Ecology, :Water_Quality;
  skos:definition "The process, also known as the hydrologic cycle, in which water travels in a sequence from the air through condensation to the earth as precipitation and back to the atmosphere by evaporation. "@en;
  skos:inScheme :epa-abg;
  skosxl:prefLabel :xl_en_eb83508e .

:xl_en_eb83508e a skosxl:Label;
  skosxl:literalForm "Water Cycle"@en .

:c_22184162 a :Terms;
  skos:broader :Ecology, :Water_Quality;
  skos:definition "The addition of sewage, industrial wastes or other harmful or objectionable material to water in concentrations or in sufficient quantities to result in measurable degradation of water quality. "@en;
  skos:inScheme :epa-abg;
  skosxl:prefLabel :xl_en_4b7c6057 .

:xl_en_4b7c6057 a skosxl:Label;
  skosxl:literalForm "Water Pollution"@en .

:c_55c4843f a :Terms;
  skos:broader :Ecology, :Water_Quality;
  skos:definition "Effluent limitations applied to dischargers when mere technology-based limitations would cause violations of water quality standards. Usually applied to discharges into small streams. "@en;
  skos:inScheme :epa-abg;
  skosxl:prefLabel :xl_en_ad4bcd43 .

:xl_en_ad4bcd43 a skosxl:Label;
  skosxl:literalForm "Water Quality-Based Limitations"@en .

:c_bd6dcbf7 a :Terms;
  skos:broader :Ecology, :Water_Quality;
  skos:definition "A permit with an effluent limit more stringent than one based on technology performance. Such limits may be necessary to protect the designated use of receiving waters (i.e., recreation, irrigation, industry or water supply). "@en;
  skos:inScheme :epa-abg;
  skosxl:prefLabel :xl_en_5dda21ff .

:xl_en_5dda21ff a skosxl:Label;
  skosxl:literalForm "Water Quality-Based Permit"@en .

:c_73d28241 a :Terms;
  skos:broader :Ecology, :Water_Quality;
  skos:definition "Levels of water quality expected to render a body of water suitable for its designated use. Criteria are based on specific levels of pollutants that would make the water harmful if used for drinking, swimming, farming, fish production, or industrial processes. "@en;
  skos:inScheme :epa-abg;
  skosxl:prefLabel :xl_en_b0f8920b .

:xl_en_b0f8920b a skosxl:Label;
  skosxl:literalForm "Water Quality Criteria"@en .

:c_2d4a117c a :Terms;
  skos:broader :Ecology, :Water_Quality;
  skos:definition "State-adopted and EPA-approved ambient standards for water bodies. The standards prescribe the use of the water body and establish the water quality criteria that must be met to protect designated uses. "@en;
  skos:inScheme :epa-abg;
  skosxl:prefLabel :xl_en_2749c8a4 .

:xl_en_2749c8a4 a skosxl:Label;
  skosxl:literalForm "Water Quality Standards"@en .

:c_e3657bb9 a :Terms;
  skos:broader :Ecology, :Water_Quality;
  skos:definition "The level or depth below the ground that is saturated with water. "@en;
  skos:inScheme :epa-abg;
  skosxl:prefLabel :xl_en_7a4e0c83 .

:xl_en_7a4e0c83 a skosxl:Label;
  skosxl:literalForm "Water Table"@en .

:c_ad742fe4 a :Terms;
  skos:broader :Ecology, :Water_Quality;
  skos:definition "Water diffused as a gas in the atmosphere. "@en;
  skos:inScheme :epa-abg;
  skosxl:prefLabel :xl_en_37f1e14a .

:xl_en_37f1e14a a skosxl:Label;
  skosxl:literalForm "Water Vapor"@en .

:c_1c8a8ea6 a :Terms;
  skos:broader :Ecology, :Water_Quality;
  skos:definition "The area of land from which rainfall (and/or snow melt) drains into a stream or other water body. Watersheds are also sometimes referred to as drainage basins or drainage areas. Ridges of higher ground generally form the boundaries between watersheds. At these boundaries, rain falling on one side flows toward the low point of one watershed, while rain falling on the other side of the boundary flows toward the low point of a different watershed. "@en;
  skos:inScheme :epa-abg;
  skosxl:prefLabel :xl_en_299b6a7b .

:xl_en_299b6a7b a skosxl:Label;
  skosxl:literalForm "Watershed"@en .

:c_5f617aa4 a :Terms;
  skos:broader :Ecology, :Water_Quality;
  skos:definition "A protected surface and subsurface zone surrounding a well or well field supplying a public water system to keep contaminants from reaching the well water. "@en;
  skos:inScheme :epa-abg;
  skosxl:prefLabel :xl_en_35b79874 .

:xl_en_35b79874 a skosxl:Label;
  skosxl:literalForm "Wellhead Protection Area"@en .

:c_421c959c a :Terms;
  skos:broader :Ecology, :Water_Quality;
  skos:definition "An area that is saturated by surface or ground water with vegetation adapted for life under those soil conditions, as swamps, bogs, fens, marshes, and estuaries. "@en;
  skos:inScheme :epa-abg;
  skosxl:prefLabel :xl_en_262e6e85 .

:xl_en_262e6e85 a skosxl:Label;
  skosxl:literalForm "Wetlands"@en .

:c_a4952f11 a :Terms;
  skos:broader :Ecology, :Water_Quality;
  skos:definition "Tiny, sometimes microscopic, floating, aquatic animals. Zooplankton generally feed upon phytoplankton and each other. "@en;
  skos:inScheme :epa-abg;
  skosxl:prefLabel :xl_en_7ad39b2e .

:xl_en_7ad39b2e a skosxl:Label;
  skosxl:literalForm "Zooplankton"@en .

:c_ccce6454 a skos:Concept;
  dct:modified "2019-09-20T18:07:06.514Z"^^xsd:dateTime;
  skos:exactMatch :c_9c396253 .

:c_aaffcb42 a skos:Concept;
  dct:modified "2019-09-20T17:59:40.837Z"^^xsd:dateTime;
  skos:exactMatch :c_09460d77 .

:c_09460d77 a skos:Concept;
  dct:modified "2019-09-20T18:00:07.703Z"^^xsd:dateTime .

:c_ced4b01e a skos:Concept .

:c_12032ab6 a skos:Concept;
  dct:modified "2019-09-26T18:03:06.676Z"^^xsd:dateTime .

:c_28a146be a skos:Concept;
  dct:modified "2019-09-26T18:03:00.217Z"^^xsd:dateTime;
  skos:topConceptOf :epa-abg .

:c_d2baf0fd a skos:Concept;
  dct:modified "2019-09-20T18:14:14.075Z"^^xsd:dateTime .

:c_5a1e1954 a skos:Concept;
  dct:modified "2019-09-20T18:14:21.209Z"^^xsd:dateTime .

:c_2f897ccc a skos:Concept;
  dct:modified "2019-09-20T18:14:29.047Z"^^xsd:dateTime .

:c_ee107987 a skos:Concept;
  dct:modified "2019-09-20T18:14:36.356Z"^^xsd:dateTime .

:c_3d964577 a skos:Concept;
  dct:modified "2019-09-20T18:14:48.730Z"^^xsd:dateTime .

:c_773b7b6c a skos:Concept;
  dct:modified "2019-09-20T18:15:00.422Z"^^xsd:dateTime .

:AL skos:broader :State_Government;
  skos:inScheme :glos;
  skosxl:prefLabel :xl_en_cd1e6cd8 .

:xl_en_cd1e6cd8 a skosxl:Label;
  skosxl:literalForm "Alabama"@en .

:AK a skos:Concept;
  skos:broader :State_Government;
  skos:inScheme :glos;
  skosxl:prefLabel :xl_en_e4e8620f .

:xl_en_e4e8620f a skosxl:Label;
  skosxl:literalForm "Alaska"@en .

:AZ a skos:Concept;
  skos:broader :State_Government;
  skos:inScheme :glos;
  skosxl:prefLabel :xl_en_5c522467 .

:xl_en_5c522467 a skosxl:Label;
  skosxl:literalForm "Arizona"@en .

:AR a skos:Concept;
  skos:broader :State_Government;
  skos:inScheme :glos;
  skosxl:prefLabel :xl_en_4f73164a .

:xl_en_4f73164a a skosxl:Label;
  skosxl:literalForm "Arkansas"@en .

:CA a skos:Concept;
  skos:broader :State_Government;
  skos:inScheme :glos;
  skosxl:prefLabel :xl_en_603dcfb7 .

:xl_en_603dcfb7 a skosxl:Label;
  skosxl:literalForm "California"@en .

:CO a skos:Concept;
  skos:broader :State_Government;
  skos:inScheme :glos;
  skosxl:prefLabel :xl_en_0d526696 .

:xl_en_0d526696 a skosxl:Label;
  skosxl:literalForm "Colorado"@en .

:CT a skos:Concept;
  skos:broader :State_Government;
  skos:inScheme :glos;
  skosxl:prefLabel :xl_en_19805012 .

:xl_en_19805012 a skosxl:Label;
  skosxl:literalForm "Connecticut"@en .

:DE a skos:Concept;
  skos:broader :State_Government;
  skos:inScheme :glos;
  skosxl:prefLabel :xl_en_39bb956f .

:xl_en_39bb956f a skosxl:Label;
  skosxl:literalForm "Delaware"@en .

:DC a skos:Concept;
  skos:broader :State_Government;
  skos:inScheme :glos;
  skosxl:prefLabel :xl_en_99ca8872 .

:xl_en_99ca8872 a skosxl:Label;
  skosxl:literalForm "District Of Columbia"@en .

:FL a skos:Concept;
  skos:broader :State_Government;
  skos:inScheme :glos;
  skosxl:prefLabel :xl_en_acbd8dcb .

:xl_en_acbd8dcb a skosxl:Label;
  skosxl:literalForm "Florida"@en .

:GA a skos:Concept;
  skos:broader :State_Government;
  skos:inScheme :glos;
  skosxl:prefLabel :xl_en_11577149 .

:xl_en_11577149 a skosxl:Label;
  skosxl:literalForm "Georgia"@en .

:HI a skos:Concept;
  skos:broader :State_Government;
  skos:inScheme :glos;
  skosxl:prefLabel :xl_en_69fba1a9 .

:xl_en_69fba1a9 a skosxl:Label;
  skosxl:literalForm "Hawaii"@en .

:ID a skos:Concept;
  skos:broader :State_Government;
  skos:inScheme :glos;
  skosxl:prefLabel :xl_en_930d43f0 .

:xl_en_930d43f0 a skosxl:Label;
  skosxl:literalForm "Idaho"@en .

:IL a skos:Concept;
  skos:broader :State_Government;
  skos:inScheme :glos;
  skosxl:prefLabel :xl_en_190d53f6 .

:xl_en_190d53f6 a skosxl:Label;
  skosxl:literalForm "Illinois"@en .

:IN a skos:Concept;
  skos:broader :State_Government;
  skos:inScheme :glos;
  skosxl:prefLabel :xl_en_e324a738 .

:xl_en_e324a738 a skosxl:Label;
  skosxl:literalForm "Indiana"@en .

:IA a skos:Concept;
  skos:broader :State_Government;
  skos:inScheme :glos;
  skosxl:prefLabel :xl_en_9ab4a9bc .

:xl_en_9ab4a9bc a skosxl:Label;
  skosxl:literalForm "Iowa"@en .

:KS a skos:Concept;
  skos:broader :State_Government;
  skos:inScheme :glos;
  skosxl:prefLabel :xl_en_5766d777 .

:xl_en_5766d777 a skosxl:Label;
  skosxl:literalForm "Kansas"@en .

:KY a skos:Concept;
  skos:broader :State_Government;
  skos:inScheme :glos;
  skosxl:prefLabel :xl_en_c6df51e3 .

:xl_en_c6df51e3 a skosxl:Label;
  skosxl:literalForm "Kentucky"@en .

:LA a skos:Concept;
  skos:broader :State_Government;
  skos:inScheme :glos;
  skosxl:prefLabel :xl_en_a973deac .

:xl_en_a973deac a skosxl:Label;
  skosxl:literalForm "Louisiana"@en .

:ME a skos:Concept;
  skos:broader :State_Government;
  skos:inScheme :glos;
  skosxl:prefLabel :xl_en_d5cae8fb .

:xl_en_d5cae8fb a skosxl:Label;
  skosxl:literalForm "Maine"@en .

:MD a skos:Concept;
  skos:broader :State_Government;
  skos:inScheme :glos;
  skosxl:prefLabel :xl_en_d25b8fdb .

:xl_en_d25b8fdb a skosxl:Label;
  skosxl:literalForm "Maryland"@en .

:MA a skos:Concept;
  skos:broader :State_Government;
  skos:inScheme :glos;
  skosxl:prefLabel :xl_en_dc7293b7 .

:xl_en_dc7293b7 a skosxl:Label;
  skosxl:literalForm "Massachusetts"@en .

:MI a skos:Concept;
  skos:broader :State_Government;
  skos:inScheme :glos;
  skosxl:prefLabel :xl_en_9c3c3626 .

:xl_en_9c3c3626 a skosxl:Label;
  skosxl:literalForm "Michigan"@en .

:MN a skos:Concept;
  skos:broader :State_Government;
  skos:inScheme :glos;
  skosxl:prefLabel :xl_en_33daef1d .

:xl_en_33daef1d a skosxl:Label;
  skosxl:literalForm "Minnesota"@en .

:MS a skos:Concept;
  skos:broader :State_Government;
  skos:inScheme :glos;
  skosxl:prefLabel :xl_en_b242837b .

:xl_en_b242837b a skosxl:Label;
  skosxl:literalForm "Mississippi"@en .

:MO a skos:Concept;
  skos:broader :State_Government;
  skos:inScheme :glos;
  skosxl:prefLabel :xl_en_16376a29 .

:xl_en_16376a29 a skosxl:Label;
  skosxl:literalForm "Missouri"@en .

:MT a skos:Concept;
  skos:broader :State_Government;
  skos:inScheme :glos;
  skosxl:prefLabel :xl_en_bbb0bdfe .

:xl_en_bbb0bdfe a skosxl:Label;
  skosxl:literalForm "Montana"@en .

:NE a skos:Concept;
  skos:broader :State_Government;
  skos:inScheme :glos;
  skosxl:prefLabel :xl_en_284bbe15 .

:xl_en_284bbe15 a skosxl:Label;
  skosxl:literalForm "Nebraska"@en .

:NV a skos:Concept;
  skos:broader :State_Government;
  skos:inScheme :glos;
  skosxl:prefLabel :xl_en_b0cb2b3a .

:xl_en_b0cb2b3a a skosxl:Label;
  skosxl:literalForm "Nevada"@en .

:NH a skos:Concept;
  skos:broader :State_Government;
  skos:inScheme :glos;
  skosxl:prefLabel :xl_en_a510697c .

:xl_en_a510697c a skosxl:Label;
  skosxl:literalForm "New Hampshire"@en .

:NJ a skos:Concept;
  skos:broader :State_Government;
  skos:inScheme :glos;
  skosxl:prefLabel :xl_en_43b772e1 .

:xl_en_43b772e1 a skosxl:Label;
  skosxl:literalForm "New Jersey"@en .

:NM a skos:Concept;
  skos:broader :State_Government;
  skos:inScheme :glos;
  skosxl:prefLabel :xl_en_da7a6531 .

:xl_en_da7a6531 a skosxl:Label;
  skosxl:literalForm "New Mexico"@en .

:NY a skos:Concept;
  skos:broader :State_Government;
  skos:inScheme :glos;
  skosxl:prefLabel :xl_en_422d1106 .

:xl_en_422d1106 a skosxl:Label;
  skosxl:literalForm "New York"@en .

:NC a skos:Concept;
  skos:broader :State_Government;
  skos:inScheme :glos;
  skosxl:prefLabel :xl_en_c60eb531 .

:xl_en_c60eb531 a skosxl:Label;
  skosxl:literalForm "North Carolina"@en .

:ND a skos:Concept;
  skos:broader :State_Government;
  skos:inScheme :glos;
  skosxl:prefLabel :xl_en_713680ea .

:xl_en_713680ea a skosxl:Label;
  skosxl:literalForm "North Dakota"@en .

:OH a skos:Concept;
  skos:broader :State_Government;
  skos:inScheme :glos;
  skosxl:prefLabel :xl_en_633f7447 .

:xl_en_633f7447 a skosxl:Label;
  skosxl:literalForm "Ohio"@en .

:OK a skos:Concept;
  skos:broader :State_Government;
  skos:inScheme :glos;
  skosxl:prefLabel :xl_en_5649f870 .

:xl_en_5649f870 a skosxl:Label;
  skosxl:literalForm "Oklahoma"@en .

:OR a skos:Concept;
  skos:broader :State_Government;
  skos:inScheme :glos;
  skosxl:prefLabel :xl_en_b10c8f21 .

:xl_en_b10c8f21 a skosxl:Label;
  skosxl:literalForm "Oregon"@en .

:PA a skos:Concept;
  skos:broader :State_Government;
  skos:inScheme :glos;
  skosxl:prefLabel :xl_en_0e9c3d02 .

:xl_en_0e9c3d02 a skosxl:Label;
  skosxl:literalForm "Pennsylvania"@en .

:PR a skos:Concept;
  skos:broader :State_Government;
  skos:inScheme :glos;
  skosxl:prefLabel :xl_en_27fef139 .

:xl_en_27fef139 a skosxl:Label;
  skosxl:literalForm "Puerto Rico"@en .

:RI a skos:Concept;
  skos:broader :State_Government;
  skos:inScheme :glos;
  skosxl:prefLabel :xl_en_c3e0021b .

:xl_en_c3e0021b a skosxl:Label;
  skosxl:literalForm "Rhode Island"@en .

:SC a skos:Concept;
  skos:broader :State_Government;
  skos:inScheme :glos;
  skosxl:prefLabel :xl_en_e66079fe .

:xl_en_e66079fe a skosxl:Label;
  skosxl:literalForm "South Carolina"@en .

:SD a skos:Concept;
  skos:broader :State_Government;
  skos:inScheme :glos;
  skosxl:prefLabel :xl_en_8ae220e3 .

:xl_en_8ae220e3 a skosxl:Label;
  skosxl:literalForm "South Dakota"@en .

:TN a skos:Concept;
  skos:broader :State_Government;
  skos:inScheme :glos;
  skosxl:prefLabel :xl_en_1a46163c .

:xl_en_1a46163c a skosxl:Label;
  skosxl:literalForm "Tennessee"@en .

:TX a skos:Concept;
  skos:broader :State_Government;
  skos:inScheme :glos;
  skosxl:prefLabel :xl_en_dced9c4f .

:xl_en_dced9c4f a skosxl:Label;
  skosxl:literalForm "Texas"@en .

:UT a skos:Concept;
  skos:broader :State_Government;
  skos:inScheme :glos;
  skosxl:prefLabel :xl_en_78528d6c .

:xl_en_78528d6c a skosxl:Label;
  skosxl:literalForm "Utah"@en .

:VT a skos:Concept;
  skos:broader :State_Government;
  skos:inScheme :glos;
  skosxl:prefLabel :xl_en_942829bc .

:xl_en_942829bc a skosxl:Label;
  skosxl:literalForm "Vermont"@en .

:VA a skos:Concept;
  skos:broader :State_Government;
  skos:inScheme :glos;
  skosxl:prefLabel :xl_en_fc786aac .

:xl_en_fc786aac a skosxl:Label;
  skosxl:literalForm "Virginia"@en .

:WA a skos:Concept;
  skos:broader :State_Government;
  skos:inScheme :glos;
  skosxl:prefLabel :xl_en_899c052e .

:xl_en_899c052e a skosxl:Label;
  skosxl:literalForm "Washington"@en .

:WV a skos:Concept;
  skos:broader :State_Government;
  skos:inScheme :glos;
  skosxl:prefLabel :xl_en_a905b930 .

:xl_en_a905b930 a skosxl:Label;
  skosxl:literalForm "West Virginia"@en .

:WI a skos:Concept;
  skos:broader :State_Government;
  skos:inScheme :glos;
  skosxl:prefLabel :xl_en_72786cee .

:xl_en_72786cee a skosxl:Label;
  skosxl:literalForm "Wisconsin"@en .

:WY a skos:Concept;
  skos:broader :State_Government;
  skos:inScheme :glos;
  skosxl:prefLabel :xl_en_e63554c9 .

:xl_en_e63554c9 a skosxl:Label;
  skosxl:literalForm "Wyoming"@en .

:CA-DWR a skos:Concept;
  dct:created "2019-09-24T19:31:58.296Z"^^xsd:dateTime;
  skos:broader :CA;
  skos:inScheme :glos;
  skosxl:altLabel :xl_en_9e4c594c;
  skosxl:prefLabel :xl_en_4e3c7492 .

:ca-dwr-g skos:definition "This glossary contains terms used in the text of California Water Plan Update 2018 as well as additional terms related to water resources." .

:xl_en_4e3c7492 a skosxl:Label;
  dct:created "2019-09-24T19:31:58.296Z"^^xsd:dateTime;
  skosxl:literalForm "California Department of Water Resources"@en .

:xl_en_9e4c594c a skosxl:Label;
  dct:created "2019-09-24T19:38:46.646Z"^^xsd:dateTime;
  skosxl:literalForm "CA-DWR"@en .

:xl_en_4a969c94 dct:modified "2019-09-24T22:04:47.229Z"^^xsd:dateTime .

:xl_en_fc31e317 dct:created "2019-09-26T17:45:03.954Z"^^xsd:dateTime .

:c_12032ab6 skos:topConceptOf :epa-abg .

:c_ced4b01e dct:modified "2019-09-26T18:02:53.894Z"^^xsd:dateTime;
  skos:topConceptOf :epa-abg .

:c_1c3d1b27 skos:broader :Water_Use .

:c_5e095931 a :Terms, skos:Concept;
  skos:broader :Beneficial_Use, :Water_Use;
  skos:definition """water use associated with the production of fish in captivity except for fish hatcheries which were in Commercial, and the raising of horses and such fur-bearing animals as rabbits and pets. 

    1985: Fish farming included in Livestock
    1990-1995: Animal specialties (excludes fish hatcheries)
    2000 and later: former Animal specialties use reported in Livestock (horses) and Aquaculture categories (fish hatcheries and fish farms)

See also aquaculture water use, fish-hatchery water use, livestock water use, and rural water use."""@en;
  skos:inScheme :usgs-wut;
  skos:topConceptOf :usgs-wut;
  skosxl:prefLabel :xl_en_8b92744d .

:xl_en_8b92744d a skosxl:Label;
  skosxl:literalForm "animal-specialties water use"@en .

:c_5cc31c7e a :Terms, skos:Concept;
  skos:broader :Beneficial_Use, :Water_Use;
  skos:definition "water use associated with the farming of finfish, shellfish, and other organisms that live in water, and offstream water use associated with fish hatcheries.     1985: Water use for fish farming included in Livestock    1990-1995: Water use was reported in Animal Specialties (fish farming) and Commercial (fish hatcheries)    2000 and later: AquacultureSee also animal-specialties water use, commercial water use, and livestock water use, and Methods for Estimating Water Withdrawals for Aquaculture in the United States, 2005."@en;
  skos:inScheme :usgs-wut;
  skos:topConceptOf :usgs-wut;
  skosxl:prefLabel :xl_en_03803609 .

:xl_en_03803609 a skosxl:Label;
  skosxl:literalForm "aquaculture water use"@en .

:c_631994db a :Terms, skos:Concept;
  skos:broader :Water_Use;
  skos:definition "see recirculation cooling system."@en;
  skos:inScheme :usgs-wut;
  skos:topConceptOf :usgs-wut;
  skosxl:prefLabel :xl_en_02fa019c .

:xl_en_02fa019c a skosxl:Label;
  skosxl:literalForm "closed-loop cooling system"@en .

:c_8d90330f a :Terms, skos:Concept;
  skos:broader :Beneficial_Use, :Water_Use;
  skos:definition """water for motels, hotels, restaurants, office buildings, other commercial facilities, military and nonmilitary institutions, and (for 1990 and 1995) offstream fish hatcheries.  Water may be obtained from a public-supply system or may be self-supplied.  Commercial water-use estimates were included in industrial water use until 1985, then were reported as a separate category. Commercial water use estimates were last reported nationally for 1995.

    1985: Self-supplied commercial water use first reported as separate category from industrial
    1990-1995: Commercial category includes offstream fish hatchery water use for some States
    2000 and later: Commercial category not estimated nationally: offstream fish hatchery water use is reported in the Aquaculture category

See also fish-hatchery water use, public-supply water use, public-supply deliveries, industrial water use, and self-supplied water use."""@en;
  skos:inScheme :usgs-wut;
  skos:topConceptOf :usgs-wut;
  skosxl:prefLabel :xl_en_da71ef82 .

:xl_en_da71ef82 a skosxl:Label;
  skosxl:literalForm "commercial water use"@en .

:c_e3620d23 a :Terms, skos:Concept;
  skos:broader :Water_Use;
  skos:definition """the part of water withdrawn that is evaporated, transpired, incorporated into products or crops, consumed by humans or livestock, or otherwise not available for immediate use.  Water returned to a different watershed than the point of withdrawal (interbasin transfer) is not considered a consumptive use. Also referred to as water consumed. 

    1960-1995: Consumptive use reported by water-use category
    2000-2010: Consumptive use not estimated nationally
    2015: Consumptive use reported for irrigation and thermoelectric power categories"""@en;
  skos:inScheme :usgs-wut;
  skos:topConceptOf :usgs-wut;
  skosxl:prefLabel :xl_en_b2e48f30 .

:xl_en_b2e48f30 a skosxl:Label;
  skosxl:literalForm "consumptive use"@en .

:c_d764033f a :Terms, skos:Concept;
  skos:broader :Water_Use;
  skos:definition """water that is lost in transit from a pipe, canal, conduit, or ditch by leakage or evaporation. Leakage from an irrigation ditch, for example, may percolate to a groundwater source and be available for further use.

    1955-1995: Conveyance losses reported nationally
    2000 and later: Conveyance losses not estimated nationally

See also irrigation water use."""@en;
  skos:inScheme :usgs-wut;
  skos:topConceptOf :usgs-wut;
  skosxl:prefLabel :xl_en_c2f431c8 .

:xl_en_c2f431c8 a skosxl:Label;
  skosxl:literalForm "conveyance loss"@en .

:c_d428b229 a :Terms, skos:Concept;
  skos:broader :Beneficial_Use, :Water_Use;
  skos:definition "an equipment system that provides water for cooling purposes, such as to condensers at power plants or at factories, subdivided into once-through or recirculation cooling system. See also industrial water use, once-through cooling system, recirculation cooling system, and thermoelectric-power water use."@en;
  skos:inScheme :usgs-wut;
  skos:topConceptOf :usgs-wut;
  skosxl:prefLabel :xl_en_66fdc9a7 .

:xl_en_66fdc9a7 a skosxl:Label;
  skosxl:literalForm "cooling-system type"@en .

:c_5fb36e22 a :Terms, skos:Concept;
  skos:broader :Beneficial_Use, :Water_Use;
  skos:definition """water used for indoor household purposes such as drinking, food preparation, bathing, washing clothes and dishes, flushing toilets, and outdoor purposes such as watering lawns and gardens. Domestic water use includes potable and non-potable water provided to households by a public water supplier (domestic deliveries) and self-supplied water.  

    1950-1955: Rural (included Livestock: estimates were retroactively allocated to Rural Domestic and Livestock in later reports)
    1960-1980: Rural Domestic
    1985 and later: Domestic

See also public-supply deliveries, public-supply water use, rural water use, and self-supplied water use."""@en;
  skos:inScheme :usgs-wut;
  skos:topConceptOf :usgs-wut;
  skosxl:prefLabel :xl_en_063c2162 .

:xl_en_063c2162 a skosxl:Label;
  skosxl:literalForm "domestic water use"@en .

:c_1ff194d9 a :Terms, skos:Concept;
  skos:broader :Beneficial_Use, :Water_Use;
  skos:definition "See  aquaculture water use, commercial water use, and animal specialities water use."@en;
  skos:inScheme :usgs-wut;
  skos:topConceptOf :usgs-wut;
  skosxl:prefLabel :xl_en_4e74bc6f .

:xl_en_4e74bc6f a skosxl:Label;
  skosxl:literalForm "fish-hatchery water use"@en .

:c_265fb99a a :Terms, skos:Concept;
  skos:broader :Water_Use;
  skos:definition "water that contains less than 1,000 milligrams per liter (mg/L) of dissolved solids.  Generally, water with more than 500 mg/L of dissolved solids is undesirable for drinking and many industrial uses. See also saline water."@en;
  skos:inScheme :usgs-wut;
  skos:topConceptOf :usgs-wut;
  skosxl:prefLabel :xl_en_6ea3daf7 .

:xl_en_6ea3daf7 a skosxl:Label;
  skosxl:literalForm "freshwater"@en .

:c_881d1b90 a :Terms, skos:Concept;
  skos:broader :Beneficial_Use, :Water_Use;
  skos:definition "see thermoelectric power water use."@en;
  skos:inScheme :usgs-wut;
  skos:topConceptOf :usgs-wut;
  skosxl:prefLabel :xl_en_62102842 .

:xl_en_62102842 a skosxl:Label;
  skosxl:literalForm "fuel-electric power"@en .

:c_a6ee839e a :Terms, skos:Concept;
  skos:broader :Beneficial_Use, :Water_Use;
  skos:definition """the use of water in the generation of electricity at plants where the turbine generators are driven by moving water. Hydroelectric water use is most commonly an instream use. Hydroelectric power water use was referred to as water power from 1950-1960.

    1950-1960: Water Power
    1965-1995: Hydroelectric Power
    2000 and later: Hydroelectric Power category not estimated nationally"""@en;
  skos:inScheme :usgs-wut;
  skos:topConceptOf :usgs-wut;
  skosxl:prefLabel :xl_en_ad44cd8a .

:xl_en_ad44cd8a a skosxl:Label;
  skosxl:literalForm "hydroelectric power water use"@en .

:c_4611a1b6 a :Terms, skos:Concept;
  skos:broader :Beneficial_Use, :Water_Use;
  skos:definition """water used for fabrication, processing, washing, and cooling.  Includes industries such as chemical and allied products, food, mining, paper and allied products, petroleum refining, and steel. 

    1950: Industrial, included thermoelectric power use
    1955: Industrial, included thermoelectric power use, subtotals for thermoelectric power use (fuel-electric power) and other provided by watershed but not by State
    1960-1980: Industrial, included thermoelectric power use, subtotals for thermoelectric power use (fuel-electric power) and \"other industrial\" uses
    1985 and later: Industrial. Separate categories for thermoelectric power, self-supplied commercial and mining split from other industrial. The term industrial water use was used 1985-1995 to describe the combined public-supply deliveries to industrial users and self-supplied industrial withdrawals.

See also thermoelectric-power water use, commercial water use, mining water use, public-supply deliveries, public-supply water use, and self-supplied water use."""@en;
  skos:inScheme :usgs-wut;
  skos:topConceptOf :usgs-wut;
  skosxl:prefLabel :xl_en_85671346 .

:xl_en_85671346 a skosxl:Label;
  skosxl:literalForm "industrial water use"@en .

:c_4f8328ff a :Terms, skos:Concept;
  skos:broader :Water_Use;
  skos:definition "water that is used, but not withdrawn, from a surface-water source for such purposes as hydroelectric-power generation, navigation, water-quality improvement, fish propagation, and recreation. Instream uses may change the flow characteristics or increase evaporative losses due to impoundments and release schedules. Instream water-use estimates for hydroelectric power were included in some previous water-use circulars but were omitted for 2000 to present."@en;
  skos:inScheme :usgs-wut;
  skos:topConceptOf :usgs-wut;
  skosxl:prefLabel :xl_en_07a12a12 .

:xl_en_07a12a12 a skosxl:Label;
  skosxl:literalForm "instream use"@en .

:c_e48beb59 a :Terms, skos:Concept;
  skos:broader :Water_Use;
  skos:definition "A transfer of water from one river basin to another. Interbasin transfers may be tracked or regulated for different levels of watersheds such as a hydrologic unit level or a set of basin delineations made by a regulatory authority."@en;
  skos:inScheme :usgs-wut;
  skos:topConceptOf :usgs-wut;
  skosxl:prefLabel :xl_en_5f354e30 .

:xl_en_5f354e30 a skosxl:Label;
  skosxl:literalForm "interbasin transfer"@en .

:c_cf4d74ad a :Terms, skos:Concept;
  skos:broader :Beneficial_Use, :Water_Use;
  skos:definition "water that is applied by an irrigation system to assist crop and pasture growth, or to maintain vegetation on recreational lands such as parks and golf courses. Irrigation includes water that is applied for pre-irrigation, frost protection, chemical application, weed control, field preparation, harvesting, dust suppression, leaching of salts from the root zone. Irrigation water use estimates also include conveyance losses.See also conveyance loss, microirrigation system, sprinkler irrigation system, and surface irrigation system."@en;
  skos:inScheme :usgs-wut;
  skos:topConceptOf :usgs-wut;
  skosxl:prefLabel :xl_en_feb6bd85 .

:xl_en_feb6bd85 a skosxl:Label;
  skosxl:literalForm "irrigation water use"@en .

:c_8b39828f a :Terms, skos:Concept;
  skos:broader :Beneficial_Use, :Water_Use;
  skos:definition """water used for livestock watering, feedlots, dairy operations, and other on-farm needs. Types of livestock include dairy cows and heifers, beef cattle and calves, sheep and lambs, goats, hogs and pigs, horses and poultry.

    1950: Rural (included self-supplied domestic: estimates were allocated to Rural Domestic and Livestock in later reports)
    1960-1980: Livestock subcatgory under Rural
    1985: Livestock, including water use for fish farming
    1990-1995: Livestock. Subcategory of Animal Specialties included horses and fish farming
    2000 and later: Livestock. Separate category of Aquaculture includes fish farming and fish hatcheries

See also animal-specialties water use, aquaculture water use, and rural water use, and Method for Estimating Water Withdrawals for Livestock in the United States, 2005."""@en;
  skos:inScheme :usgs-wut;
  skos:topConceptOf :usgs-wut;
  skosxl:prefLabel :xl_en_7752f9e7 .

:xl_en_7752f9e7 a skosxl:Label;
  skosxl:literalForm "livestock water use"@en .

:c_86ddc733 a :Terms, skos:Concept;
  skos:broader :Beneficial_Use, :Water_Use;
  skos:definition "an irrigation system that wets only a discrete portion of the soil surface in the vicinity of the plant by means of applicators (such as orifices, emitters, porous tubing, or perforated pipe) and operated under low pressure. The applicators may be placed on or below the surface of the ground or suspended from supports. See also irrigation water use, sprinkler irrigation system, and surface irrigation system."@en;
  skos:inScheme :usgs-wut;
  skos:topConceptOf :usgs-wut;
  skosxl:prefLabel :xl_en_7470e31c .

:xl_en_7470e31c a skosxl:Label;
  skosxl:literalForm "microirrigation system"@en .

:c_7adbbea3 a :Terms, skos:Concept;
  skos:broader :Beneficial_Use, :Water_Use;
  skos:definition """water used for the extraction of naturally occurring minerals including solids (such as coal, sand, gravel, and other ores), liquids (such as crude petroleum), and gases (such as natural gas).  Also includes uses associated with quarrying, milling and other preparations customarily done at the mine site, injection of water for secondary oil recovery or for unconventional oil and gas recovery (such as hydraulic fracturing), and other operations associated with mining activity.  Does not include water associated with dewatering of the aquifer that is not put to beneficial use. Also does not include water used in processing, such as smelting, refining petroleum, or slurry pipeline operations.  These processing uses are included in industrial water use.

    1950-1980: included in Industrial
    1985 and later: Mining

See also industrial water use and self-supplied water use, and Methods for Estimating Water Withdrawals for Mining in the United States, 2005."""@en;
  skos:inScheme :usgs-wut;
  skos:topConceptOf :usgs-wut;
  skosxl:prefLabel :xl_en_db063011 .

:xl_en_db063011 a skosxl:Label;
  skosxl:literalForm "mining water use"@en .

:c_85a58854 a :Terms, skos:Concept;
  skos:broader :Beneficial_Use, :Water_Use;
  skos:definition """public supply water use. Term used in 1950 water-use circular.

four-digit codes established by the Office of Management and Budget, published in 1987, and used in the classification of establishments by type of activity in which they are engaged."""@en;
  skos:inScheme :usgs-wut;
  skos:topConceptOf :usgs-wut;
  skosxl:prefLabel :xl_en_e74af7d8 .

:xl_en_e74af7d8 a skosxl:Label;
  skosxl:literalForm "municipal water use"@en .

:c_50185a6b a :Terms, skos:Concept;
  skos:broader :Beneficial_Use, :Water_Use;
  skos:definition "classification system used by Federal statistical agencies to classify establishments according to type of production or other economic activity. NAICS was adopted in 1997 to replace the Standard Industrial Classification system. "@en;
  skos:inScheme :usgs-wut;
  skos:topConceptOf :usgs-wut;
  skosxl:altLabel :xl_en_92a9e138;
  skosxl:prefLabel :xl_en_51a6ece9 .

:xl_en_51a6ece9 a skosxl:Label;
  skosxl:literalForm "North American Industry Classification System "@en .

:xl_en_92a9e138 a skosxl:Label;
  skosxl:literalForm "NAICS"@en .

:c_333fbc4c a :Terms, skos:Concept;
  skos:broader :Water_Use;
  skos:definition "water withdrawn or diverted from a groundwater or surface-water source for aquaculture, commercial, domestic self-supply, industrial, irrigation, livestock, mining, public supply, thermoelectric power, and other uses. See also entries for each of these categories of use."@en;
  skos:inScheme :usgs-wut;
  skos:topConceptOf :usgs-wut;
  skosxl:prefLabel :xl_en_e9e0af2f .

:xl_en_e9e0af2f a skosxl:Label;
  skosxl:literalForm "offstream use"@en .

:c_9180b163 a :Terms, skos:Concept;
  skos:broader :Beneficial_Use, :Water_Use;
  skos:definition "also known as open-loop cooling system. Cooling system in which the water is withdrawn from a source, circulated through the heat exchangers, and then returned to a body of water at a higher temperature. See also cooling system, cooling-system type, industrial water use, and thermoelectric-power water use."@en;
  skos:inScheme :usgs-wut;
  skos:topConceptOf :usgs-wut;
  skosxl:prefLabel :xl_en_1fac4c8a .

:xl_en_1fac4c8a a skosxl:Label;
  skosxl:literalForm "once-through cooling system"@en .

:c_fba4615d a :Terms, skos:Concept;
  skos:broader :Water_Use;
  skos:definition """amount of water delivered from a public supplier to users for domestic, commercial, industrial, thermoelectric-power, or public-use purposes.  

    1960-1965: combined estimate of deliveries for industrial and commercial use broken down by air conditioning and other, and combined estimate for domestic deliveries and losses
    1970-1975: combined estimate of deliveries for industrial and commercial use, and combined estimate for domestic use and losses
    1980: combined estimate of deliveries for industrial and commercial use, and combined estimate for domestic and public use including losses
    1985-1995: estimates of deliveries for domestic, commercial, industrial, thermoelectric power, and public use and losses
    2000: no estimates of deliveries
    2005 and later: estimates of deliveries for domestic use and a combined estimate of all other uses and system losses

See also commercial water use, domestic water use, industrial water use, public-supply water use, public water use, and thermoelectric-power use."""@en;
  skos:inScheme :usgs-wut;
  skos:topConceptOf :usgs-wut;
  skosxl:prefLabel :xl_en_ea146e7b .

:xl_en_ea146e7b a skosxl:Label;
  skosxl:literalForm "public-supply deliveries"@en .

:c_8a622cfa a :Terms, skos:Concept;
  skos:broader :Beneficial_Use, :Water_Use;
  skos:definition """water withdrawn by public and private water suppliers that furnish water to at least 25 people or have a minimum of 15 connections. Public suppliers provide water for a variety of uses, such as domestic, commercial, industrial, thermoelectric-power, and public water use.  See also commercial water use, domestic water use, industrial water use, public-supply deliveries, public water use, and thermoelectric-power water use.

    1950: Municipal
    1955 and later: Public Supply"""@en;
  skos:inScheme :usgs-wut;
  skos:topConceptOf :usgs-wut;
  skosxl:prefLabel :xl_en_0266c241 .

:xl_en_0266c241 a skosxl:Label;
  skosxl:literalForm "public-supply water use"@en .

:c_0e2ae3ff a :Terms, skos:Concept;
  skos:broader :Beneficial_Use, :Water_Use;
  skos:definition "water supplied from a public supplier and used for such purposes as firefighting, street washing, flushing of water lines, and maintaining municipal parks and swimming pools. Generally, public-use water is not billed by the public supplier. See also public-supply deliveries and public-supply water use."@en;
  skos:inScheme :usgs-wut;
  skos:topConceptOf :usgs-wut;
  skosxl:prefLabel :xl_en_7e3e0f3e .

:xl_en_7e3e0f3e a skosxl:Label;
  skosxl:literalForm "public water use"@en .

:c_50848288 a :Terms, skos:Concept;
  skos:broader :Beneficial_Use, :Water_Use;
  skos:definition "also known as closed-loop cooling system. Water is withdrawn from a source, circulated through heat exchangers, cooled, and then re-used in the same process. Recirculation cooling systems may use induced draft cooling towers, forced draft cooling towers, cooling ponds, or canals. See also cooling system, cooling-system type, industrial water use, and thermoelectric-power water use."@en;
  skos:inScheme :usgs-wut;
  skos:topConceptOf :usgs-wut;
  skosxl:prefLabel :xl_en_be353910 .

:xl_en_be353910 a skosxl:Label;
  skosxl:literalForm "recirculation cooling system"@en .

:c_34f548c8 a :Terms, skos:Concept;
  skos:broader :Beneficial_Use, :Water_Use;
  skos:definition "wastewater-treatment plant effluent that has been diverted for beneficial uses such as irrigation, industry, or thermoelectric cooling instead of being released to a natural waterway or aquifer.  See also water use."@en;
  skos:inScheme :usgs-wut;
  skos:topConceptOf :usgs-wut;
  skosxl:prefLabel :xl_en_099f0819 .

:xl_en_099f0819 a skosxl:Label;
  skosxl:literalForm "reclaimed wastewater"@en .

:c_a17e96f1 a :Terms, skos:Concept;
  skos:broader :Water_Use;
  skos:definition "water that reaches a groundwater or surface-water source after release from the point of use and thus becomes available for further use. Term used in previous water-use circulars. See also water use."@en;
  skos:inScheme :usgs-wut;
  skos:topConceptOf :usgs-wut;
  skosxl:prefLabel :xl_en_1dadd8e0 .

:xl_en_1dadd8e0 a skosxl:Label;
  skosxl:literalForm "return flow"@en .

:c_0bfdabb7 a :Terms, skos:Concept;
  skos:broader :Beneficial_Use, :Water_Use;
  skos:definition """self-supplied water used in suburban or farm areas for domestic and livestock needs, and includes domestic use, drinking water for livestock, and other uses such as dairy sanitation, cleaning, and waste disposal.

    1950-1955: Rural, included self-supplied domestic and livestock uses
    1960-1980: Rural, subcategories of rural domestic and livestock
    1985 and later: replaced by Domestic and Livestock categories

See also animal-specialties water use, domestic water use, livestock water use, and self-supplied water use."""@en;
  skos:inScheme :usgs-wut;
  skos:topConceptOf :usgs-wut;
  skosxl:prefLabel :xl_en_46ff0d90 .

:xl_en_46ff0d90 a skosxl:Label;
  skosxl:literalForm "rural water use"@en .

:c_e635df5e a :Terms, skos:Concept;
  skos:broader :Water_Use;
  skos:definition "water that contains 1,000 mg/L or more of dissolved solids. See also freshwater."@en;
  skos:inScheme :usgs-wut;
  skos:topConceptOf :usgs-wut;
  skosxl:prefLabel :xl_en_97016514 .

:xl_en_97016514 a skosxl:Label;
  skosxl:literalForm "saline water"@en .

:c_9501f5bb a :Terms, skos:Concept;
  skos:broader :Water_Use;
  skos:definition "water withdrawn from a groundwater or surface-water source by a user rather than being obtained from a public supply."@en;
  skos:inScheme :usgs-wut;
  skos:topConceptOf :usgs-wut;
  skosxl:prefLabel :xl_en_0351508b .

:xl_en_0351508b a skosxl:Label;
  skosxl:literalForm "self-supplied water use"@en .

:c_bc61313f a :Terms, skos:Concept;
  skos:broader :Beneficial_Use, :Water_Use;
  skos:definition "an irrigation system in which water is applied by means of perforated pipes or nozzles operated under pressure so as to form a spray pattern. See also irrigation water use, microirrigation system, and surface irrigation system."@en;
  skos:inScheme :usgs-wut;
  skos:topConceptOf :usgs-wut;
  skosxl:prefLabel :xl_en_5a41a1b2 .

:xl_en_5a41a1b2 a skosxl:Label;
  skosxl:literalForm "sprinkler irrigation system"@en .

:c_c19ed656 a :Terms, skos:Concept;
  skos:broader :Beneficial_Use, :Water_Use;
  skos:definition "codes established by the Office of Management and Budget in 1987 and used in the classification of establishments by type of activity in which they are engaged. Largely replaced by the North American Industry Classification System (NAICS)."@en;
  skos:inScheme :usgs-wut;
  skos:topConceptOf :usgs-wut;
  skosxl:altLabel :xl_en_90dfd2ae;
  skosxl:prefLabel :xl_en_19bfe664 .

:xl_en_19bfe664 a skosxl:Label;
  skosxl:literalForm "Standard Industrial Classification codes"@en .

:xl_en_90dfd2ae a skosxl:Label;
  skosxl:literalForm "SIC"@en .

:c_651b42f6 a :Terms, skos:Concept;
  skos:broader :Beneficial_Use, :Water_Use;
  skos:definition "irrigation by means of flood, furrow, or gravity. Flood irrigation is the application of irrigation water in which the entire soil surface is covered by ponded water. Furrow is a partial surface-flooding method of irrigation normally used with clean-tilled crops in which water is applied in furrows or rows of sufficient capacity to contain the design irrigation stream. Gravity is an irrigation method in which water is not pumped, but flows in ditches or pipes and is distributed by gravity. See also irrigation water use, microirrigation system, and sprinkler irrigation system."@en;
  skos:inScheme :usgs-wut;
  skos:topConceptOf :usgs-wut;
  skosxl:prefLabel :xl_en_d025baf4 .

:xl_en_d025baf4 a skosxl:Label;
  skosxl:literalForm "surface irrigation system"@en .

:c_f5b5ce44 a :Terms, skos:Concept;
  skos:broader :Beneficial_Use, :Water_Use;
  skos:definition """water used in the process of generating electricity with steam-driven turbine generators. Term used in previous water-use circulars to describe the combined public-supply deliveries to thermoelectric-power plants and self-supplied thermoelectric-power withdrawals.

    1950: Included in Industrial
    1955: Fuel-electric power subcategory in Industrial (data presented by watershed but not by State)
    1960-1980: Fuel-electric power subcategory in Industrial
    1985-1995: Thermoelectric power, subcategories by fuel type (fossil fuel, geothermal, nuclear)
    2000 and later: Thermoelectric power, subcategories by cooling-system type (once-through, closed-loop/recirculation)

See also cooling system, cooling-system type, public-supply water use, industrial water use, and self-supplied water use. and Methods for estimating water consumption for thermoelectric power plants in the United States.
"""@en;
  skos:inScheme :usgs-wut;
  skos:topConceptOf :usgs-wut;
  skosxl:prefLabel :xl_en_deea4cc8 .

:xl_en_deea4cc8 a skosxl:Label;
  skosxl:literalForm "thermoelectric-power water use"@en .

:c_d4c2baf8 a :Terms, skos:Concept;
  skos:broader :Water_Use;
  skos:definition "water returned to the hydrologic system by wastewater-treatment facilities. Wastewater-treatment return flows were referred to as sewage treatment in 1985. Wastewater treatment return flows were last reported in 1995. See also water use."@en;
  skos:inScheme :usgs-wut;
  skos:topConceptOf :usgs-wut;
  skosxl:prefLabel :xl_en_bef5227b .

:xl_en_bef5227b a skosxl:Label;
  skosxl:literalForm "wastewater-treatment return flow"@en .

:c_91d53bd4 a :Terms, skos:Concept;
  skos:broader :Beneficial_Use, :Water_Use;
  skos:definition "hydroelectric power water use"@en;
  skos:inScheme :usgs-wut;
  skos:topConceptOf :usgs-wut;
  skosxl:prefLabel :xl_en_60014877 .

:xl_en_60014877 a skosxl:Label;
  skosxl:literalForm "water power, waterpower"@en .

:c_d306080f a :Terms, skos:Concept;
  skos:broader :Water_Use;
  skos:definition "in a restrictive sense, the term refers to water that is withdrawn for a specific purpose, such as for public supply, domestic use, irrigation, thermoelectric-power cooling, or industrial processing.  In previous water-use circulars, water use for the domestic, commercial, industrial, and thermoelectric categories included both self-supplied withdrawals and deliveries from public supply. More broadly, water use pertains to the interaction of humans with and influence on the hydrologic cycle, and includes elements such as water withdrawal, delivery, consumptive use, wastewater release, reclaimed wastewater, return flow, and instream use.  See also offstream use and instream use."@en;
  skos:inScheme :usgs-wut;
  skos:topConceptOf :usgs-wut;
  skosxl:prefLabel :xl_en_2038ed07 .

:xl_en_2038ed07 a skosxl:Label;
  skosxl:literalForm "water use"@en .

:c_1c3d1b27 a :Terms, skos:Concept;
  skos:definition "water removed from the ground or diverted from a surface-water source for use. See also offstream use and self-supplied water.   "@en;
  skos:inScheme :usgs-wut;
  skos:topConceptOf :usgs-wut;
  skosxl:prefLabel :xl_en_096ffda8 .

:xl_en_096ffda8 a skosxl:Label;
  skosxl:literalForm "water withdrawal"@en .

:c_007145c9 a skos:Concept;
  dct:modified "2019-10-01T14:12:59.593Z"^^xsd:dateTime;
  skos:topConceptOf :epa-abg .

:c_044ab9ac a skos:Concept;
  dct:modified "2019-10-01T14:14:14.713Z"^^xsd:dateTime;
  skos:topConceptOf :epa-abg .

:c_0274cc14 a skos:Concept;
  dct:modified "2019-10-01T14:13:40.347Z"^^xsd:dateTime;
  skos:topConceptOf :epa-abg .

:c_ff73992f a skos:Concept;
  dct:modified "2019-10-01T14:14:29.578Z"^^xsd:dateTime;
  skos:topConceptOf :epa-abg .

:c_0419e86c a skos:Concept;
  dct:modified "2019-10-01T14:14:02.672Z"^^xsd:dateTime;
  skos:topConceptOf :epa-abg .

:c_27833921 a skos:Concept;
  dct:modified "2019-10-01T14:18:50.855Z"^^xsd:dateTime;
  skos:topConceptOf :epa-abg .

:c_06bb3cf2 a skos:Concept;
  dct:modified "2019-10-01T14:19:25.184Z"^^xsd:dateTime;
  skos:topConceptOf :epa-abg .

:c_276979f7 a skos:Concept;
  dct:modified "2019-10-01T14:18:59.342Z"^^xsd:dateTime;
  skos:topConceptOf :epa-abg .

:c_062b396a a skos:Concept;
  dct:modified "2019-10-01T14:19:14.302Z"^^xsd:dateTime;
  skos:topConceptOf :epa-abg .

skos:member rdfs:range _:node1dm3s2690x4 .

_:node1dm3s2690x4 a owl:Class;
  owl:unionOf _:node1dm3s2690x5 .

_:node1dm3s2690x5 rdf:first skos:Concept;
  rdf:rest _:node1dm3s2690x6 .

_:node1dm3s2690x6 rdf:first skos:Collection;
  rdf:rest rdf:nil .

:c_48ea95f3 a skos:Concept .

:c_99baa24b a skos:Concept .

:c_53de4e31 a skos:Concept .

:c_0d6ff9cd a skos:Concept .

:c_f33909f1 a skos:Concept .

:c_0a03c69e a skos:Concept .

:c_3a50aaaf a skos:Concept .

:c_5f11be9d a skos:Concept .

:c_f563ac9c a skos:Concept .

:c_dfdea833 a skos:Concept .

:c_5d486d0b a skos:Concept .

:c_9c396253 a skos:Concept .

:c_817edf3c a skos:Concept .

:c_d1f703d0 a skos:Concept .

:c_ac554243 a skos:Concept .

:c_d0a5258b a skos:Concept .

:c_c5fe43e8 a skos:Concept .

:c_178eed3e a skos:Concept .

:c_b79034fb a skos:Concept .

:c_2508ee26 a skos:Concept .

:c_60251af7 a skos:Concept .

:c_681f119a a skos:Concept .

:c_def1eb08 a skos:Concept .

:c_a2bba777 a skos:Concept .

:c_9481cd83 a skos:Concept .

:c_1b17940f a skos:Concept .

:c_87daa77c a skos:Concept .

:c_990217f6 a skos:Concept .

:c_40c2a3c5 a skos:Concept .

:c_6bf2dc94 a skos:Concept .

:c_a2ee4156 a skos:Concept .

:c_4f154be7 a skos:Concept .

:c_edc84aa8 a skos:Concept .

:c_c4ce4107 a skos:Concept .

:c_10b9fb11 a skos:Concept .

:c_74d63618 a skos:Concept .

:c_ec689587 a skos:Concept .

:c_e2f415cb a skos:Concept .

:c_da4f8325 a skos:Concept .

:c_1c3eebed a skos:Concept .

:c_2d5a5a40 a skos:Concept .

:c_bc8e39e5 a skos:Concept .

:c_4a50fa88 a skos:Concept .

:c_bd5b34d7 a skos:Concept .

:c_9f076510 a skos:Concept .

:c_40ca3850 a skos:Concept .

:c_95dd9832 a skos:Concept .

:c_18db2546 a skos:Concept .

:c_a2353449 a skos:Concept .

:c_c88fb39c a skos:Concept .

:c_58e5c7cb a skos:Concept .

:c_0c2cf147 a skos:Concept .

:c_9a9b73b9 a skos:Concept .

:c_3fac87b5 a skos:Concept .

:c_f7336870 a skos:Concept .

:c_47a36070 a skos:Concept .

:c_ad1766fd a skos:Concept .

:c_e3340e37 a skos:Concept .

:c_71390156 a skos:Concept .

:c_35665364 a skos:Concept .

:c_c78898ec a skos:Concept .

:c_1d6ffa67 a skos:Concept .

:c_11b47abe a skos:Concept .

:c_8071067c a skos:Concept .

:c_2d43db08 a skos:Concept .

:c_36b2800e a skos:Concept .

:c_f4d62c40 a skos:Concept .

:c_0e833719 a skos:Concept .

:c_278b73ec a skos:Concept .

:c_2fd5bb59 a skos:Concept .

:c_06e09c9b a skos:Concept .

:c_91457516 a skos:Concept .

:c_fc45de6f a skos:Concept .

:c_29e7234c a skos:Concept .

:c_baa4c68e a skos:Concept .

:c_2baef830 a skos:Concept .

:c_71153440 a skos:Concept .

:c_7b00a71a a skos:Concept .

:c_0fcdf7be a skos:Concept .

:c_4996f7cf a skos:Concept .

:c_76da11b5 a skos:Concept .

:c_8709c7ed a skos:Concept .

:c_f12f6680 a skos:Concept .

:c_34dd7e7e a skos:Concept .

:c_b3984ed0 a skos:Concept .

:c_8cac60a2 a skos:Concept .

:c_86af95fd a skos:Concept .

:c_97f17ef2 a skos:Concept .

:c_7a79bc61 a skos:Concept .

:c_74ad006c a skos:Concept .

:c_baa72ff1 a skos:Concept .

:c_756e2d70 a skos:Concept .

:c_8c62431e a skos:Concept .

:c_0c0ff1cc a skos:Concept .

:c_8df339dc a skos:Concept .

:c_c9d2869c a skos:Concept .

:c_06c154fe a skos:Concept .

:c_0f5bbd8a a skos:Concept .

:c_525e18f0 a skos:Concept .

:c_3bb891cf a skos:Concept .

:c_07861457 a skos:Concept .

:c_d0fa72e2 a skos:Concept .

:c_5d4cbc0a a skos:Concept .

:c_79a78368 a skos:Concept .

:c_61777e73 a skos:Concept .

:c_fb2cf0cd a skos:Concept .

:c_c1291eab a skos:Concept .

:c_24cc3016 a skos:Concept .

:c_21006d83 a skos:Concept .

:c_5810681a a skos:Concept .

:c_afee82d5 a skos:Concept .

:c_92f02cd4 a skos:Concept .

:c_eecca9b8 a skos:Concept .

:c_88319145 a skos:Concept .

:c_62d4bfb6 a skos:Concept .

:c_8e256c3d a skos:Concept .

:c_3a974a14 a skos:Concept .

:c_b176fb27 a skos:Concept .

:c_62d17e1d a skos:Concept .

:c_13cbbc62 a skos:Concept .

:c_b519ac68 a skos:Concept .

:c_cfba7d50 a skos:Concept .

:c_334faf2c a skos:Concept .

:c_8d3599bf a skos:Concept .

:c_b47d3731 a skos:Concept .

:c_5b685993 a skos:Concept .

:c_dd843071 a skos:Concept .

:c_fceba1d7 a skos:Concept .

:c_bf04de70 a skos:Concept .

:c_ecad58cf a skos:Concept .

:c_4f14be71 a skos:Concept .

:c_c578ab81 a skos:Concept .

:c_fe1af19f a skos:Concept .

:c_5ddc6dcc a skos:Concept .

:c_a050c59f a skos:Concept .

:c_35edc6f7 a skos:Concept .

:c_75b4a3a0 a skos:Concept .

:c_bd7d9638 a skos:Concept .

:c_8def1e2e a skos:Concept .

:c_f98834e6 a skos:Concept .

:c_17f6d6d9 a skos:Concept .

:c_37656125 a skos:Concept .

:c_56a11087 a skos:Concept .

:c_1da88ee3 a skos:Concept .

:c_24c2a3d7 a skos:Concept .

:c_9929c59d a skos:Concept .

:c_d2921141 a skos:Concept .

:c_74745111 a skos:Concept .

:c_871c0928 a skos:Concept .

:c_d3a88eef a skos:Concept .

:c_c397370b a skos:Concept .

:c_2b934ca8 a skos:Concept;
  skos:topConceptOf :epa-abg .

:c_2ff144c8 a skos:Concept;
  skos:topConceptOf :epa-abg .

:c_db1de5cc a skos:Concept;
  skos:topConceptOf :epa-abg .

:c_271b7032 a skos:Concept;
  skos:topConceptOf :epa-abg .

:c_3394f41e a skos:Concept;
  skos:topConceptOf :epa-abg .

:c_c29e378a a skos:Concept;
  skos:topConceptOf :epa-abg .

:c_84e77ccd a skos:Concept;
  skos:topConceptOf :epa-abg .

:c_64990663 a skos:Concept;
  skos:topConceptOf :epa-abg .

:c_7e8fb6ba a skos:Concept;
  skos:topConceptOf :epa-abg .

:c_d54bff58 a skos:Concept;
  skos:topConceptOf :epa-abg .

:c_a709c1ee a skos:Concept;
  skos:topConceptOf :epa-abg .

:c_2d97a8c4 a skos:Concept;
  skos:topConceptOf :epa-abg .

:c_1769f129 a skos:Concept;
  skos:topConceptOf :epa-abg .

:c_9da283c9 a skos:Concept;
  skos:topConceptOf :epa-abg .

:c_67b80a28 a skos:Concept;
  skos:topConceptOf :epa-abg .

:c_51ac3765 a skos:Concept;
  skos:topConceptOf :epa-abg .

:c_35819cc0 a skos:Concept;
  skos:topConceptOf :epa-abg .

:c_074149dd a skos:Concept;
  skos:topConceptOf :epa-abg .

:c_9ee7e4e6 a skos:Concept;
  skos:topConceptOf :epa-abg .

:c_1a1186ee a skos:Concept;
  skos:topConceptOf :epa-abg .

:c_ba09dc70 a skos:Concept;
  skos:topConceptOf :epa-abg .

:c_4d16deb7 a skos:Concept;
  skos:topConceptOf :epa-abg .

:c_29198b40 a skos:Concept;
  skos:topConceptOf :epa-abg .

:c_cb7d7def a skos:Concept;
  skos:topConceptOf :epa-abg .

:c_22184162 a skos:Concept;
  skos:topConceptOf :epa-abg .

:c_55c4843f a skos:Concept;
  skos:topConceptOf :epa-abg .

:c_bd6dcbf7 a skos:Concept;
  skos:topConceptOf :epa-abg .

:c_73d28241 a skos:Concept;
  skos:topConceptOf :epa-abg .

:c_2d4a117c a skos:Concept;
  skos:topConceptOf :epa-abg .

:c_e3657bb9 a skos:Concept;
  skos:topConceptOf :epa-abg .

:c_ad742fe4 a skos:Concept;
  skos:topConceptOf :epa-abg .

:c_1c8a8ea6 a skos:Concept;
  skos:topConceptOf :epa-abg .

:c_5f617aa4 a skos:Concept;
  skos:topConceptOf :epa-abg .

:c_421c959c a skos:Concept;
  skos:topConceptOf :epa-abg .

:c_a4952f11 a skos:Concept;
  skos:topConceptOf :epa-abg .

:c_09460d77 skos:topConceptOf :epa-abg .

:c_d2baf0fd skos:topConceptOf :epa-abg .

:c_5a1e1954 skos:topConceptOf :epa-abg .

:c_2f897ccc skos:topConceptOf :epa-abg .

:c_ee107987 skos:topConceptOf :epa-abg .

:c_3d964577 skos:topConceptOf :epa-abg .

:c_773b7b6c skos:topConceptOf :epa-abg .

:c_48ea95f3 skos:topConceptOf :epa-abg .

:c_99baa24b skos:topConceptOf :epa-abg .

:c_53de4e31 skos:topConceptOf :epa-abg .

:c_0d6ff9cd skos:topConceptOf :epa-abg .

:c_f33909f1 skos:topConceptOf :epa-abg .

:c_0a03c69e skos:topConceptOf :epa-abg .

:c_3a50aaaf skos:topConceptOf :epa-abg .

:c_5f11be9d skos:topConceptOf :epa-abg .

:c_f563ac9c skos:topConceptOf :epa-abg .

:c_dfdea833 skos:topConceptOf :epa-abg .

:c_ccce6454 skos:topConceptOf :epa-abg .

:c_5d486d0b skos:topConceptOf :epa-abg .

:c_9c396253 skos:topConceptOf :epa-abg .

:c_817edf3c skos:topConceptOf :epa-abg .

:c_d1f703d0 skos:topConceptOf :epa-abg .

:c_ac554243 skos:topConceptOf :epa-abg .

:c_d0a5258b skos:topConceptOf :epa-abg .

:c_c5fe43e8 skos:topConceptOf :epa-abg .

:c_178eed3e skos:topConceptOf :epa-abg .

:c_b79034fb skos:topConceptOf :epa-abg .

:c_2508ee26 skos:topConceptOf :epa-abg .

:c_60251af7 skos:topConceptOf :epa-abg .

:c_681f119a skos:topConceptOf :epa-abg .

:c_def1eb08 skos:topConceptOf :epa-abg .

:c_a2bba777 skos:topConceptOf :epa-abg .

:c_9481cd83 skos:topConceptOf :epa-abg .

:c_1b17940f skos:topConceptOf :epa-abg .

:c_87daa77c skos:topConceptOf :epa-abg .

:c_990217f6 skos:topConceptOf :epa-abg .

:c_40c2a3c5 skos:topConceptOf :epa-abg .

:c_6bf2dc94 skos:topConceptOf :epa-abg .

:c_a2ee4156 skos:topConceptOf :epa-abg .

:c_4f154be7 skos:topConceptOf :epa-abg .

:c_edc84aa8 skos:topConceptOf :epa-abg .

:c_c4ce4107 skos:topConceptOf :epa-abg .

:c_10b9fb11 skos:topConceptOf :epa-abg .

:c_74d63618 skos:topConceptOf :epa-abg .

:c_ec689587 skos:topConceptOf :epa-abg .

:c_e2f415cb skos:topConceptOf :epa-abg .

:c_da4f8325 skos:topConceptOf :epa-abg .

:c_1c3eebed skos:topConceptOf :epa-abg .

:c_2d5a5a40 skos:topConceptOf :epa-abg .

:c_bc8e39e5 skos:topConceptOf :epa-abg .

:c_4a50fa88 skos:topConceptOf :epa-abg .

:c_bd5b34d7 skos:topConceptOf :epa-abg .

:c_9f076510 skos:topConceptOf :epa-abg .

:c_40ca3850 skos:topConceptOf :epa-abg .

:c_95dd9832 skos:topConceptOf :epa-abg .

:c_18db2546 skos:topConceptOf :epa-abg .

:c_a2353449 skos:topConceptOf :epa-abg .

:c_c88fb39c skos:topConceptOf :epa-abg .

:c_58e5c7cb skos:topConceptOf :epa-abg .

:c_0c2cf147 skos:topConceptOf :epa-abg .

:c_9a9b73b9 skos:topConceptOf :epa-abg .

:c_3fac87b5 skos:topConceptOf :epa-abg .

:c_f7336870 skos:topConceptOf :epa-abg .

:c_47a36070 skos:topConceptOf :epa-abg .

:c_ad1766fd skos:topConceptOf :epa-abg .

:c_e3340e37 skos:topConceptOf :epa-abg .

:c_71390156 skos:topConceptOf :epa-abg .

:c_35665364 skos:topConceptOf :epa-abg .

:c_c78898ec skos:topConceptOf :epa-abg .

:c_1d6ffa67 skos:topConceptOf :epa-abg .

:c_11b47abe skos:topConceptOf :epa-abg .

:c_8071067c skos:topConceptOf :epa-abg .

:c_2d43db08 skos:topConceptOf :epa-abg .

:c_36b2800e skos:topConceptOf :epa-abg .

:c_f4d62c40 skos:topConceptOf :epa-abg .

:c_0e833719 skos:topConceptOf :epa-abg .

:c_278b73ec skos:topConceptOf :epa-abg .

:c_2fd5bb59 skos:topConceptOf :epa-abg .

:c_06e09c9b skos:topConceptOf :epa-abg .

:c_91457516 skos:topConceptOf :epa-abg .

:c_fc45de6f skos:topConceptOf :epa-abg .

:c_29e7234c skos:topConceptOf :epa-abg .

:c_baa4c68e skos:topConceptOf :epa-abg .

:c_2baef830 skos:topConceptOf :epa-abg .

:c_71153440 skos:topConceptOf :epa-abg .

:c_7b00a71a skos:topConceptOf :epa-abg .

:c_0fcdf7be skos:topConceptOf :epa-abg .

:c_4996f7cf skos:topConceptOf :epa-abg .

:c_76da11b5 skos:topConceptOf :epa-abg .

:c_8709c7ed skos:topConceptOf :epa-abg .

:c_f12f6680 skos:topConceptOf :epa-abg .

:c_34dd7e7e skos:topConceptOf :epa-abg .

:c_b3984ed0 skos:topConceptOf :epa-abg .

:c_8cac60a2 skos:topConceptOf :epa-abg .

:c_86af95fd skos:topConceptOf :epa-abg .

:c_97f17ef2 skos:topConceptOf :epa-abg .

:c_7a79bc61 skos:topConceptOf :epa-abg .

:c_74ad006c skos:topConceptOf :epa-abg .

:c_baa72ff1 skos:topConceptOf :epa-abg .

:c_756e2d70 skos:topConceptOf :epa-abg .

:c_8c62431e skos:topConceptOf :epa-abg .

:c_0c0ff1cc skos:topConceptOf :epa-abg .

:c_8df339dc skos:topConceptOf :epa-abg .

:c_c9d2869c skos:topConceptOf :epa-abg .

:c_aaffcb42 skos:topConceptOf :epa-abg .

:c_06c154fe skos:topConceptOf :epa-abg .

:c_0f5bbd8a skos:topConceptOf :epa-abg .

:c_525e18f0 skos:topConceptOf :epa-abg .

:c_3bb891cf skos:topConceptOf :epa-abg .

:c_07861457 skos:topConceptOf :epa-abg .

:xl_en_9c1894ee dct:modified "2019-10-02T05:09:23.233Z"^^xsd:dateTime .

:c_50185a6b dct:modified "2019-10-02T03:23:06.862Z"^^xsd:dateTime;
  skos:broader :Data .

:c_c19ed656 dct:modified "2019-10-02T03:23:19.771Z"^^xsd:dateTime;
  skos:broader :Data .

:c_e635df5e dct:modified "2019-10-02T03:25:29.358Z"^^xsd:dateTime;
  skos:related :c_007145c9 .

:ca-dwr-g a skos:ConceptScheme;
  dct:created "2019-10-02T03:59:11.858Z"^^xsd:dateTime;
  dct:modified "2019-10-02T04:01:33.607Z"^^xsd:dateTime;
  skos:note "https://water.ca.gov/Water-Basics/Glossary"^^rdf:HTML;
  skos:scopeNote :CA-DWR;
  skosxl:prefLabel :xl_en_7087f22a .

:CA-DWR a :Organizations;
  rdfs:isDefinedBy "https://water.ca.gov"^^rdf:HTML .

:xl_en_7087f22a a skosxl:Label;
  dct:created "2019-10-02T03:59:11.858Z"^^xsd:dateTime;
  skosxl:literalForm "CA-DWR Glossary"@en .

:Legal_and_Regulatory a :Themes, skos:Concept;
  dct:created "2019-10-02T05:05:07.667Z"^^xsd:dateTime;
  dct:modified "2019-10-02T05:06:58.464Z"^^xsd:dateTime;
  skos:broader :Theme;
  skos:inScheme :glos;
  skosxl:prefLabel :xl_en_0c972522 .

:xl_en_0c972522 a skosxl:Label;
  dct:created "2019-10-02T05:05:07.667Z"^^xsd:dateTime;
  skosxl:literalForm "Legal and Regulatory"@en .

:c_43eb1b10 skos:broader :Environment_and_Ecology;
  skos:definition "Includes farmland; ranches; forests; wetlands; mines; water bodies; and other natural resource lands, both private and public. "@en;
  skos:topConceptOf :ca-dwr-g;
  skosxl:prefLabel :xl_en_ea83f1f4 .

:xl_en_ea83f1f4 a skosxl:Label;
  skosxl:literalForm "working landscape "@en .

:c_d508285a a :Terms, skos:Concept;
  skos:broader :Legal_and_Regulatory;
  skos:definition "A flood event with a 1 percent chance of being equaled or exceeded in any given year (also known as a base flood)."@en;
  skos:inScheme :ca-dwr-g;
  skos:topConceptOf :ca-dwr-g;
  skosxl:prefLabel :xl_en_62c5b1ad .

:xl_en_62c5b1ad a skosxl:Label;
  skosxl:literalForm "100-year flood event "@en .

:c_b1adfc02 a :Terms, skos:Concept;
  skos:broader :Legal_and_Regulatory;
  skos:definition "A flood event with a 0.2 percent chance of being equaled or exceeded in any given year."@en;
  skos:inScheme :ca-dwr-g;
  skos:topConceptOf :ca-dwr-g;
  skosxl:prefLabel :xl_en_5a7122ad .

:xl_en_5a7122ad a skosxl:Label;
  skosxl:literalForm "500-year flood event "@en .

:c_b00a30e9 a :Terms, skos:Concept;
  skos:broader :Legal_and_Regulatory, :Water_use;
  skos:definition "A well whose use has been permanently discontinued or which is in a state of such disrepair that no water can be produced. Because abandonment is a state that also involves intent on the part of the well owner, a definition that prescribes a set of conditions and a time limit for use in applying standards appears in Section 21 of Chapter II (Standards), of the California Well Standards 74-81, available at https://water.ca.gov/Programs/Groundwater-Management/Wells. Abandoned wells pose a groundwater quality concern because they provide a vertical conduit for contamination of the aquifer. State law (Health and Safety Code Section 115700) requires that all permanently inactive wells or abandoned wells be properly destroyed."@en;
  skos:inScheme :ca-dwr-g;
  skos:topConceptOf :ca-dwr-g;
  skosxl:prefLabel :xl_en_d804b5c3 .

:xl_en_d804b5c3 a skosxl:Label;
  skosxl:literalForm "abandoned well "@en .

:Water_use a skos:Concept .

:c_ff5a1512 a :Terms, skos:Concept;
  skos:broader :Data_, :Water_Use;
  skos:definition "The volume of water that would cover 1 acre to a depth of 1 foot; equal to 43,560 cubic feet or 325,851 gallons. An acre-foot of water is considered enough water to meet the needs of two families of four for one year."@en;
  skos:inScheme :ca-dwr-g;
  skos:topConceptOf :ca-dwr-g;
  skosxl:prefLabel :xl_en_da2e611c .

:xl_en_da2e611c a skosxl:Label;
  skosxl:literalForm "acre-foot (af) "@en .

:Data_ a skos:Concept .

:c_8db56211 a :Terms, skos:Concept;
  skos:broader :Environment_and_Ecology, :Infrastructure;
  skos:definition "Adjustments to natural and human systems to moderate harm or to exploit beneficial opportunities in response to actual or expected effects of climate change."@en;
  skos:inScheme :ca-dwr-g;
  skos:topConceptOf :ca-dwr-g;
  skosxl:prefLabel :xl_en_2cd1aa50 .

:xl_en_2cd1aa50 a skosxl:Label;
  skosxl:literalForm "adaptation (measures/strategies) "@en .

:Environment_and_Ecology a skos:Concept .

:c_baa9f27a a :Terms, skos:Concept;
  skos:broader :Environment_and_Ecology;
  skos:definition "The ability of systems, organizations, and individuals to (1) adjust to actual or potential adverse changes and events; (2) take advantage of existing and emerging opportunities that support essential functions or relationships; or (3) cope with adverse consequences, mitigate damages, and recover from system failures. Adaptive capacity is an indicator of how well a system will adjust to or recover from external changes or large perturbations (e.g., severe floods or droughts). See also resilience."@en;
  skos:inScheme :ca-dwr-g;
  skos:topConceptOf :ca-dwr-g;
  skosxl:prefLabel :xl_en_6fe36bea .

:xl_en_6fe36bea a skosxl:Label;
  skosxl:literalForm "adaptive capacity "@en .

:c_ce67e033 a :Terms, skos:Concept;
  skos:broader :Legal_and_Regulatory, :Water_Use;
  skos:definition "A determination of water rights for a stream or groundwater basin, or parts of those waters. In the context of an adjudicated groundwater basin, landowners or other parties have turned to the courts to settle disputes over how much groundwater can be extracted by each party to the decision."@en;
  skos:inScheme :ca-dwr-g;
  skos:topConceptOf :ca-dwr-g;
  skosxl:prefLabel :xl_en_81b1c061 .

:xl_en_81b1c061 a skosxl:Label;
  skosxl:literalForm "adjudication (water rights) "@en .

:c_df3eaee0 a :Terms, skos:Concept;
  skos:broader :Infrastructure, :Utilities, :Water_Quality;
  skos:definition "Any wastewater treatment processes beyond tertiary treatment. The types of treatment processes may include reverse osmosis, micro- or nanofiltration, ozonation, or advanced oxidation."@en;
  skos:inScheme :ca-dwr-g;
  skos:topConceptOf :ca-dwr-g;
  skosxl:prefLabel :xl_en_cda56421 .

:xl_en_cda56421 a skosxl:Label;
  skosxl:literalForm "advanced treatment "@en .

:c_8f63ad9d a :Terms, skos:Concept;
  skos:broader :Legal_and_Regulatory, :Water_Quality;
  skos:definition "This represents the State and federal water-quality regulations regarding discharge of water used for agricultural production to streams, rivers, groundwater aquifers, or evaporation ponds."@en;
  skos:inScheme :ca-dwr-g;
  skos:topConceptOf :ca-dwr-g;
  skosxl:prefLabel :xl_en_984fb079 .

:xl_en_984fb079 a skosxl:Label;
  skosxl:literalForm "agricultural discharge standards"@en .

:c_ff3a50ad a :Terms, skos:Concept;
  skos:broader :Environment_and_Ecology;
  skos:definition "Farm and ranch landowners, the stewards of the state's agricultural land, producing public environmental benefits in conjunction with the food and fiber they have historically provided while keeping land in private ownership to the greatest extent feasible."@en;
  skos:inScheme :ca-dwr-g;
  skos:topConceptOf :ca-dwr-g;
  skosxl:prefLabel :xl_en_19a1ba33 .

:xl_en_19a1ba33 a skosxl:Label;
  skosxl:literalForm "agricultural land stewardship "@en .

:c_3abd961d a :Terms, skos:Concept;
  skos:broader :Water_use;
  skos:definition "The ratio of the amount of water required to sustain agricultural productivity to the total applied water. Efficiency is increased through the application of less water to achieve the same beneficial productivity or by achieving more productivity while applying the same amount of water."@en;
  skos:inScheme :ca-dwr-g;
  skos:topConceptOf :ca-dwr-g;
  skosxl:prefLabel :xl_en_e8630c6f .

:xl_en_e8630c6f a skosxl:Label;
  skosxl:literalForm "agricultural water use efficiency "@en .

:c_fbe9be9e a :Terms, skos:Concept;
  skos:broader :Water_use;
  skos:definition "The practice of ceasing irrigation to an alfalfa field in the mid-summer months when forage quality and yield may be low while water demand is high. Then resuming irrigation in the fall when temperatures are cooler."@en;
  skos:inScheme :ca-dwr-g;
  skos:topConceptOf :ca-dwr-g;
  skosxl:prefLabel :xl_en_b1244f22 .

:xl_en_b1244f22 a skosxl:Label;
  skosxl:literalForm "alfalfa summer dry-down"@en .

:c_60cf58a5 a :Terms, skos:Concept;
  skos:broader :Environment_and_Ecology, :Hydrology;
  skos:definition "A general term for clay, silt, sand, gravel, or similar unconsolidated detrital material deposited during comparatively recent geologic time by a stream or other body of running water, as a sorted or semi-sorted sediment in the bed of the stream or on its floodplain or delta, as a cone or fan at the base of a mountain slope."@en;
  skos:inScheme :ca-dwr-g;
  skos:topConceptOf :ca-dwr-g;
  skosxl:prefLabel :xl_en_42a127c9 .

:xl_en_42a127c9 a skosxl:Label;
  skosxl:literalForm "alluvial/alluvium "@en .

:c_1d6b78b4 a :Terms, skos:Concept;
  skos:broader :Environment_and_Ecology, :Hydrology;
  skos:definition "A fan-shaped deposit formed where a fast-flowing stream flattens, slows, and spreads, typically at the exit of a canyon onto a flatter plain."@en;
  skos:inScheme :ca-dwr-g;
  skos:topConceptOf :ca-dwr-g;
  skosxl:prefLabel :xl_en_be8c7773 .

:xl_en_be8c7773 a skosxl:Label;
  skosxl:literalForm "alluvial fan "@en .

:c_5392749f a :Terms, skos:Concept;
  skos:broader :Environment_and_Ecology, :Hydrology;
  skos:definition "Flows of shallow depth and high velocity, with sediment transport, along uncertain flow paths on the surface and at the toe of alluvial fans. Typically caused by localized rainstorms, often with snowmelt."@en;
  skos:inScheme :ca-dwr-g;
  skos:topConceptOf :ca-dwr-g;
  skosxl:prefLabel :xl_en_d8327539 .

:xl_en_d8327539 a skosxl:Label;
  skosxl:literalForm "alluvial fan flooding "@en .

:c_0575a7d1 a :Terms, skos:Concept;
  skos:broader :Environment_and_Ecology;
  skos:definition "Migratory fish that are born in freshwater, migrate to the ocean where they live their adult life, and migrate back to fresh water to lay their eggs. Salmon and steelhead are two very common anadromous fish in California."@en;
  skos:inScheme :ca-dwr-g;
  skos:topConceptOf :ca-dwr-g;
  skosxl:prefLabel :xl_en_49cf41c7 .

:xl_en_49cf41c7 a skosxl:Label;
  skosxl:literalForm "anadromous fish "@en .

:c_f2b58d12 a :Terms, skos:Concept;
  skos:broader :Environment_and_Ecology;
  skos:definition "The human aspect of biodiversity that denotes the value of varied human habitats (e.g., rural, suburban and urban), to support contemporary cultures, heritages and lifestyles. Examples of human habitat attributes (which are valued differently by individuals and/or cultures) include, but are not limited to, climate, built environment, crime rate, proximity to recreational opportunities, ability to engage in animal husbandry or agriculture at the household scale, proximity to family and family heritage, belief systems and values, quality and level of public service (e.g., schools, roads), proximity to medical care, and so forth."@en;
  skos:inScheme :ca-dwr-g;
  skos:topConceptOf :ca-dwr-g;
  skosxl:prefLabel :xl_en_322d2070 .

:xl_en_322d2070 a skosxl:Label;
  skosxl:literalForm "anthrodiversity "@en .

:c_f573b209 a :Terms, skos:Concept;
  skos:broader :Environment_and_Ecology;
  skos:definition "Of human origin or resulting from human activity."@en;
  skos:inScheme :ca-dwr-g;
  skos:topConceptOf :ca-dwr-g;
  skosxl:prefLabel :xl_en_4b143240 .

:xl_en_4b143240 a skosxl:Label;
  skosxl:literalForm "anthropogenic "@en .

:c_c9a3d027 a :Terms, skos:Concept;
  skos:broader :Water_Use;
  skos:definition "A decrease in the amount of water needed to meet the demand for beneficial use. Applied water reduction can be a supply for both new (real) water and reused water. See also new water."@en;
  skos:inScheme :ca-dwr-g;
  skos:topConceptOf :ca-dwr-g;
  skosxl:prefLabel :xl_en_b4806bb2 .

:xl_en_b4806bb2 a skosxl:Label;
  skosxl:literalForm "applied water reduction "@en .

:c_1ca997f1 a :Terms, skos:Concept;
  skos:broader :Water_Use;
  skos:definition "Refers to the volume of water that was applied and used by urban and agricultural sectors and was dedicated to the environment."@en;
  skos:inScheme :ca-dwr-g;
  skos:topConceptOf :ca-dwr-g;
  skosxl:prefLabel :xl_en_334c655f .

:xl_en_334c655f a skosxl:Label;
  skosxl:literalForm "applied water "@en .

:c_0cf37e0a a :Terms, skos:Concept;
  skos:broader :Water_Use;
  skos:definition "The total amount of water diverted from any source and applied to meet the uses of urban and agricultural sectors and dedicated to the environment, including water applied for groundwater recharge. Applied water is the quantity of water delivered to the intake to a city water system, a factory, or a farm headgate, either directly or by incidental flows to a marsh or wetland for wildlife areas. For existing instream use, applied water is the portion of the streamflow dedicated to instream use or reserved under the federal or State Wild and Scenic Rivers acts, or the flow needed to meet standards in the Sacramento-San Joaquin Delta under State Water Resources Control Board. Applied water includes consumptive use, reuse, and outflows. Applied water includes all sources of supply (surface water, groundwater, reuse, and recycled water)."@en;
  skos:inScheme :ca-dwr-g;
  skos:topConceptOf :ca-dwr-g;
  skosxl:prefLabel :xl_en_5ec948bd .

:xl_en_5ec948bd a skosxl:Label;
  skosxl:literalForm "applied water use "@en .

:c_90198d8e a :Terms, skos:Concept;
  skos:broader :Legal_and_Regulatory, :Water_Use;
  skos:definition "The right to use water that is diverted or extracted by a nonriparian or nonoverlying party for nonriparian or nonoverlying beneficial uses. In California, surface water appropriative rights are subject to a statutory permitting process, while groundwater appropriation is not. See also riparian right and pueblo right."@en;
  skos:inScheme :ca-dwr-g;
  skos:topConceptOf :ca-dwr-g;
  skosxl:prefLabel :xl_en_29c0296d .

:xl_en_29c0296d a skosxl:Label;
  skosxl:literalForm "appropriative right "@en .

:c_704b3b1b a :Terms, skos:Concept;
  skos:broader :Hydrology;
  skos:definition "A body of rock or sediment that is sufficiently porous and permeable to store, transmit, and yield significant quantities of groundwater to wells and springs."@en;
  skos:inScheme :ca-dwr-g;
  skos:topConceptOf :ca-dwr-g;
  skosxl:prefLabel :xl_en_67195f97 .

:xl_en_67195f97 a skosxl:Label;
  skosxl:literalForm "aquifer "@en .

:c_b5c13b33 a :Terms, skos:Concept;
  skos:broader :Hydrology, :Water_Use;
  skos:definition "See groundwater remediation/aquifer remediation."@en;
  skos:inScheme :ca-dwr-g;
  skos:topConceptOf :ca-dwr-g;
  skosxl:prefLabel :xl_en_d892ca6d .

:xl_en_d892ca6d a skosxl:Label;
  skosxl:literalForm "aquifer remediation "@en .

:c_156fb19f a :Terms, skos:Concept;
  skos:broader :Hydrology;
  skos:definition "A confining bed or formation composed of rock or sediment that retards but does not prevent the flow of water to or from an adjacent aquifer. It does not readily yield water to wells or springs, but stores groundwater."@en;
  skos:inScheme :ca-dwr-g;
  skos:topConceptOf :ca-dwr-g;
  skosxl:prefLabel :xl_en_d6ead20b .

:xl_en_d6ead20b a skosxl:Label;
  skosxl:literalForm "aquitard "@en .

:c_b2cb4c70 a :Terms, skos:Concept;
  skos:broader :Legal_and_Regulatory;
  skos:definition "State of California legislative acts providing special assurances to those counties and areas where the State's water resources originate, so as to allow for their own population and economic growth. See also area of origin, as defined in California Water Code Sections 10500-10506 and 11460-11463."@en;
  skos:inScheme :ca-dwr-g;
  skos:topConceptOf :ca-dwr-g;
  skosxl:prefLabel :xl_en_4cef0261 .

:xl_en_4cef0261 a skosxl:Label;
  skosxl:literalForm "area of origin acts "@en .

:c_a0992bd8 a :Terms, skos:Concept;
  skos:broader :Hydrology;
  skos:definition "A body of rock or sediment containing groundwater that is under greater than hydrostatic pressure (i.e., a confined aquifer). When an artesian aquifer is penetrated by a well, the water level will rise above the top of the aquifer. See also confined aquifer, semi-confined aquifer, and unconfined aquifer."@en;
  skos:inScheme :ca-dwr-g;
  skos:topConceptOf :ca-dwr-g;
  skosxl:prefLabel :xl_en_6ac6d0a6 .

:xl_en_6ac6d0a6 a skosxl:Label;
  skosxl:literalForm "artesian aquifer "@en .

:c_21a39aff a :Terms, skos:Concept;
  skos:broader :Hydrology;
  skos:definition "Hydrostatic pressure of artesian water, often expressed in terms of pounds per square inch; or the height, in feet above the land surface, of a column of water that would be supported by the pressure."@en;
  skos:inScheme :ca-dwr-g;
  skos:topConceptOf :ca-dwr-g;
  skosxl:prefLabel :xl_en_b614516d .

:xl_en_b614516d a skosxl:Label;
  skosxl:literalForm "artesian pressure "@en .

:c_7b1b744b a :Terms, skos:Concept;
  skos:broader :Hydrology, :Water_Use;
  skos:definition "ee also Groundwater recharge."@en;
  skos:inScheme :ca-dwr-g;
  skos:topConceptOf :ca-dwr-g;
  skosxl:prefLabel :xl_en_34fc9ee1 .

:xl_en_34fc9ee1 a skosxl:Label;
  skosxl:literalForm "artificial recharge "@en .

:c_a8a752b2 a :Terms, skos:Concept;
  skos:broader :Data_, :Legal_and_Regulatory;
  skos:definition "The Open and Transparent Water Data Act directs the California Department of Water Resources, in consultation with the California Water Quality Monitoring Council, the State Water Resources Control Board, and the California Department of Fish and Wildlife, to create, operate, and maintain a statewide integrated water data platform; and to develop protocols for data sharing, documentation, quality control, public access, and promotion of open-source platforms and decision support tools related to water data. The implementation of AB 1755 takes a user-centered approach intended to build the relationships and investments necessary across State, federal, and Tribal agencies, and among stakeholders to ensure its near-term and long-term success. The AB 1755 webpage (https://water.ca.gov/ab1755) provides additional resources, announcements, and other information."@en;
  skos:inScheme :ca-dwr-g;
  skos:topConceptOf :ca-dwr-g;
  skosxl:prefLabel :xl_en_6abc22e7 .

:xl_en_6abc22e7 a skosxl:Label;
  skosxl:literalForm "Assembly Bill (AB) 1755 "@en .

:c_e79d7893 a :Terms, skos:Concept;
  skos:broader :Hydrology;
  skos:definition "A weather pattern that forms a narrow corridor of concentrated moisture in the atmosphere that drops significant rain and snow as it passes over land."@en;
  skos:inScheme :ca-dwr-g;
  skos:topConceptOf :ca-dwr-g;
  skosxl:prefLabel :xl_en_6b03e23f .

:xl_en_6b03e23f a skosxl:Label;
  skosxl:literalForm "atmospheric river "@en .

:c_fb389530 a :Terms, skos:Concept;
  skos:broader :Hydrology;
  skos:definition "The volume of a groundwater basin that is unsaturated and capable of storing groundwater."@en;
  skos:inScheme :ca-dwr-g;
  skos:topConceptOf :ca-dwr-g;
  skosxl:prefLabel :xl_en_e5557090 .

:xl_en_e5557090 a skosxl:Label;
  skosxl:literalForm "available groundwater storage capacity "@en .

:c_3af85da3 a :Terms, skos:Concept;
  skos:broader :Hydrology;
  skos:definition "The amount of water held in the soil that can be extracted by a crop; available soil water is often expressed in inches per foot of soil depth. It is the amount of water released between in situ field capacity and the permanent wilting point."@en;
  skos:inScheme :ca-dwr-g;
  skos:topConceptOf :ca-dwr-g;
  skosxl:prefLabel :xl_en_e607ecf4 .

:xl_en_e607ecf4 a skosxl:Label;
  skosxl:literalForm "available soil water "@en .

:c_1cf8b61b a :Terms, skos:Concept;
  skos:broader :Data_, :Hydrology;
  skos:definition "The average value of total annual runoff volume calculated for a selected period of record, at a specified location or area."@en;
  skos:inScheme :ca-dwr-g;
  skos:topConceptOf :ca-dwr-g;
  skosxl:prefLabel :xl_en_b743af6c .

:xl_en_b743af6c a skosxl:Label;
  skosxl:literalForm "average annual runoff "@en .

:c_ec2f8a85 a :Terms, skos:Concept;
  skos:broader :Data_, :Hydrology;
  skos:definition "Demand for water under average hydrologic conditions for a specific level of development."@en;
  skos:inScheme :ca-dwr-g;
  skos:topConceptOf :ca-dwr-g;
  skosxl:prefLabel :xl_en_65a475ff .

:xl_en_65a475ff a skosxl:Label;
  skosxl:literalForm "average year water demand "@en .

:c_832f51ec a :Terms, skos:Concept;
  skos:broader :Water_Use;
  skos:definition "This represents water conservation occurring independent of best management practices and efficient water management practices (e.g., plumbing code changes, natural placement, and actions that water users implement on their own)."@en;
  skos:inScheme :ca-dwr-g;
  skos:topConceptOf :ca-dwr-g;
  skosxl:prefLabel :xl_en_7cac3012 .

:xl_en_7cac3012 a skosxl:Label;
  skosxl:literalForm "background water conservation "@en .

:c_36879372 a :Terms, skos:Concept;
  skos:broader :Hydrology;
  skos:definition "See hydrologic basin."@en;
  skos:inScheme :ca-dwr-g;
  skos:topConceptOf :ca-dwr-g;
  skosxl:prefLabel :xl_en_49612a8e .

:xl_en_49612a8e a skosxl:Label;
  skosxl:literalForm "basin "@en .

:c_246bea91 a :Terms, skos:Concept;
  skos:broader :Water_Use;
  skos:definition "Irrigation by flooding areas of level land surrounded by dikes. Basin irrigation is used interchangeably with level border irrigation but usually refers to smaller areas."@en;
  skos:inScheme :ca-dwr-g;
  skos:topConceptOf :ca-dwr-g;
  skosxl:prefLabel :xl_en_60940905 .

:xl_en_60940905 a skosxl:Label;
  skosxl:literalForm "basin irrigation "@en .

:c_0b5074dd a :Terms, skos:Concept;
  skos:broader :Legal_and_Regulatory;
  skos:definition "See management objectives."@en;
  skos:inScheme :ca-dwr-g;
  skos:topConceptOf :ca-dwr-g;
  skosxl:altLabel :xl_en_8aac3c5a;
  skosxl:prefLabel :xl_en_2a6894e8 .

:xl_en_2a6894e8 a skosxl:Label;
  skosxl:literalForm "basin management objectives "@en .

:xl_en_8aac3c5a a skosxl:Label;
  skosxl:literalForm "BMO"@en .

:c_0c56b1c2 a :Terms, skos:Concept;
  skos:broader :Legal_and_Regulatory;
  skos:definition "A basin plan or water quality control plan establishes a comprehensive program of actions designed to preserve, enhance, and restore water quality in all water bodies in California. The basin plan is each regional water quality control board's master water quality control planning document, and it designates beneficial uses of surface water and groundwater. The basin plan contains numeric and/or narrative water quality objectives and spells out a program by which the objectives can be achieved with their boundaries."@en;
  skos:inScheme :ca-dwr-g;
  skos:topConceptOf :ca-dwr-g;
  skosxl:prefLabel :xl_en_3d61f316 .

:xl_en_3d61f316 a skosxl:Label;
  skosxl:literalForm "basin plan "@en .

:c_9fd2a0bf a :Terms, skos:Concept;
  skos:broader :Legal_and_Regulatory, :Water_Use;
  skos:definition "(1) As part of the nine regional water quality control boards' basin planning efforts, up to 25 water-quality beneficial use categories for water have been identified for mostly human and instream uses. From Section 13050(f) of California's Porter-Cologne Water Quality Control Act: 'Beneficial uses' of the waters of the state that may be protected against water quality degradation include, but are not necessarily limited to, domestic, municipal, agricultural, and industrial supply; power generation; recreation; aesthetic enjoyment; navigation; and preservation and enhancement of fish, wildlife, and other aquatic resources or preserves. (2) As part of the State Water Resources Control Board's water rights program, the California Water Code Section 1240 states, The appropriation must be for some useful or beneficial purpose, and when the appropriator or his successor in interest ceases to use it for such a purpose [typically five years or greater] the right ceases. In the water rights process, beneficial uses are defined in the California Code of Regulations. Categories of beneficial uses recognized in California include aquaculture, domestic, fire protection, fish and wildlife, frost protection, heat control, industrial use, mining, municipal, power, recreation, stockwatering, and water quality control."@en;
  skos:inScheme :ca-dwr-g;
  skos:topConceptOf :ca-dwr-g;
  skosxl:prefLabel :xl_en_40dc1d7b .

:xl_en_40dc1d7b a skosxl:Label;
  skosxl:literalForm "beneficial use "@en .

:c_4155cdfd a :Terms, skos:Concept;
  skos:broader :Environment_and_Ecology;
  skos:definition "A region with a high amount of biodiversity that experiences habitat loss by human activity. To qualify as a biodiversity hotspot, according to Conservation International, a region must contain at least 1,500 species of vascular plants (more than 0.5 percent of the world's total) as endemics, and it must have lost at least 70 percent of its original habitat."@en;
  skos:inScheme :ca-dwr-g;
  skos:topConceptOf :ca-dwr-g;
  skosxl:prefLabel :xl_en_1877adad .

:xl_en_1877adad a skosxl:Label;
  skosxl:literalForm "Biodiversity hotspot "@en .

:c_9f6140b2 a :Terms, skos:Concept;
  skos:broader :Environment_and_Ecology;
  skos:definition "A relatively large area of land or water that characterizes a geographically distinct assemblage of natural communities and species."@en;
  skos:inScheme :ca-dwr-g;
  skos:topConceptOf :ca-dwr-g;
  skosxl:prefLabel :xl_en_80dfdb54 .

:xl_en_80dfdb54 a skosxl:Label;
  skosxl:literalForm "bioregion "@en .

:c_a5423dd0 a :Terms, skos:Concept;
  skos:broader :Legal_and_Regulatory, :Water_Quality;
  skos:definition "Wastewater treatment residuals, not including material removed during preliminary treatment, treated to levels that allow agronomic use in accordance with federal law."@en;
  skos:inScheme :ca-dwr-g;
  skos:topConceptOf :ca-dwr-g;
  skosxl:prefLabel :xl_en_27934a95 .

:xl_en_27934a95 a skosxl:Label;
  skosxl:literalForm "biosolids "@en .

:c_086653f9 a :Terms, skos:Concept;
  skos:broader :Water_Quality;
  skos:definition "A process of reducing the concentration of a contaminant in one water source by blending or dilution with water that has a lower concentration."@en;
  skos:inScheme :ca-dwr-g;
  skos:topConceptOf :ca-dwr-g;
  skosxl:prefLabel :xl_en_f1d1163f .

:xl_en_f1d1163f a skosxl:Label;
  skosxl:literalForm "blending treatment "@en .

:c_71a36eb1 a :Terms, skos:Concept;
  skos:broader :Hydrology;
  skos:definition "Fresh surface water and groundwater (i.e., the water in freshwater lakes, rivers, and aquifers) (definition taken in part from Hoekstra et al. 2011). The California Water Plan quantifies components of blue water in the water portfolios. See, for example, water portfolio components for groundwater net change in storage, surface water total available Storage, applied water, instream flows, Wild and Scenic rivers net water use, and various return flow definitions. "@en;
  skos:inScheme :ca-dwr-g;
  skos:topConceptOf :ca-dwr-g;
  skosxl:prefLabel :xl_en_5ab503df .

:xl_en_5ab503df a skosxl:Label;
  skosxl:literalForm "blue water "@en .

:c_a1490cd6 a :Terms, skos:Concept;
  skos:broader :Hydrology, :Water_Use;
  skos:definition "The volume of surface water and groundwater consumed as a result of the production of a good or service. Consumption refers to the volume of fresh water used and then evaporated or incorporated into a product. It also includes water abstracted from surface or groundwater in a catchment and returned to another catchment or the sea. It is the amount of water abstracted from groundwater or surface water that does not return to the catchment from which it was withdrawn, unless the water is reused in a downstream process. In the latter case, the second use is a second blue water footprint for the same water (definition taken in part from Hoekstra et al. 2011). The California Water Plan quantifies components of blue water footprint in the water portfolios as net water use (demand)."@en;
  skos:inScheme :ca-dwr-g;
  skos:topConceptOf :ca-dwr-g;
  skosxl:prefLabel :xl_en_d513a682 .

:xl_en_d513a682 a skosxl:Label;
  skosxl:literalForm "blue water footprint "@en .

:c_ef52ef04 a :Terms, skos:Concept;
  skos:broader :Water_Use;
  skos:definition "Irrigation by flooding strips of land, rectangular in shape and cross-leveled, bordered by dikes. Water is applied at a rate sufficient to move it down the strip in a uniform sheet. Border strips having no downfield slope are referred to as level border systems. Border systems constructed on terraced lands are commonly referred to as benched borders."@en;
  skos:inScheme :ca-dwr-g;
  skos:topConceptOf :ca-dwr-g;
  skosxl:prefLabel :xl_en_f103aa7c .

:xl_en_f103aa7c a skosxl:Label;
  skosxl:literalForm "border irrigation "@en .

:c_2d95cb4d a :Terms, skos:Concept;
  skos:broader :Hydrology;
  skos:definition "Water with a salinity that exceeds normally acceptable standards for municipal, domestic, and irrigation uses but has less salinity than seawater."@en;
  skos:inScheme :ca-dwr-g;
  skos:topConceptOf :ca-dwr-g;
  skosxl:prefLabel :xl_en_d14c33f1 .

:xl_en_d14c33f1 a skosxl:Label;
  skosxl:literalForm "brackish water "@en .

:c_c9b39657 a :Terms, skos:Concept;
  skos:broader :Environment_and_Ecology, :Legal_and_Regulatory;
  skos:definition "Generally speaking, brownfields are abandoned or unused industrial and commercial facilities/sites where expansion or redevelopment is complicated by real or perceived environmental contamination. They can be in urban, suburban, or rural areas. The U.S. Environmental Protection Agency's Brownfields Program helps communities mitigate potential health risks and restore the economic viability of such areas or properties."@en;
  skos:inScheme :ca-dwr-g;
  skos:topConceptOf :ca-dwr-g;
  skosxl:prefLabel :xl_en_225bea50 .

:xl_en_225bea50 a skosxl:Label;
  skosxl:literalForm "brownfields "@en .

:c_846697ed a :Terms, skos:Concept;
  skos:broader :Legal_and_Regulatory;
  skos:definition "California's official publication on the occurrence and nature of groundwater statewide. The bulletin includes regional and statewide information on groundwater management and recommendations for the future. In addition, it provides groundwater sustainability agencies, related stakeholders, and the public, with three critical pieces of information regarding groundwater basins: Critical Conditions of Overdraft, Basin Boundaries, and Basin Priority. Bulletin 118 will be updated in 2020, and every five years after that."@en;
  skos:inScheme :ca-dwr-g;
  skos:topConceptOf :ca-dwr-g;
  skosxl:prefLabel :xl_en_5a5f4f6b .

:xl_en_5a5f4f6b a skosxl:Label;
  skosxl:literalForm "Bulletin No. 118 "@en .

:c_9e9695e4 a :Terms, skos:Concept;
  skos:broader :Data_, :Hydrology;
  skos:definition "An integrated numerical model that simulates water movement through the linked land surface, groundwater, and surface water flow systems in California's Central Valley. The C2VSim model contains monthly historical stream inflows, surface water diversions, precipitation, land use, and crop acreages from October 1921 through September 2009. C2VSim dynamically calculates crop water demands, allocates contributions from precipitation, soil moisture, and surface water diversions, and calculates the groundwater pumpage required to meet the remaining demand. The model simulates the historical response of the Central Valley's groundwater and surface water flow system to historical stresses and can be used to simulate the response to projected future stresses. Additional information is available at: https://water.ca.gov/Library/Modeling-and-Analysis/Central-Valley-models-and-tools/C2VSim"@en;
  skos:inScheme :ca-dwr-g;
  skos:topConceptOf :ca-dwr-g;
  skosxl:altLabel :xl_en_3aa1c5f9;
  skosxl:prefLabel :xl_en_e5c79b71 .

:xl_en_e5c79b71 a skosxl:Label;
  skosxl:literalForm "California Central Valley Groundwater-Surface Water Simulation Model"@en .

:xl_en_3aa1c5f9 a skosxl:Label;
  skosxl:literalForm "C2VSim"@en .

:c_23f93add a :Terms, skos:Concept;
  skos:broader :Data_, :Water_Use;
  skos:definition "CIMIS is a network of automated weather stations that are owned and operated cooperatively between the California Department of Water Resources and local agencies. The stations are installed in most of the agricultural and urban areas in the state and provide farm and large landscape irrigation managers and researchers with real time weather data to estimate reference evapotranspiration (ETo) use to estimate crop and landscape evapotranspiration (ET) rates and make irrigation management decisions."@en;
  skos:inScheme :ca-dwr-g;
  skos:topConceptOf :ca-dwr-g;
  skosxl:altLabel :xl_en_e9c498ef;
  skosxl:prefLabel :xl_en_bea6295f .

:xl_en_bea6295f a skosxl:Label;
  skosxl:literalForm "California Irrigation Management Information System "@en .

:xl_en_e9c498ef a skosxl:Label;
  skosxl:literalForm "CIMIS"@en .

:c_8592d0ef a :Terms, skos:Concept;
  skos:broader :Legal_and_Regulatory;
  skos:definition "A federally recognized California Native American Tribe or a non-federally recognized California Native American Tribe that is on the contact list maintained by the Native American Heritage Commission."@en;
  skos:inScheme :ca-dwr-g;
  skos:topConceptOf :ca-dwr-g;
  skosxl:prefLabel :xl_en_040adff3 .

:xl_en_040adff3 a skosxl:Label;
  skosxl:literalForm "California Native American Tribes "@en .

:c_c6148ab4 a :Terms, skos:Concept;
  skos:broader :Data_, :Hydrology, :Legal_and_Regulatory;
  skos:definition "The California Department of Water Resources (DWR) developed the CASGEM program in response to Senate Bill X7 6 (Chapter 1, Statutes of 2009) that added provisions of groundwater monitoring to Division 6 of the California Water Code (Section 10920 et seq.). The intent of the CASGEM program is to establish a permanent, locally managed program of regular and systematic monitoring in all of California's alluvial groundwater basins. The CASGEM program will rely and build on the many established, local, long-term groundwater monitoring and management programs. DWR's role is to coordinate the CASGEM program, to work cooperatively with local entities, and to maintain the collected elevation data in a readily and widely available public database."@en;
  skos:inScheme :ca-dwr-g;
  skos:topConceptOf :ca-dwr-g;
  skosxl:altLabel :xl_en_ec939406;
  skosxl:prefLabel :xl_en_fe9cf077 .

:xl_en_fe9cf077 a skosxl:Label;
  skosxl:literalForm "California Statewide Groundwater Elevation Monitoring "@en .

:xl_en_ec939406 a skosxl:Label;
  skosxl:literalForm "CASGEM"@en .

:c_6d6c6f84 a :Terms, skos:Concept;
  skos:broader :Data_, :Hydrology;
  skos:definition "A surface water storage allocation model developed by the California Department of Water Resources (DWR) - for the State Water Project. CALSIM II is the latest application of the generic CALSIM model to simulate State Water Project/Central Valley Project operations. The model is a product of joint development between DWR and the U.S. Bureau of Reclamation. See also water resource integrated modeling system."@en;
  skos:inScheme :ca-dwr-g;
  skos:topConceptOf :ca-dwr-g;
  skosxl:altLabel :xl_en_5029e911;
  skosxl:prefLabel :xl_en_93c015db .

:xl_en_93c015db a skosxl:Label;
  skosxl:literalForm "California Water Resources Simulation Model "@en .

:xl_en_5029e911 a skosxl:Label;
  skosxl:literalForm "CALSIM"@en .

:c_c91f7626 a :Terms, skos:Concept;
  skos:broader :Legal_and_Regulatory;
  skos:definition "Capacity building is the process of equipping entities, usually public agencies, with certain skills or competencies or abilities for general upgrading of its performance capability by providing assistance, funding, resources, training, and more. For example, capacity building is one of three fundamental elements of conjunctive water use management, along with project construction and groundwater management."@en;
  skos:inScheme :ca-dwr-g;
  skos:topConceptOf :ca-dwr-g;
  skosxl:prefLabel :xl_en_3d0e6f82 .

:xl_en_3d0e6f82 a skosxl:Label;
  skosxl:literalForm "capacity building "@en .

:c_4c2cbf1b a :Terms, skos:Concept;
  skos:broader :Environment_and_Ecology;
  skos:definition "This represents the probability and magnitude of potential negative economic, public health, and environmental impacts associated with water management actions."@en;
  skos:inScheme :ca-dwr-g;
  skos:topConceptOf :ca-dwr-g;
  skosxl:prefLabel :xl_en_59e0432a .

:xl_en_59e0432a a skosxl:Label;
  skosxl:literalForm "catastrophic vulnerability "@en .

:c_2a161254 a :Terms, skos:Concept;
  skos:broader :Hydrology;
  skos:definition "The area of land that catches and collects water above a reservoir or other storage structure."@en;
  skos:inScheme :ca-dwr-g;
  skos:topConceptOf :ca-dwr-g;
  skosxl:prefLabel :xl_en_db841bd3 .

:xl_en_db841bd3 a skosxl:Label;
  skosxl:literalForm "catchment "@en .

:c_948238c5 a :Terms, skos:Concept;
  skos:broader :Legal_and_Regulatory;
  skos:definition "An area that is an active recharge area at the present time under the control of water management agencies. The infiltration rate at these areas is high, and they are carefully managed to maintain that high infiltration rate and to protect the quality of the water that is being recharged. At most sites, monitoring activities track groundwater levels, the rate of movement of the recharged water into the aquifer, and chemical changes. "@en;
  skos:inScheme :ca-dwr-g;
  skos:topConceptOf :ca-dwr-g;
  skosxl:prefLabel :xl_en_0c49fd50 .

:xl_en_0c49fd50 a skosxl:Label;
  skosxl:literalForm "Category 1 recharge area "@en .

:c_c53eb32b a :Terms, skos:Concept;
  skos:broader :Legal_and_Regulatory;
  skos:definition "An area that is known to have a fairly high infiltration rate but that is not under the control of a water management agency. There may be little or no monitoring of these areas. Programs should be considered that monitor recharge, prevent potential contaminating activities, and educate the public about the importance of protecting the quantity and quality of their water supply, to enable people to select appropriate actions to protect water quality."@en;
  skos:inScheme :ca-dwr-g;
  skos:topConceptOf :ca-dwr-g;
  skosxl:prefLabel :xl_en_874eccf1 .

:xl_en_874eccf1 a skosxl:Label;
  skosxl:literalForm "Category 2 recharge area "@en .

:c_ca5d9bda a :Terms, skos:Concept;
  skos:broader :Legal_and_Regulatory;
  skos:definition "An area with a lower infiltration rate making the area much less suitable for an artificial recharge program managed by a local water agency. These areas may have a lower degree of monitoring and management of potential contaminating activities."@en;
  skos:inScheme :ca-dwr-g;
  skos:topConceptOf :ca-dwr-g;
  skosxl:prefLabel :xl_en_a94a61b2 .

:xl_en_a94a61b2 a skosxl:Label;
  skosxl:literalForm "Category 3 recharge area "@en .

:c_22c544d6 a :Terms, skos:Concept;
  skos:broader :Infrastructure;
  skos:definition "Cathodic protection wells are installed to protect metallic objects in contact with the ground from electrolytic corrosion. Such objects include petroleum, natural gas, and water pipelines, and related storage facilities; power lines; telephone cables; and switchyards. Cathodic protection wells are sometimes used to control electrolytic corrosion in large water wells."@en;
  skos:inScheme :ca-dwr-g;
  skos:topConceptOf :ca-dwr-g;
  skosxl:prefLabel :xl_en_c240024c .

:xl_en_c240024c a skosxl:Label;
  skosxl:literalForm "cathodic protection well "@en .

:c_0c56f851 a :Terms, skos:Concept;
  skos:broader :Legal_and_Regulatory;
  skos:definition "The CVFPP is a State plan that describes the challenges, opportunities, and a vision for improving flood management in the context of integrated water management in the Central Valley. The CVFPP documents the current and future risks associated with flooding and recommends improvements to the Federal-State flood protection system to reduce the occurrence of major flooding and the consequence of flood damage that could result. The plan is updated every five years."@en;
  skos:inScheme :ca-dwr-g;
  skos:topConceptOf :ca-dwr-g;
  skosxl:altLabel :xl_en_14387a7c;
  skosxl:prefLabel :xl_en_80da86a1 .

:xl_en_80da86a1 a skosxl:Label;
  skosxl:literalForm "Central Valley Flood Protection Plan "@en .

:xl_en_14387a7c a skosxl:Label;
  skosxl:literalForm "CVFPP"@en .

:c_d53fc5f8 a :Terms, skos:Concept;
  skos:broader :Infrastructure, :Water_Use;
  skos:definition "The volume of surface water supplied to a given area through the Central Valley Project."@en;
  skos:inScheme :ca-dwr-g;
  skos:topConceptOf :ca-dwr-g;
  skosxl:prefLabel :xl_en_8c168c05 .

:xl_en_8c168c05 a skosxl:Label;
  skosxl:literalForm "Central Valley Project (CVP) deliveries "@en .

:c_b688b211 a :Terms, skos:Concept;
  skos:broader :Infrastructure, :Water_Use;
  skos:definition "The delivery of prior rights water to Central Valley Project base or settlement contractors."@en;
  skos:inScheme :ca-dwr-g;
  skos:topConceptOf :ca-dwr-g;
  skosxl:prefLabel :xl_en_4de022b8 .

:xl_en_4de022b8 a skosxl:Label;
  skosxl:literalForm "Central Valley Project (CVP) base deliveries "@en .

:c_5c388454 a :Terms, skos:Concept;
  skos:broader :Infrastructure, :Water_Use;
  skos:definition "The delivery of project water to Central Valley Project contractors. "@en;
  skos:inScheme :ca-dwr-g;
  skos:topConceptOf :ca-dwr-g;
  skosxl:prefLabel :xl_en_0202024a .

:xl_en_0202024a a skosxl:Label;
  skosxl:literalForm "Central Valley Project (CVP) project deliveries "@en .

:c_a55e8009 a :Terms, skos:Concept;
  skos:broader :Legal_and_Regulatory, :Water_Quality;
  skos:definition "CVSALTS is a collaborative stakeholder-driven and -managed program to develop sustainable salinity and nitrate management planning for the Central Valley."@en;
  skos:inScheme :ca-dwr-g;
  skos:topConceptOf :ca-dwr-g;
  skosxl:prefLabel :xl_en_0e46ffd3 .

:xl_en_0e46ffd3 a skosxl:Label;
  skosxl:literalForm "Central Valley Salinity Alternatives for Long-Term Sustainability (CV-SALTS) "@en .

:c_c4c2db15 a :Terms, skos:Concept;
  skos:broader :Infrastructure, :Water_Use;
  skos:definition "Modification of a border strip with small earth ridges or restrictions (checks) constructed or inserted at intervals to retain water as it flows down the strip."@en;
  skos:inScheme :ca-dwr-g;
  skos:topConceptOf :ca-dwr-g;
  skosxl:prefLabel :xl_en_36605055 .

:xl_en_36605055 a skosxl:Label;
  skosxl:literalForm "check irrigation "@en .

:c_bb8d81e4 a :Terms, skos:Concept;
  skos:broader :Legal_and_Regulatory, :Utilities, :Water_Quality;
  skos:definition "Constituents, such as personal care products and pharmaceuticals, that may be present in wastewater and may not be easily removed by most wastewater treatment processes. "@en;
  skos:inScheme :ca-dwr-g;
  skos:topConceptOf :ca-dwr-g;
  skosxl:altLabel :xl_en_5c8d0df7;
  skosxl:prefLabel :xl_en_261a9171 .

:xl_en_261a9171 a skosxl:Label;
  skosxl:literalForm "chemical of emerging concern (CEC) "@en .

:xl_en_5c8d0df7 a skosxl:Label;
  skosxl:literalForm "CEC"@en .

:c_2c104198 a :Terms, skos:Concept;
  skos:broader :Legal_and_Regulatory, :Water_Quality;
  skos:definition "Federal legislation enacted in 1972 to restore and maintain the chemical, physical, and biological integrity of the surface waters of the United States. The stated goals of the act are that all waters be fishable and swimmable."@en;
  skos:inScheme :ca-dwr-g;
  skos:topConceptOf :ca-dwr-g;
  skosxl:altLabel :xl_en_9efc48bc;
  skosxl:prefLabel :xl_en_24f692e4 .

:xl_en_24f692e4 a skosxl:Label;
  skosxl:literalForm "Clean Water Act "@en .

:xl_en_9efc48bc a skosxl:Label;
  skosxl:literalForm "CWA"@en .

:c_1b9d71f1 a :Terms, skos:Concept;
  skos:broader :Environment_and_Ecology;
  skos:definition "Changes in long-term average temperature, precipitation, wind, or other variables in a specific region. "@en;
  skos:inScheme :ca-dwr-g;
  skos:topConceptOf :ca-dwr-g;
  skosxl:prefLabel :xl_en_eb4b9383 .

:xl_en_eb4b9383 a skosxl:Label;
  skosxl:literalForm "climate change "@en .

:c_5f7d6793 a :Terms, skos:Concept;
  skos:broader :Hydrology;
  skos:definition "A basin in which no stream naturally exits the basin into another river or ocean."@en;
  skos:inScheme :ca-dwr-g;
  skos:topConceptOf :ca-dwr-g;
  skosxl:prefLabel :xl_en_fbfeaaad .

:xl_en_fbfeaaad a skosxl:Label;
  skosxl:literalForm "closed basin "@en .

:c_27f0b1b5 a :Terms, skos:Concept;
  skos:broader :Environment_and_Ecology;
  skos:definition "Typically occurs in the wintertime where special substances (e.g., silver iodide) are injected into the clouds that enable snowflakes and raindrops to form more easily. See also precipitation enhancement."@en;
  skos:inScheme :ca-dwr-g;
  skos:topConceptOf :ca-dwr-g;
  skosxl:prefLabel :xl_en_380d5ccb .

:xl_en_380d5ccb a skosxl:Label;
  skosxl:literalForm "cloud seeding "@en .

:c_c1907269 a :Terms, skos:Concept;
  skos:broader :Hydrology, :Infrastructure;
  skos:definition "Inundation at locations normally above the level of high tide and often caused by storm surges occurring with high tides. Impacts include property damage and beach erosion."@en;
  skos:inScheme :ca-dwr-g;
  skos:topConceptOf :ca-dwr-g;
  skosxl:prefLabel :xl_en_3628863c .

:xl_en_3628863c a skosxl:Label;
  skosxl:literalForm "coastal flooding "@en .

:c_a7f37e5d a :Terms, skos:Concept;
  skos:broader :Water_Use;
  skos:definition "The volume of water diverted from the mainstem Colorado River by Metropolitan Water District of Southern California, Imperial Irrigation District, Coachella Valley Water District, the Yuma Project, and others under California's consumptive use entitlement to use Colorado River water. "@en;
  skos:inScheme :ca-dwr-g;
  skos:topConceptOf :ca-dwr-g;
  skosxl:prefLabel :xl_en_bd300a39 .

:xl_en_bd300a39 a skosxl:Label;
  skosxl:literalForm "Colorado River deliveries "@en .

:c_7241f915 a :Terms, skos:Concept;
  skos:broader :Water_Use;
  skos:definition "This represents the mix of high- and low-water-using commercial activity. Note that commercial activity is broken into two factors: total commercial activity and commercial activity mix. The latter allows designation of the type of commercial activity that is occurring. See also total commercial activity. "@en;
  skos:inScheme :ca-dwr-g;
  skos:topConceptOf :ca-dwr-g;
  skosxl:prefLabel :xl_en_848fa0de .

:xl_en_848fa0de a skosxl:Label;
  skosxl:literalForm "commercial activity mix "@en .

:c_c4df16d3 a :Terms, skos:Concept;
  skos:broader :Utilities, :Water_Use;
  skos:definition "A public water system that serves at least 15 service connections used by yearlong residents or that regularly serves at least 25 year-long residents. See also public water system."@en;
  skos:inScheme :ca-dwr-g;
  skos:topConceptOf :ca-dwr-g;
  skosxl:prefLabel :xl_en_a047f69a .

:xl_en_a047f69a a skosxl:Label;
  skosxl:literalForm "community water system "@en .

:c_fa7c78ac a :Terms, skos:Concept;
  skos:broader :Water_Use;
  skos:definition "Refers to 60,000 acre-feet of transfer water that the Yuba County Water Agency (YCWA), as part of a purchase agreement under the Yuba Accord, agreed to provide to the California Department of Water Resources, to be shared equally with the U.S. Bureau of Reclamation. C1water is typically surface water stored in YCWA's New Bullards Bar Reservoir, and available quantities of C1 water depend on operational limitations of the YCWA's Yuba Project."@en;
  skos:inScheme :ca-dwr-g;
  skos:topConceptOf :ca-dwr-g;
  skosxl:prefLabel :xl_en_69eadf2f .

:xl_en_69eadf2f a skosxl:Label;
  skosxl:literalForm "component 1 (C1) water "@en .

:c_34d23115 a :Terms, skos:Concept;
  skos:broader :Hydrology;
  skos:definition "An aquifer that is bounded above and below by formations of distinctly lower permeability than that of the aquifer itself. An aquifer containing confined groundwater. See also artesian aquifer, unconfined aquifer, and semi-confined aquifer."@en;
  skos:inScheme :ca-dwr-g;
  skos:topConceptOf :ca-dwr-g;
  skosxl:prefLabel :xl_en_8f1fc4b9 .

:xl_en_8f1fc4b9 a skosxl:Label;
  skosxl:literalForm "confined aquifer "@en .

:c_0b883395 a :Terms, skos:Concept;
  skos:broader :Hydrology, :Infrastructure;
  skos:definition "Coordinated and planned management of both surface and groundwater resources to maximize the efficient use of the resource; that is, the planned and managed operation of a groundwater basin and a surface water storage system combined through a coordinated conveyance infrastructure. Water is stored in the groundwater basin for later and planned use by intentionally recharging the basin during years of above-average surface water supply. Surface water and groundwater resources typically differ significantly in their availability, quality, management needs, and development and use costs. Managing both resources together, rather than in isolation from one another, allows water managers to use the advantages of both resources for maximum benefit."@en;
  skos:inScheme :ca-dwr-g;
  skos:topConceptOf :ca-dwr-g;
  skosxl:prefLabel :xl_en_165e2f9e .

:xl_en_165e2f9e a skosxl:Label;
  skosxl:literalForm "conjunctive management (use) of surface and groundwater storage "@en .

:c_9ae201dc a :Terms, skos:Concept;
  skos:broader :Water_Use;
  skos:definition "Actions by the developer of a proposed project to save water at or above the demand level of the project."@en;
  skos:inScheme :ca-dwr-g;
  skos:topConceptOf :ca-dwr-g;
  skosxl:prefLabel :xl_en_0e170b21 .

:xl_en_0e170b21 a skosxl:Label;
  skosxl:literalForm "conservation offset "@en .

:c_ef87c156 a :Terms, skos:Concept;
  skos:broader :Environment_and_Ecology, :Water_Use;
  skos:definition "A tillage practice that leaves plant residues on the soil surface for erosion control and moisture conservation."@en;
  skos:inScheme :ca-dwr-g;
  skos:topConceptOf :ca-dwr-g;
  skosxl:prefLabel :xl_en_0be98ee9 .

:xl_en_0be98ee9 a skosxl:Label;
  skosxl:literalForm "conservation tillage "@en .

:c_be5b444e a :Terms, skos:Concept;
  skos:broader :Water_Use;
  skos:definition "The portion of agricultural applied irrigation water that satisfies evapotranspiration."@en;
  skos:inScheme :ca-dwr-g;
  skos:topConceptOf :ca-dwr-g;
  skosxl:prefLabel :xl_en_4ec99cb9 .

:xl_en_4ec99cb9 a skosxl:Label;
  skosxl:literalForm "consumed fraction "@en .

:c_a26b32ac a :Terms, skos:Concept;
  skos:broader :Water_Use;
  skos:definition "The amount of applied water used and not available for reuse as a source of supply. It includes water that evaporates, transpires, or is incorporated into products, plant tissue, or animal tissue."@en;
  skos:inScheme :ca-dwr-g;
  skos:topConceptOf :ca-dwr-g;
  skosxl:prefLabel :xl_en_b6281798 .

:xl_en_b6281798 a skosxl:Label;
  skosxl:literalForm "consumptive use "@en .

:c_469db688 a :Terms, skos:Concept;
  skos:broader :Water_Quality;
  skos:definition "Any substance or property preventing the use of, or reducing the usability of, water for ordinary purposes such as drinking, preparing food, bathing, washing, recreation, and cooling. Any solute or cause of change in physical properties that renders water unfit for a given use. (Generally considered synonymous with pollutant.)"@en;
  skos:inScheme :ca-dwr-g;
  skos:topConceptOf :ca-dwr-g;
  skosxl:prefLabel :xl_en_6680b684 .

:xl_en_6680b684 a skosxl:Label;
  skosxl:literalForm "contaminant "@en .

:c_0305dee7 a :Terms, skos:Concept;
  skos:broader :Water_Quality;
  skos:definition "A mixture of chemicals or leachate in groundwater at a certain concentration or toxicity."@en;
  skos:inScheme :ca-dwr-g;
  skos:topConceptOf :ca-dwr-g;
  skosxl:prefLabel :xl_en_457ebf23 .

:xl_en_457ebf23 a skosxl:Label;
  skosxl:literalForm "contaminant plume "@en .

:c_ce5f39fc a :Terms, skos:Concept;
  skos:broader :Infrastructure, :Water_Use;
  skos:definition "A conveyance provides for the movement of water, either natural or manmade. Conveyance infrastructures include natural watercourses, such as streams, rivers, and groundwater aquifers; and constructed facilities, such as canals and pipelines, including control structures such as weirs. Conveyance facilities range in size from small, local, end-user distribution systems to large systems that deliver water to or drain areas as large as multiple hydrologic regions. Conveyance facilities also require associated infrastructure, such as pumping plants and power supply, diversion structures, fish ladders, and fish screens."@en;
  skos:inScheme :ca-dwr-g;
  skos:topConceptOf :ca-dwr-g;
  skosxl:prefLabel :xl_en_4c221b05 .

:xl_en_4c221b05 a skosxl:Label;
  skosxl:literalForm "conveyance "@en .

:c_c6704ea3 a :Terms, skos:Concept;
  skos:broader :Infrastructure, :Water_Use;
  skos:definition "he amount of applied water used to convey water from the source to the use (e.g., if 200 acre-feet is diverted into a canal and 180 acre-feet arrive at its place of use, then 20 acre-feet is the amount of conveyance applied water). This includes water that is both recoverable (outflows such as seepage and deep percolation) and irrecoverable (depletions such as evapotranspiration, evaporation, or deep percolation to a salt sink)."@en;
  skos:inScheme :ca-dwr-g;
  skos:topConceptOf :ca-dwr-g;
  skosxl:prefLabel :xl_en_9c9c9af7 .

:xl_en_9c9c9af7 a skosxl:Label;
  skosxl:literalForm "conveyance applied water "@en .

:c_fad1a243 a :Terms, skos:Concept;
  skos:broader :Infrastructure, :Water_Use;
  skos:definition "The water evaporated into the atmosphere from conveyance systems and evapotranspired by vegetation in and near canals.conveyance facilities - Canals, pipelines, pump lifts, ditches, etc., used to move water from one area to another."@en;
  skos:inScheme :ca-dwr-g;
  skos:topConceptOf :ca-dwr-g;
  skosxl:prefLabel :xl_en_978cf49d .

:xl_en_978cf49d a skosxl:Label;
  skosxl:literalForm "conveyance evaporation and evapotranspiration "@en .

:c_7d5f4b18 a :Terms, skos:Concept;
  skos:broader :Infrastructure, :Water_Use;
  skos:definition "The portion of conveyance water that seeps through channels and returns as surface flow in another area."@en;
  skos:inScheme :ca-dwr-g;
  skos:topConceptOf :ca-dwr-g;
  skosxl:prefLabel :xl_en_e728cc31 .

:xl_en_e728cc31 a skosxl:Label;
  skosxl:literalForm "conveyance return flows to developed supply "@en .

:c_bbf44254 a :Terms, skos:Concept;
  skos:broader :Infrastructure, :Water_Use;
  skos:definition "n of conveyance water that seeps through channels and returns to surface or groundwater."@en;
  skos:inScheme :ca-dwr-g;
  skos:topConceptOf :ca-dwr-g;
  skosxl:prefLabel :xl_en_4d229b6d .

:xl_en_4d229b6d a skosxl:Label;
  skosxl:literalForm "conveyance seepage "@en .

:c_23bdcd07 a :Terms, skos:Concept;
  skos:broader :Infrastructure, :Utilities;
  skos:definition "Designates who (marginal or existing users) pays the marginal and existing water costs. It also specifies circumstances where other revenue sources are used to recover costs. Costs can include capital, operation and maintenance, financing, and environmental compliance (documentation, permitting, and mitigation)."@en;
  skos:inScheme :ca-dwr-g;
  skos:topConceptOf :ca-dwr-g;
  skosxl:prefLabel :xl_en_3c21d3d7 .

:xl_en_3c21d3d7 a skosxl:Label;
  skosxl:literalForm "cost recovery "@en .

:c_a05ff475 a :Terms, skos:Concept;
  skos:broader :Water_Use;
  skos:definition "A close-growing crop that provides soil protection, seeding protection, and soil improvement between periods of normal crop production or between trees in orchards and vines in vineyards. When plowed under and incorporated into the soil, cover crops may be referred to as green manure crops."@en;
  skos:inScheme :ca-dwr-g;
  skos:topConceptOf :ca-dwr-g;
  skosxl:prefLabel :xl_en_92765bca .

:xl_en_92765bca a skosxl:Label;
  skosxl:literalForm "cover crop "@en .

:c_72dda436 a :Terms, skos:Concept;
  skos:broader :Environment_and_Ecology;
  skos:definition "An ongoing or imminent problem (e.g., increasing flood risk, declining ecosystems) that adversely affects public health and safety, the state's economy, ecosystems, or opportunities for enriching experiences."@en;
  skos:inScheme :ca-dwr-g;
  skos:topConceptOf :ca-dwr-g;
  skosxl:prefLabel :xl_en_00daae1b .

:xl_en_00daae1b a skosxl:Label;
  skosxl:literalForm "critical challenge "@en .

:c_a70ef476 a :Terms, skos:Concept;
  skos:broader :Legal_and_Regulatory, :Water_Use;
  skos:definition "Critical conditions of overdraft refers to a groundwater basin in which a continuation of present practices would probably result in significant adverse overdraft-related environmental, social, or economic impacts. The definition was created after an extensive public input process during the development of the California Department of Water Resources' Bulletin 118-80 report."@en;
  skos:inScheme :ca-dwr-g;
  skos:topConceptOf :ca-dwr-g;
  skosxl:prefLabel :xl_en_33946010 .

:xl_en_33946010 a skosxl:Label;
  skosxl:literalForm "critical conditions of overdraft "@en .

:c_837d4277 a :Terms, skos:Concept;
  skos:broader :Water_Use;
  skos:definition "The portion of applied water solely for crop production. This does not include groundwater recharge applied water or conveyance applied water."@en;
  skos:inScheme :ca-dwr-g;
  skos:topConceptOf :ca-dwr-g;
  skosxl:prefLabel :xl_en_f96d6d11 .

:xl_en_f96d6d11 a skosxl:Label;
  skosxl:literalForm "Crop production applied water "@en .

:c_af8ae3cd a :Terms, skos:Concept;
  skos:broader :Data_, :Water_Use;
  skos:definition "A numerical factor (normally identified as Kp or Kc) that relates the evapotranspiration (ET) of an individual crop (ETc) to reference evaporation or some other index."@en;
  skos:inScheme :ca-dwr-g;
  skos:topConceptOf :ca-dwr-g;
  skosxl:prefLabel :xl_en_13bc6340 .

:xl_en_13bc6340 a skosxl:Label;
  skosxl:literalForm "crop coefficient "@en .

:c_983cd38e a :Terms, skos:Concept;
  skos:broader :Water_Use;
  skos:definition "This represents the temporary or permanent fallowing of land previously under irrigation that results in a reduction in stresses to a water system (e.g., alternate land use must result in a reduction in water use or an enhancement of water quality, or both)."@en;
  skos:inScheme :ca-dwr-g;
  skos:topConceptOf :ca-dwr-g;
  skosxl:prefLabel :xl_en_d8bf056e .

:xl_en_d8bf056e a skosxl:Label;
  skosxl:literalForm "crop idling"@en .

:c_4a8c8042 a :Terms, skos:Concept;
  skos:broader :Water_Use;
  skos:definition "A system of farming in which a succession of different crops is planted on the same land area, as opposed to growing the same crop time after time (monoculture)."@en;
  skos:inScheme :ca-dwr-g;
  skos:topConceptOf :ca-dwr-g;
  skosxl:prefLabel :xl_en_8b33f5c4 .

:xl_en_8b33f5c4 a skosxl:Label;
  skosxl:literalForm "crop rotation "@en .

:c_6b48d3f1 a :Terms, skos:Concept;
  skos:broader :Data_, :Water_Use;
  skos:definition "This represents the volume of irrigation water used per unit area of land, commonly expressed in acre-feet per acre. As used in scenario evaluation, a change in unit water use can be a function of evapotranspiration rates and cultural practices but not agricultural use efficiency, which is captured under its own distinct factor."@en;
  skos:inScheme :ca-dwr-g;
  skos:topConceptOf :ca-dwr-g;
  skosxl:prefLabel :xl_en_3ea9e12c .

:xl_en_3ea9e12c a skosxl:Label;
  skosxl:literalForm "crop unit water use"@en .

:c_3f926c02 a :Terms, skos:Concept;
  skos:broader :Infrastructure, :Utilities;
  skos:definition "An unprotected actual or potential connection between a drinking water system and any source or system containing unapproved water or a substance that cannot be approved as safe, wholesome, and potable. Cross-connection is defined in the California Code of Regulations, Title 17, Section 7583."@en;
  skos:inScheme :ca-dwr-g;
  skos:topConceptOf :ca-dwr-g;
  skosxl:prefLabel :xl_en_dc643851 .

:xl_en_dc643851 a skosxl:Label;
  skosxl:literalForm "cross-connection "@en .

:c_ac2934f3 a :Terms, skos:Concept;
  skos:broader :Legal_and_Regulatory, :Water_Quality;
  skos:definition "Cryptosporidium is a significant concern in drinking water because it contaminates most surface waters used as drinking water sources in the United States, is resistant to chlorine and other disinfectants, and has caused waterborne disease outbreaks in the United States. Consuming water with Cryptosporidium can cause gastrointestinal illness, which may be severe and sometimes fatal for people with weakened immune systems (which may include infants, the elderly, and people who have AIDS). In 2006 the U.S. Environmental Protection Agency promulgated the Long Term 2 Enhanced Surface Water Treatment Rule (LT2ESWTR) to reduce illness linked to the contaminant Cryptosporidium and other pathogenic microorganisms in drinking water."@en;
  skos:inScheme :ca-dwr-g;
  skos:topConceptOf :ca-dwr-g;
  skosxl:prefLabel :xl_en_b9f972e4 .

:xl_en_b9f972e4 a skosxl:Label;
  skosxl:literalForm "Cryptosporidium "@en .

:c_63cbc5fe a :Terms, skos:Concept;
  skos:broader :Legal_and_Regulatory, :Water_Quality;
  skos:definition " health concern at certain levels of exposure, and a primary drinking water standard has been established for this contaminant. DBCP was once a popular pesticide; however, agricultural use of this pesticide was suspended in California in 1977."@en;
  skos:inScheme :ca-dwr-g;
  skos:topConceptOf :ca-dwr-g;
  skosxl:prefLabel :xl_en_a48ecf34 .

:xl_en_a48ecf34 a skosxl:Label;
  skosxl:literalForm "DBCP (or 1,2-dibromo-3-chloropropane) "@en .

:c_fbd56c5a a :Terms, skos:Concept;
  skos:broader :Environment_and_Ecology;
  skos:definition "Flows made up of water, liquefied mud, and debris that can form and accelerate quickly, reach high velocities, and travel great distances. They are commonly caused by heavy localized rainfall on hillsides denuded of vegetation."@en;
  skos:inScheme :ca-dwr-g;
  skos:topConceptOf :ca-dwr-g;
  skosxl:prefLabel :xl_en_3c595876 .

:xl_en_3c595876 a skosxl:Label;
  skosxl:literalForm "debris flow flooding "@en .

:c_5edfa8d0 a :Terms, skos:Concept;
  skos:broader :Infrastructure, :Water_Use;
  skos:definition "Water provided for urban and agricultural uses, and dedicated to the environment. Sources of supply include surface water, groundwater, reuse, and recycled water. In any year, some of the dedicated supply includes water that is used multiple times (reuse) and water held in storage from previous years. On average, this equals 40 to 50 percent of precipitation."@en;
  skos:inScheme :ca-dwr-g;
  skos:topConceptOf :ca-dwr-g;
  skosxl:prefLabel :xl_en_5aac3113 .

:xl_en_5aac3113 a skosxl:Label;
  skosxl:literalForm "dedicated and developed water supplies "@en .

:c_7b902159 a :Terms, skos:Concept;
  skos:broader :Hydrology;
  skos:definition "Vertical movement of water through the soil/unsaturated zones and reaches the saturated zone of the aquifer (groundwater system)."@en;
  skos:inScheme :ca-dwr-g;
  skos:topConceptOf :ca-dwr-g;
  skosxl:prefLabel :xl_en_3cb925e5 .

:xl_en_3cb925e5 a skosxl:Label;
  skosxl:literalForm "deep percolation "@en .

:c_e07e2b25 a :Terms, skos:Concept;
  skos:broader :Hydrology;
  skos:definition "Freshwater outflow from the Sacramento-San Joaquin Delta (Delta). See minimum required Delta Outflow."@en;
  skos:inScheme :ca-dwr-g;
  skos:topConceptOf :ca-dwr-g;
  skosxl:prefLabel :xl_en_1d6fa91e .

:xl_en_1d6fa91e a skosxl:Label;
  skosxl:literalForm "Delta outflow "@en .

:c_c54c5047 a :Terms, skos:Concept;
  skos:broader :Legal_and_Regulatory;
  skos:definition "This zone is the Sacramento-San Joaquin Delta (Delta) land and water area of primary State concern and statewide significance, as described in Section 12220 of the California Water Code, but not within either the urban limit line or sphere of influence line of any local government's general plan or studies existing as of January 1, 1992. California Public Resources Code Section 29728 states: The precise boundary lines of the Delta Primary Zone includes the land and water areas as shown on the map titled 'Delta Protection Zones' on file with the California State Lands Commission. Where the boundary between the primary zone and secondary zone is a river, stream, channel, or waterway, the boundary line shall be the middle of that river, stream, channel, or waterway. The Delta Primary Zone consists of approximately 500,000 acres. "@en;
  skos:inScheme :ca-dwr-g;
  skos:topConceptOf :ca-dwr-g;
  skosxl:prefLabel :xl_en_e278d992 .

:xl_en_e278d992 a skosxl:Label;
  skosxl:literalForm "Delta Primary Zone "@en .

:c_ac0e3181 a :Terms, skos:Concept;
  skos:broader :Legal_and_Regulatory;
  skos:definition "This zone is the Sacramento-San Joaquin Delta (Delta) land and water area within the boundaries of the legal Delta not included within the Delta Primary Zone, subject to the land use authority of local government, and which includes the land and water areas shown on the map referenced in Delta Primary Zone, above. The Secondary Zone consists of approximately 238,000 acres. (California Public Resources Code Section 29731.)"@en;
  skos:inScheme :ca-dwr-g;
  skos:topConceptOf :ca-dwr-g;
  skosxl:prefLabel :xl_en_17119c30 .

:xl_en_17119c30 a skosxl:Label;
  skosxl:literalForm "Delta Secondary Zone "@en .

:c_24d3a0aa a :Terms, skos:Concept;
  skos:broader :Water_Use;
  skos:definition "The quantity of water consumed within a service area and no longer available as a source of supply. Depletion includes evaporation, evapotranspiration, and outflow to a salt sink."@en;
  skos:inScheme :ca-dwr-g;
  skos:topConceptOf :ca-dwr-g;
  skosxl:prefLabel :xl_en_7151e235 .

:xl_en_7151e235 a skosxl:Label;
  skosxl:literalForm "depletion "@en .

:c_83574b5f a :Terms, skos:Concept;
  skos:broader :Water_Quality;
  skos:definition "A treatment process to remove salts from water to produce a water of lesser salinity than the source water."@en;
  skos:inScheme :ca-dwr-g;
  skos:topConceptOf :ca-dwr-g;
  skosxl:prefLabel :xl_en_a83f06bf .

:xl_en_a83f06bf a skosxl:Label;
  skosxl:literalForm "desalination "@en .

:c_731ddd39 a :Terms, skos:Concept;
  skos:broader :Legal_and_Regulatory, :Water_Use;
  skos:definition "A subsection of a planning area. The smallest hydrologic study area for the analysis of water supply and use balances by the California Water Plan. DAUs are often split by county, so the smallest study area used in the water balances is DAU by county (DAUCO). Many planning studies begin at the DAUCO, DAU, or planning area level, depending on available data, and the results are aggregated to county or hydrologic region for presentation."@en;
  skos:inScheme :ca-dwr-g;
  skos:topConceptOf :ca-dwr-g;
  skosxl:altLabel :xl_en_5dc5b376;
  skosxl:prefLabel :xl_en_52636b67 .

:xl_en_52636b67 a skosxl:Label;
  skosxl:literalForm "detailed analysis units "@en .

:xl_en_5dc5b376 a skosxl:Label;
  skosxl:literalForm "DAU"@en .

:c_60755a9c a :Terms, skos:Concept;
  skos:broader :Infrastructure, :Utilities;
  skos:definition "A basin that stores stormwater for a limited amount of time and is designed to reduce stormwater flows downstream of the basin."@en;
  skos:inScheme :ca-dwr-g;
  skos:topConceptOf :ca-dwr-g;
  skosxl:prefLabel :xl_en_39085b5a .

:xl_en_39085b5a a skosxl:Label;
  skosxl:literalForm "detention basin "@en .

:c_e860becb a :Terms, skos:Concept;
  skos:broader :Infrastructure;
  skos:definition "Desalination through humidification and subsequent dehumidification (collection of evaporated water)."@en;
  skos:inScheme :ca-dwr-g;
  skos:topConceptOf :ca-dwr-g;
  skosxl:prefLabel :xl_en_b82a1289 .

:xl_en_b82a1289 a skosxl:Label;
  skosxl:literalForm "dewvaporation (atmospheric pressure desalination) "@en .

:c_974a3f57 a :Terms, skos:Concept;
  skos:broader :Utilities, :Water_Quality, :Water_Use;
  skos:definition "The planned introduction of [highly treated] recycled water either directly into a (potable) public water supply distribution system downstream of any water treatment plant, or into a raw water supply immediately upstream of a water treatment plant (California Water Code Section 13561[b])."@en;
  skos:inScheme :ca-dwr-g;
  skos:topConceptOf :ca-dwr-g;
  skosxl:prefLabel :xl_en_e319fb04 .

:xl_en_e319fb04 a skosxl:Label;
  skosxl:literalForm "direct potable reuse "@en .

:c_55d08d57 a :Terms, skos:Concept;
  skos:broader :Utilities, :Water_Quality, :Water_Use;
  skos:definition "The use of recycled water that has been transported from a wastewater treatment plant to a reuse site without passing through a natural surface water body or groundwater. "@en;
  skos:inScheme :ca-dwr-g;
  skos:topConceptOf :ca-dwr-g;
  skosxl:prefLabel :xl_en_cfbbf8c9 .

:xl_en_cfbbf8c9 a skosxl:Label;
  skosxl:literalForm "direct reuse "@en .

:c_30b8292a a :Terms, skos:Concept;
  skos:broader :Legal_and_Regulatory;
  skos:definition "A community with an annual median household income less than 80percent of the statewide average."@en;
  skos:inScheme :ca-dwr-g;
  skos:topConceptOf :ca-dwr-g;
  skosxl:prefLabel :xl_en_0781c1b9 .

:xl_en_0781c1b9 a skosxl:Label;
  skosxl:literalForm "Disadvantaged community "@en .

:c_b9e91f62 a :Terms, skos:Concept;
  skos:broader :Hydrology;
  skos:definition "An area where the groundwater that has been recharged flows out of the aquifer under natural conditions or is removed from the aquifer by wells. See also recharge area."@en;
  skos:inScheme :ca-dwr-g;
  skos:topConceptOf :ca-dwr-g;
  skosxl:prefLabel :xl_en_bc411dc1 .

:xl_en_bc411dc1 a skosxl:Label;
  skosxl:literalForm "discharge area "@en .

:c_73478388 a :Terms, skos:Concept;
  skos:broader :Infrastructure, :Utilities;
  skos:definition "(1) A system of ditches or conduits and their controls that conveys water from a supply canal to points of delivery. (2) An interconnected series of pipes, storage facilities, and components that convey treated drinking water and meet the fire protection needs for cities, homes, schools, hospitals, businesses, industries, and various facilities. Public water systems depend on distribution systems to provide an uninterrupted supply of pressurized safe drinking water to all consumers."@en;
  skos:inScheme :ca-dwr-g;
  skos:topConceptOf :ca-dwr-g;
  skosxl:prefLabel :xl_en_88bbfa07 .

:xl_en_88bbfa07 a skosxl:Label;
  skosxl:literalForm "distribution system (or water distribution system) "@en .

:c_0acce633 a :Terms, skos:Concept;
  skos:broader :Legal_and_Regulatory, :Water_Use;
  skos:definition "A water well used to supply water for the domestic needs of an individual residence or local small water system of four or fewer service connections or homes. Small water systems with 1-4 service connections are not defined by either the California Health and Safety Code or Title 22 of the California Code of Regulations. The California Department of Public Health and various county environmental health agencies throughout the state, acting as the drinking water program primacy agency for state small water systems or small community water systems, generally define private domestic wells as wells serving up to four service connections. On the other hand, some local health agencies define a private domestic well as serving an individual residence (single connection) and a local small (or shared) water system as having two to four service connections (Governor's Drinking Water Stakeholder Group 2014)."@en;
  skos:inScheme :ca-dwr-g;
  skos:topConceptOf :ca-dwr-g;
  skosxl:prefLabel :xl_en_638e4380 .

:xl_en_638e4380 a skosxl:Label;
  skosxl:literalForm "domestic well "@en .

:c_1a58f459 a :Terms, skos:Concept;
  skos:broader :Hydrology;
  skos:definition "See watershed."@en;
  skos:inScheme :ca-dwr-g;
  skos:topConceptOf :ca-dwr-g;
  skosxl:prefLabel :xl_en_2dc39f8c .

:xl_en_2dc39f8c a skosxl:Label;
  skosxl:literalForm "drainage basin "@en .

:c_d117ace7 a :Terms, skos:Concept;
  skos:broader :Legal_and_Regulatory, :Utilities, :Water_Quality;
  skos:definition "State and federal regulations regarding drinking water quality delivered by public water systems to customers. Primary drinking water standards, called maximum contaminant levels or MCLs, are established to protect public health by limiting the levels of contaminants in drinking water. Secondary drinking water standards, called secondary maximum contaminant levels or SMCLs, are established for aesthetic considerations, such as taste, color, and odor. These contaminants are not considered to present a risk to human health at the SMCL."@en;
  skos:inScheme :ca-dwr-g;
  skos:topConceptOf :ca-dwr-g;
  skosxl:prefLabel :xl_en_bc50fc09 .

:xl_en_bc50fc09 a skosxl:Label;
  skosxl:literalForm "drinking water standards "@en .

:c_db322ec3 a :Terms, skos:Concept;
  skos:broader :Legal_and_Regulatory, :Utilities;
  skos:definition "See public water system and community water system."@en;
  skos:inScheme :ca-dwr-g;
  skos:topConceptOf :ca-dwr-g;
  skosxl:prefLabel :xl_en_3bc73a86 .

:xl_en_3bc73a86 a skosxl:Label;
  skosxl:literalForm "drinking water system "@en .

:c_89b14706 a :Terms, skos:Concept;
  skos:broader :Infrastructure, :Utilities, :Water_Quality;
  skos:definition "Drinking water treatment refers to the physical, biological, and chemical processes that make water suitable for drinking by ensuring that drinking water standards are met. A drinking water distribution system is an interconnected series of pipes, storage facilities, and components that convey drinking water and meet the fire protection needs of customers. Public water systems depend on distribution systems to provide an uninterrupted supply of pressurized safe drinking water to all consumers."@en;
  skos:inScheme :ca-dwr-g;
  skos:topConceptOf :ca-dwr-g;
  skosxl:prefLabel :xl_en_e6e51854 .

:xl_en_e6e51854 a skosxl:Label;
  skosxl:literalForm "drinking water treatment and distribution "@en .

:c_bf95ee58 a :Terms, skos:Concept;
  skos:broader :Water_Use;
  skos:definition "A method of micro irrigation wherein water is applied to the soil surface as drops or small streams through emitters. Discharge rates are generally less than 8 liters per hour (2 gallons per hour) for single-outlet emitters and 12 liters per hour (3 gallons per hour) per meter for line-source emitters."@en;
  skos:inScheme :ca-dwr-g;
  skos:topConceptOf :ca-dwr-g;
  skosxl:prefLabel :xl_en_1be66c15 .

:xl_en_1be66c15 a skosxl:Label;
  skosxl:literalForm "drip irrigation "@en .

:c_44b15b9a a :Terms, skos:Concept;
  skos:broader :Hydrology;
  skos:definition "Hydrologic conditions during a defined period, greater than one dry year, when precipitation and runoff are much less than average."@en;
  skos:inScheme :ca-dwr-g;
  skos:topConceptOf :ca-dwr-g;
  skosxl:prefLabel :xl_en_4e1e6974 .

:xl_en_4e1e6974 a skosxl:Label;
  skosxl:literalForm "drought condition "@en .

:c_e35897e7 a :Terms, skos:Concept;
  skos:broader :Environment_and_Ecology, :Water_Use;
  skos:definition "The magnitude and probability of economic, social, or environmental consequences that would occur as a result of a sustained drought under a given study plan. Evaluation criteria measure the drought tolerance of study plans. "@en;
  skos:inScheme :ca-dwr-g;
  skos:topConceptOf :ca-dwr-g;
  skosxl:prefLabel :xl_en_730cd6a1 .

:xl_en_730cd6a1 a skosxl:Label;
  skosxl:literalForm "drought preparedness "@en .

:c_7b7e15ce a :Terms, skos:Concept;
  skos:broader :Data_, :Water_Use;
  skos:definition "The average annual supply of a water development system during a defined drought period."@en;
  skos:inScheme :ca-dwr-g;
  skos:topConceptOf :ca-dwr-g;
  skosxl:prefLabel :xl_en_3a40bcb6 .

:xl_en_3a40bcb6 a skosxl:Label;
  skosxl:literalForm "drought year supply "@en .

:c_113ae23f a :Terms, skos:Concept;
  skos:broader :Water_Quality;
  skos:definition "Dry-weather runoff occurs when, for example, excess landscape irrigation water flows to a storm drain. It is a concern because it can carry a significant amount of pollutants to surface waters."@en;
  skos:inScheme :ca-dwr-g;
  skos:topConceptOf :ca-dwr-g;
  skosxl:prefLabel :xl_en_0ed72842 .

:xl_en_0ed72842 a skosxl:Label;
  skosxl:literalForm "dry-weather runoff "@en .

:c_7cfe9e5d a :Terms, skos:Concept;
  skos:broader :Water_Use;
  skos:definition "The total volume of irrigation water required to mature a particular type of crop. It includes consumptive use, evaporation, and seepage, as well as the water returned to streams by percolation and surface water."@en;
  skos:inScheme :ca-dwr-g;
  skos:topConceptOf :ca-dwr-g;
  skosxl:prefLabel :xl_en_6c256f2a .

:xl_en_6c256f2a a skosxl:Label;
  skosxl:literalForm "duty of water "@en .

:c_5aff0f0d a :Terms, skos:Concept;
  skos:broader :Legal_and_Regulatory;
  skos:definition "Financial assistance and pricing policies intended to influence water management, including amount of use, time of use, wastewater volume, and source of supply, among other related factors."@en;
  skos:inScheme :ca-dwr-g;
  skos:topConceptOf :ca-dwr-g;
  skosxl:prefLabel :xl_en_881d009a .

:xl_en_881d009a a skosxl:Label;
  skosxl:literalForm "economic incentives "@en .

:c_26bdcf2b a :Terms, skos:Concept;
  skos:broader :Environment_and_Ecology;
  skos:definition "The activity of improving the condition of natural landscapes and biotic communities. "@en;
  skos:inScheme :ca-dwr-g;
  skos:topConceptOf :ca-dwr-g;
  skosxl:prefLabel :xl_en_25dc4377 .

:xl_en_25dc4377 a skosxl:Label;
  skosxl:literalForm "ecosystem restoration "@en .

:c_1e0adab7 a :Terms, skos:Concept;
  skos:broader :Environment_and_Ecology, :Legal_and_Regulatory;
  skos:definition "Ecosystems perform a multitude of complex and interrelated functions that not only provide basic biological support, but also provide valuable goods and services to society (e.g., enhanced water supply and quality, flood damage reduction, recreation). If these goods and services can be identified and measured, then it may be possible to place monetary values on them by using market or non-market valuation methods."@en;
  skos:inScheme :ca-dwr-g;
  skos:topConceptOf :ca-dwr-g;
  skosxl:prefLabel :xl_en_10b13ad5 .

:xl_en_10b13ad5 a skosxl:Label;
  skosxl:literalForm "ecosystem valuation methods "@en .

:c_475bbb48 a :Terms, skos:Concept;
  skos:broader :Environment_and_Ecology;
  skos:definition "See bioregion."@en;
  skos:inScheme :ca-dwr-g;
  skos:topConceptOf :ca-dwr-g;
  skosxl:prefLabel :xl_en_93df441d .

:xl_en_93df441d a skosxl:Label;
  skosxl:literalForm "ecozone "@en .

:c_5b0484be a :Terms, skos:Concept;
  skos:broader :Hydrology;
  skos:definition "The interconnected portion of the total voids or open spaces in alluvium and rocks that is capable of transmitting fluids."@en;
  skos:inScheme :ca-dwr-g;
  skos:topConceptOf :ca-dwr-g;
  skosxl:prefLabel :xl_en_c8cfb3b4 .

:xl_en_c8cfb3b4 a skosxl:Label;
  skosxl:literalForm "effective porosity "@en .

:c_fe072a80 a :Terms, skos:Concept;
  skos:broader :Hydrology;
  skos:definition "That portion of precipitation stored in the root zone that is available for plant evapotranspiration. This includes precipitation stored in the soil before and during the growing season. Effective precipitation is sometimes referred to as consumptive use of precipitation."@en;
  skos:inScheme :ca-dwr-g;
  skos:topConceptOf :ca-dwr-g;
  skosxl:prefLabel :xl_en_f8785039 .

:xl_en_f8785039 a skosxl:Label;
  skosxl:literalForm "effective precipitation "@en .

:c_e5cb9229 a :Terms, skos:Concept;
  skos:broader :Hydrology;
  skos:definition "The depth from which soil moisture is extracted; it is determined by the crop rooting characteristics and soil depth limitations."@en;
  skos:inScheme :ca-dwr-g;
  skos:topConceptOf :ca-dwr-g;
  skosxl:prefLabel :xl_en_10a34f9b .

:xl_en_10a34f9b a skosxl:Label;
  skosxl:literalForm "effective rooting depth "@en .

:c_3209e9a1 a :Terms, skos:Concept;
  skos:broader :Legal_and_Regulatory, :Water_Use;
  skos:definition "Technology or procedures employed by an agricultural water supplier to increase the beneficial use of water. There are 16 EWMPs defined in California Water Code Section 10608.48."@en;
  skos:inScheme :ca-dwr-g;
  skos:topConceptOf :ca-dwr-g;
  skosxl:altLabel :xl_en_dfbf579f;
  skosxl:prefLabel :xl_en_a5bdb4a5 .

:xl_en_a5bdb4a5 a skosxl:Label;
  skosxl:literalForm "efficient water management practice "@en .

:xl_en_dfbf579f a skosxl:Label;
  skosxl:literalForm "EWMP"@en .

:c_1ac6de27 a :Terms, skos:Concept;
  skos:broader :Data_, :Legal_and_Regulatory, :Water_Quality;
  skos:definition "The measure of water's ability to conduct an electrical current. Conductivity depends on the ion concentration and temperature and can be used to approximate the total dissolved solids in the water."@en;
  skos:inScheme :ca-dwr-g;
  skos:topConceptOf :ca-dwr-g;
  skosxl:altLabel :xl_en_20e37d5e;
  skosxl:prefLabel :xl_en_73cf5bf6 .

:xl_en_73cf5bf6 a skosxl:Label;
  skosxl:literalForm "electrical conductivity"@en .

:xl_en_20e37d5e a skosxl:Label;
  skosxl:literalForm "EC"@en .

:c_958d8831 a :Terms, skos:Concept;
  skos:broader :Infrastructure, :Utilities;
  skos:definition "This represents the cost of energy use related to producing, conveying, and applying water. It also refers to the cost of energy use for processes and inputs not directly related to water but which can affect the demand for water (e.g., the cost of nitrogen fertilizer or tractor manufacturing)."@en;
  skos:inScheme :ca-dwr-g;
  skos:topConceptOf :ca-dwr-g;
  skosxl:prefLabel :xl_en_f88fc50d .

:xl_en_f88fc50d a skosxl:Label;
  skosxl:literalForm "energy costs "@en .

:c_05bd4e7b a :Terms, skos:Concept;
  skos:broader :Infrastructure, :Utilities;
  skos:definition "Both instantaneous capacity (megawatt) and energy produced (kilowatt hours)."@en;
  skos:inScheme :ca-dwr-g;
  skos:topConceptOf :ca-dwr-g;
  skosxl:prefLabel :xl_en_44e33c85 .

:xl_en_44e33c85 a skosxl:Label;
  skosxl:literalForm "energy production "@en .

:c_7f495983 a :Terms, skos:Concept;
  skos:broader :Environment_and_Ecology, :Legal_and_Regulatory;
  skos:definition "Equal protection from environmental hazards for individuals, groups, or communities regardless of race, ethnicity, or economic status. The fair treatment of people of all races, cultures, and incomes with respect to the development, adoption, implementation, and enforcement of environmental laws, regulations, and policies (Government Code Section 65040.12[e])."@en;
  skos:inScheme :ca-dwr-g;
  skos:topConceptOf :ca-dwr-g;
  skosxl:prefLabel :xl_en_d961b02b .

:xl_en_d961b02b a skosxl:Label;
  skosxl:literalForm "environmental equity/justice "@en .

:c_05da0658 a :Terms, skos:Concept;
  skos:broader :Legal_and_Regulatory, :Water_Use;
  skos:definition "Minimum flow levels of a specific quality needed to ensure the continued viability of fish and wildlife resources for a particular water body. This is water used to maintain and enhance beneficial uses related to the preservation and enhancement of fish, wildlife, and other aquatic resources or preserves, as specified in the Porter-Cologne Water Quality Control Act."@en;
  skos:inScheme :ca-dwr-g;
  skos:topConceptOf :ca-dwr-g;
  skosxl:prefLabel :xl_en_798398ff .

:xl_en_798398ff a skosxl:Label;
  skosxl:literalForm "environmental water "@en .

:c_b4ce81c3 a :Terms, skos:Concept;
  skos:broader :Infrastructure, :Legal_and_Regulatory;
  skos:definition "An element of the CALFED Bay-Delta Program's overall management strategy for the San Francisco Bay/Sacramento-San Joaquin Delta ecosystem. Its purpose is to protect fish of the Bay-Delta estuary through environmentally beneficial changes in the operations of the Central Valley Project and State Water Project."@en;
  skos:inScheme :ca-dwr-g;
  skos:topConceptOf :ca-dwr-g;
  skosxl:prefLabel :xl_en_a480cdf5 .

:xl_en_a480cdf5 a skosxl:Label;
  skosxl:literalForm "Environmental Water Account "@en .

:c_109ebcca a :Terms, skos:Concept;
  skos:broader :Water_Quality;
  skos:definition "Water quality in terms of ecosystem health, recreation, salinity intrusion, usability per sector, treatment costs, etc. Aquatic species and water bodies are vulnerable to changes in water quality. "@en;
  skos:inScheme :ca-dwr-g;
  skos:topConceptOf :ca-dwr-g;
  skosxl:prefLabel :xl_en_2edfaa97 .

:xl_en_2edfaa97 a skosxl:Label;
  skosxl:literalForm "environmental water quality "@en .

:c_5bbe6673 a :Terms, skos:Concept;
  skos:broader :Water_Quality;
  skos:definition "dibromide is a health concern at certain levels of exposure, and a primary drinking water standard has been established for this contaminant. Ethylene dibromide was once a popular pesticide and was used as a gasoline additive, but both uses have now been discontinued."@en;
  skos:inScheme :ca-dwr-g;
  skos:topConceptOf :ca-dwr-g;
  skosxl:prefLabel :xl_en_f61a5487 .

:xl_en_f61a5487 a skosxl:Label;
  skosxl:literalForm "ethylene dibromide "@en .

:c_98d57989 a :Terms, skos:Concept;
  skos:broader :Hydrology, :Water_Use;
  skos:definition "The evapotranspiration rate from an extended surface of 3- to 6-inch-tall (8- to 15-centimeter-tall) green grass cover of uniform height, actively growing, completely shading the ground, and not short on water (the reference evapotranspiration rate reported by the California Irrigation Management Irrigation System)."@en;
  skos:inScheme :ca-dwr-g;
  skos:topConceptOf :ca-dwr-g;
  skosxl:prefLabel :xl_en_e33cb2c5 .

:xl_en_e33cb2c5 a skosxl:Label;
  skosxl:literalForm "ETo (reference evapotranspiration) "@en .

:c_92e4baf7 a :Terms, skos:Concept;
  skos:broader :Water_Quality;
  skos:definition "Eutrophic conditions exist in a body of water that has high primary productivity resulting from excessive nutrients and is subject to algal blooms, resulting in poor water quality. Typically, such a body of water is deficient in oxygen in the deeper regions - ranging from hypoxic to anoxic. These conditions do not favor fish species, such as trout, which require or prefer cold, well-oxygenated water."@en;
  skos:inScheme :ca-dwr-g;
  skos:topConceptOf :ca-dwr-g;
  skosxl:prefLabel :xl_en_cd2c64b6 .

:xl_en_cd2c64b6 a skosxl:Label;
  skosxl:literalForm "eutrophic conditions "@en .

:c_ba75192f a :Terms, skos:Concept;
  skos:broader :Legal_and_Regulatory;
  skos:definition "The technical information used to compare the favorability of different response packages of resource management strategies against future scenarios in the California Water Plan They are designed to identify and measure potential effects on water supply, the environment, energy use or production, recreational opportunities, groundwater overdraft, and more."@en;
  skos:inScheme :ca-dwr-g;
  skos:topConceptOf :ca-dwr-g;
  skosxl:prefLabel :xl_en_dd86a6b3 .

:xl_en_dd86a6b3 a skosxl:Label;
  skosxl:literalForm "evaluation criteria "@en .

:c_843fe30d a :Terms, skos:Concept;
  skos:broader :Hydrology;
  skos:definition "The physical process by which a liquid or solid is transformed to a gaseous state. "@en;
  skos:inScheme :ca-dwr-g;
  skos:topConceptOf :ca-dwr-g;
  skosxl:prefLabel :xl_en_668467aa .

:xl_en_668467aa a skosxl:Label;
  skosxl:literalForm "evaporation "@en .

:c_4a3624a9 a :Terms, skos:Concept;
  skos:broader :Hydrology;
  skos:definition "The collective influence of all climatic factors on the rate of evaporation of water."@en;
  skos:inScheme :ca-dwr-g;
  skos:topConceptOf :ca-dwr-g;
  skosxl:prefLabel :xl_en_09cc3f5e .

:xl_en_09cc3f5e a skosxl:Label;
  skosxl:literalForm "evaporative demand "@en .

:c_6ad9de70 a :Terms, skos:Concept;
  skos:broader :Hydrology, :Water_Use;
  skos:definition "The amount of water transpired by plants, retained in plant tissues, and evaporated from plant tissues and surrounding soil surfaces. See also green water. "@en;
  skos:inScheme :ca-dwr-g;
  skos:topConceptOf :ca-dwr-g;
  skosxl:altLabel :xl_en_7674da64;
  skosxl:prefLabel :xl_en_fd813294 .

:xl_en_fd813294 a skosxl:Label;
  skosxl:literalForm "evapotranspiration"@en .

:xl_en_7674da64 a skosxl:Label;
  skosxl:literalForm "ET"@en .

:c_127863e4 a :Terms, skos:Concept;
  skos:broader :Water_Use;
  skos:definition "The amount of consumptive use by crops, landscapes, or other vegetation. ETAW is the portion of evapotranspiration (ET) that was provided by applied irrigation water."@en;
  skos:inScheme :ca-dwr-g;
  skos:topConceptOf :ca-dwr-g;
  skosxl:altLabel :xl_en_fff18ecb;
  skosxl:prefLabel :xl_en_68b52ca1 .

:xl_en_68b52ca1 a skosxl:Label;
  skosxl:literalForm "evapotranspiration of applied water "@en .

:xl_en_fff18ecb a skosxl:Label;
  skosxl:literalForm "ETAW"@en .

:c_741debac a :Terms, skos:Concept;
  skos:broader :Legal_and_Regulatory;
  skos:definition "The freshwater outflow from the Sacramento-San Joaquin Delta that exceeds the amount required by law."@en;
  skos:inScheme :ca-dwr-g;
  skos:topConceptOf :ca-dwr-g;
  skosxl:prefLabel :xl_en_809b4ba5 .

:xl_en_809b4ba5 a skosxl:Label;
  skosxl:literalForm "excess Delta outflow "@en .

:c_64dc3f51 a :Terms, skos:Concept;
  skos:broader :Data_, :Legal_and_Regulatory;
  skos:definition "EAD is the value that measures the severity of flood loss in any given year. EAD does not mean that this amount of damage will occur in any particular year, but rather that over a long period, the average damages will tend to approach that amount."@en;
  skos:inScheme :ca-dwr-g;
  skos:topConceptOf :ca-dwr-g;
  skosxl:altLabel :xl_en_d4ef5268;
  skosxl:prefLabel :xl_en_9bcd49a9 .

:xl_en_9bcd49a9 a skosxl:Label;
  skosxl:literalForm "expected annual damage "@en .

:xl_en_d4ef5268 a skosxl:Label;
  skosxl:literalForm "EAD"@en .

:c_44a8cf2f a :Terms, skos:Concept;
  skos:broader :Infrastructure, :Water_Use;
  skos:definition "In the process of extracting groundwater for remediation, groundwater flows through the aquifer(s) toward the extraction wells, where it is removed for treatment."@en;
  skos:inScheme :ca-dwr-g;
  skos:topConceptOf :ca-dwr-g;
  skosxl:prefLabel :xl_en_689190b4 .

:xl_en_689190b4 a skosxl:Label;
  skosxl:literalForm "extraction wells "@en .

:c_29168cb1 a :Terms, skos:Concept;
  skos:broader :Infrastructure, :Water_Use;
  skos:definition "The sum of Central Valley Project and other federal deliveries volumes."@en;
  skos:inScheme :ca-dwr-g;
  skos:topConceptOf :ca-dwr-g;
  skosxl:prefLabel :xl_en_cbd98e4e .

:xl_en_cbd98e4e a skosxl:Label;
  skosxl:literalForm "federal projects "@en .

:c_15b98061 a :Terms, skos:Concept;
  skos:broader :Utilities;
  skos:definition "Finished water is treated or conditioned to the point that it meets drinking water standards and is suitable for distribution to consumers for all drinking water uses."@en;
  skos:inScheme :ca-dwr-g;
  skos:topConceptOf :ca-dwr-g;
  skosxl:prefLabel :xl_en_d60df464 .

:xl_en_d60df464 a skosxl:Label;
  skosxl:literalForm "finished water "@en .

:c_eb72b427 a :Terms, skos:Concept;
  skos:broader :Legal_and_Regulatory;
  skos:definition "The Central Valley Project Improvement Act Section 3406(d) (Refuge Water Supply) establishes the primary goal of providing a firm water supply for wildlife refuges. See also firm-yield approach."@en;
  skos:inScheme :ca-dwr-g;
  skos:topConceptOf :ca-dwr-g;
  skosxl:prefLabel :xl_en_7f2a0b93 .

:xl_en_7f2a0b93 a skosxl:Label;
  skosxl:literalForm "firm water supply "@en .

:c_169b2829 a :Terms, skos:Concept;
  skos:broader :Legal_and_Regulatory;
  skos:definition "To deliver the same amount of water every year regardless of water supply conditions."@en;
  skos:inScheme :ca-dwr-g;
  skos:topConceptOf :ca-dwr-g;
  skosxl:prefLabel :xl_en_0bcc4e96 .

:xl_en_0bcc4e96 a skosxl:Label;
  skosxl:literalForm "firm-yield approach "@en .

:c_62cd83cf a :Terms, skos:Concept;
  skos:broader :Hydrology;
  skos:definition "Quickly forming floods with high-velocity flows often caused by stationary or slow-moving storms. Flash floods typically occur on steep slopes and impermeable surfaces, and in areas adjacent to local streams and creeks."@en;
  skos:inScheme :ca-dwr-g;
  skos:topConceptOf :ca-dwr-g;
  skosxl:prefLabel :xl_en_dc1e3c8f .

:xl_en_dc1e3c8f a skosxl:Label;
  skosxl:literalForm "flash flooding "@en .

:c_cd69cce5 a :Terms, skos:Concept;
  skos:broader :Infrastructure, :Legal_and_Regulatory;
  skos:definition "The emergency measures used to prevent levee failure from seepage, erosion, or overtopping during high water."@en;
  skos:inScheme :ca-dwr-g;
  skos:topConceptOf :ca-dwr-g;
  skosxl:prefLabel :xl_en_4f2bf428 .

:xl_en_4f2bf428 a skosxl:Label;
  skosxl:literalForm "flood fight "@en .

:c_d7d9c476 a :Terms, skos:Concept;
  skos:broader :Legal_and_Regulatory;
  skos:definition "The Federal Emergency Management Agency defines a flood hazard as any flood event or condition with the potential to cause fatalities, injuries, property damage, infrastructure damage, agricultural loss, environmental damage, business interruption, or other loss."@en;
  skos:inScheme :ca-dwr-g;
  skos:topConceptOf :ca-dwr-g;
  skosxl:prefLabel :xl_en_c28edb18 .

:xl_en_c28edb18 a skosxl:Label;
  skosxl:literalForm "flood hazard "@en .

:c_d3a1b9b3 a :Terms, skos:Concept;
  skos:broader :Legal_and_Regulatory;
  skos:definition "A FIRM is the official map of a community on which the Federal Emergency Management Agency has delineated the special flood hazard areas, the base flood elevations, and the risk premium zones applicable to the community."@en;
  skos:inScheme :ca-dwr-g;
  skos:topConceptOf :ca-dwr-g;
  skosxl:altLabel :xl_en_566de8c9;
  skosxl:prefLabel :xl_en_802c185c .

:xl_en_802c185c a skosxl:Label;
  skosxl:literalForm "flood insurance rate map "@en .

:xl_en_566de8c9 a skosxl:Label;
  skosxl:literalForm "FIRM"@en .

:c_8e62969e a :Terms, skos:Concept;
  skos:broader :Water_Use;
  skos:definition "A method of irrigation in which water is applied to the soil surface without flow controls, such as furrows, borders, or corrugations."@en;
  skos:inScheme :ca-dwr-g;
  skos:topConceptOf :ca-dwr-g;
  skosxl:prefLabel :xl_en_6082d1aa .

:xl_en_6082d1aa a skosxl:Label;
  skosxl:literalForm "flood irrigation "@en .

:c_862440bd a :Terms, skos:Concept;
  skos:broader :Legal_and_Regulatory, :Water_Use;
  skos:definition "An integrated and voluntary resource management strategy that uses floodwater resulting from, or in anticipation of, rainfall or snowmelt for managed aquifer recharge on agricultural lands; working landscapes; and managed natural landscapes, including but not limited to refuges, floodplains, and flood bypasses."@en;
  skos:inScheme :ca-dwr-g;
  skos:topConceptOf :ca-dwr-g;
  skosxl:altLabel :xl_en_3782aec2;
  skosxl:prefLabel :xl_en_246a1567 .

:xl_en_246a1567 a skosxl:Label;
  skosxl:literalForm "Flood-managed aquifer recharge "@en .

:xl_en_3782aec2 a skosxl:Label;
  skosxl:literalForm "Flood-MAR"@en .

:c_399271af a :Terms, skos:Concept;
  skos:broader :Legal_and_Regulatory;
  skos:definition "See flood risk management."@en;
  skos:inScheme :ca-dwr-g;
  skos:topConceptOf :ca-dwr-g;
  skosxl:prefLabel :xl_en_3062611c .

:xl_en_3062611c a skosxl:Label;
  skosxl:literalForm "flood management "@en .

:c_57905db2 a :Terms, skos:Concept;
  skos:broader :Legal_and_Regulatory;
  skos:definition "Flood risk is the likelihood of consequence of inundation within an identified area, given a specified climate condition, land use condition, and flood management system (existing or planned) in place. The consequence may be direct or indirect economic cost, loss of life, environmental impact, or other specified measure of flood effect. Flood risk is a function of the following components: "@en;
  skos:inScheme :ca-dwr-g;
  skos:topConceptOf :ca-dwr-g;
  skosxl:prefLabel :xl_en_17f805be .

:xl_en_17f805be a skosxl:Label;
  skosxl:literalForm "flood risk "@en .

:c_0432193d a :Terms, skos:Concept;
  skos:broader :Infrastructure, :Legal_and_Regulatory;
  skos:definition "Flood risk management seeks to reduce flood risks by managing the floodwaters to reduce the probability of flooding (including by levees and dams) and by managing the floodplains to reduce the consequences of flooding. Flood risk management requires integrating and synchronizing programs at various levels of government designed to reduce flood risk. (U.S. Army Corps of Engineers 2019)"@en;
  skos:inScheme :ca-dwr-g;
  skos:topConceptOf :ca-dwr-g;
  skosxl:prefLabel :xl_en_6aaf938a .

:xl_en_6aaf938a a skosxl:Label;
  skosxl:literalForm "flood risk management "@en .

:c_f56468de a :Terms, skos:Concept;
  skos:broader :Legal_and_Regulatory;
  skos:definition "The extent of the flood hazard for a 100-year (1 percent chance of exceedance in a given year) or 500-year (0.2 percent chance of exceedance in a given year) event, as determined by the Central Valley Flood Protection Plan, Federal Emergency Management Agency, or U.S. Army Corps of Engineers."@en;
  skos:inScheme :ca-dwr-g;
  skos:topConceptOf :ca-dwr-g;
  skosxl:prefLabel :xl_en_ec33841f .

:xl_en_ec33841f a skosxl:Label;
  skosxl:literalForm "floodplain "@en .

:c_168fee0b a :Terms, skos:Concept;
  skos:broader :Legal_and_Regulatory;
  skos:definition "Actions designed to reduce risks to life, property, and the environment resulting from flooding. Actions can include watershed management, infrastructure construction and operation, variations in land use practices, floodway designations, etc."@en;
  skos:inScheme :ca-dwr-g;
  skos:topConceptOf :ca-dwr-g;
  skosxl:prefLabel :xl_en_27550593 .

:xl_en_27550593 a skosxl:Label;
  skosxl:literalForm "floodplain management "@en .

:c_0091abed a :Terms, skos:Concept;
  skos:broader :Legal_and_Regulatory;
  skos:definition "FloodSAFE California refers to the California Department of Water Resources multi-faceted initiative launched in 2006 to improve public safety through flood management, in the context of integrated water management, and to reduce potential flood damages in areas of the state with the highest risk. Although led at the State level and initially funded by bond money from Propositions 1E (2006) and 84 (2006), FloodSAFE implementation relies on the cooperation and assistance of federal partners, tribal entities, local sponsors, and other stakeholders. The FloodSAFE vision is a sustainable system of flood management, with an integrated water management approach and emergency response throughout California, which improves public safety, protects and enhances environmental and cultural resources, and supports economic growth by reducing the probability of destructive floods, promoting beneficial floodplain processes, and lowering the damages caused by flooding."@en;
  skos:inScheme :ca-dwr-g;
  skos:topConceptOf :ca-dwr-g;
  skosxl:prefLabel :xl_en_685a0657 .

:xl_en_685a0657 a skosxl:Label;
  skosxl:literalForm "FloodSAFE California "@en .

:c_8efb42aa a :Terms, skos:Concept;
  skos:broader :Hydrology;
  skos:definition "A diagram that characterizes a region's hydrologic cycle by documenting sources of water, such as precipitation and inflows, and tracks the water as it flows (through many different uses) to its ultimate destinations."@en;
  skos:inScheme :ca-dwr-g;
  skos:topConceptOf :ca-dwr-g;
  skosxl:prefLabel :xl_en_dfd9fd36 .

:xl_en_dfd9fd36 a skosxl:Label;
  skosxl:literalForm "flow diagram "@en .

:c_6ef2985b a :Terms, skos:Concept;
  skos:broader :Hydrology;
  skos:definition "An itemized listing of all the categories contained in a flow diagram organized by inputs and withdrawals."@en;
  skos:inScheme :ca-dwr-g;
  skos:topConceptOf :ca-dwr-g;
  skosxl:prefLabel :xl_en_7a5458d7 .

:xl_en_7a5458d7 a skosxl:Label;
  skosxl:literalForm "flow diagram table "@en .

:c_a9193747 a :Terms, skos:Concept;
  skos:broader :Hydrology;
  skos:definition "The processes associated with rivers and streams comprising the motion of sediment and erosion of or deposition on the river bed. "@en;
  skos:inScheme :ca-dwr-g;
  skos:topConceptOf :ca-dwr-g;
  skosxl:prefLabel :xl_en_9cadaf9b .

:xl_en_9cadaf9b a skosxl:Label;
  skosxl:literalForm "fluvial "@en .

:c_4d301402 a :Terms, skos:Concept;
  skos:broader :Infrastructure;
  skos:definition "Forecast-coordinated operations refers to improving tools to forecast precipitation and river flows to allow drawing down flood management reservoirs in anticipation of major runoff so that more reservoir space is available to control downstream flood releases from a reservoir without affecting water supply."@en;
  skos:inScheme :ca-dwr-g;
  skos:topConceptOf :ca-dwr-g;
  skosxl:altLabel :xl_en_f872671d;
  skosxl:prefLabel :xl_en_2d7fa157 .

:xl_en_2d7fa157 a skosxl:Label;
  skosxl:literalForm "forecast-coordinated operations  "@en .

:xl_en_f872671d a skosxl:Label;
  skosxl:literalForm "FCO"@en .

:c_35c75cfa a :Terms, skos:Concept;
  skos:broader :Water_Use;
  skos:definition "The difference between the quantity of water demanded and the supply available for use."@en;
  skos:inScheme :ca-dwr-g;
  skos:topConceptOf :ca-dwr-g;
  skosxl:prefLabel :xl_en_7b1f4d52 .

:xl_en_7b1f4d52 a skosxl:Label;
  skosxl:literalForm "forgone use "@en .

:c_a81b351d a :Terms, skos:Concept;
  skos:broader :Environment_and_Ecology, :Legal_and_Regulatory;
  skos:definition "(1) All monetary costs associated with project planning, implementation, financing, or impact mitigation plus any recurring costs required to sustain benefits; plus (2) all nonmonetary costs that are incurred either at implementation or on a recurring basis, such as unmitigable environmental or cultural impacts, public trust, environmental justice, or other nonmarket-based societal values. (Coincides with California Environmental Quality Act/National Environmental Policy Act study requirements and other permitting requirements.)"@en;
  skos:inScheme :ca-dwr-g;
  skos:topConceptOf :ca-dwr-g;
  skosxl:prefLabel :xl_en_07ea823d .

:xl_en_07ea823d a skosxl:Label;
  skosxl:literalForm "full cost "@en .

:c_d91f4fae a :Terms, skos:Concept;
  skos:broader :Water_Use;
  skos:definition "A method of surface irrigation in which water is supplied to small ditches or furrows and guided across a field."@en;
  skos:inScheme :ca-dwr-g;
  skos:topConceptOf :ca-dwr-g;
  skosxl:prefLabel :xl_en_fbfed636 .

:xl_en_fbfed636 a skosxl:Label;
  skosxl:literalForm "furrow irrigation "@en .

:c_aacbcf4a a :Terms, skos:Concept;
  skos:definition "Geomorphology looks at the processes that shape and alter the surface features of the land. By studying landforms, including their origin and patterns, scientists attempt to comprehend the history and dynamics of landscapes."@en;
  skos:inScheme :ca-dwr-g;
  skos:topConceptOf :ca-dwr-g;
  skosxl:prefLabel :xl_en_c9d63023 .

:xl_en_c9d63023 a skosxl:Label;
  skosxl:literalForm "geomorphology "@en .

:c_a37bd2b5 a :Terms, skos:Concept;
  skos:broader :Legal_and_Regulatory, :Water_Quality;
  skos:definition "Giardia is a significant concern in drinking water, because consuming water with giardia can cause gastrointestinal illness. Since 1971, giardia has been the most commonly identified pathogen in waterborne outbreaks reported in the United States. In 1989 the U.S. Environmental Protection Agency promulgated the Surface Water Treatment Rule (SWTR) to prevent waterborne disease caused by viruses, legionella, and giardia lamblia."@en;
  skos:inScheme :ca-dwr-g;
  skos:topConceptOf :ca-dwr-g;
  skosxl:prefLabel :xl_en_80e34b7a .

:xl_en_80e34b7a a skosxl:Label;
  skosxl:literalForm "giardia "@en .

:c_3fe13fed a :Terms, skos:Concept;
  skos:broader :Legal_and_Regulatory;
  skos:definition "The California Water Plan goals are the desired outcomes and are founded on the statewide vision. Meeting the goals requires coordination among State, federal, tribal, and local governments and agencies."@en;
  skos:inScheme :ca-dwr-g;
  skos:topConceptOf :ca-dwr-g;
  skosxl:prefLabel :xl_en_44549d09 .

:xl_en_44549d09 a skosxl:Label;
  skosxl:literalForm "goals "@en .

:c_916ce6ee a :Terms, skos:Concept;
  skos:broader :Legal_and_Regulatory, :Water_Quality;
  skos:definition "Untreated wastewater that has not been affected by infectious, contaminated, or unhealthy bodily wastes, and which does not present a threat from contamination by unhealthful processing, manufacturing, or operating wastes. Gray water includes, but is not limited to, wastewater from bathtubs, showers, bathroom washbasins, clothes washing machines, and laundry tubs, but does not include wastewater from kitchen sinks or dishwashers. (California Water Code Section 14876 and Health and Safety Code Section 17922.12)"@en;
  skos:inScheme :ca-dwr-g;
  skos:topConceptOf :ca-dwr-g;
  skosxl:prefLabel :xl_en_3135bede .

:xl_en_3135bede a skosxl:Label;
  skosxl:literalForm "gray water "@en .

:c_11b6e312 a :Terms, skos:Concept;
  skos:broader :Water_Quality;
  skos:definition "The gray water footprint of a product is an indicator of freshwater pollution that can be associated with the production of a product over its full supply chain. It is defined as the volume of fresh water that is required to assimilate the load of pollutants based on existing ambient water quality standards. It is calculated as the volume of water that is required to dilute pollutants to such an extent that the quality of the water remains above agreed-upon water quality standards. This definition differs from general urban water use terms in which gray water is any wastewater that comes from an urban dwelling that does not contain bodily wastes (e.g., washing machine effluent) (definition taken in part from Hoekstra et al. 2011). See also urban wastewater produced."@en;
  skos:inScheme :ca-dwr-g;
  skos:topConceptOf :ca-dwr-g;
  skosxl:prefLabel :xl_en_c318a86d .

:xl_en_c318a86d a skosxl:Label;
  skosxl:literalForm "gray water footprint "@en .

:c_557f8834 a :Terms, skos:Concept;
  skos:broader :Environment_and_Ecology;
  skos:definition "See brownfields."@en;
  skos:inScheme :ca-dwr-g;
  skos:topConceptOf :ca-dwr-g;
  skosxl:prefLabel :xl_en_f37519dd .

:xl_en_f37519dd a skosxl:Label;
  skosxl:literalForm "grayfield land "@en .

:c_3feff4c2 a :Terms, skos:Concept;
  skos:broader :Hydrology;
  skos:definition "The precipitation on land that does not run off or recharge the groundwater but is stored in the soil or temporarily stays on top of the soil or vegetation. Eventually, this part of precipitation evaporates or transpires through plants. Green water can be made productive for crop growth (but not all green water can be taken up by crops, because there will always be evaporation from the soil and because not all periods of the year or areas are suitable for crop growth) (definition taken in part from Hoekstra et al. 2011). See also conveyance seepage - ag and ag effective precipitation on irrigated lands."@en;
  skos:inScheme :ca-dwr-g;
  skos:topConceptOf :ca-dwr-g;
  skosxl:prefLabel :xl_en_5861565d .

:xl_en_5861565d a skosxl:Label;
  skosxl:literalForm "green water "@en .

:c_a690911f a :Terms, skos:Concept;
  skos:broader :Hydrology, :Water_Use;
  skos:definition "The volume of rainwater consumed during the production process. This is particularly relevant for agricultural and forestry products (products based on crops or wood), where it refers to the total rainwater evapotranspiration (from fields and plantations) plus the water incorporated into the harvested crop or wood (definition taken in part from Hoekstra et al. 2011). See also ag effective precipitation on irrigated lands."@en;
  skos:inScheme :ca-dwr-g;
  skos:topConceptOf :ca-dwr-g;
  skosxl:prefLabel :xl_en_cf99b8fb .

:xl_en_cf99b8fb a skosxl:Label;
  skosxl:literalForm "green water footprint "@en .

:c_c0f84b41 a :Terms, skos:Concept;
  skos:broader :Environment_and_Ecology;
  skos:definition "Also referred to as carbon intensity or carbon footprint. The storage and transport of water generates hydroelectricity, which is California's largest source of energy that does not produce GHG emissions. At the same time, though, water conveyance, groundwater extraction, water and wastewater treatment, and especially water use can involve the use of substantial amounts of carbon-based energy, which in turn results in GHG emissions that contribute to climate change. Each water management strategy should be evaluated for its contribution to the accumulation of GHGs in our atmosphere."@en;
  skos:inScheme :ca-dwr-g;
  skos:topConceptOf :ca-dwr-g;
  skosxl:altLabel :xl_en_c8c8f712;
  skosxl:prefLabel :xl_en_f11e6f6f .

:xl_en_f11e6f6f a skosxl:Label;
  skosxl:literalForm "greenhouse gas emissions "@en .

:xl_en_c8c8f712 a skosxl:Label;
  skosxl:literalForm "GHG"@en .

:c_f47f101c a :Terms, skos:Concept;
  skos:broader :Hydrology;
  skos:definition "Water that occurs beneath the land surface and fills the pore spaces of the alluvium, soil, or rock formation in which it is situated. It excludes soil moisture, which refers to water held by capillary action in the upper unsaturated zones of soil or rock. Groundwater classified as underflow of a surface water system, a subterranean stream flowing through a known and definite channel, is subject to statutory permitting processes. However, most groundwater in California is presumed to be percolating water (i.e., water in underground basins and groundwater that has escaped from streams and is not subject to a permitting process). See also subterranean stream."@en;
  skos:inScheme :ca-dwr-g;
  skos:topConceptOf :ca-dwr-g;
  skosxl:prefLabel :xl_en_fc3b2834 .

:xl_en_fc3b2834 a skosxl:Label;
  skosxl:literalForm "groundwater "@en .

:c_fd731aa5 a :Terms, skos:Concept;
  skos:broader :Hydrology, :Water_Use;
  skos:definition "Consist of water that is banked during wet or above-normal water years. The water to be banked is provided by the entity that will receive the water in times of need. Although transfers or exchanges may be needed to get the water to the bank and from the bank to the water user, groundwater banks are not transfers in the typical sense. The water user stores water for future use; this is not a sale or lease of water rights. It is typical for fees to apply to the use of groundwater banks."@en;
  skos:inScheme :ca-dwr-g;
  skos:topConceptOf :ca-dwr-g;
  skosxl:prefLabel :xl_en_83913f1e .

:xl_en_83913f1e a skosxl:Label;
  skosxl:literalForm "groundwater banks "@en .

:c_8a621ce9 a :Terms, skos:Concept;
  skos:broader :Hydrology;
  skos:definition "An alluvial aquifer or a stacked series of alluvial aquifers with reasonably well-defined boundaries in a lateral direction and having a definable bottom. See also recharge basin."@en;
  skos:inScheme :ca-dwr-g;
  skos:topConceptOf :ca-dwr-g;
  skosxl:prefLabel :xl_en_d96add9d .

:xl_en_d96add9d a skosxl:Label;
  skosxl:literalForm "groundwater basin "@en .

:c_2711987c a :Terms, skos:Concept;
  skos:broader :Hydrology;
  skos:definition "A numerical accounting - the groundwater equation - of the recharge, discharge, and changes in storage of an aquifer, part of an aquifer, or a system of aquifers. A numerical accounting of inflows to and outflows from the groundwater system within a water budget zone, including the change in groundwater storage."@en;
  skos:inScheme :ca-dwr-g;
  skos:topConceptOf :ca-dwr-g;
  skosxl:prefLabel :xl_en_b46359c6 .

:xl_en_b46359c6 a skosxl:Label;
  skosxl:literalForm "groundwater budget "@en .

:c_0fd656d1 a :Terms, skos:Concept;
  skos:broader :Legal_and_Regulatory, :Water_Use;
  skos:definition "The amount of water withdrawn from basins that have been adjudicated."@en;
  skos:inScheme :ca-dwr-g;
  skos:topConceptOf :ca-dwr-g;
  skosxl:prefLabel :xl_en_a20d4507 .

:xl_en_a20d4507 a skosxl:Label;
  skosxl:literalForm "groundwater extractions - adjudicated"@en .

:c_c5925fce a :Terms, skos:Concept;
  skos:broader :Legal_and_Regulatory, :Water_Use;
  skos:definition "The amount of water withdrawn from formal interagency banking programs."@en;
  skos:inScheme :ca-dwr-g;
  skos:topConceptOf :ca-dwr-g;
  skosxl:prefLabel :xl_en_0c9a43be .

:xl_en_0c9a43be a skosxl:Label;
  skosxl:literalForm "groundwater extractions - banked "@en .

:c_994a6a70 a :Terms, skos:Concept;
  skos:broader :Legal_and_Regulatory, :Water_Use;
  skos:definition "The amount of water withdrawn from basins or fractured bedrock that are not adjudicated or part of a contract banking program."@en;
  skos:inScheme :ca-dwr-g;
  skos:topConceptOf :ca-dwr-g;
  skosxl:prefLabel :xl_en_da5530f4 .

:xl_en_da5530f4 a skosxl:Label;
  skosxl:literalForm "groundwater extractions - unadjudicated "@en .

:c_1d5bbfb7 a :Terms, skos:Concept;
  skos:broader :Hydrology;
  skos:definition "The quantity of water in the zone of saturation."@en;
  skos:inScheme :ca-dwr-g;
  skos:topConceptOf :ca-dwr-g;
  skosxl:prefLabel :xl_en_98edfe01 .

:xl_en_98edfe01 a skosxl:Label;
  skosxl:literalForm "groundwater in storage "@en .

:c_b6b676a4 a :Terms, skos:Concept;
  skos:broader :Water_Use;
  skos:definition "The planned and coordinated management of a groundwater basin or portion of a groundwater basin with a goal of long-term sustainability of the resource."@en;
  skos:inScheme :ca-dwr-g;
  skos:topConceptOf :ca-dwr-g;
  skosxl:prefLabel :xl_en_bfd2616f .

:xl_en_bfd2616f a skosxl:Label;
  skosxl:literalForm "groundwater management "@en .

:c_6fefeaba a :Terms, skos:Concept;
  skos:broader :Legal_and_Regulatory, :Water_Use;
  skos:definition "A comprehensive document developed for the purpose of groundwater management and adopted by an agency having appropriate legal or statutory authority."@en;
  skos:inScheme :ca-dwr-g;
  skos:topConceptOf :ca-dwr-g;
  skosxl:prefLabel :xl_en_4ac11511 .

:xl_en_4ac11511 a skosxl:Label;
  skosxl:literalForm "groundwater management plan "@en .

:c_3b80246f a :Terms, skos:Concept;
  skos:broader :Water_Use;
  skos:definition "The process, deliberate or inadvertent, of extracting groundwater from a source at a rate in excess of the replenishment rate such that the groundwater level declines persistently, threatening exhaustion of the supply or at least a decline of pumping levels to uneconomic depths."@en;
  skos:inScheme :ca-dwr-g;
  skos:topConceptOf :ca-dwr-g;
  skosxl:prefLabel :xl_en_c17b4179 .

:xl_en_c17b4179 a skosxl:Label;
  skosxl:literalForm "groundwater mining "@en .

:c_028d0a5e a :Terms, skos:Concept;
  skos:broader :Data_;
  skos:definition "A series of monitoring wells at appropriate locations and depths to effectively cover the area of interest. Scale and density of monitoring wells are dependent on the size and complexity of the area of interest and the objective of monitoring."@en;
  skos:inScheme :ca-dwr-g;
  skos:topConceptOf :ca-dwr-g;
  skosxl:prefLabel :xl_en_0fe075cf .

:xl_en_0fe075cf a skosxl:Label;
  skosxl:literalForm "groundwater monitoring network "@en .

:c_a03c1af0 a :Terms, skos:Concept;
  skos:broader :Water_Use;
  skos:definition "The condition of a groundwater basin in which the amount of water withdrawn by pumping exceeds the amount of water that recharges the basin over a period of years during which water supply conditions approximate average conditions."@en;
  skos:inScheme :ca-dwr-g;
  skos:topConceptOf :ca-dwr-g;
  skosxl:prefLabel :xl_en_2ec4b4d5 .

:xl_en_2ec4b4d5 a skosxl:Label;
  skosxl:literalForm "groundwater overdraft "@en .

:c_dcdb65a4 a :Terms, skos:Concept;
  skos:broader :Hydrology, :Water_Quality;
  skos:definition "Groundwater quality is a measure of the chemical, physical, bacteriological, and radiological characteristics of groundwater. Groundwater may be contaminated by either naturally occurring or anthropogenic (human-caused) sources of contamination. Groundwater that becomes contaminated by anthropogenic sources is difficult to cleanup and may take on the order of decades for the water cycle to displace the contaminated groundwater with clean water. See also water quality."@en;
  skos:inScheme :ca-dwr-g;
  skos:topConceptOf :ca-dwr-g;
  skosxl:prefLabel :xl_en_216d7a7b .

:xl_en_216d7a7b a skosxl:Label;
  skosxl:literalForm "groundwater quality "@en .

:c_c6e3e8d1 a :Terms, skos:Concept;
  skos:broader :Hydrology;
  skos:definition "The natural or managed infiltration or injection of water into a groundwater aquifer."@en;
  skos:inScheme :ca-dwr-g;
  skos:topConceptOf :ca-dwr-g;
  skosxl:prefLabel :xl_en_c533665a .

:xl_en_c533665a a skosxl:Label;
  skosxl:literalForm "groundwater recharge "@en .

:c_8128a726 a :Terms, skos:Concept;
  skos:broader :Hydrology, :Water_Use;
  skos:definition "The amount of water that is intentionally recharged through deep percolation methods into a water bank or other unconfined alluvial aquifer system for storage for future use. This may also include recharge from applied water outflow or return flow from developed supply."@en;
  skos:inScheme :ca-dwr-g;
  skos:topConceptOf :ca-dwr-g;
  skosxl:prefLabel :xl_en_0be549fe .

:xl_en_0be549fe a skosxl:Label;
  skosxl:literalForm "groundwater recharge applied water"@en .

:c_a5da63ba a :Terms, skos:Concept;
  skos:broader :Hydrology, :Water_Use;
  skos:definition "The amount of evaporation and evapotranspiration occurring from intentional groundwater recharge."@en;
  skos:inScheme :ca-dwr-g;
  skos:topConceptOf :ca-dwr-g;
  skosxl:prefLabel :xl_en_404d3349 .

:xl_en_404d3349 a skosxl:Label;
  skosxl:literalForm "groundwater recharge evaporation and evapotranspiration "@en .

:c_ec9e352a a :Terms, skos:Concept;
  skos:broader :Infrastructure;
  skos:definition "A structure that serves to conduct surface water into the ground for the purpose of replenishing groundwater. The facility may consist of dug or constructed spreading basins, pits, ditches, furrows, streambed modifications, or injection wells."@en;
  skos:inScheme :ca-dwr-g;
  skos:topConceptOf :ca-dwr-g;
  skosxl:prefLabel :xl_en_a552ab59 .

:xl_en_a552ab59 a skosxl:Label;
  skosxl:literalForm "groundwater recharge facility "@en .

:c_a85e5f4c a :Terms, skos:Concept;
  skos:broader :Hydrology, :Legal_and_Regulatory;
  skos:definition "The amount of water recharged into groundwater basins that have been adjudicated by a court of law."@en;
  skos:inScheme :ca-dwr-g;
  skos:topConceptOf :ca-dwr-g;
  skosxl:prefLabel :xl_en_79d60f68 .

:xl_en_79d60f68 a skosxl:Label;
  skosxl:literalForm "groundwater recharge - adjudicated basins "@en .

:c_2246dcc7 a :Terms, skos:Concept;
  skos:broader :Hydrology, :Legal_and_Regulatory;
  skos:definition "The amount of water recharged into groundwater basins under formal contract programs."@en;
  skos:inScheme :ca-dwr-g;
  skos:topConceptOf :ca-dwr-g;
  skosxl:prefLabel :xl_en_3d1a7361 .

:xl_en_3d1a7361 a skosxl:Label;
  skosxl:literalForm "groundwater recharge - contract banking "@en .

:c_fb43c082 a :Terms, skos:Concept;
  skos:broader :Hydrology, :Legal_and_Regulatory;
  skos:definition "The amount of water recharged into groundwater basins that are neither adjudicated nor part of formal contract banking programs."@en;
  skos:inScheme :ca-dwr-g;
  skos:topConceptOf :ca-dwr-g;
  skosxl:prefLabel :xl_en_5a3a86c6 .

:xl_en_5a3a86c6 a skosxl:Label;
  skosxl:literalForm "groundwater recharge - unadjudicated basins "@en .

:c_f8543278 a :Terms, skos:Concept;
  skos:broader :Water_Quality;
  skos:definition "Groundwater remediation involves extracting contaminated groundwater from an aquifer, treating it, and then either returning it to the aquifer or using it for agricultural or municipal purposes. Aquifer remediation is usually accomplished by treating groundwater while it is still in the aquifer by using in-situ methods involving biological, physical, or chemical treatment or electrokinetics."@en;
  skos:inScheme :ca-dwr-g;
  skos:topConceptOf :ca-dwr-g;
  skosxl:prefLabel :xl_en_3410e98b .

:xl_en_3410e98b a skosxl:Label;
  skosxl:literalForm "groundwater remediation/aquifer remediation "@en .

:c_837f948e a :Terms, skos:Concept;
  skos:broader :Hydrology, :Water_Use;
  skos:definition "An area where groundwater may be found in economically retrievable quantities outside of normally defined groundwater basins. This generally refers to areas of fractured bedrock in foothill and mountainous terrain where groundwater development is based on successful well penetration through interconnecting fracture systems. Well yields are generally lower in fractured bedrock than within groundwater basins. See also groundwater basin."@en;
  skos:inScheme :ca-dwr-g;
  skos:topConceptOf :ca-dwr-g;
  skosxl:prefLabel :xl_en_4ca8f112 .

:xl_en_4ca8f112 a skosxl:Label;
  skosxl:literalForm "groundwater source area "@en .

:c_91389d7d a :Terms, skos:Concept;
  skos:broader :Hydrology;
  skos:definition "Groundwater storage can be defined in three different ways, depending on the context of its use: (a) the quantity of water that occurs beneath the land surface and fills the pore spaces of the alluvium, soil, or rock formation beneath the land surface; (b) the volume of usable physical space available to store water in the pore spaces of the alluvium, soil, or rock formation beneath the land surface; or (c) the act of storing water in the pore spaces of the alluvium, soil, or rock formation beneath the land surface."@en;
  skos:inScheme :ca-dwr-g;
  skos:topConceptOf :ca-dwr-g;
  skosxl:prefLabel :xl_en_2f9cbd95 .

:xl_en_2f9cbd95 a skosxl:Label;
  skosxl:literalForm "groundwater storage "@en .

:c_f94e3970 a :Terms, skos:Concept;
  skos:broader :Hydrology;
  skos:definition "The volume of void space that can be occupied by water in a given volume of a formation, aquifer, or groundwater basin."@en;
  skos:inScheme :ca-dwr-g;
  skos:topConceptOf :ca-dwr-g;
  skosxl:prefLabel :xl_en_bb2b33a7 .

:xl_en_bb2b33a7 a skosxl:Label;
  skosxl:literalForm "groundwater storage capacity "@en .

:c_df2ec571 a :Terms, skos:Concept;
  skos:broader :Hydrology;
  skos:definition "A subdivision of a groundwater basin created by dividing the basin by using geologic and hydrologic conditions or institutional boundaries. See groundwater basin."@en;
  skos:inScheme :ca-dwr-g;
  skos:topConceptOf :ca-dwr-g;
  skosxl:prefLabel :xl_en_2cd0a092 .

:xl_en_2cd0a092 a skosxl:Label;
  skosxl:literalForm "groundwater subbasin "@en .

:c_5b258ca8 a :Terms, skos:Concept;
  skos:broader :Hydrology;
  skos:definition "The amount of water that flows into a region underground."@en;
  skos:inScheme :ca-dwr-g;
  skos:topConceptOf :ca-dwr-g;
  skosxl:prefLabel :xl_en_92aae60d .

:xl_en_92aae60d a skosxl:Label;
  skosxl:literalForm "groundwater subsurface inflow "@en .

:c_bf76dd42 a :Terms, skos:Concept;
  skos:broader :Hydrology;
  skos:definition "The amount of water that flows underground and out of a region, basin, or study area."@en;
  skos:inScheme :ca-dwr-g;
  skos:topConceptOf :ca-dwr-g;
  skosxl:prefLabel :xl_en_ed025c85 .

:xl_en_ed025c85 a skosxl:Label;
  skosxl:literalForm "groundwater subsurface outflow "@en .

:c_f134da0e a :Terms, skos:Concept;
  skos:broader :Hydrology;
  skos:definition "The upper surface of the zone of saturation in an unconfined aquifer."@en;
  skos:inScheme :ca-dwr-g;
  skos:topConceptOf :ca-dwr-g;
  skosxl:prefLabel :xl_en_65b2dddf .

:xl_en_65b2dddf a skosxl:Label;
  skosxl:literalForm "groundwater table "@en .

:c_4fcb3f0f a :Terms, skos:Concept;
  skos:broader :Legal_and_Regulatory;
  skos:definition "The guiding principles of the California Water plan describe the core values and philosophies that dictate how to achieve a vision, mission, and goals. In other words, guiding principles describe how to make decisions and do business."@en;
  skos:inScheme :ca-dwr-g;
  skos:topConceptOf :ca-dwr-g;
  skosxl:prefLabel :xl_en_366c10df .

:xl_en_366c10df a skosxl:Label;
  skosxl:literalForm "guiding principles "@en .

:c_eb1e49fc a :Terms, skos:Concept;
  skos:broader :Environment_and_Ecology;
  skos:definition "Highly salt-tolerant grasses."@en;
  skos:inScheme :ca-dwr-g;
  skos:topConceptOf :ca-dwr-g;
  skosxl:prefLabel :xl_en_f5b9cab3 .

:xl_en_f5b9cab3 a skosxl:Label;
  skosxl:literalForm "halophytes "@en .

:c_7ef55e41 a :Terms, skos:Concept;
  skos:broader :Environment_and_Ecology, :Water_Quality;
  skos:definition "Waste that poses a present or potential danger to human beings or other organisms because it is toxic, flammable, radioactive, or explosive, or has some other property that produces substantial risk to life."@en;
  skos:inScheme :ca-dwr-g;
  skos:topConceptOf :ca-dwr-g;
  skosxl:prefLabel :xl_en_9a825368 .

:xl_en_9a825368 a skosxl:Label;
  skosxl:literalForm "hazardous waste "@en .

:c_1eb4da03 a :Terms, skos:Concept;
  skos:broader :Hydrology, :Infrastructure;
  skos:definition "A barrier created by injecting fresh water to control seawater intrusion in an aquifer or that is created by injecting water to control migration of contaminants in an aquifer."@en;
  skos:inScheme :ca-dwr-g;
  skos:topConceptOf :ca-dwr-g;
  skosxl:prefLabel :xl_en_02b13d65 .

:xl_en_02b13d65 a skosxl:Label;
  skosxl:literalForm "hydraulic barrier "@en .

:c_27bd5c36 a :Terms, skos:Concept;
  skos:broader :Hydrology;
  skos:definition "A measure of the capacity for a rock or soil to transmit water; this generally is expressed in units of feet per day or centimeters per second."@en;
  skos:inScheme :ca-dwr-g;
  skos:topConceptOf :ca-dwr-g;
  skosxl:prefLabel :xl_en_dbda0783 .

:xl_en_dbda0783 a skosxl:Label;
  skosxl:literalForm "hydraulic conductivity "@en .

:c_68ff8515 a :Terms, skos:Concept;
  skos:broader :Hydrology;
  skos:definition "A graph that shows some property of groundwater or surface water as a function of time at a given point."@en;
  skos:inScheme :ca-dwr-g;
  skos:topConceptOf :ca-dwr-g;
  skosxl:prefLabel :xl_en_66c168c5 .

:xl_en_66c168c5 a skosxl:Label;
  skosxl:literalForm "hydrograph "@en .

:c_666bb0b2 a :Terms, skos:Concept;
  skos:broader :Hydrology;
  skos:definition "Where conceptually any drop of water that falls in the basin will flow to a stream or groundwater basin within it. A subset is the groundwater basin, which can be within a hydrologic basin. The California Department of Water Resources' hydrologic regions are collections of the larger hydrologic basins. Basin names are based on published and unpublished reports, topographic maps, and local terminology. Names of more recently delineated basins or subbasins are based on the principal geographic feature, which in most cases corresponds to the name of a valley. In the case of a subbasin, its formal name should include the name of the basin (e.g., Sacramento Valley Groundwater Basin, North American Subbasin). However, both locally and informally, the term subbasin is used interchangeably with basin (e.g., North American Basin)."@en;
  skos:inScheme :ca-dwr-g;
  skos:topConceptOf :ca-dwr-g;
  skosxl:prefLabel :xl_en_a0e755a0 .

:xl_en_a0e755a0 a skosxl:Label;
  skosxl:literalForm "hydrologic basin "@en .

:c_42eae4be a :Terms, skos:Concept;
  skos:broader :Hydrology;
  skos:definition "The circulation of water from the ocean through the atmosphere to the land and ultimately back to the ocean."@en;
  skos:inScheme :ca-dwr-g;
  skos:topConceptOf :ca-dwr-g;
  skosxl:prefLabel :xl_en_0a8dbbed .

:xl_en_0a8dbbed a skosxl:Label;
  skosxl:literalForm "hydrologic cycle "@en .

:c_a1ca5fc5 a :Terms, skos:Concept;
  skos:broader :Hydrology, :Legal_and_Regulatory;
  skos:definition "A geographical division of the state based on the local hydrologic basins. The California Department of Water Resources divides California into 10 hydrologic regions that correspond to the state's major water drainage basins: North Coast, North Lahontan, Sacramento River, San Francisco Bay, Central Coast, San Joaquin River, Tulare Lake, South Coast, South Lahontan, and Colorado River."@en;
  skos:inScheme :ca-dwr-g;
  skos:topConceptOf :ca-dwr-g;
  skosxl:prefLabel :xl_en_78c702d9 .

:xl_en_78c702d9 a skosxl:Label;
  skosxl:literalForm "hydrologic region "@en .

:c_516a0cf9 a :Terms, skos:Concept;
  skos:broader :Hydrology;
  skos:definition "The United States is divided and subdivided into successively smaller hydrologic units, which are classified into four levels: regions, subregions, accounting units, and cataloging units. The hydrologic units are arranged within each other, from the smallest (cataloging units) to the largest (regions). Each hydrologic unit is identified by a unique hydrologic unit code (HUC) consisting of two to eight digits, based on the four levels of classification in the hydrologic unit system. (Visit http://water.usgs.gov/GIS/huc.html for more information.)"@en;
  skos:inScheme :ca-dwr-g;
  skos:topConceptOf :ca-dwr-g;
  skosxl:prefLabel :xl_en_adebd722 .

:xl_en_adebd722 a skosxl:Label;
  skosxl:literalForm "hydrologic unit "@en .

:c_f878aab9 a :Terms, skos:Concept;
  skos:broader :Hydrology;
  skos:definition "A science related to the occurrence and distribution of natural water on Earth, including the annual volume and the monthly timing of runoff. "@en;
  skos:inScheme :ca-dwr-g;
  skos:topConceptOf :ca-dwr-g;
  skosxl:prefLabel :xl_en_4def5798 .

:xl_en_4def5798 a skosxl:Label;
  skosxl:literalForm "hydrology "@en .

:c_41b6c833 a :Terms, skos:Concept;
  skos:broader :Hydrology;
  skos:definition "Channel modification (channelization), flow alterations, levees, and dams."@en;
  skos:inScheme :ca-dwr-g;
  skos:topConceptOf :ca-dwr-g;
  skosxl:prefLabel :xl_en_70cc58c1 .

:xl_en_70cc58c1 a skosxl:Label;
  skosxl:literalForm "hydromodification "@en .

:c_8d0b3a60 a :Terms, skos:Concept;
  skos:broader :Hydrology;
  skos:definition "A geologic framework consisting of a body of rock having considerable lateral extent and composing a reasonably distinct hydrologic system."@en;
  skos:inScheme :ca-dwr-g;
  skos:topConceptOf :ca-dwr-g;
  skosxl:prefLabel :xl_en_c03c3b4d .

:xl_en_c03c3b4d a skosxl:Label;
  skosxl:literalForm "hydrostratigraphy "@en .

:c_231bf4e4 a :Terms, skos:Concept;
  skos:broader :Hydrology;
  skos:definition "Substances that take up water from the air. Some hygroscopic materials are being tried as supplemental cloud-seeding agents."@en;
  skos:inScheme :ca-dwr-g;
  skos:topConceptOf :ca-dwr-g;
  skosxl:prefLabel :xl_en_65aaa98f .

:xl_en_65aaa98f a skosxl:Label;
  skosxl:literalForm "hygroscopic materials "@en .

:c_a182f734 a :Terms, skos:Concept;
  skos:broader :Hydrology;
  skos:definition "The region of saturated sediments beneath and alongside the active channel, which contains some proportion of surface water that was part of the flow in the surface channel and went back underground and could mix with groundwater. "@en;
  skos:inScheme :ca-dwr-g;
  skos:topConceptOf :ca-dwr-g;
  skosxl:prefLabel :xl_en_ff7abebc .

:xl_en_ff7abebc a skosxl:Label;
  skosxl:literalForm "hyporheic zone "@en .

:c_8fd8eb37 a :Terms, skos:Concept;
  skos:broader :Hydrology, :Water_Quality;
  skos:definition "As defined by the U.S. Geological Survey's Toxic Substances Hydrology Program, Zones of hypoxia develop in water bodies, typically estuaries and coastal waters, when dissolved oxygen concentrations fall below the level to sustain most aquatic animal life. Hypoxia can be caused by a variety of factors, including excess nutrients, primarily nitrogen and phosphorus, and water body stratification due to saline or temperature gradients. These excess nutrients, eutrophication, promote algal growth. As dead algae decompose, oxygen is consumed in the process, resulting in low levels of oxygen in the water."@en;
  skos:inScheme :ca-dwr-g;
  skos:topConceptOf :ca-dwr-g;
  skosxl:prefLabel :xl_en_92604d71 .

:xl_en_92604d71 a skosxl:Label;
  skosxl:literalForm "hypoxic zone "@en .

:c_bc34877b a :Terms, skos:Concept;
  skos:broader :Legal_and_Regulatory, :Water_Quality;
  skos:definition "A water body that has been determined under State and federal law as not meeting water quality standards or having the potential to not meet such standards in the future. Impaired waters are included on California's 303(d) list."@en;
  skos:inScheme :ca-dwr-g;
  skos:topConceptOf :ca-dwr-g;
  skosxl:prefLabel :xl_en_07ebce6f .

:xl_en_07ebce6f a skosxl:Label;
  skosxl:literalForm "impaired waters "@en .

:c_1cd974a7 a :Terms, skos:Concept;
  skos:broader :Legal_and_Regulatory, :Utilities, :Water_Use;
  skos:definition "The planned use of recycled water for replenishment of a groundwater basin or an aquifer that has been designated as a source of water supply for a public water system (California Water Code 13561[c]). See also surface water augmentation. "@en;
  skos:inScheme :ca-dwr-g;
  skos:topConceptOf :ca-dwr-g;
  skosxl:prefLabel :xl_en_daf80f7e .

:xl_en_daf80f7e a skosxl:Label;
  skosxl:literalForm "indirect potable reuse "@en .

:c_cceb9650 a :Terms, skos:Concept;
  skos:broader :Water_Use;
  skos:definition "The reuse of recycled water after it has been discharged into and comingled with a natural surface water body."@en;
  skos:inScheme :ca-dwr-g;
  skos:topConceptOf :ca-dwr-g;
  skosxl:prefLabel :xl_en_cc757de3 .

:xl_en_cc757de3 a skosxl:Label;
  skosxl:literalForm "indirect reuse "@en .

:c_5ff2cc24 a :Terms, skos:Concept;
  skos:broader :Water_Use;
  skos:definition "This represents a mix of high- and low-water-using industrial activity. Note that industrial activity is broken into two factors: total industrial activity and industrial activity mix. The latter factor allows designation of the type of industry that is occurring. This is necessary to account for the large variation in water demands by industry type. See also total industrial activity."@en;
  skos:inScheme :ca-dwr-g;
  skos:topConceptOf :ca-dwr-g;
  skosxl:prefLabel :xl_en_abe566d9 .

:xl_en_abe566d9 a skosxl:Label;
  skosxl:literalForm "industrial activity mix "@en .

:c_dd40016e a :Terms, skos:Concept;
  skos:broader :Hydrology;
  skos:definition "The flow of water downward from the land surface into and through the upper soil layers."@en;
  skos:inScheme :ca-dwr-g;
  skos:topConceptOf :ca-dwr-g;
  skosxl:prefLabel :xl_en_fc006e94 .

:xl_en_fc006e94 a skosxl:Label;
  skosxl:literalForm "infiltration "@en .

:c_c3dddc23 a :Terms, skos:Concept;
  skos:broader :Hydrology;
  skos:definition "A shallow basin designed to infiltrate stormwater into the ground."@en;
  skos:inScheme :ca-dwr-g;
  skos:topConceptOf :ca-dwr-g;
  skosxl:prefLabel :xl_en_c0a4f5bc .

:xl_en_c0a4f5bc a skosxl:Label;
  skosxl:literalForm "infiltration basin "@en .

:c_9a9564f1 a :Terms, skos:Concept;
  skos:broader :Hydrology;
  skos:definition "The maximum rate at which infiltration can occur under specific conditions of soil moisture."@en;
  skos:inScheme :ca-dwr-g;
  skos:topConceptOf :ca-dwr-g;
  skosxl:prefLabel :xl_en_ebcd6733 .

:xl_en_ebcd6733 a skosxl:Label;
  skosxl:literalForm "infiltration capacity "@en .

:c_0ca37211 a :Terms, skos:Concept;
  skos:broader :Hydrology;
  skos:definition "The quantity of water that can enter the soil in a specified time interval."@en;
  skos:inScheme :ca-dwr-g;
  skos:topConceptOf :ca-dwr-g;
  skosxl:prefLabel :xl_en_b08828d2 .

:xl_en_b08828d2 a skosxl:Label;
  skosxl:literalForm "Infiltration rate "@en .

:c_e4c46bb1 a :Terms, skos:Concept;
  skos:broader :Legal_and_Regulatory;
  skos:definition "The New River and Alamo River inflows from Mexico."@en;
  skos:inScheme :ca-dwr-g;
  skos:topConceptOf :ca-dwr-g;
  skosxl:prefLabel :xl_en_0fd63bfc .

:xl_en_0fd63bfc a skosxl:Label;
  skosxl:literalForm "inflow from Mexico "@en .

:c_f794de80 a :Terms, skos:Concept;
  skos:broader :Legal_and_Regulatory;
  skos:definition "The Klamath River inflow from Oregon."@en;
  skos:inScheme :ca-dwr-g;
  skos:topConceptOf :ca-dwr-g;
  skosxl:prefLabel :xl_en_90a10260 .

:xl_en_90a10260 a skosxl:Label;
  skosxl:literalForm "inflow from Oregon "@en .

:c_fc31fdc1 a :Terms, skos:Concept;
  skos:broader :Infrastructure;
  skos:definition "The underlying foundation or basic framework of a system. For water supply, this includes the canals, pipelines, pumps, reservoirs, and treatment plants that make up a treatment and delivery system."@en;
  skos:inScheme :ca-dwr-g;
  skos:topConceptOf :ca-dwr-g;
  skosxl:prefLabel :xl_en_7cd8cb08 .

:xl_en_7cd8cb08 a skosxl:Label;
  skosxl:literalForm "infrastructure "@en .

:c_d4fda29f a :Terms, skos:Concept;
  skos:broader :Infrastructure;
  skos:definition "Injection wells are used primarily to recharge confined aquifers. The design of an injection well for artificial recharge is similar to that of a water supply well. The principal difference is that water flows from the injection well into the surrounding aquifer under either a gravity head or a head maintained by an injection pump."@en;
  skos:inScheme :ca-dwr-g;
  skos:topConceptOf :ca-dwr-g;
  skosxl:prefLabel :xl_en_205a6e3e .

:xl_en_205a6e3e a skosxl:Label;
  skosxl:literalForm "injection wells "@en .

:c_994452b1 a :Terms, skos:Concept;
  skos:broader :Hydrology, :Water_Use;
  skos:definition "The practice of providing surplus surface water to historical groundwater users, thereby leaving groundwater in storage for later use. See also groundwater recharge."@en;
  skos:inScheme :ca-dwr-g;
  skos:topConceptOf :ca-dwr-g;
  skosxl:prefLabel :xl_en_1dea5df8 .

:xl_en_1dea5df8 a skosxl:Label;
  skosxl:literalForm "in-lieu recharge "@en .

:c_729af641 a :Terms, skos:Concept;
  skos:broader :Environment_and_Ecology, :Hydrology, :Legal_and_Regulatory, :Water_Use;
  skos:definition "The volume of water in a stream dedicated for instream flow requirements, wild and scenic rivers, and minimum required Delta outflow."@en;
  skos:inScheme :ca-dwr-g;
  skos:topConceptOf :ca-dwr-g;
  skosxl:prefLabel :xl_en_8275ac33 .

:xl_en_8275ac33 a skosxl:Label;
  skosxl:literalForm "instream environmental "@en .

:c_1416eb53 a :Terms, skos:Concept;
  skos:broader :Legal_and_Regulatory, :Water_Use;
  skos:definition "The amount of water within its natural watercourse as specified in an agreement, water rights permit, court order, Federal Energy Regulatory Commission license, etc., to support natural ecosystems, create habitat for plants and animals, and possibly provide additional benefits, such as recreation. See also required instream flows."@en;
  skos:inScheme :ca-dwr-g;
  skos:topConceptOf :ca-dwr-g;
  skosxl:prefLabel :xl_en_09851cdb .

:xl_en_09851cdb a skosxl:Label;
  skosxl:literalForm "instream flow requirements "@en .

:c_2681cc6c a :Terms, skos:Concept;
  skos:broader :Hydrology, :Water_Use;
  skos:definition "Recharge that allows water to percolate through a streambed itself."@en;
  skos:inScheme :ca-dwr-g;
  skos:topConceptOf :ca-dwr-g;
  skosxl:prefLabel :xl_en_f0202315 .

:xl_en_f0202315 a skosxl:Label;
  skosxl:literalForm "instream recharge "@en .

:c_80dd6550 a :Terms, skos:Concept;
  skos:broader :Water_Use;
  skos:definition "The beneficial uses of water within a stream or river without diversion from the stream."@en;
  skos:inScheme :ca-dwr-g;
  skos:topConceptOf :ca-dwr-g;
  skosxl:prefLabel :xl_en_4923f0be .

:xl_en_4923f0be a skosxl:Label;
  skosxl:literalForm "instream uses "@en .

:c_3fbbc37a a :Terms, skos:Concept;
  skos:broader :Water_Use;
  skos:definition "An integrated agricultural water management system that applies subsurface drainage water to a sequence of increasingly salt-tolerant crops."@en;
  skos:inScheme :ca-dwr-g;
  skos:topConceptOf :ca-dwr-g;
  skosxl:prefLabel :xl_en_6437ed8f .

:xl_en_6437ed8f a skosxl:Label;
  skosxl:literalForm "integrated on-farm drainage management "@en .

:c_6dcb21a1 a :Terms, skos:Concept;
  skos:broader :Water_Quality, :Water_Use;
  skos:definition "IRWM is a collaborative effort to manage all aspects of water resources in a region and is the application of integrated water management principals at the regional scale to improve public safety, environmental stewardship, and economic stability. IRWM is based on regional water managers and resource planners being best suited and best positioned to manage regional and local water resources to meet regional needs."@en;
  skos:inScheme :ca-dwr-g;
  skos:topConceptOf :ca-dwr-g;
  skosxl:altLabel :xl_en_c5181fcc;
  skosxl:prefLabel :xl_en_82b306a7 .

:xl_en_82b306a7 a skosxl:Label;
  skosxl:literalForm "integrated regional water management "@en .

:xl_en_c5181fcc a skosxl:Label;
  skosxl:literalForm "IWRM"@en .

:c_d754806d a :Terms, skos:Concept;
  skos:broader :Legal_and_Regulatory, :Water_Quality, :Water_Use;
  skos:definition "IWM is a comprehensive and collaborative approach for managing water to concurrently achieve social, environmental, and economic objectives. In the California Water Plan, these objectives are focused toward improving public safety, fostering environmental stewardship, and supporting economic stability. The integrated approach delivers higher value for investments by considering all interests, providing multiple benefits, and working across jurisdictional boundaries at the appropriate geographic scale. Examples of multiple benefits include improved water quality, better flood management, restored and enhanced ecosystems, and more reliable water supplies."@en;
  skos:inScheme :ca-dwr-g;
  skos:topConceptOf :ca-dwr-g;
  skosxl:altLabel :xl_en_877d0149;
  skosxl:prefLabel :xl_en_aa79df36 .

:xl_en_aa79df36 a skosxl:Label;
  skosxl:literalForm "integrated water management "@en .

:xl_en_877d0149 a skosxl:Label;
  skosxl:literalForm "IWM"@en .

:c_3e6aa537 a :Terms, skos:Concept;
  skos:broader :Legal_and_Regulatory;
  skos:definition "A coordinated effort among agencies and organizations to manage watersheds or groundwater basins for sustainability."@en;
  skos:inScheme :ca-dwr-g;
  skos:topConceptOf :ca-dwr-g;
  skosxl:prefLabel :xl_en_ef286d4c .

:xl_en_ef286d4c a skosxl:Label;
  skosxl:literalForm "integrated watershed management "@en .

:c_e400084a a :Terms, skos:Concept;
  skos:broader :Data_;
  skos:definition "IWRIS is a discontinued data management tool for water resources data. It is a web-based geographic information system (GIS) application that allows one to access, integrate, query, and visualize multiple sets of data. Some of the databases include the California Department of Water Resources' Water Data Library, the California Data Exchange Center (CDEC), U.S. Geological Survey streamflow, Local Groundwater Assistance Grants (AB 303), and data from local agencies. See also Water PIE."@en;
  skos:inScheme :ca-dwr-g;
  skos:topConceptOf :ca-dwr-g;
  skosxl:altLabel :xl_en_637e5fd3;
  skosxl:prefLabel :xl_en_bd965129 .

:xl_en_bd965129 a skosxl:Label;
  skosxl:literalForm "Integrated Water Resources Information System "@en .

:xl_en_637e5fd3 a skosxl:Label;
  skosxl:literalForm "IWRIS"@en .

:c_55d976b4 a :Terms, skos:Concept;
  skos:broader :Legal_and_Regulatory;
  skos:definition "Intended results from an action taken."@en;
  skos:inScheme :ca-dwr-g;
  skos:topConceptOf :ca-dwr-g;
  skosxl:prefLabel :xl_en_9292c4ee .

:xl_en_9292c4ee a skosxl:Label;
  skosxl:literalForm "intended outcome "@en .

:c_3c677d63 a :Terms, skos:Concept;
  skos:broader :Environment_and_Ecology;
  skos:definition "The simultaneous planting of two or more crops in the same field. The practice is used to help control pest populations that can occur on monoculture crops; it is sometimes called polycropping or plant stratification."@en;
  skos:inScheme :ca-dwr-g;
  skos:topConceptOf :ca-dwr-g;
  skosxl:prefLabel :xl_en_990d9b83 .

:xl_en_990d9b83 a skosxl:Label;
  skosxl:literalForm "intercropping "@en .

:c_a98d3a1f a :Terms, skos:Concept;
  skos:broader :Hydrology;
  skos:definition "Smaller watersheds or areas outside of the larger watershed boundaries used at the regional planning scale. "@en;
  skos:inScheme :ca-dwr-g;
  skos:topConceptOf :ca-dwr-g;
  skosxl:prefLabel :xl_en_496f120e .

:xl_en_496f120e a skosxl:Label;
  skosxl:literalForm "interfluves "@en .

:c_771dbbd8 a :Terms, skos:Concept;
  skos:broader :Infrastructure, :Water_Use;
  skos:definition "This represents the movement of water between hydrologic regions through such mechanisms as the State Water Project and federal water projects."@en;
  skos:inScheme :ca-dwr-g;
  skos:topConceptOf :ca-dwr-g;
  skosxl:prefLabel :xl_en_b3f39c11 .

:xl_en_b3f39c11 a skosxl:Label;
  skosxl:literalForm "interregional import projects"@en .

:c_7d6194f2 a :Terms, skos:Concept;
  skos:broader :Infrastructure, :Utilities;
  skos:definition "An interconnection permitting passage of utility service (e.g., water or electricity) between two or more systems, such as electric and water utility systems."@en;
  skos:inScheme :ca-dwr-g;
  skos:topConceptOf :ca-dwr-g;
  skosxl:prefLabel :xl_en_08e2bb3b .

:xl_en_08e2bb3b a skosxl:Label;
  skosxl:literalForm "interties "@en .

:c_c3382946 a :Terms, skos:Concept;
  skos:broader :Environment_and_Ecology;
  skos:definition "Non-indigenous plants or animals that adversely affect the habitats they invade economically, environmentally, and/or ecologically."@en;
  skos:inScheme :ca-dwr-g;
  skos:topConceptOf :ca-dwr-g;
  skosxl:prefLabel :xl_en_49c7d732 .

:xl_en_49c7d732 a skosxl:Label;
  skosxl:literalForm "invasive species "@en .

:c_cf91957e a :Terms, skos:Concept;
  skos:broader :Water_Quality;
  skos:definition "Processes of purification, separation, and decontamination of aqueous and other ion-containing solutions with solid ion exchangers, such as sodium carbonate used for water softening."@en;
  skos:inScheme :ca-dwr-g;
  skos:topConceptOf :ca-dwr-g;
  skosxl:prefLabel :xl_en_19b7af1f .

:xl_en_19b7af1f a skosxl:Label;
  skosxl:literalForm "ion exchange "@en .

:c_b28d562d a :Terms, skos:Concept;
  skos:broader :Water_Use;
  skos:definition "The amount of water that flows or percolates to a salt sink, is used by the growth process of plants (evapotranspiration), or evaporates from a conveyance facility or drainage canal. See also recoverable water."@en;
  skos:inScheme :ca-dwr-g;
  skos:topConceptOf :ca-dwr-g;
  skosxl:prefLabel :xl_en_64384305 .

:xl_en_64384305 a skosxl:Label;
  skosxl:literalForm "irrecoverable water "@en .

:c_e115a4e4 a :Terms, skos:Concept;
  skos:broader :Legal_and_Regulatory, :Water_Quality;
  skos:definition "State Water Resources Control Board and Regional Water Quality Control Board program regulating discharges from irrigated agriculture through conditional waivers of Waste Discharge Requirements."@en;
  skos:inScheme :ca-dwr-g;
  skos:topConceptOf :ca-dwr-g;
  skosxl:prefLabel :xl_en_de32281f .

:xl_en_de32281f a skosxl:Label;
  skosxl:literalForm "Irrigated Lands Regulatory Program "@en .

:c_7131da38 a :Terms, skos:Concept;
  skos:broader :Water_Use;
  skos:definition "The efficiency of water application and use, calculated by dividing a portion of applied water that is beneficially used by the total applied water, expressed as a percentage. The two main beneficial uses are crop water use (evapotranspiration or ET) and leaching to maintain a salt balance. "@en;
  skos:inScheme :ca-dwr-g;
  skos:topConceptOf :ca-dwr-g;
  skosxl:altLabel :xl_en_e081230b;
  skosxl:prefLabel :xl_en_a2978d5f .

:xl_en_a2978d5f a skosxl:Label;
  skosxl:literalForm "irrigation efficiency "@en .

:xl_en_e081230b a skosxl:Label;
  skosxl:literalForm "IE"@en .

:c_f2e48bfe a :Terms, skos:Concept;
  skos:broader :Water_Use;
  skos:definition "The quantity of water, exclusive of precipitation, that is required for various irrigation purposes."@en;
  skos:inScheme :ca-dwr-g;
  skos:topConceptOf :ca-dwr-g;
  skosxl:prefLabel :xl_en_f56c5bc2 .

:xl_en_f56c5bc2 a skosxl:Label;
  skosxl:literalForm "irrigation water requirements "@en .

:c_ef563605 a :Terms, skos:Concept;
  skos:broader :Legal_and_Regulatory;
  skos:definition "An agreement entered into by two or more public agencies that allows them to jointly exercise any power common to the contracting parties. JPA is defined in California Government Code Title 1, Division 7, Chapter 5 (commencing with Section 6500)."@en;
  skos:inScheme :ca-dwr-g;
  skos:topConceptOf :ca-dwr-g;
  skosxl:altLabel :xl_en_aa1bf508;
  skosxl:prefLabel :xl_en_84f4efb1 .

:xl_en_84f4efb1 a skosxl:Label;
  skosxl:literalForm "joint powers agreement "@en .

:xl_en_aa1bf508 a skosxl:Label;
  skosxl:literalForm "JPA"@en .

:c_625e2fbf a :Terms, skos:Concept;
  skos:broader :Infrastructure, :Water_Use;
  skos:definition "Keyline systems of water and soil conservation were developed in Australia during the 1950s by mining geologist and inventor P.A. Yeomans, as a response to increasing desertification and erosion of the landscape. Keyline agriculture is a permaculture farming technique offering holistic farm design. Keyline is a set of principles, techniques, and systems that coordinates into a development plan for rural and urban landscapes. The result is a strategic master plan to develop the natural or existing landscape through regeneration and enhancement. On Keyline properties, the typical vistas are of lakes with water birds, roads along the contours and ridge lines, contour tree belts, healthy crops, and green pasture growing in dark, biologically fertile soil."@en;
  skos:inScheme :ca-dwr-g;
  skos:topConceptOf :ca-dwr-g;
  skosxl:prefLabel :xl_en_bd927913 .

:xl_en_bd927913 a skosxl:Label;
  skosxl:literalForm "Keyline systems "@en .

:c_7efb9a88 a :Terms, skos:Concept;
  skos:broader :Hydrology;
  skos:definition "Natural lake, pond, and human-made reservoir ecosystems."@en;
  skos:inScheme :ca-dwr-g;
  skos:topConceptOf :ca-dwr-g;
  skosxl:prefLabel :xl_en_1a836eb9 .

:xl_en_1a836eb9 a skosxl:Label;
  skosxl:literalForm "lacustrine "@en .

:c_cd4ac51d a :Terms, skos:Concept;
  skos:broader :Hydrology, :Water_Use;
  skos:definition "Land subsidence occurs in areas experiencing significant declines in groundwater levels. When groundwater is extracted from aquifers in sufficient quantity, the groundwater level is lowered and the water pressure, which supports the sediment grains structure, decreases. In unconsolidated deposits, as aquifer pressures decrease, the increased weight from overlying sediments may compact the fine-grained sediments and permanently decrease the porosity of the aquifer and the ability of the aquifer to store water. Elastic land subsidence is the reversible and temporary fluctuation of the earth's surface in response to seasonal groundwater extraction and recharge. Inelastic land subsidence is the irreversible and permanent decline in the earth's surface due to the collapse or compaction of the pore structure within the fine-grained portions of an aquifer system (U.S. Geological Survey 1999). Inelastic land subsidence thus results in irreversible compaction of the aquifer and permanent loss of aquifer storage capacity and can have serious effects on groundwater supply and development. Land subsidence due to aquifer compaction can cause costly damage to the gradient and flood capacity of conveyance channels, to water system infrastructure (including wells), and to farming operations."@en;
  skos:inScheme :ca-dwr-g;
  skos:topConceptOf :ca-dwr-g;
  skosxl:prefLabel :xl_en_f99e4a70 .

:xl_en_f99e4a70 a skosxl:Label;
  skosxl:literalForm "land subsidence "@en .

:c_b98c6832 a :Terms, skos:Concept;
  skos:broader :Water_Use;
  skos:definition "People will purchase less of a good or service as its price increases. "@en;
  skos:inScheme :ca-dwr-g;
  skos:topConceptOf :ca-dwr-g;
  skosxl:prefLabel :xl_en_6f6e33dc .

:xl_en_6f6e33dc a skosxl:Label;
  skosxl:literalForm "law of demand "@en .

:c_8e69c936 a :Terms, skos:Concept;
  skos:broader :Hydrology, :Water_Quality;
  skos:definition "The ratio of the average salt concentration in drainage water to an average salt concentration in the soil water of the root zone when near field capacity."@en;
  skos:inScheme :ca-dwr-g;
  skos:topConceptOf :ca-dwr-g;
  skosxl:prefLabel :xl_en_0b50524f .

:xl_en_0b50524f a skosxl:Label;
  skosxl:literalForm "leaching efficiency "@en .

:c_8070048b a :Terms, skos:Concept;
  skos:broader :Hydrology;
  skos:definition "The fraction of water entering the soil that must pass through the root zone to prevent soil salinity from exceeding a specific value."@en;
  skos:inScheme :ca-dwr-g;
  skos:topConceptOf :ca-dwr-g;
  skosxl:prefLabel :xl_en_2fa27d3a .

:xl_en_2fa27d3a a skosxl:Label;
  skosxl:literalForm "leaching requirements "@en .

:c_0f929f29 a :Terms, skos:Concept;
  skos:broader :Hydrology;
  skos:definition "A low-permeability layer that can transmit water at sufficient rates to furnish some recharge from an adjacent aquifer to a well."@en;
  skos:inScheme :ca-dwr-g;
  skos:topConceptOf :ca-dwr-g;
  skosxl:prefLabel :xl_en_62f187fa .

:xl_en_62f187fa a skosxl:Label;
  skosxl:literalForm "leaky confining layer "@en .

:c_0e4c5f7f a :Terms, skos:Concept;
  skos:broader :Environment_and_Ecology;
  skos:definition "Inheritance of negative impacts from anthropogenically induced change, such as legacy pollution and legacy changes to ecosystems or individual species."@en;
  skos:inScheme :ca-dwr-g;
  skos:topConceptOf :ca-dwr-g;
  skosxl:prefLabel :xl_en_c89c8c24 .

:xl_en_c89c8c24 a skosxl:Label;
  skosxl:literalForm "legacy impacts "@en .

:c_8a60fef3 a :Terms, skos:Concept;
  skos:broader :Legal_and_Regulatory, :Water_Quality;
  skos:definition "Examples of legacy pollutants are mercury, extracted from the Coast Ranges and used to process gold in the Sierra Nevada mines in the 19th century; industrial chemicals, such as polychlorinated biphenyls (PCBs), used in electrical transformers; and pesticides, such as dichloro-diphenyl-trichloroethane (DDT)."@en;
  skos:inScheme :ca-dwr-g;
  skos:topConceptOf :ca-dwr-g;
  skosxl:prefLabel :xl_en_8ad508b6 .

:xl_en_8ad508b6 a skosxl:Label;
  skosxl:literalForm "legacy pollutants "@en .

:c_6858e553 a :Terms, skos:Concept;
  skos:broader :Data_, :Hydrology;
  skos:definition "A record of the lithology of the soils, sediments, or rock encountered in a borehole from the surface to the bottom."@en;
  skos:inScheme :ca-dwr-g;
  skos:topConceptOf :ca-dwr-g;
  skosxl:prefLabel :xl_en_bd413b1e .

:xl_en_bd413b1e a skosxl:Label;
  skosxl:literalForm "lithologic log "@en .

:c_5b573556 a :Terms, skos:Concept;
  skos:broader :Hydrology;
  skos:definition "The description of rocks, especially in hand specimens and in outcrops, on the basis of such characteristics as color, mineralogic composition, and grain size."@en;
  skos:inScheme :ca-dwr-g;
  skos:topConceptOf :ca-dwr-g;
  skosxl:prefLabel :xl_en_6b2c9711 .

:xl_en_6b2c9711 a skosxl:Label;
  skosxl:literalForm "lithology "@en .

:c_c8b5c496 a :Terms, skos:Concept;
  skos:broader :Water_Use;
  skos:definition "The amount of water delivered by local water agencies and individuals. It includes direct deliveries of water from streamflows, as well as local water-storage facilities. It also includes water supply that remains in the stream for instream requirements and Wild and Scenic rivers."@en;
  skos:inScheme :ca-dwr-g;
  skos:topConceptOf :ca-dwr-g;
  skosxl:prefLabel :xl_en_8ea3fe9b .

:xl_en_8ea3fe9b a skosxl:Label;
  skosxl:literalForm "local deliveries "@en .

:c_3584afe3 a :Terms, skos:Concept;
  skos:broader :Water_Use;
  skos:definition "The amount of water transferred by local agencies from other regions of the state."@en;
  skos:inScheme :ca-dwr-g;
  skos:topConceptOf :ca-dwr-g;
  skosxl:prefLabel :xl_en_224d25a2 .

:xl_en_224d25a2 a skosxl:Label;
  skosxl:literalForm "local imported deliveries "@en .

:c_6cfe78b8 a :Terms, skos:Concept;
  skos:broader :Water_Use;
  skos:definition "The amount of water from local water storage facilities."@en;
  skos:inScheme :ca-dwr-g;
  skos:topConceptOf :ca-dwr-g;
  skosxl:prefLabel :xl_en_b31f2feb .

:xl_en_b31f2feb a skosxl:Label;
  skosxl:literalForm "local projects "@en .

:c_743aadb1 a :Terms, skos:Concept;
  skos:broader :Infrastructure;
  skos:definition "LID uses site design and stormwater management to maintain the site's pre-development runoff rates and volumes. Design techniques filtrate, filter, store, evaporate, and detain runoff close to the source of rainfall. LID can be used to benefit water quality and to address the modifications to the hydrologic cycle, and it can be a means to augment local water supply through either infiltration or water harvesting. LID is seen in California as an alternative to conventional stormwater management."@en;
  skos:inScheme :ca-dwr-g;
  skos:topConceptOf :ca-dwr-g;
  skosxl:altLabel :xl_en_f0f190f6;
  skosxl:prefLabel :xl_en_96733fbc .

:xl_en_96733fbc a skosxl:Label;
  skosxl:literalForm "low-impact development "@en .

:xl_en_f0f190f6 a skosxl:Label;
  skosxl:literalForm "LID"@en .

:c_63f5f252 a :Terms, skos:Concept;
  skos:broader :Environment_and_Ecology, :Legal_and_Regulatory;
  skos:definition "Impounded freshwater and nontidal brackish water wetlands."@en;
  skos:inScheme :ca-dwr-g;
  skos:topConceptOf :ca-dwr-g;
  skosxl:prefLabel :xl_en_9819bfe7 .

:xl_en_9819bfe7 a skosxl:Label;
  skosxl:literalForm "managed wetlands "@en .

:c_86467770 a :Terms, skos:Concept;
  skos:broader :Legal_and_Regulatory, :Water_Use;
  skos:definition "The percentage of available water that an irrigator will allow plants to deplete before irrigating, or the depth of water that an irrigator will allow plants to extract from the root zone between irrigations."@en;
  skos:inScheme :ca-dwr-g;
  skos:topConceptOf :ca-dwr-g;
  skosxl:altLabel :xl_en_95729505;
  skosxl:prefLabel :xl_en_2b91463e .

:xl_en_2b91463e a skosxl:Label;
  skosxl:literalForm "management allowable depletion "@en .

:xl_en_95729505 a skosxl:Label;
  skosxl:literalForm "MAD"@en .

:c_4567cbb6 a :Terms, skos:Concept;
  skos:broader :Legal_and_Regulatory;
  skos:definition "Objectives that set forth the priorities and measurable criteria of water management (e.g., improve water quality, augment water supplies, improve water use efficiency). "@en;
  skos:inScheme :ca-dwr-g;
  skos:topConceptOf :ca-dwr-g;
  skosxl:prefLabel :xl_en_5253af8e .

:xl_en_5253af8e a skosxl:Label;
  skosxl:literalForm "management objectives "@en .

:c_f93286de a :Terms, skos:Concept;
  skos:broader :Legal_and_Regulatory, :Water_Quality, :Water_Use;
  skos:definition "A resource management strategy recognizing that not all water uses require the same quality of water. High-quality water sources can be used for drinking and industrial purposes that benefit from higher quality water, whereas lesser quality water is adequate for other uses. "@en;
  skos:inScheme :ca-dwr-g;
  skos:topConceptOf :ca-dwr-g;
  skosxl:prefLabel :xl_en_cb50d96b .

:xl_en_cb50d96b a skosxl:Label;
  skosxl:literalForm "matching water quality to use "@en .

:c_8ef8be29 a :Terms, skos:Concept;
  skos:broader :Legal_and_Regulatory, :Water_Quality;
  skos:definition "The maximum permissible level of a contaminant in drinking water delivered to any user of a public water system. MCLs are drinking water standards set in federal and State Safe Drinking Water Act regulations."@en;
  skos:inScheme :ca-dwr-g;
  skos:topConceptOf :ca-dwr-g;
  skosxl:altLabel :xl_en_9a56c486;
  skosxl:prefLabel :xl_en_b7289f4a .

:xl_en_b7289f4a a skosxl:Label;
  skosxl:literalForm "maximum contaminant level "@en .

:xl_en_9a56c486 a skosxl:Label;
  skosxl:literalForm "MCL"@en .

:c_ccb129ad a :Terms, skos:Concept;
  skos:broader :Environment_and_Ecology;
  skos:definition "Most of California has this type of climate, characterized by cool, rainy winters and dry summers."@en;
  skos:inScheme :ca-dwr-g;
  skos:topConceptOf :ca-dwr-g;
  skosxl:prefLabel :xl_en_6b191a8d .

:xl_en_6b191a8d a skosxl:Label;
  skosxl:literalForm "Mediterranean climate "@en .

:c_b526b769 a :Terms, skos:Concept;
  skos:broader :Data_;
  skos:definition "Chemical contaminants in water are often measured in micrograms per liter  or parts per billion."@en;
  skos:inScheme :ca-dwr-g;
  skos:topConceptOf :ca-dwr-g;
  skosxl:prefLabel :xl_en_db54ca65 .

:xl_en_db54ca65 a skosxl:Label;
  skosxl:literalForm "micrograms per liter "@en .

:c_32d84bc0 a :Terms, skos:Concept;
  skos:broader :Water_Use;
  skos:definition "The frequent application of small quantities of water as drops, tiny streams, or miniature sprays through emitters or applicators placed along a water delivery line. Microirrigation encompasses a number of methods or concepts, such as bubbler, drip, trickle, mist, and spray irrigation."@en;
  skos:inScheme :ca-dwr-g;
  skos:topConceptOf :ca-dwr-g;
  skosxl:prefLabel :xl_en_88288ce5 .

:xl_en_88288ce5 a skosxl:Label;
  skosxl:literalForm "microirrigation "@en .

:c_9b270cf8 a :Terms, skos:Concept;
  skos:broader :Data_;
  skos:definition "Chemical contaminants in water are often measured in milligrams per liter (mg/L) or parts per million."@en;
  skos:inScheme :ca-dwr-g;
  skos:topConceptOf :ca-dwr-g;
  skosxl:prefLabel :xl_en_3e907d06 .

:xl_en_3e907d06 a skosxl:Label;
  skosxl:literalForm "milligrams per liter "@en .

:c_252cf466 a :Terms, skos:Concept;
  skos:broader :Water_Use;
  skos:definition "The minimum volume of freshwater outflow from the Sacramento-San Joaquin Delta required by law to maintain flow and water quality standards to protect the beneficial uses within the Delta."@en;
  skos:inScheme :ca-dwr-g;
  skos:topConceptOf :ca-dwr-g;
  skosxl:prefLabel :xl_en_812a0604 .

:xl_en_812a0604 a skosxl:Label;
  skosxl:literalForm "minimum required Detla outflow "@en .

:c_596b08e7 a :Terms, skos:Concept;
  skos:broader :Legal_and_Regulatory;
  skos:definition "The California Water Plan's mission statement describes the collaborative efforts to prepare for California's most pressing statewide and regional water management issues and challenges, the California Water plan's unique purpose, and its overarching reason for existence. It identifies what the water plan should do, why, and for whom."@en;
  skos:inScheme :ca-dwr-g;
  skos:topConceptOf :ca-dwr-g;
  skosxl:prefLabel :xl_en_d436a755 .

:xl_en_d436a755 a skosxl:Label;
  skosxl:literalForm "mission statement "@en .

:c_67bc957c a :Terms, skos:Concept;
  skos:broader :Environment_and_Ecology;
  skos:definition "In the context of climate change, this represents the reduction of human activities that affect global climate change; it includes strategies to reduce greenhouse gas emissions."@en;
  skos:inScheme :ca-dwr-g;
  skos:topConceptOf :ca-dwr-g;
  skosxl:prefLabel :xl_en_d397b12b .

:xl_en_d397b12b a skosxl:Label;
  skosxl:literalForm "mitigation (measurements/strategies) "@en .

:c_7f9b5949 a :Terms, skos:Concept;
  skos:broader :Water_Quality;
  skos:definition "An additive originally put in gasoline to reduce air pollution, but later found to be a source of groundwater pollution. The State of California ordered a phase-out of its use in California gasoline by the end of 2003."@en;
  skos:inScheme :ca-dwr-g;
  skos:topConceptOf :ca-dwr-g;
  skosxl:altLabel :xl_en_7b6e7c57;
  skosxl:prefLabel :xl_en_f0d6cc54 .

:xl_en_f0d6cc54 a skosxl:Label;
  skosxl:literalForm "methyl tertiary butyl ether "@en .

:xl_en_7b6e7c57 a skosxl:Label;
  skosxl:literalForm "MTBE"@en .

:c_9b412e66 a :Terms, skos:Concept;
  skos:broader :Data_;
  skos:definition "A well used to obtain water quality samples or measure groundwater levels."@en;
  skos:inScheme :ca-dwr-g;
  skos:topConceptOf :ca-dwr-g;
  skosxl:prefLabel :xl_en_8b8917c9 .

:xl_en_8b8917c9 a skosxl:Label;
  skosxl:literalForm "monitoring well "@en .

:c_6d38d74b a :Terms, skos:Concept;
  skos:broader :Legal_and_Regulatory;
  skos:definition "A project that accomplishes two or more intended outcomes. These projects are the result of collaboration among water management sectors, are multi-disciplinary, and leverage multiple funding sources. "@en;
  skos:inScheme :ca-dwr-g;
  skos:topConceptOf :ca-dwr-g;
  skosxl:prefLabel :xl_en_f1f1c64a .

:xl_en_f1f1c64a a skosxl:Label;
  skosxl:literalForm "multi-benefit projects "@en .

:c_3c9e0525 a :Terms, skos:Concept;
  skos:broader :Water_Use;
  skos:definition "The practice of growing one or more crops on the same field two or more times within a year. For example, in a single field, broccoli may be grown in the spring and lettuce in the fall."@en;
  skos:inScheme :ca-dwr-g;
  skos:topConceptOf :ca-dwr-g;
  skosxl:prefLabel :xl_en_c9da01c9 .

:xl_en_c9da01c9 a skosxl:Label;
  skosxl:literalForm "multicropping"@en .

:c_45356f34 a :Terms, skos:Concept;
  skos:broader :Utilities, :Water_Use;
  skos:definition "Recycled water that wholly or in part is derived from municipal wastewater and is subsequently beneficially reused. Beneficial reuses are not limited to municipal applications."@en;
  skos:inScheme :ca-dwr-g;
  skos:topConceptOf :ca-dwr-g;
  skosxl:prefLabel :xl_en_040f423b .

:xl_en_040f423b a skosxl:Label;
  skosxl:literalForm "municipal recycled water "@en .

:c_b69a720d a :Terms, skos:Concept;
  skos:broader :Legal_and_Regulatory, :Utilities;
  skos:definition "A system of pipes, ditches, or gullies that is owned and/or operated by a municipal government entity for collecting and conveying stormwater and is separate from the collection system for municipal wastewater."@en;
  skos:inScheme :ca-dwr-g;
  skos:topConceptOf :ca-dwr-g;
  skosxl:altLabel :xl_en_e4db9d93;
  skosxl:prefLabel :xl_en_e1cfc9ac .

:xl_en_e1cfc9ac a skosxl:Label;
  skosxl:literalForm "Municipal Separate Storm Sewer System "@en .

:xl_en_e4db9d93 a skosxl:Label;
  skosxl:literalForm "MS4"@en .

:c_d9785981 a :Terms, skos:Concept;
  skos:broader :Utilities;
  skos:definition "Municipal wastewater comes primarily from domestic sources but also includes wastewater from commercial, industrial, and institutional sources that discharge to a common collection system, where it mixes with domestic wastewater before treatment."@en;
  skos:inScheme :ca-dwr-g;
  skos:topConceptOf :ca-dwr-g;
  skosxl:prefLabel :xl_en_26a4dcc6 .

:xl_en_26a4dcc6 a skosxl:Label;
  skosxl:literalForm "municipal wastewater "@en .

:c_53a13cc7 a :Terms, skos:Concept;
  skos:broader :Legal_and_Regulatory;
  skos:definition "The NFIP is a federal program created by the U.S. Congress to mitigate future flood losses nationwide. The NFIP requires local communities to enforce building and zoning ordinances in exchange for access to affordable, federally backed flood insurance protection for property owners."@en;
  skos:inScheme :ca-dwr-g;
  skos:topConceptOf :ca-dwr-g;
  skosxl:altLabel :xl_en_6b1a7c01;
  skosxl:prefLabel :xl_en_06b4b8f0 .

:xl_en_06b4b8f0 a skosxl:Label;
  skosxl:literalForm "National Flood Insurance Program "@en .

:xl_en_6b1a7c01 a skosxl:Label;
  skosxl:literalForm "NFIP"@en .

:c_c6fe3cbd a :Terms, skos:Concept;
  skos:broader :Legal_and_Regulatory, :Water_Quality;
  skos:definition "A provision of the Clean Water Act that prohibits discharge of pollutants into waters of the United States unless a permit is issued that complies with the Clean Water Act. The State and regional boards issue waste discharge requirements that serve as NPDES permits in California."@en;
  skos:inScheme :ca-dwr-g;
  skos:topConceptOf :ca-dwr-g;
  skosxl:altLabel :xl_en_7ed781cb;
  skosxl:prefLabel :xl_en_7034c8ad .

:xl_en_7034c8ad a skosxl:Label;
  skosxl:literalForm "National Pollutant Discharge Elimination System "@en .

:xl_en_7ed781cb a skosxl:Label;
  skosxl:literalForm "NPDES"@en .

:c_f4cb1eb9 a :Terms, skos:Concept;
  skos:broader :Environment_and_Ecology, :Legal_and_Regulatory;
  skos:definition "The U.S. Environmental Protection Agency's list of the most serious uncontrolled or abandoned hazardous waste sites identified for possible long-term remedial action under Superfund. The list is based primarily on the score a site receives from the Hazard Ranking System. The EPA is required to update the NPL at least once a year. A site must be on the NPL to receive money for remedial action from the Superfund Trust Fund."@en;
  skos:inScheme :ca-dwr-g;
  skos:topConceptOf :ca-dwr-g;
  skosxl:altLabel :xl_en_0bb9ef9b;
  skosxl:prefLabel :xl_en_a67e510c .

:xl_en_a67e510c a skosxl:Label;
  skosxl:literalForm "National Priorities List "@en .

:xl_en_0bb9ef9b a skosxl:Label;
  skosxl:literalForm "NPL"@en .

:c_68cd1707 a :Terms, skos:Concept;
  skos:broader :Hydrology;
  skos:definition "Replenishment of an aquifer generally from snowmelt and runoff, through seepage from the surface. Recharge of an aquifer that occurs without human interference - also referred to as unintentional recharge."@en;
  skos:inScheme :ca-dwr-g;
  skos:topConceptOf :ca-dwr-g;
  skosxl:prefLabel :xl_en_3eff36ff .

:xl_en_3eff36ff a skosxl:Label;
  skosxl:literalForm "natural recharge "@en .

:c_66b55c65 a :Terms, skos:Concept;
  skos:broader :Hydrology, :Water_Quality;
  skos:definition "Application of natural processes, such as wetlands or aquifer treatment, to filter or biologically remove contaminants from water. "@en;
  skos:inScheme :ca-dwr-g;
  skos:topConceptOf :ca-dwr-g;
  skosxl:prefLabel :xl_en_485d921a .

:xl_en_485d921a a skosxl:Label;
  skosxl:literalForm "natural treatment "@en .

:c_8fa112aa a :Terms, skos:Concept;
  skos:broader :Hydrology;
  skos:definition "See background water conservation."@en;
  skos:inScheme :ca-dwr-g;
  skos:topConceptOf :ca-dwr-g;
  skosxl:prefLabel :xl_en_89f0d76e .

:xl_en_89f0d76e a skosxl:Label;
  skosxl:literalForm "naturally occurring conservation "@en .

:c_f9173d20 a :Terms, skos:Concept;
  skos:broader :Legal_and_Regulatory, :Water_Quality;
  skos:definition "Contaminants that exist naturally in the environment (e.g., arsenic, uranium, fluoride) and are not human-made or human-introduced. Naturally occurring contaminants are considered pollutants when they exceed a maximum contaminant level (MCL)."@en;
  skos:inScheme :ca-dwr-g;
  skos:topConceptOf :ca-dwr-g;
  skosxl:prefLabel :xl_en_b91a8357 .

:xl_en_b91a8357 a skosxl:Label;
  skosxl:literalForm "naturally occurring contaminants "@en .

:c_5aa409b8 a :Terms, skos:Concept;
  skos:broader :Hydrology, :Water_Use;
  skos:definition "The amount of groundwater extraction in excess of recoverable deep percolation."@en;
  skos:inScheme :ca-dwr-g;
  skos:topConceptOf :ca-dwr-g;
  skosxl:prefLabel :xl_en_8691f370 .

:xl_en_8691f370 a skosxl:Label;
  skosxl:literalForm "net groundwater extraction "@en .

:c_9ccbc79c a :Terms, skos:Concept;
  skos:broader :Water_Use;
  skos:definition "In the context of agricultural water use efficiency, this represents the reduction in the amount of water used that becomes available for other purposes while maintaining or improving crop yield."@en;
  skos:inScheme :ca-dwr-g;
  skos:topConceptOf :ca-dwr-g;
  skosxl:prefLabel :xl_en_381ed291 .

:xl_en_381ed291 a skosxl:Label;
  skosxl:literalForm "net water savings "@en .

:c_143f104a a :Terms, skos:Concept;
  skos:broader :Water_Use;
  skos:definition "The amount of water needed in a water service area to meet all requirements. It includes the consumptive use of applied water, irrecoverable water from the distribution system, and the outflow leaving the service area. It does not include reuse of water within a service area, including recoverable deep percolation. See also applied water use."@en;
  skos:inScheme :ca-dwr-g;
  skos:topConceptOf :ca-dwr-g;
  skosxl:prefLabel :xl_en_f530769a .

:xl_en_f530769a a skosxl:Label;
  skosxl:literalForm "net water use "@en .

:c_3bb37502 a :Terms, skos:Concept;
  skos:broader :Water_Use;
  skos:definition "Water that is legally and empirically available for a beneficial use; it can be developed through many strategies, such as capture of surplus water, desalination of ocean water, and reductions in depletion. (This is the same as real water.) The term denotes, in part, recycled water that is an augmentation to the state's overall water supply, such as the reuse of wastewater discharged to the ocean, rather than planned reuse of wastewater inland where unplanned indirect reuse may already be occurring downstream. The Recycled Water Task Force made this distinction in estimating future potential. Of an estimated potential of 1.5 million acre-feet per year of additional recycled water use by 2030, 1.2 million acre-feet per year was estimated to be new water. See also saved water."@en;
  skos:inScheme :ca-dwr-g;
  skos:topConceptOf :ca-dwr-g;
  skosxl:prefLabel :xl_en_79a90b44 .

:xl_en_79a90b44 a skosxl:Label;
  skosxl:literalForm "new water "@en .

:c_aaf963a0 a :Terms, skos:Concept;
  skos:broader :Water_Quality;
  skos:definition "Water that is unsafe to drink because it contains contaminants and/or is untreated. See also potable."@en;
  skos:inScheme :ca-dwr-g;
  skos:topConceptOf :ca-dwr-g;
  skosxl:prefLabel :xl_en_ec6de41d .

:xl_en_ec6de41d a skosxl:Label;
  skosxl:literalForm "non-potable "@en .

:c_6ac7b4e3 a :Terms, skos:Concept;
  skos:broader :Water_Use;
  skos:definition "Water dedicated to instream environmental needs that does not reduce the available water supply downstream for other uses."@en;
  skos:inScheme :ca-dwr-g;
  skos:topConceptOf :ca-dwr-g;
  skosxl:prefLabel :xl_en_a165a8a8 .

:xl_en_a165a8a8 a skosxl:Label;
  skosxl:literalForm "nonconsumptive environmental water use "@en .

:c_830ce8b8 a :Terms, skos:Concept;
  skos:broader :Legal_and_Regulatory, :Water_Quality;
  skos:definition "Diffuse pollution sources that are not subject to National Pollutant Discharge Elimination System (NPDES) permitting. The pollutants are generally carried off the land by runoff. Common non-point sources are agriculture, forestry, mining, dams, channels, and saltwater intrusion. See also point-source."@en;
  skos:inScheme :ca-dwr-g;
  skos:topConceptOf :ca-dwr-g;
  skosxl:prefLabel :xl_en_9b0367d6 .

:xl_en_9b0367d6 a skosxl:Label;
  skosxl:literalForm "non-point-source pollution "@en .

:c_0069a726 a :Terms, skos:Concept;
  skos:broader :Legal_and_Regulatory, :Utilities;
  skos:definition "A public water system that is not a community water system and that regularly serves the same non-residential users for at least six months per year. Examples include schools, places of employment, and institutions. See also community water system, transient noncommunity water system."@en;
  skos:inScheme :ca-dwr-g;
  skos:topConceptOf :ca-dwr-g;
  skosxl:prefLabel :xl_en_5dec5d95 .

:xl_en_5dec5d95 a skosxl:Label;
  skosxl:literalForm "nontransient-noncommunity water system "@en .

:c_e2a30d00 a :Terms, skos:Concept;
  skos:broader :Legal_and_Regulatory;
  skos:definition "Methods not widely used by the State to generate funds for implementing California Water Plan actions. These methods can be administered by local, regional, or State government."@en;
  skos:inScheme :ca-dwr-g;
  skos:topConceptOf :ca-dwr-g;
  skosxl:prefLabel :xl_en_00c738df .

:xl_en_00c738df a skosxl:Label;
  skosxl:literalForm "novel funding mechanism "@en .

:c_7f500a64 a :Terms, skos:Concept;
  skos:broader :Legal_and_Regulatory;
  skos:definition "Objectives tell what we will do and why we are doing it in order to accomplish one or more goals."@en;
  skos:inScheme :ca-dwr-g;
  skos:topConceptOf :ca-dwr-g;
  skosxl:prefLabel :xl_en_8bb3dd6c .

:xl_en_8bb3dd6c a skosxl:Label;
  skosxl:literalForm "objectives "@en .

:c_c2c543c5 a :Terms, skos:Concept;
  skos:broader :Infrastructure, :Water_Use;
  skos:definition "Offstream recharge uses suitable recharge sites outside a streambed. In some operations, water must be pumped some distance from its source to an offstream recharge area."@en;
  skos:inScheme :ca-dwr-g;
  skos:topConceptOf :ca-dwr-g;
  skosxl:prefLabel :xl_en_741e9585 .

:xl_en_741e9585 a skosxl:Label;
  skosxl:literalForm "offstream recharge "@en .

:c_c3ecf87e a :Terms, skos:Concept;
  skos:broader :Hydrology;
  skos:definition "Deep clear lake with few nutrients, little organic matter, and a high dissolved-oxygen level. (Lake Tahoe is an example)."@en;
  skos:inScheme :ca-dwr-g;
  skos:topConceptOf :ca-dwr-g;
  skosxl:prefLabel :xl_en_bf2d5441 .

:xl_en_bf2d5441 a skosxl:Label;
  skosxl:literalForm "oligotrophic lake "@en .

:c_2e9eb4b0 a :Terms, skos:Concept;
  skos:broader :Infrastructure, :Water_Quality;
  skos:definition "Any individual residential sewage treatment and wastewater dispersal system, such as a septic system."@en;
  skos:inScheme :ca-dwr-g;
  skos:topConceptOf :ca-dwr-g;
  skosxl:altLabel :xl_en_1ea3f035;
  skosxl:prefLabel :xl_en_90d8789b .

:xl_en_90d8789b a skosxl:Label;
  skosxl:literalForm "onsite wastewater treatment system"@en .

:xl_en_1ea3f035 a skosxl:Label;
  skosxl:literalForm "OWTS"@en .

:c_750e2aeb a :Terms, skos:Concept;
  skos:definition "The temporal or spatial operational efficiency of existing and proposed infrastructure to maximize benefits."@en;
  skos:inScheme :ca-dwr-g;
  skos:topConceptOf :ca-dwr-g;
  skosxl:prefLabel :xl_en_11c350e1 .

:xl_en_11c350e1 a skosxl:Label;
  skosxl:literalForm "operational flexibility "@en .

:c_1d70e47d a :Terms, skos:Concept;
  skos:broader :Water_Quality;
  skos:definition "When a water treatment facility and distribution system are able to provide a consistent level of fluoride at the appropriate prophylactic level."@en;
  skos:inScheme :ca-dwr-g;
  skos:topConceptOf :ca-dwr-g;
  skosxl:prefLabel :xl_en_b2c08815 .

:xl_en_b2c08815 a skosxl:Label;
  skosxl:literalForm "optimal fluoridation "@en .

:c_6d8486a4 a :Terms, skos:Concept;
  skos:broader :Legal_and_Regulatory;
  skos:definition "A law set forth by a governmental authority."@en;
  skos:inScheme :ca-dwr-g;
  skos:topConceptOf :ca-dwr-g;
  skosxl:prefLabel :xl_en_f5c7fbdc .

:xl_en_f5c7fbdc a skosxl:Label;
  skosxl:literalForm "ordinance "@en .

:c_f350a214 a :Terms, skos:Concept;
  skos:broader :Water_Use;
  skos:definition "The sum of deliveries from federal projects other than the Central Valley Project."@en;
  skos:inScheme :ca-dwr-g;
  skos:topConceptOf :ca-dwr-g;
  skosxl:prefLabel :xl_en_db349115 .

:xl_en_db349115 a skosxl:Label;
  skosxl:literalForm "other federal deliveries "@en .

:c_ff580113 a :Terms, skos:Concept;
  skos:broader :Hydrology, :Water_Use;
  skos:definition "The amount of water leaving a service area. "@en;
  skos:inScheme :ca-dwr-g;
  skos:topConceptOf :ca-dwr-g;
  skosxl:prefLabel :xl_en_13a6d3f9 .

:xl_en_13a6d3f9 a skosxl:Label;
  skosxl:literalForm "outflow "@en .

:c_795400de a :Terms, skos:Concept;
  skos:broader :Water_Use;
  skos:definition "See groundwater overdraft."@en;
  skos:inScheme :ca-dwr-g;
  skos:topConceptOf :ca-dwr-g;
  skosxl:prefLabel :xl_en_9984332d .

:xl_en_9984332d a skosxl:Label;
  skosxl:literalForm "overdraft "@en .

:c_9bae42d3 a :Terms, skos:Concept;
  skos:broader :Legal_and_Regulatory, :Water_Use;
  skos:definition "Property owners above a common aquifer possess a mutual right to the reasonable and beneficial use of a groundwater resource on land overlying the aquifer from which the water is taken. Overlying rights are correlative (related to one another), and overlying users of a common water source must share the resource on a pro rata basis in times of shortage. A proper overlying use takes precedence over all non-overlying uses."@en;
  skos:inScheme :ca-dwr-g;
  skos:topConceptOf :ca-dwr-g;
  skosxl:prefLabel :xl_en_fec754e4 .

:xl_en_fec754e4 a skosxl:Label;
  skosxl:literalForm "overlying right "@en .

:c_ab7fab40 a :Terms, skos:Concept;
  skos:broader :Environment_and_Ecology;
  skos:definition "Fish that live in open water, often near the surface. Many river-dwelling anadromous fishes, such as shad, are also pelagic spawners."@en;
  skos:inScheme :ca-dwr-g;
  skos:topConceptOf :ca-dwr-g;
  skosxl:prefLabel :xl_en_150aa08d .

:xl_en_150aa08d a skosxl:Label;
  skosxl:literalForm "pelagic fish "@en .

:c_d6cbe0fb a :Terms, skos:Concept;
  skos:broader :Hydrology;
  skos:definition "Groundwater supported by a zone of material of low permeability located above an underlying main body of groundwater."@en;
  skos:inScheme :ca-dwr-g;
  skos:topConceptOf :ca-dwr-g;
  skosxl:prefLabel :xl_en_8680f1b5 .

:xl_en_8680f1b5 a skosxl:Label;
  skosxl:literalForm "perched groundwater "@en .

:c_c6980ed4 a :Terms, skos:Concept;
  skos:broader :Hydrology;
  skos:definition "Water in underground basins and groundwater that has escaped from streams and is not subject to a permitting process."@en;
  skos:inScheme :ca-dwr-g;
  skos:topConceptOf :ca-dwr-g;
  skosxl:prefLabel :xl_en_730c6b0f .

:xl_en_730c6b0f a skosxl:Label;
  skosxl:literalForm "percolating water "@en .

:c_a1a47312 a :Terms, skos:Concept;
  skos:broader :Hydrology;
  skos:definition "The process in which water moves through a porous material, usually surface water migrating through soil toward a groundwater aquifer."@en;
  skos:inScheme :ca-dwr-g;
  skos:topConceptOf :ca-dwr-g;
  skosxl:prefLabel :xl_en_3db5f874 .

:xl_en_3db5f874 a skosxl:Label;
  skosxl:literalForm "percolation "@en .

:c_faceaeb3 a :Terms, skos:Concept;
  skos:broader :Hydrology;
  skos:definition "The capability of soil or other geologic formations to transmit water."@en;
  skos:inScheme :ca-dwr-g;
  skos:topConceptOf :ca-dwr-g;
  skosxl:prefLabel :xl_en_191493dc .

:xl_en_191493dc a skosxl:Label;
  skosxl:literalForm "permeability "@en .

:c_d5b8e7f9 a :Terms, skos:Concept;
  skos:broader :Environment_and_Ecology;
  skos:definition "Any of a class of chemicals used for killing insects, weeds, or other undesirable entities. Pesticides are most commonly associated with agricultural activities, but they also have significant domestic use in California."@en;
  skos:inScheme :ca-dwr-g;
  skos:topConceptOf :ca-dwr-g;
  skosxl:prefLabel :xl_en_e2c83b43 .

:xl_en_e2c83b43 a skosxl:Label;
  skosxl:literalForm "pesticide "@en .

:c_cba631f9 a :Terms, skos:Concept;
  skos:definition "The pleasant smell that accompanies the first rain after a dry spell."@en;
  skos:inScheme :ca-dwr-g;
  skos:topConceptOf :ca-dwr-g;
  skosxl:prefLabel :xl_en_8107a510 .

:xl_en_8107a510 a skosxl:Label;
  skosxl:literalForm "petrichor"@en .

:c_3e6a7252 a :Terms, skos:Concept;
  skos:broader :Water_Use;
  skos:definition "The deliberate direct or indirect use of recycled water without relinquishing control over the water during its delivery."@en;
  skos:inScheme :ca-dwr-g;
  skos:topConceptOf :ca-dwr-g;
  skosxl:prefLabel :xl_en_09eab1d6 .

:xl_en_09eab1d6 a skosxl:Label;
  skosxl:literalForm "planned reuse "@en .

:c_07783a2f a :Terms, skos:Concept;
  skos:broader :Hydrology, :Legal_and_Regulatory;
  skos:definition "A subsection of a hydrologic region containing a number of detailed analysis units (DAUs)."@en;
  skos:inScheme :ca-dwr-g;
  skos:topConceptOf :ca-dwr-g;
  skosxl:prefLabel :xl_en_b8c6f79c .

:xl_en_b8c6f79c a skosxl:Label;
  skosxl:literalForm "planning area (PA) "@en .

:c_bf40ceb9 a :Terms, skos:Concept;
  skos:broader :Infrastructure, :Legal_and_Regulatory, :Water_Quality;
  skos:definition "A specific site from which wastewater or polluted water is discharged into a water body. See also non-point-source pollution."@en;
  skos:inScheme :ca-dwr-g;
  skos:topConceptOf :ca-dwr-g;
  skosxl:prefLabel :xl_en_a55a77b4 .

:xl_en_a55a77b4 a skosxl:Label;
  skosxl:literalForm "point source "@en .

:c_00292758 a :Terms, skos:Concept;
  skos:broader :Water_Quality;
  skos:definition "The alteration of physical, chemical, or biological properties of water by the introduction of any substance into it that adversely affects the water's beneficial uses."@en;
  skos:inScheme :ca-dwr-g;
  skos:topConceptOf :ca-dwr-g;
  skosxl:prefLabel :xl_en_a4fe3066 .

:xl_en_a4fe3066 a skosxl:Label;
  skosxl:literalForm "pollution (of water) "@en .

:c_10c7fed4 a :Terms, skos:Concept;
  skos:broader :Water_Quality;
  skos:definition "Improving water quality for all beneficial uses by protecting water at its source, and thus reducing the need and cost for other water management actions and treatment."@en;
  skos:inScheme :ca-dwr-g;
  skos:topConceptOf :ca-dwr-g;
  skosxl:prefLabel :xl_en_14f176e5 .

:xl_en_14f176e5 a skosxl:Label;
  skosxl:literalForm "pollution prevention "@en .

:c_6e01a716 a :Terms, skos:Concept;
  skos:broader :Data_, :Water_Use;
  skos:definition "This represents the average number of people per square mile for a planning area."@en;
  skos:inScheme :ca-dwr-g;
  skos:topConceptOf :ca-dwr-g;
  skosxl:prefLabel :xl_en_215366b2 .

:xl_en_215366b2 a skosxl:Label;
  skosxl:literalForm "population density"@en .

:c_1400283b a :Terms, skos:Concept;
  skos:broader :Data_;
  skos:definition "This represents the geographic location within California of the population projection."@en;
  skos:inScheme :ca-dwr-g;
  skos:topConceptOf :ca-dwr-g;
  skosxl:prefLabel :xl_en_4855c0eb .

:xl_en_4855c0eb a skosxl:Label;
  skosxl:literalForm "population distribution "@en .

:c_b7702fd6 a :Terms, skos:Concept;
  skos:broader :Data_;
  skos:definition "This represents the 2050 forecast of population made by the California Department of Finance or other agencies."@en;
  skos:inScheme :ca-dwr-g;
  skos:topConceptOf :ca-dwr-g;
  skosxl:prefLabel :xl_en_301803f4 .

:xl_en_301803f4 a skosxl:Label;
  skosxl:literalForm "population projection "@en .

:c_796249df a :Terms, skos:Concept;
  skos:broader :Hydrology;
  skos:definition "The ratio of the voids or open spaces in a mass to the total volume of the mass. For example, soil porosity is the ratio of voids in alluvium and rocks to the total volume of the alluvium or rock mass."@en;
  skos:inScheme :ca-dwr-g;
  skos:topConceptOf :ca-dwr-g;
  skosxl:prefLabel :xl_en_9989ab1d .

:xl_en_9989ab1d a skosxl:Label;
  skosxl:literalForm "porosity"@en .

:c_b03986ca a :Terms, skos:Concept;
  skos:broader :Legal_and_Regulatory, :Water_Quality;
  skos:definition "Human activities that are actual or potential origins of contamination for a drinking water source. PCAs include sources of both microbiological and chemical contaminants that could have an adverse effect on drinking water sources."@en;
  skos:inScheme :ca-dwr-g;
  skos:topConceptOf :ca-dwr-g;
  skosxl:altLabel :xl_en_3edfa342;
  skosxl:prefLabel :xl_en_eea2ad9a .

:xl_en_eea2ad9a a skosxl:Label;
  skosxl:literalForm "possible contaminating activity "@en .

:xl_en_3edfa342 a skosxl:Label;
  skosxl:literalForm "PCA"@en .

:c_b03c4439 a :Terms, skos:Concept;
  skos:broader :Water_Quality;
  skos:definition "Water that is safe for drinking and cooking. See also non-potable."@en;
  skos:inScheme :ca-dwr-g;
  skos:topConceptOf :ca-dwr-g;
  skosxl:prefLabel :xl_en_17ce00be .

:xl_en_17ce00be a skosxl:Label;
  skosxl:literalForm "potable "@en .

:c_3e2a5431 a :Terms, skos:Concept;
  skos:broader :Legal_and_Regulatory;
  skos:definition "When an activity raises threats to the environment or human health, precautionary measures are taken even if some cause-and-effect relationships are not fully established. Key elements of the principle include exercising precaution in the face of scientific uncertainty; exploring alternatives to possibly harmful actions; placing the burden of proof on proponents of an activity rather than on victims or potential victims of the activity; and using democratic processes to carry out and enforce the principle, including the public right to informed consent."@en;
  skos:inScheme :ca-dwr-g;
  skos:topConceptOf :ca-dwr-g;
  skosxl:prefLabel :xl_en_85a47e65 .

:xl_en_85a47e65 a skosxl:Label;
  skosxl:literalForm "precautionary principle approach "@en .

:c_c09d8e96 a :Terms, skos:Concept;
  skos:broader :Hydrology;
  skos:definition "he amount of water that falls to the earth as rain, snow, hail, or is formed on the earth as dew, and frost."@en;
  skos:inScheme :ca-dwr-g;
  skos:topConceptOf :ca-dwr-g;
  skosxl:prefLabel :xl_en_f151df02 .

:xl_en_f151df02 a skosxl:Label;
  skosxl:literalForm "precipitation"@en .

:c_bccb2d81 a :Terms, skos:Concept;
  skos:definition "The action of artificially stimulating clouds (cloud seeding) to produce more rainfall/snowfall than would occur naturally."@en;
  skos:inScheme :ca-dwr-g;
  skos:topConceptOf :ca-dwr-g;
  skosxl:prefLabel :xl_en_6f438f4c .

:xl_en_6f438f4c a skosxl:Label;
  skosxl:literalForm "precipitation enhancement "@en .

:c_947ea310 a :Terms, skos:Concept;
  skos:broader :Legal_and_Regulatory, :Water_Use;
  skos:definition "Rights obtained through the open and notorious adverse use of another's water rights. By definition, adverse use is not the use of a surplus, but the use of non-surplus water to the direct detriment of the original rights holder."@en;
  skos:inScheme :ca-dwr-g;
  skos:topConceptOf :ca-dwr-g;
  skosxl:prefLabel :xl_en_f29eb7fa .

:xl_en_f29eb7fa a skosxl:Label;
  skosxl:literalForm "prescriptive right "@en .

:c_a7bea862 a :Terms, skos:Concept;
  skos:broader :Utilities, :Water_Quality;
  skos:definition "The initial stage of wastewater treatment involving physical mechanisms such as screens, sedimentation tanks, or filters to remove material from wastewater."@en;
  skos:inScheme :ca-dwr-g;
  skos:topConceptOf :ca-dwr-g;
  skosxl:prefLabel :xl_en_9120bc16 .

:xl_en_9120bc16 a skosxl:Label;
  skosxl:literalForm "primary treatment "@en .

:c_3c40b00a a :Terms, skos:Concept;
  skos:broader :Utilities;
  skos:definition "These include investor-owned utilities, mutual water companies, mobile home parks, and water associations. They also may include various commercial enterprises, such as restaurants, hotels, resorts, and employee housing, which have their own water supply."@en;
  skos:inScheme :ca-dwr-g;
  skos:topConceptOf :ca-dwr-g;
  skosxl:prefLabel :xl_en_485dda12 .

:xl_en_485dda12 a skosxl:Label;
  skosxl:literalForm "privately owned water systems "@en .

:c_876a2c9a a :Terms, skos:Concept;
  skos:definition "Public goods are resources or services common to all individuals in society that everyone benefits from or enjoys. These resources or services may include water quality protection, flood management, environmental protection, and national parks. Public goods usually are not exchanged in a market place, and consumption of these goods by one individual does not preclude consumption by other individuals."@en;
  skos:inScheme :ca-dwr-g;
  skos:topConceptOf :ca-dwr-g;
  skosxl:prefLabel :xl_en_3cb4423f .

:xl_en_3cb4423f a skosxl:Label;
  skosxl:literalForm "public goods "@en .

:c_9e0ea714 a :Terms, skos:Concept;
  skos:broader :Legal_and_Regulatory;
  skos:definition "A legal doctrine recognizing public rights in the beds, banks, and waters of navigable waterways, and the State's power and duty to exercise continued supervision over them as trustee for the benefit of the people."@en;
  skos:inScheme :ca-dwr-g;
  skos:topConceptOf :ca-dwr-g;
  skosxl:prefLabel :xl_en_c1e913d1 .

:xl_en_c1e913d1 a skosxl:Label;
  skosxl:literalForm "public trust doctrine "@en .

:c_32755429 a :Terms, skos:Concept;
  skos:broader :Legal_and_Regulatory, :Utilities;
  skos:definition "A system for the provision of water for human consumption through pipes or other constructed conveyances that has 15 or more service connections or regularly serves at least 25 individuals daily at least 60 days out of the year. See also community water system."@en;
  skos:inScheme :ca-dwr-g;
  skos:topConceptOf :ca-dwr-g;
  skosxl:prefLabel :xl_en_e847fd17 .

:xl_en_e847fd17 a skosxl:Label;
  skosxl:literalForm "public water system "@en .

:c_4c5804bd a :Terms, skos:Concept;
  skos:broader :Legal_and_Regulatory, :Water_Use;
  skos:definition "A water right possessed by a municipality that, as a successor of a Spanish or Mexican pueblo, is entitled to the beneficial use of all needed naturally occurring surface water and groundwater of the original pueblo watershed. Pueblo rights are paramount to all other claims."@en;
  skos:inScheme :ca-dwr-g;
  skos:topConceptOf :ca-dwr-g;
  skosxl:prefLabel :xl_en_3d6eb40d .

:xl_en_3d6eb40d a skosxl:Label;
  skosxl:literalForm "pueblo right "@en .

:c_6ddcb3bd a :Terms, skos:Concept;
  skos:broader :Infrastructure;
  skos:definition "Part of a dual piping network. Purple pipe is used to distribute municipal recycled water to distinguish it from pipelines that distribute potable drinking water."@en;
  skos:inScheme :ca-dwr-g;
  skos:topConceptOf :ca-dwr-g;
  skosxl:prefLabel :xl_en_bf97f675 .

:xl_en_bf97f675 a skosxl:Label;
  skosxl:literalForm "purple pipes "@en .

:c_bbe61fd2 a :Terms, skos:Concept;
  skos:broader :Water_Use;
  skos:definition "crop consumptive water use is provided directly by rainfall."@en;
  skos:inScheme :ca-dwr-g;
  skos:topConceptOf :ca-dwr-g;
  skosxl:prefLabel :xl_en_fa6eb55e .

:xl_en_fa6eb55e a skosxl:Label;
  skosxl:literalForm "rainfed agriculture"@en .

:c_86aa0b0a a :Terms, skos:Concept;
  skos:broader :Infrastructure;
  skos:definition "l wells adjacent to or under the bed of a stream."@en;
  skos:inScheme :ca-dwr-g;
  skos:topConceptOf :ca-dwr-g;
  skosxl:prefLabel :xl_en_a8ca58e4 .

:xl_en_a8ca58e4 a skosxl:Label;
  skosxl:literalForm "Ranney collectors"@en .

:c_13d443b3 a :Terms, skos:Concept;
  skos:broader :Legal_and_Regulatory, :Water_Use;
  skos:definition "Designates the rate basis for cost recovery (e.g., flat, uniform, or tiered). Block/tiered rates are assumed to provide cost signals to consumers. Costs can include capital, operation and maintenance, financing, environmental compliance (e.g., documentation, permitting and mitigation), and so forth."@en;
  skos:inScheme :ca-dwr-g;
  skos:topConceptOf :ca-dwr-g;
  skosxl:prefLabel :xl_en_025f2099 .

:xl_en_025f2099 a skosxl:Label;
  skosxl:literalForm "rate structure "@en .

:c_f3ef5fe7 a :Terms, skos:Concept;
  skos:broader :Water_Use;
  skos:definition "An untreated water supply."@en;
  skos:inScheme :ca-dwr-g;
  skos:topConceptOf :ca-dwr-g;
  skosxl:prefLabel :xl_en_3a95bbe8 .

:xl_en_3a95bbe8 a skosxl:Label;
  skosxl:literalForm "raw water "@en .

:c_f7b7f176 a :Terms, skos:Concept;
  skos:broader :Environment_and_Ecology, :Hydrology, :Water_Use;
  skos:definition "Estimates of real water are the estimates of the water supply benefits from the transfer within the water system. There is a risk that these estimates will be inaccurate and that the transfers will result in unintended consequences to other water users, local economies, or the environment. A key challenge is to improve methods for quantifying these uncertainties and include adequate monitoring and assurances when implementing water transfers. See also new water and water transfers."@en;
  skos:inScheme :ca-dwr-g;
  skos:topConceptOf :ca-dwr-g;
  skosxl:prefLabel :xl_en_583bd9ef .

:xl_en_583bd9ef a skosxl:Label;
  skosxl:literalForm "real water "@en .

:c_39406cb6 a :Terms, skos:Concept;
  skos:broader :Hydrology;
  skos:definition "See groundwater recharge."@en;
  skos:inScheme :ca-dwr-g;
  skos:topConceptOf :ca-dwr-g;
  skosxl:prefLabel :xl_en_b8effcce .

:xl_en_b8effcce a skosxl:Label;
  skosxl:literalForm "recharge "@en .

:c_af165748 a :Terms, skos:Concept;
  skos:broader :Hydrology;
  skos:definition "An area where surface water infiltrates into the ground and reaches a saturated zone in either an unconfined aquifer or a confined aquifer. The recharge area for an unconfined aquifer is the ground surface above the aquifer. The recharge area for a confined aquifer is always some distance away from the area where wells have been built that extract groundwater from the aquifer. In other cases, recharge of the confined aquifer may occur only where a stream has eroded through the aquitard into the confined aquifer, allowing recharge to occur through the stream bottom. See also discharge area."@en;
  skos:inScheme :ca-dwr-g;
  skos:topConceptOf :ca-dwr-g;
  skosxl:prefLabel :xl_en_0740e012 .

:xl_en_0740e012 a skosxl:Label;
  skosxl:literalForm "recharge area "@en .

:c_16138340 a :Terms, skos:Concept;
  skos:broader :Hydrology, :Legal_and_Regulatory;
  skos:definition "The action of keeping recharge areas from being paved over or otherwise developed and guarding the recharge areas so they do not become contaminated."@en;
  skos:inScheme :ca-dwr-g;
  skos:topConceptOf :ca-dwr-g;
  skosxl:prefLabel :xl_en_f96275cb .

:xl_en_f96275cb a skosxl:Label;
  skosxl:literalForm "recharge area protection "@en .

:c_1e80a191 a :Terms, skos:Concept;
  skos:broader :Hydrology;
  skos:definition "A surface facility constructed to infiltrate surface water into a groundwater basin. Recharge basins are frequently used to recharge unconfined aquifers. Water is spread over the surface of a basin or pond in order to increase the quantity of water infiltrating into the ground and then percolating to the water table. Recharge basins concentrate a large volume of infiltrating water on the surface. As a result, a groundwater mound forms beneath the basin. See also groundwater recharge and groundwater recharge facility."@en;
  skos:inScheme :ca-dwr-g;
  skos:topConceptOf :ca-dwr-g;
  skosxl:prefLabel :xl_en_351f642c .

:xl_en_351f642c a skosxl:Label;
  skosxl:literalForm "recharge basin "@en .

:c_99cb99f9 a :Terms, skos:Concept;
  skos:broader :Hydrology, :Water_Use;
  skos:definition "See recycled water."@en;
  skos:inScheme :ca-dwr-g;
  skos:topConceptOf :ca-dwr-g;
  skosxl:prefLabel :xl_en_f30a09e1 .

:xl_en_f30a09e1 a skosxl:Label;
  skosxl:literalForm "reclaimed water "@en .

:c_b3e22b1f a :Terms, skos:Concept;
  skos:broader :Hydrology, :Water_Use;
  skos:definition "The amount of water that is available for supply or reuse, including surface runoff to non-saline bodies of water and deep percolation that becomes groundwater. See irrecoverable water."@en;
  skos:inScheme :ca-dwr-g;
  skos:topConceptOf :ca-dwr-g;
  skosxl:prefLabel :xl_en_e0a4bf9a .

:xl_en_e0a4bf9a a skosxl:Label;
  skosxl:literalForm "recoverable water "@en .

:c_6d0e0a2a a :Terms, skos:Concept;
  skos:broader :Water_Use;
  skos:definition "This represents the water-dependent recreation activities that are consumptive (e.g., parks), flat-water (e.g., boating), or flow-based (e.g., whitewater rafting)."@en;
  skos:inScheme :ca-dwr-g;
  skos:topConceptOf :ca-dwr-g;
  skosxl:prefLabel :xl_en_f0034af2 .

:xl_en_f0034af2 a skosxl:Label;
  skosxl:literalForm "recreation"@en .

:c_b4ede41c a :Terms, skos:Concept;
  skos:broader :Water_Use;
  skos:definition "Flat-water recreation, such as boating and skiing, in the form of future storage facilities as well as operation of existing surface storage facilities."@en;
  skos:inScheme :ca-dwr-g;
  skos:topConceptOf :ca-dwr-g;
  skosxl:prefLabel :xl_en_d1a2ea33 .

:xl_en_d1a2ea33 a skosxl:Label;
  skosxl:literalForm "recreation (reservoir-based) "@en .

:c_e0513dcb a :Terms, skos:Concept;
  skos:broader :Water_Use;
  skos:definition "Activities that are dependent on instream flows, such as whitewater rafting."@en;
  skos:inScheme :ca-dwr-g;
  skos:topConceptOf :ca-dwr-g;
  skosxl:prefLabel :xl_en_0d07b555 .

:xl_en_0d07b555 a skosxl:Label;
  skosxl:literalForm "recreation (watercourse-based) "@en .

:c_11eafb53 a :Terms, skos:Concept;
  skos:broader :Water_Use;
  skos:definition "Volume of water that, as a result of treatment of waste, is suitable for a direct beneficial use or a controlled use, which would not otherwise occur. It includes wastewater treated, stored, distributed, and reused or recirculated for beneficial use. "@en;
  skos:inScheme :ca-dwr-g;
  skos:topConceptOf :ca-dwr-g;
  skosxl:prefLabel :xl_en_1811bf94 .

:xl_en_1811bf94 a skosxl:Label;
  skosxl:literalForm "recycled water "@en .

:c_b03c3f1d a :Terms, skos:Concept;
  skos:broader :Hydrology, :Water_Use;
  skos:definition "water transferred out of a hydrologic region."@en;
  skos:inScheme :ca-dwr-g;
  skos:topConceptOf :ca-dwr-g;
  skosxl:prefLabel :xl_en_8454d143 .

:xl_en_8454d143 a skosxl:Label;
  skosxl:literalForm "regional exports "@en .

:c_8bff6b1b a :Terms, skos:Concept;
  skos:broader :Hydrology, :Water_Use;
  skos:definition "water transferred into a hydrologic region from an adjoining area."@en;
  skos:inScheme :ca-dwr-g;
  skos:topConceptOf :ca-dwr-g;
  skosxl:prefLabel :xl_en_b1329f1d .

:xl_en_b1329f1d a skosxl:Label;
  skosxl:literalForm "regional imports "@en .

:c_19ac0184 a :Terms, skos:Concept;
  skos:broader :Legal_and_Regulatory, :Water_Use;
  skos:definition "In the California Water Plan, the 12 regional reports each describe the watersheds and water conditions, population and land use, and activities that influence a region's water use and supply reliability. The regional reports focus on California's 10 hydrologic regions, which correspond to the state's major water drainage basins, and two important regional areas that overlie hydrologic boundaries but encompass communities that share common water issues or interests: the Sacramento-San Joaquin Delta region and the Mountain Counties area, which includes the foothills and mountains of the western slope of the Sierra Nevada and a portion of the Cascade Range."@en;
  skos:inScheme :ca-dwr-g;
  skos:topConceptOf :ca-dwr-g;
  skosxl:prefLabel :xl_en_fc5f6f76 .

:xl_en_fc5f6f76 a skosxl:Label;
  skosxl:literalForm "regional reports "@en .

:c_d5698dab a :Terms, skos:Concept;
  skos:broader :Legal_and_Regulatory;
  skos:definition "The degree to which a regional area implements regional water management options, such that it can provide all its needs for water from within its borders."@en;
  skos:inScheme :ca-dwr-g;
  skos:topConceptOf :ca-dwr-g;
  skosxl:prefLabel :xl_en_22ac86b6 .

:xl_en_22ac86b6 a skosxl:Label;
  skosxl:literalForm "regional self-sufficiency "@en .

:c_66df36cc a :Terms, skos:Concept;
  skos:broader :Legal_and_Regulatory;
  skos:definition "Related actions are part of the California Water Plan Update 2013 strategic plan and tell how objectives will be carried out. They describe specific actions in measurable, time-based statements of intent. They emphasize the results of actions at the end of a specific time. Some related actions must be undertaken by State government or communities over which the California Department of Water Resources has no authority. In these cases, measure and time must be part of the entities' own strategic plans."@en;
  skos:inScheme :ca-dwr-g;
  skos:topConceptOf :ca-dwr-g;
  skosxl:prefLabel :xl_en_77b09ded .

:xl_en_77b09ded a skosxl:Label;
  skosxl:literalForm "related action "@en .

:c_18cd5b6f a :Terms, skos:Concept;
  skos:broader :Legal_and_Regulatory, :Water_Use;
  skos:definition "he volume of freshwater outflow from the Sacramento-San Joaquin Delta required by law to protect the beneficial uses within the Delta from the incursion of saline water."@en;
  skos:inScheme :ca-dwr-g;
  skos:topConceptOf :ca-dwr-g;
  skosxl:prefLabel :xl_en_a8d742df .

:xl_en_a8d742df a skosxl:Label;
  skosxl:literalForm "required Delta outflow "@en .

:c_dcb106f4 a :Terms, skos:Concept;
  skos:broader :Legal_and_Regulatory, :Water_Use;
  skos:definition "The amount of water required for instream use by agreement, water rights permit, or State/federal acts."@en;
  skos:inScheme :ca-dwr-g;
  skos:topConceptOf :ca-dwr-g;
  skosxl:prefLabel :xl_en_fe55c717 .

:xl_en_fe55c717 a skosxl:Label;
  skosxl:literalForm "required instream flow "@en .

:c_b455dbbf a :Terms, skos:Concept;
  skos:broader :Data_, :Infrastructure;
  skos:definition "ResSim can simulate a range of reservoir operating conditions and accurately simulate downstream flows at specific control-point locations."@en;
  skos:inScheme :ca-dwr-g;
  skos:topConceptOf :ca-dwr-g;
  skosxl:prefLabel :xl_en_e2edfc94 .

:xl_en_e2edfc94 a skosxl:Label;
  skosxl:literalForm "Reservoir System Simulation (ResSim) "@en .

:c_c8ec3bcb a :Terms, skos:Concept;
  skos:broader :Legal_and_Regulatory;
  skos:definition "Residual risk is the likelihood of damage or other adverse consequence remaining after flood management actions are taken."@en;
  skos:inScheme :ca-dwr-g;
  skos:topConceptOf :ca-dwr-g;
  skosxl:prefLabel :xl_en_e25108cd .

:xl_en_e25108cd a skosxl:Label;
  skosxl:literalForm "residual risk "@en .

:c_9568f008 a :Terms, skos:Concept;
  skos:broader :Environment_and_Ecology;
  skos:definition "The capacity of a resource/natural or constructed system to adapt to and recover from changed conditions after a disturbance."@en;
  skos:inScheme :ca-dwr-g;
  skos:topConceptOf :ca-dwr-g;
  skosxl:prefLabel :xl_en_9d427dcb .

:xl_en_9d427dcb a skosxl:Label;
  skosxl:literalForm "resilience "@en .

:c_97ad0c20 a :Terms, skos:Concept;
  skos:broader :Legal_and_Regulatory, :Water_Use;
  skos:definition "A project, program, or policy that helps federal, State, or local agencies manage water and related resources. Resource management strategies in the California Water Plan are grouped by the following management objectives: reduce water demand, improve operational efficiency and transfers, increase water supply, improve water quality, practice resource stewardship, improve flood management, and recognize people's relationship to water."@en;
  skos:inScheme :ca-dwr-g;
  skos:topConceptOf :ca-dwr-g;
  skosxl:prefLabel :xl_en_63383514 .

:xl_en_63383514 a skosxl:Label;
  skosxl:literalForm "resource management strategy "@en .

:c_ebd52733 a :Terms, skos:Concept;
  skos:broader :Hydrology, :Water_Use;
  skos:definition "The volume of applied water returning to the surface water system."@en;
  skos:inScheme :ca-dwr-g;
  skos:topConceptOf :ca-dwr-g;
  skosxl:prefLabel :xl_en_9fdf3836 .

:xl_en_9fdf3836 a skosxl:Label;
  skosxl:literalForm "return flow "@en .

:c_519f5c0f a :Terms, skos:Concept;
  skos:broader :Hydrology, :Water_Use;
  skos:definition "The surface return flows that were discharged into storage from uses the previous year instead of being depleted, then supplied for uses the next year."@en;
  skos:inScheme :ca-dwr-g;
  skos:topConceptOf :ca-dwr-g;
  skosxl:prefLabel :xl_en_a85a115d .

:xl_en_a85a115d a skosxl:Label;
  skosxl:literalForm "return flow to carryover storage (from previous years) "@en .

:c_b50e357d a :Terms, skos:Concept;
  skos:broader :Legal_and_Regulatory, :Water_Use;
  skos:definition "The surface return flows to channels that are available for use in another detailed analysis unit by county (DAUCO), planning area (PA) and/or hydrologic region (HR)."@en;
  skos:inScheme :ca-dwr-g;
  skos:topConceptOf :ca-dwr-g;
  skosxl:prefLabel :xl_en_44ff4610 .

:xl_en_44ff4610 a skosxl:Label;
  skosxl:literalForm "return flow to developed supply "@en .

:c_aba4405f a :Terms, skos:Concept;
  skos:broader :Hydrology, :Water_Use;
  skos:definition "The volume of return flows evaporation and/or evapotranspiration by weeds and other vegetation in fringes of fields and in and near agricultural drains and sump areas."@en;
  skos:inScheme :ca-dwr-g;
  skos:topConceptOf :ca-dwr-g;
  skosxl:prefLabel :xl_en_46f044d8 .

:xl_en_46f044d8 a skosxl:Label;
  skosxl:literalForm "return flows evaporation and evapotranspiration"@en .

:c_5e3be78b a :Terms, skos:Concept;
  skos:broader :Hydrology, :Water_Use;
  skos:definition "The volume of return flows that go to saline water bodies, such as the Salton Sea or the ocean, or to saline groundwater basins."@en;
  skos:inScheme :ca-dwr-g;
  skos:topConceptOf :ca-dwr-g;
  skosxl:prefLabel :xl_en_1b77f4c4 .

:xl_en_1b77f4c4 a skosxl:Label;
  skosxl:literalForm "return flows to salt sink "@en .

:c_e9c36e05 a :Terms, skos:Concept;
  skos:broader :Infrastructure, :Water_Use;
  skos:definition "A system of pipelines or ditches to collect and convey surface or subsurface runoff from an irrigated field or landscape for reuse."@en;
  skos:inScheme :ca-dwr-g;
  skos:topConceptOf :ca-dwr-g;
  skosxl:prefLabel :xl_en_f3a1698f .

:xl_en_f3a1698f a skosxl:Label;
  skosxl:literalForm "return-flow system "@en .

:c_fbf60f0b a :Terms, skos:Concept;
  skos:broader :Water_Use;
  skos:definition "The amount of recoverable deep percolation from untreated raw applied and conveyance water."@en;
  skos:inScheme :ca-dwr-g;
  skos:topConceptOf :ca-dwr-g;
  skosxl:prefLabel :xl_en_735daa06 .

:xl_en_735daa06 a skosxl:Label;
  skosxl:literalForm "reuse groundwater"@en .

:c_031a4e22 a :Terms, skos:Concept;
  skos:broader :Water_Use;
  skos:definition "The amount of the reuse of agricultural irrigation system tailwater and return flows to local distribution systems and streams within a region; this does not include reuse of excess applied water that percolates to groundwater."@en;
  skos:inScheme :ca-dwr-g;
  skos:topConceptOf :ca-dwr-g;
  skosxl:prefLabel :xl_en_98b9e99e .

:xl_en_98b9e99e a skosxl:Label;
  skosxl:literalForm "reuse of return flows within region - ag "@en .

:c_2504adf0 a :Terms, skos:Concept;
  skos:broader :Water_Use;
  skos:definition "The amount of the reuse of urban tailwater and return flows to local distribution systems and streams within a region; this does not include reuse of excess applied water that percolates to groundwater."@en;
  skos:inScheme :ca-dwr-g;
  skos:topConceptOf :ca-dwr-g;
  skosxl:prefLabel :xl_en_99bfacd6 .

:xl_en_99bfacd6 a skosxl:Label;
  skosxl:literalForm "reuse of return flows within region - urban "@en .

:c_e81d56a3 a :Terms, skos:Concept;
  skos:broader :Water_Use;
  skos:definition "The amount of the reuse of managed wetlands irrigation system tailwater and return flows, wild and scenic river flows, and required instream flows to local distribution systems and streams within a region; this does not include reuse of excess applied water that percolates to groundwater."@en;
  skos:inScheme :ca-dwr-g;
  skos:topConceptOf :ca-dwr-g;
  skosxl:prefLabel :xl_en_85a3de01 .

:xl_en_85a3de01 a skosxl:Label;
  skosxl:literalForm "reuse of return flows within region - wetlands, wild and scenic, instream "@en .

:c_4fa26730 a :Terms, skos:Concept;
  skos:broader :Water_Use;
  skos:definition "The amount of untreated raw applied water recaptured for use through surface drainage facilities."@en;
  skos:inScheme :ca-dwr-g;
  skos:topConceptOf :ca-dwr-g;
  skosxl:prefLabel :xl_en_f50888d4 .

:xl_en_f50888d4 a skosxl:Label;
  skosxl:literalForm "reuse surface water "@en .

:c_e5501bb3 a :Terms, skos:Concept;
  skos:broader :Water_Use;
  skos:definition "Water that is used by more than one grower and is, therefore, not available for reallocation should one grower become increasingly efficient (i.e., applied water reductions minus real water equals zero)."@en;
  skos:inScheme :ca-dwr-g;
  skos:topConceptOf :ca-dwr-g;
  skosxl:prefLabel :xl_en_a02f73ce .

:xl_en_a02f73ce a skosxl:Label;
  skosxl:literalForm "reused agricultural water "@en .

:c_977713c8 a :Terms, skos:Concept;
  skos:broader :Water_Use;
  skos:definition "The application of previously used water to meet a beneficial use, whether treated or not prior to the subsequent use. See also recycled water."@en;
  skos:inScheme :ca-dwr-g;
  skos:topConceptOf :ca-dwr-g;
  skosxl:prefLabel :xl_en_ca6b8dd8 .

:xl_en_ca6b8dd8 a skosxl:Label;
  skosxl:literalForm "reused water "@en .

:c_3aeaaa67 a :Terms, skos:Concept;
  skos:broader :Infrastructure, :Water_Quality;
  skos:definition "A method of purifying water by applying pressure to force a solution of saline water through a membrane, retaining the solute (higher concentrated saline water) on one side and allowing the pure solvent (water) to pass to the other side. This is the reverse of the normal osmosis process, which is the natural movement of solvent (water) from an area of low solute concentration, through a membrane, to an area of high solute concentration (saline water) when no pressure is applied. Reverse osmosis removes most drinking water contaminants and is also used in wastewater treatment."@en;
  skos:inScheme :ca-dwr-g;
  skos:topConceptOf :ca-dwr-g;
  skosxl:prefLabel :xl_en_b0ff0ff2 .

:xl_en_b0ff0ff2 a skosxl:Label;
  skosxl:literalForm "reverse osmosis "@en .

:c_545f3d79 a :Terms, skos:Concept;
  skos:broader :Environment_and_Ecology;
  skos:definition "Areas adjacent to rivers and streams with a differing density, diversity, and productivity of plant and animal species relative to nearby uplands."@en;
  skos:inScheme :ca-dwr-g;
  skos:topConceptOf :ca-dwr-g;
  skosxl:prefLabel :xl_en_f16ee04c .

:xl_en_f16ee04c a skosxl:Label;
  skosxl:literalForm "riparian habitat "@en .

:c_7d406de3 a :Terms, skos:Concept;
  skos:broader :Water_Use;
  skos:definition "A water right that comes with the ownership of land adjacent to a water source wherein owners of land adjacent to a stream have the right to make reasonable use of a correlative share of the natural flow stream. These rights are senior to most appropriative rights. See also appropriate right and pueblo right."@en;
  skos:inScheme :ca-dwr-g;
  skos:topConceptOf :ca-dwr-g;
  skosxl:prefLabel :xl_en_cdf2cb45 .

:xl_en_cdf2cb45 a skosxl:Label;
  skosxl:literalForm "riparian right "@en .

:c_4ec4de9d a :Terms, skos:Concept;
  skos:definition "Most risks originate from such hazards as floods, earthquakes, and droughts that would occur even if all uncertainty could be eliminated. Reducing uncertainty provides a clearer view of what the risks to the system are. Risk is the probability of the occurrence (multiplied by) consequences of the occurrence over a range of potential events."@en;
  skos:inScheme :ca-dwr-g;
  skos:topConceptOf :ca-dwr-g;
  skosxl:prefLabel :xl_en_f2cd26f1 .

:xl_en_f2cd26f1 a skosxl:Label;
  skosxl:literalForm "risk "@en .

:c_a2a21658 a :Terms, skos:Concept;
  skos:broader :Water_Use;
  skos:definition "Balances increasing deliveries in a given year with the risk of not meeting full deliveries in a subsequent dry year."@en;
  skos:inScheme :ca-dwr-g;
  skos:topConceptOf :ca-dwr-g;
  skosxl:prefLabel :xl_en_4ca9ba9a .

:xl_en_4ca9ba9a a skosxl:Label;
  skosxl:literalForm "risk-based water deliveries "@en .

:c_11e1948d a :Terms, skos:Concept;
  skos:broader :Legal_and_Regulatory;
  skos:definition "This is a new approach to decision support when conditions present deep uncertainty. RDM uses computational methods to identify the scenarios most likely to break assumptions embedded in a long-term resource management plan."@en;
  skos:inScheme :ca-dwr-g;
  skos:topConceptOf :ca-dwr-g;
  skosxl:altLabel :xl_en_3b152e5c;
  skosxl:prefLabel :xl_en_2e6c5445 .

:xl_en_2e6c5445 a skosxl:Label;
  skosxl:literalForm "robust decision-making "@en .

:xl_en_3b152e5c a skosxl:Label;
  skosxl:literalForm "RDM"@en .

:c_379d1c83 a :Terms, skos:Concept;
  skos:broader :Hydrology;
  skos:definition "The portion of the soil profile through which plant roots readily penetrate to obtain water and plant nutrients, expressed in inches or feet of depth."@en;
  skos:inScheme :ca-dwr-g;
  skos:topConceptOf :ca-dwr-g;
  skosxl:prefLabel :xl_en_0cdb5f89 .

:xl_en_0cdb5f89 a skosxl:Label;
  skosxl:literalForm "root zone "@en .

:c_6c18f1e4 a :Terms, skos:Concept;
  skos:broader :Hydrology;
  skos:definition "(1) Rainfall, snowmelt, or irrigation water in excess of what can infiltrate the soil surface and be stored in small surface depressions. A major transporter of nonpoint-source pollutants to rivers, streams, and lakes. (2) The volume of surface flow from an area."@en;
  skos:inScheme :ca-dwr-g;
  skos:topConceptOf :ca-dwr-g;
  skosxl:prefLabel :xl_en_1378367f .

:xl_en_1378367f a skosxl:Label;
  skosxl:literalForm "runoff"@en .

:c_54e52e7c a :Terms, skos:Concept;
  skos:broader :Hydrology;
  skos:definition "The portion of precipitation that would have been used by natural vegetation but now contributes to runoff. This is a result of roads, paved areas, building roofs, land drainage systems, fields developed for irrigation, and other changes in land use. "@en;
  skos:inScheme :ca-dwr-g;
  skos:topConceptOf :ca-dwr-g;
  skosxl:prefLabel :xl_en_cc1f2e33 .

:xl_en_cc1f2e33 a skosxl:Label;
  skosxl:literalForm "runoff-incidental"@en .

:c_1bf274e9 a :Terms, skos:Concept;
  skos:broader :Hydrology;
  skos:definition "The portion of precipitation that runs off the land and makes up the natural flow in rivers."@en;
  skos:inScheme :ca-dwr-g;
  skos:topConceptOf :ca-dwr-g;
  skosxl:prefLabel :xl_en_c018d45a .

:xl_en_c018d45a a skosxl:Label;
  skosxl:literalForm "runoff-natural"@en .

:c_d7989046 a :Terms, skos:Concept;
  skos:broader :Legal_and_Regulatory, :Water_Quality, :Water_Use;
  skos:definition "The Delta Reform Act established a new governance approach for the Sacramento-San Joaquin Delta that is focused on achieving the coequal goals of protecting, restoring, and enhancing the Delta ecosystem, and providing a more reliable water supply for California. The Delta Reform Act created the Delta Stewardship Council and gave it the direction and authority to serve two primary governance roles: (1) set a comprehensive, legally enforceable direction for how the State manages important water and environmental resources in the Delta through the adoption of a Delta Plan, and (2) ensure coherent and integrated implementation of that direction through coordination and oversight of State and local agencies proposing to fund, carry out, and approve Delta-related activities."@en;
  skos:inScheme :ca-dwr-g;
  skos:topConceptOf :ca-dwr-g;
  skosxl:prefLabel :xl_en_23d9a40a .

:xl_en_23d9a40a a skosxl:Label;
  skosxl:literalForm "Sacramento-San Joaquin Delta Reform Act of 2009 "@en .

:c_dbd68ce5 a :Terms, skos:Concept;
  skos:broader :Legal_and_Regulatory, :Utilities, :Water_Quality;
  skos:definition "The federal Safe Drinking Water Act (SDWA) was passed in 1974 to protect public health by regulating the nation's public drinking water supply. Under the SDWA, the U.S. Environmental Protection Agency sets standards for drinking water quality and oversees the states, localities, and water suppliers who implement those standards. In addition, the State has enacted the California SDWA to ensure that all residents have safe drinking water."@en;
  skos:inScheme :ca-dwr-g;
  skos:topConceptOf :ca-dwr-g;
  skosxl:prefLabel :xl_en_f6c23777 .

:xl_en_f6c23777 a skosxl:Label;
  skosxl:literalForm "Safe Drinking Water Act "@en .

:c_04f4bfc8 a :Terms, skos:Concept;
  skos:broader :Hydrology;
  skos:definition "Soils with both salt and sodium accumulation requiring special management; these soils are common in the San Joaquin Valley."@en;
  skos:inScheme :ca-dwr-g;
  skos:topConceptOf :ca-dwr-g;
  skosxl:prefLabel :xl_en_3252b043 .

:xl_en_3252b043 a skosxl:Label;
  skosxl:literalForm "saline-sodic soils"@en .

:c_602fbc52 a :Terms, skos:Concept;
  skos:broader :Hydrology;
  skos:definition "Generally, the concentration of mineral salts dissolved in water. Salinity may be expressed in terms of concentration or as electrical conductivity. When describing salinity influenced by sea water, salinity often refers to the concentration of chlorides in the water."@en;
  skos:inScheme :ca-dwr-g;
  skos:topConceptOf :ca-dwr-g;
  skosxl:prefLabel :xl_en_b9d63dd0 .

:xl_en_b9d63dd0 a skosxl:Label;
  skosxl:literalForm "salinity "@en .

:c_c186e4a9 a :Terms, skos:Concept;
  skos:broader :Hydrology;
  skos:definition "The movement of salt water into a body of fresh surface water or groundwater. It may be called seawater intrusion if it comes from the ocean."@en;
  skos:inScheme :ca-dwr-g;
  skos:topConceptOf :ca-dwr-g;
  skosxl:prefLabel :xl_en_567a66f1 .

:xl_en_567a66f1 a skosxl:Label;
  skosxl:literalForm "salt water intrusion "@en .

:c_0d2609dc a :Terms, skos:Concept;
  skos:broader :Hydrology;
  skos:definition "Minerals that cause salinity. Water may pick up additional salts as it passes through the air, over and under the ground, or as households and industry use it."@en;
  skos:inScheme :ca-dwr-g;
  skos:topConceptOf :ca-dwr-g;
  skosxl:prefLabel :xl_en_bfe9bc1d .

:xl_en_bfe9bc1d a skosxl:Label;
  skosxl:literalForm "salts "@en .

:c_581d0d3c a :Terms, skos:Concept;
  skos:broader :Hydrology;
  skos:definition "The zone in which all interconnected openings are filled with water, usually underlying the unsaturated zone."@en;
  skos:inScheme :ca-dwr-g;
  skos:topConceptOf :ca-dwr-g;
  skosxl:prefLabel :xl_en_807873e9 .

:xl_en_807873e9 a skosxl:Label;
  skosxl:literalForm "saturated zone "@en .

:c_64faae37 a :Terms, skos:Concept;
  skos:broader :Hydrology, :Water_Use;
  skos:definition "Saved water is water that is prevented from evaporating from soil or flowing to salt sinks, such as saline surface or groundwater or ocean. See new water."@en;
  skos:inScheme :ca-dwr-g;
  skos:topConceptOf :ca-dwr-g;
  skosxl:prefLabel :xl_en_a0299977 .

:xl_en_a0299977 a skosxl:Label;
  skosxl:literalForm "saved water "@en .

:c_146ec688 a :Terms, skos:Concept;
  skos:broader :Environment_and_Ecology;
  skos:definition "Scenarios capture a broad range of uncertain factors that affect water management, but over which water managers have little control. Scenarios are used to test the robustness of strategies by evaluating how well strategies perform across a wide range of possible future conditions. The California Water Plan organizes scenarios around themes of population growth, land use patterns, and climate change."@en;
  skos:inScheme :ca-dwr-g;
  skos:topConceptOf :ca-dwr-g;
  skosxl:prefLabel :xl_en_5aec0273 .

:xl_en_5aec0273 a skosxl:Label;
  skosxl:literalForm "scenarios "@en .

:c_ab7ffc4d a :Terms, skos:Concept;
  skos:broader :Environment_and_Ecology;
  skos:definition "An increase in the height of the average or peak sea level at coastal or tidal locations, usually with regard to projected impacts resulting from climate change."@en;
  skos:inScheme :ca-dwr-g;
  skos:topConceptOf :ca-dwr-g;
  skosxl:prefLabel :xl_en_728047e8 .

:xl_en_728047e8 a skosxl:Label;
  skosxl:literalForm "sea level rise "@en .

:c_1a173b7d a :Terms, skos:Concept;
  skos:broader :Water_Use;
  skos:definition "This represents the shift in crop type between seasonal and permanent. This factor depicts the diminished ability to reduce water use during times of increased water scarcity (due to shifting from seasonal to permanent crops). In other words, shortage losses increase when shifting from seasonal to permanent."@en;
  skos:inScheme :ca-dwr-g;
  skos:topConceptOf :ca-dwr-g;
  skosxl:prefLabel :xl_en_cc47344e .

:xl_en_cc47344e a skosxl:Label;
  skosxl:literalForm "seasonal vs. permanent crop mix "@en .

:c_5682c0f7 a :Terms, skos:Concept;
  skos:broader :Hydrology;
  skos:definition "A system designed to retard, cease, or repel the advancement of seawater intrusion into potable groundwater supplies along coastal portions of California. The system may be a series of specifically placed injection wells or a combination of injection and pumping wells where water is injected or pumped to form a hydraulic barrier. "@en;
  skos:inScheme :ca-dwr-g;
  skos:topConceptOf :ca-dwr-g;
  skosxl:prefLabel :xl_en_e7ab1698 .

:xl_en_e7ab1698 a skosxl:Label;
  skosxl:literalForm "seawater intrusion barrier "@en .

:c_0e6ad6fd a :Terms, skos:Concept;
  skos:broader :Data_, :Water_Quality;
  skos:definition "White disk of specific size used to measure the depth clarity of a water body."@en;
  skos:inScheme :ca-dwr-g;
  skos:topConceptOf :ca-dwr-g;
  skosxl:prefLabel :xl_en_90afe4dc .

:xl_en_90afe4dc a skosxl:Label;
  skosxl:literalForm "Secchi disk"@en .

:c_f39b9004 a :Terms, skos:Concept;
  skos:broader :Hydrology;
  skos:definition "Voids in a rock formed after the rock has been deposited; not formed with the genesis of the rock, but later, as a result of other processes. Fractures in granite and caverns in limestone are examples of secondary openings."@en;
  skos:inScheme :ca-dwr-g;
  skos:topConceptOf :ca-dwr-g;
  skosxl:prefLabel :xl_en_eb8e4871 .

:xl_en_eb8e4871 a skosxl:Label;
  skosxl:literalForm "secondary porosity "@en .

:c_df373f28 a :Terms, skos:Concept;
  skos:broader :Water_Quality;
  skos:definition "The second stage of wastewater treatment focused on removal of dissolved and suspended organic matter remaining after primary treatment. It is usually accomplished by micro-organisms converting suspended waste solids into biomass that settles out."@en;
  skos:inScheme :ca-dwr-g;
  skos:topConceptOf :ca-dwr-g;
  skosxl:prefLabel :xl_en_c2c922e2 .

:xl_en_c2c922e2 a skosxl:Label;
  skosxl:literalForm "secondary treatment "@en .

:c_8ec67572 a :Terms, skos:Concept;
  skos:broader :Hydrology;
  skos:definition "The gradual movement of water into, through, or from a porous medium; also, infiltration of water into soil from canals, ditches, laterals, watercourses, reservoirs, storage facilities, or other water bodies, or from a field."@en;
  skos:inScheme :ca-dwr-g;
  skos:topConceptOf :ca-dwr-g;
  skosxl:prefLabel :xl_en_d9d8e427 .

:xl_en_d9d8e427 a skosxl:Label;
  skosxl:literalForm "seepage "@en .

:c_149d4949 a :Terms, skos:Concept;
  skos:broader :Hydrology;
  skos:definition "A semi-confined aquifer, or leaky confined aquifer, is an aquifer that has aquitards either above or below that allow water to leak into or out of the aquifer, depending on the direction of the hydraulic gradient. See also artesian aquifer, confined aquifer, and unconfined aquifer."@en;
  skos:inScheme :ca-dwr-g;
  skos:topConceptOf :ca-dwr-g;
  skosxl:prefLabel :xl_en_ec3d3cda .

:xl_en_ec3d3cda a skosxl:Label;
  skosxl:literalForm "semi-confined aquifer "@en .

:c_2e53732c a :Terms, skos:Concept;
  skos:broader :Utilities;
  skos:definition "The geographic area served by a water agency."@en;
  skos:inScheme :ca-dwr-g;
  skos:topConceptOf :ca-dwr-g;
  skosxl:prefLabel :xl_en_66424f5c .

:xl_en_66424f5c a skosxl:Label;
  skosxl:literalForm "service area "@en .

:c_50c3dc4a a :Terms, skos:Concept;
  skos:broader :Hydrology;
  skos:definition "Slow rise flooding occurs as a gradual inundation as waterways or lakes overflow their banks and is most often caused by heavy precipitation, especially with heavy snowmelt. It includes riverine flooding in deep floodplains and ponding of water in low-lying urban areas, as well as gradual flooding in areas adjacent to local streams and creeks."@en;
  skos:inScheme :ca-dwr-g;
  skos:topConceptOf :ca-dwr-g;
  skosxl:prefLabel :xl_en_e131ea86 .

:xl_en_e131ea86 a skosxl:Label;
  skosxl:literalForm "slow rise flooding "@en .

:c_294332a4 a :Terms, skos:Concept;
  skos:broader :Data_, :Hydrology;
  skos:definition "The water in soils; usually expressed as a percentage of the dry weight of the soil. It may also be expressed on a wet weight or a volume basis."@en;
  skos:inScheme :ca-dwr-g;
  skos:topConceptOf :ca-dwr-g;
  skosxl:prefLabel :xl_en_7903b1be .

:xl_en_7903b1be a skosxl:Label;
  skosxl:literalForm "soil moisture "@en .

:c_6280f744 a :Terms, skos:Concept;
  skos:broader :Data_, :Hydrology;
  skos:definition "Soil texture refers to the percentage of sand, silt, and clay particles in a soil. Sand, silt, and clay particles are defined by their size. Soil texture has important effects on soil properties, such as water-holding capacity, drainage class, consistence, and chemical properties."@en;
  skos:inScheme :ca-dwr-g;
  skos:topConceptOf :ca-dwr-g;
  skosxl:prefLabel :xl_en_e7f0e25f .

:xl_en_e7f0e25f a skosxl:Label;
  skosxl:literalForm "soil texture "@en .

:c_75f5e9dc a :Terms, skos:Concept;
  skos:broader :Infrastructure, :Water_Use;
  skos:definition "An enhanced evaporation system that uses timed sprinklers or other equipment that allows the discharge rate to be set and adjusted as necessary to avoid standing water within the surface of the solar evaporator."@en;
  skos:inScheme :ca-dwr-g;
  skos:topConceptOf :ca-dwr-g;
  skosxl:prefLabel :xl_en_ab160ca2 .

:xl_en_ab160ca2 a skosxl:Label;
  skosxl:literalForm "solar evaporator "@en .

:c_a5a94020 a :Terms, skos:Concept;
  skos:broader :Data_, :Hydrology, :Water_Quality;
  skos:definition "The ability to analyze and predict the movement of solutes in groundwater systems in order to determine the impacts of groundwater contamination."@en;
  skos:inScheme :ca-dwr-g;
  skos:topConceptOf :ca-dwr-g;
  skosxl:prefLabel :xl_en_ab0a318a .

:xl_en_ab0a318a a skosxl:Label;
  skosxl:literalForm "solute transport (analysis) "@en .

:c_35f3c132 a :Terms, skos:Concept;
  skos:broader :Water_Use;
  skos:definition "The body of water from which water is taken for beneficial use."@en;
  skos:inScheme :ca-dwr-g;
  skos:topConceptOf :ca-dwr-g;
  skosxl:prefLabel :xl_en_9f012cb5 .

:xl_en_9f012cb5 a skosxl:Label;
  skosxl:literalForm "source water "@en .

:c_af75572b a :Terms, skos:Concept;
  skos:broader :Hydrology;
  skos:definition "The ratio of the volume of water a rock or sediment will retain against the pull of gravity to the total volume of the rock or sediment. "@en;
  skos:inScheme :ca-dwr-g;
  skos:topConceptOf :ca-dwr-g;
  skosxl:prefLabel :xl_en_0db691e6 .

:xl_en_0db691e6 a skosxl:Label;
  skosxl:literalForm "specific retention "@en .

:c_d16c8772 a :Terms, skos:Concept;
  skos:broader :Hydrology;
  skos:definition "A location where groundwater flows naturally to the land surface or a surface water body. See also artesian aquifer."@en;
  skos:inScheme :ca-dwr-g;
  skos:topConceptOf :ca-dwr-g;
  skosxl:prefLabel :xl_en_f90553ca .

:xl_en_f90553ca a skosxl:Label;
  skosxl:literalForm "spring "@en .

:c_b7679bcd a :Terms, skos:Concept;
  skos:broader :Water_Use;
  skos:definition "A method of irrigation in which water is sprayed or sprinkled through the air to the ground surface."@en;
  skos:inScheme :ca-dwr-g;
  skos:topConceptOf :ca-dwr-g;
  skosxl:prefLabel :xl_en_16f206ef .

:xl_en_16f206ef a skosxl:Label;
  skosxl:literalForm "sprinkler irrigation "@en .

:c_b564c7e8 a :Terms, skos:Concept;
  skos:broader :Legal_and_Regulatory;
  skos:definition "Individuals or groups who can affect or be affected by an organization's activities; or individuals or groups with an interest or stake in what happens as a result of any decision or action. Stakeholders do not necessarily use the products or receive the services of a program."@en;
  skos:inScheme :ca-dwr-g;
  skos:topConceptOf :ca-dwr-g;
  skosxl:prefLabel :xl_en_938a4276 .

:xl_en_938a4276 a skosxl:Label;
  skosxl:literalForm "stakeholder "@en .

:c_2e1a9570 a :Terms, skos:Concept;
  skos:broader :Legal_and_Regulatory;
  skos:definition "Collectively, the facilities, lands, programs, conditions, and mode of operation and maintenance for the State-Federal flood protection system in the Central Valley."@en;
  skos:inScheme :ca-dwr-g;
  skos:topConceptOf :ca-dwr-g;
  skosxl:altLabel :xl_en_963e7b6d;
  skosxl:prefLabel :xl_en_852edf3b .

:xl_en_852edf3b a skosxl:Label;
  skosxl:literalForm "State Plan of Flood Control "@en .

:xl_en_963e7b6d a skosxl:Label;
  skosxl:literalForm "SPFC"@en .

:c_02f477b6 a :Terms, skos:Concept;
  skos:broader :Water_Use;
  skos:definition "The sum of all deliveries to State Water Project contractors."@en;
  skos:inScheme :ca-dwr-g;
  skos:topConceptOf :ca-dwr-g;
  skosxl:prefLabel :xl_en_2eae7de5 .

:xl_en_2eae7de5 a skosxl:Label;
  skosxl:literalForm "State Water Project (SWP) deliveries "@en .

:c_b0a23958 a :Terms, skos:Concept;
  skos:broader :Infrastructure, :Legal_and_Regulatory, :Utilities, :Water_Quality, :Water_Use;
  skos:definition "These include physical facilities (more than 1,200 State, federal, and local reservoirs, as well as canals, treatment plants, and levees), which make up the backbone of water management in California; and statewide water management programs, which include water-quality standards, monitoring programs, economic incentives, water pricing policies, and statewide water-efficiency programs, such as appliance standards, labeling, and education."@en;
  skos:inScheme :ca-dwr-g;
  skos:topConceptOf :ca-dwr-g;
  skosxl:prefLabel :xl_en_4a87e1c1 .

:xl_en_4a87e1c1 a skosxl:Label;
  skosxl:literalForm "statewide water management systems "@en .

:c_dce7567f a :Terms, skos:Concept;
  skos:broader :Legal_and_Regulatory, :Water_Use;
  skos:definition "A water rights permitting system defined in the California Water Code and administered by the State Water Resources Control Board."@en;
  skos:inScheme :ca-dwr-g;
  skos:topConceptOf :ca-dwr-g;
  skosxl:prefLabel :xl_en_e9d1311b .

:xl_en_e9d1311b a skosxl:Label;
  skosxl:literalForm "statutory permitting system "@en .

:c_02101666 a :Terms, skos:Concept;
  skos:broader :Hydrology, :Infrastructure, :Legal_and_Regulatory, :Utilities, :Water_Quality;
  skos:definition "Water that is originated during a precipitation event and may collect and concentrate diffused pollutants and carry them to watercourses, causing degradation. Runoff in the urban environment, both storm-generated and dry-weather flows, has been shown to be a significant source of pollutants to the surface waters of the nation."@en;
  skos:inScheme :ca-dwr-g;
  skos:topConceptOf :ca-dwr-g;
  skosxl:prefLabel :xl_en_eed3ade9 .

:xl_en_eed3ade9 a skosxl:Label;
  skosxl:literalForm "stormwater runoff "@en .

:c_d856a1a6 a :Terms, skos:Concept;
  skos:broader :Legal_and_Regulatory;
  skos:definition "The long-term goals of an organization or program and an outline of how they will be achieved (e.g., adopting specific strategies, approaches, and methodologies). "@en;
  skos:inScheme :ca-dwr-g;
  skos:topConceptOf :ca-dwr-g;
  skosxl:prefLabel :xl_en_ae144bc5 .

:xl_en_ae144bc5 a skosxl:Label;
  skosxl:literalForm "strategic plan "@en .

:c_ea16b8d0 a :Terms, skos:Concept;
  skos:broader :Hydrology;
  skos:definition "The science of rocks. It is concerned with the original succession and age relations of rock strata and their form, distribution, lithologic composition, fossil content, geophysical and geochemical properties - all characters and attributes of rocks as strata - and their interpretation in terms of environment, mode of origin, and geologic history."@en;
  skos:inScheme :ca-dwr-g;
  skos:topConceptOf :ca-dwr-g;
  skosxl:prefLabel :xl_en_e655857d .

:xl_en_e655857d a skosxl:Label;
  skosxl:literalForm "stratigraphy "@en .

:c_cab84190 a :Terms, skos:Concept;
  skos:broader :Environment_and_Ecology;
  skos:definition "Stream ecosystems are labeled according to their inhabitants; thus, area streams are referred to by these labels: conifer forest snowmelt streams, trout headwater streams, trout/sculpin streams, sucker/dace/redside streams, and whitefish cutthroat/sucker streams."@en;
  skos:inScheme :ca-dwr-g;
  skos:topConceptOf :ca-dwr-g;
  skosxl:prefLabel :xl_en_c1c2b6d1 .

:xl_en_c1c2b6d1 a skosxl:Label;
  skosxl:literalForm "stream ecosystems "@en .

:c_2be29e3e a :Terms, skos:Concept;
  skos:broader :Hydrology;
  skos:definition "A systematic process for describing the degree of branching of a stream network within a watershed."@en;
  skos:inScheme :ca-dwr-g;
  skos:topConceptOf :ca-dwr-g;
  skosxl:prefLabel :xl_en_3c8413a1 .

:xl_en_3c8413a1 a skosxl:Label;
  skosxl:literalForm "stream order "@en .

:c_d1073c0f a :Terms, skos:Concept;
  skos:broader :Water_Use;
  skos:definition "Application of irrigation water below the ground surface by raising the water table to within or near the root zone."@en;
  skos:inScheme :ca-dwr-g;
  skos:topConceptOf :ca-dwr-g;
  skosxl:prefLabel :xl_en_26e1b7f8 .

:xl_en_26e1b7f8 a skosxl:Label;
  skosxl:literalForm "subirrigation "@en .

:c_1096468e a :Terms, skos:Concept;
  skos:broader :Hydrology, :Water_Use;
  skos:definition "See land subsidence."@en;
  skos:inScheme :ca-dwr-g;
  skos:topConceptOf :ca-dwr-g;
  skosxl:prefLabel :xl_en_6f0fcef2 .

:xl_en_6f0fcef2 a skosxl:Label;
  skosxl:literalForm "subsidence "@en .

:c_11cfc339 a :Terms, skos:Concept;
  skos:broader :Water_Use;
  skos:definition "Application of water below the soil surface through emitters, with discharge rates generally in the same range as drip irrigation. This method of water application is different from and not to be confused with subirrigation, where the root zone is irrigated by water table control."@en;
  skos:inScheme :ca-dwr-g;
  skos:topConceptOf :ca-dwr-g;
  skosxl:prefLabel :xl_en_9a20e412 .

:xl_en_9a20e412 a skosxl:Label;
  skosxl:literalForm "subsurface drip irrigation "@en .

:c_876ecd7b a :Terms, skos:Concept;
  skos:broader :Hydrology;
  skos:definition "Subterranean streams flowing through known and definite channels are regulated by California's surface water rights system. The following physical conditions must be present in a subterranean stream flowing in a known and definite channel: (1) a subsurface channel must be present, (2) the channel must have relatively impermeable bed and banks, (3) the course of the channel must be known or capable of being determined by reasonable inference, and (4) groundwater must be flowing in the channel."@en;
  skos:inScheme :ca-dwr-g;
  skos:topConceptOf :ca-dwr-g;
  skosxl:prefLabel :xl_en_d5f7a7f1 .

:xl_en_d5f7a7f1 a skosxl:Label;
  skosxl:literalForm "subterranean stream "@en .

:c_4f168cd3 a :Terms, skos:Concept;
  skos:broader :Water_Use;
  skos:definition "Irrigation in which the soil surface is used as the conduit, as in furrow and border irrigation, and as opposed to sprinkler, drip, and subirrigation. "@en;
  skos:inScheme :ca-dwr-g;
  skos:topConceptOf :ca-dwr-g;
  skosxl:prefLabel :xl_en_1a57bac8 .

:xl_en_1a57bac8 a skosxl:Label;
  skosxl:literalForm "surface irrigation "@en .

:c_f6a0b67c a :Terms, skos:Concept;
  skos:broader :Infrastructure;
  skos:definition "Reservoirs to collect water for later release and use."@en;
  skos:inScheme :ca-dwr-g;
  skos:topConceptOf :ca-dwr-g;
  skosxl:prefLabel :xl_en_b9d404d1 .

:xl_en_b9d404d1 a skosxl:Label;
  skosxl:literalForm "surface storage "@en .

:c_6f2da491 a :Terms, skos:Concept;
  skos:broader :Water_Use;
  skos:definition "Water supply obtained from streams, lakes, and reservoirs."@en;
  skos:inScheme :ca-dwr-g;
  skos:topConceptOf :ca-dwr-g;
  skosxl:prefLabel :xl_en_be109d25 .

:xl_en_be109d25 a skosxl:Label;
  skosxl:literalForm "surface supply "@en .

:c_f39e286d a :Terms, skos:Concept;
  skos:broader :Hydrology, :Legal_and_Regulatory;
  skos:definition "As defined under the California Surface Water Treatment Rule, California Code of Regulations Title 22, Section 64651.83, surface water means all water open to the atmosphere and subject to surface runoff and hence would include all lakes, rivers, streams, and other water bodies. Surface water includes all groundwater sources that are deemed to be under the influence of surface water (i.e., springs, shallow wells, wells close to rivers, etc.), which must comply with the same level of treatment as surface water."@en;
  skos:inScheme :ca-dwr-g;
  skos:topConceptOf :ca-dwr-g;
  skosxl:prefLabel :xl_en_2b752394 .

:xl_en_2b752394 a skosxl:Label;
  skosxl:literalForm "surface water "@en .

:c_9aa5b5f0 a :Terms, skos:Concept;
  skos:broader :Infrastructure, :Water_Use;
  skos:definition "The planned placement of recycled water into a surface water reservoir used as a source of domestic drinking water supply (California Water Code Section 13561(d)) or into any surface water when discharged for the purpose of aquatic habitat enhancement. See also indirect potable reuse."@en;
  skos:inScheme :ca-dwr-g;
  skos:topConceptOf :ca-dwr-g;
  skosxl:prefLabel :xl_en_3aefb4e5 .

:xl_en_3aefb4e5 a skosxl:Label;
  skosxl:literalForm "surface water augmentation "@en .

:c_6ee39087 a :Terms, skos:Concept;
  skos:broader :Hydrology;
  skos:definition "The difference between beginning of year and end of year surface water storage."@en;
  skos:inScheme :ca-dwr-g;
  skos:topConceptOf :ca-dwr-g;
  skosxl:prefLabel :xl_en_abd76ca3 .

:xl_en_abd76ca3 a skosxl:Label;
  skosxl:literalForm "surface water change in storage "@en .

:c_2d7795ea a :Terms, skos:Concept;
  skos:broader :Water_Use;
  skos:definition "A surface irrigation technique wherein flow is applied to furrows (or, less commonly, borders) intermittently during a single irrigation set."@en;
  skos:inScheme :ca-dwr-g;
  skos:topConceptOf :ca-dwr-g;
  skosxl:prefLabel :xl_en_5cff1bb6 .

:xl_en_5cff1bb6 a skosxl:Label;
  skosxl:literalForm "surge irrigation "@en .

:c_095b0be4 a :Terms, skos:Concept;
  skos:broader :Water_Use;
  skos:definition "Water that is not being used directly or indirectly to benefit environmental, agricultural, or urban use sectors."@en;
  skos:inScheme :ca-dwr-g;
  skos:topConceptOf :ca-dwr-g;
  skosxl:prefLabel :xl_en_6a7fb0cd .

:xl_en_6a7fb0cd a skosxl:Label;
  skosxl:literalForm "surplus water "@en .

:c_0a5579c2 a :Terms, skos:Concept;
  skos:broader :Environment_and_Ecology;
  skos:definition "Sustainability of California's water systems means meeting current needs - expressed by water stakeholders as public health and safety, healthy economy, ecosystem vitality, and opportunities for enriching experiences - without compromising the needs of future generations."@en;
  skos:inScheme :ca-dwr-g;
  skos:topConceptOf :ca-dwr-g;
  skosxl:prefLabel :xl_en_0cca821d .

:xl_en_0cca821d a skosxl:Label;
  skosxl:literalForm "sustainability "@en .

:c_2729bb2b a :Terms, skos:Concept;
  skos:broader :Environment_and_Ecology, :Infrastructure;
  skos:definition "See sustainability. "@en;
  skos:inScheme :ca-dwr-g;
  skos:topConceptOf :ca-dwr-g;
  skosxl:prefLabel :xl_en_e02384a2 .

:xl_en_e02384a2 a skosxl:Label;
  skosxl:literalForm "sustainable development "@en .

:c_aa9478fd a :Terms, skos:Concept;
  skos:broader :Utilities;
  skos:definition "Changing existing water system operation and management procedures or priorities to either meet competing beneficial uses or derive more total benefits from the water system by operating more efficiently."@en;
  skos:inScheme :ca-dwr-g;
  skos:topConceptOf :ca-dwr-g;
  skosxl:prefLabel :xl_en_643341bd .

:xl_en_643341bd a skosxl:Label;
  skosxl:literalForm "system reoperation "@en .

:c_b5078dd8 a :Terms, skos:Concept;
  skos:definition "Outdated, ineffective, or inflexible statutes, policies, or practices that increase the time, effort, or cost to mitigate adverse effects from critical challenges."@en;
  skos:inScheme :ca-dwr-g;
  skos:topConceptOf :ca-dwr-g;
  skosxl:prefLabel :xl_en_5e62b17a .

:xl_en_5e62b17a a skosxl:Label;
  skosxl:literalForm "systemic and institutional challenges "@en .

:c_2880c478 a :Terms, skos:Concept;
  skos:broader :Legal_and_Regulatory;
  skos:definition "Table A is an exhibit that corresponds to the contracts between the California Department of Water Resources and the 29 State Water Project (SWP) water contractors, in which are defined the terms and conditions governing the water delivery and cost repayment for the SWP. All water-supply-related costs of the SWP are paid by the contractors, and Table A serves as a basis for allocating some of the costs among the contractors. In addition, Table A plays a key role in the annual allocation of available supply among contractors. Table A is simply contractual language for apportioning available supply and cost obligations under the contract."@en;
  skos:inScheme :ca-dwr-g;
  skos:topConceptOf :ca-dwr-g;
  skosxl:prefLabel :xl_en_f4deb4e2 .

:xl_en_f4deb4e2 a skosxl:Label;
  skosxl:literalForm "Table A "@en .

:c_0666aae1 a :Terms, skos:Concept;
  skos:broader :Legal_and_Regulatory, :Water_Use;
  skos:definition "The maximum amount of State Water Project (SWP) water that the State agreed to make available to an SWP contractor for delivery during the year. Table A amounts determine the maximum water a contractor may request each year from the California Department of Water Resources. The State and SWP contractors also use Table A amounts to serve as a basis for allocation of some SWP costs among the contractors."@en;
  skos:inScheme :ca-dwr-g;
  skos:topConceptOf :ca-dwr-g;
  skosxl:prefLabel :xl_en_6b3e9baa .

:xl_en_6b3e9baa a skosxl:Label;
  skosxl:literalForm "Table A Water "@en .

:c_8bc9e04c a :Terms, skos:Concept;
  skos:broader :Hydrology, :Water_Use;
  skos:definition "The runoff of irrigation water from the lower end of an irrigated field."@en;
  skos:inScheme :ca-dwr-g;
  skos:topConceptOf :ca-dwr-g;
  skosxl:prefLabel :xl_en_643adfd8 .

:xl_en_643adfd8 a skosxl:Label;
  skosxl:literalForm "tailwater "@en .

:c_5e51c354 a :Terms, skos:Concept;
  skos:broader :Utilities, :Water_Quality;
  skos:definition "Water treatment processes beyond secondary treatment. Granular media, such as sand or anthracite coal, or a membrane are used to filter out most of the solids remaining after secondary treatment. After filtration, finish water is usually disinfected with chlorine or ultraviolet light to inactivate bacteria, viruses, and other microorganisms prior to discharge or recycling."@en;
  skos:inScheme :ca-dwr-g;
  skos:topConceptOf :ca-dwr-g;
  skosxl:prefLabel :xl_en_7e3ef027 .

:xl_en_7e3ef027 a skosxl:Label;
  skosxl:literalForm "tertiary treatment "@en .

:c_316ae151 a :Terms, skos:Concept;
  skos:broader :Legal_and_Regulatory;
  skos:definition "The occurrence of incidental economic impacts on parties not directly related to impact-causing water management actions. For example, agricultural land retirement can affect local tax revenues or labor conditions."@en;
  skos:inScheme :ca-dwr-g;
  skos:topConceptOf :ca-dwr-g;
  skosxl:prefLabel :xl_en_96d6e06a .

:xl_en_96d6e06a a skosxl:Label;
  skosxl:literalForm "third-party impacts "@en .

:c_b7f44969 a :Terms, skos:Concept;
  skos:broader :Water_Use;
  skos:definition "The water drained from agricultural fields by the practice of removing excess water from the subsurface of soil with a network of underground pipes that allow subsurface water to move out from between soil particles and into the tile line. Water flowing through tile lines is often ultimately deposited into surface water. Water enters the tile line either via the gaps between tile sections, in the case of older tile designs, or through small perforations in modern plastic tile. Tile drainage brings soil moisture levels down for optimal crop growth and is used as a primary method of controlling soil salinity."@en;
  skos:inScheme :ca-dwr-g;
  skos:topConceptOf :ca-dwr-g;
  skosxl:prefLabel :xl_en_78bb1f40 .

:xl_en_78bb1f40 a skosxl:Label;
  skosxl:literalForm "tile water (tile drainage) "@en .

:c_d3b55acf a :Terms, skos:Concept;
  skos:broader :Infrastructure, :Legal_and_Regulatory;
  skos:definition "The total monetary cost required for turnkey implementation, including environmental and third-party impact mitigation, storage, conveyance, energy, capitalized operations and maintenance, administrative costs, planning costs, legal costs, and engineering costs."@en;
  skos:inScheme :ca-dwr-g;
  skos:topConceptOf :ca-dwr-g;
  skosxl:prefLabel :xl_en_67f4658d .

:xl_en_67f4658d a skosxl:Label;
  skosxl:literalForm "total capital cost "@en .

:c_1359766f a :Terms, skos:Concept;
  skos:broader :Water_Use;
  skos:definition "This represents the amount of commercial activity (e.g., employment, productivity, commercial land use) that occurs in a given study area. This factor is a driver of (and indicator for) commercial water use and includes institutional water use (e.g., government offices, schools), as well. See also commercial activity mix."@en;
  skos:inScheme :ca-dwr-g;
  skos:topConceptOf :ca-dwr-g;
  skosxl:prefLabel :xl_en_cd6187ce .

:xl_en_cd6187ce a skosxl:Label;
  skosxl:literalForm "total commercial activity "@en .

:c_62c7a88a a :Terms, skos:Concept;
  skos:broader :Data_, :Water_Quality;
  skos:definition "A measure of the residual minerals dissolved in water and that remain after evaporation of a solution. Usually expressed in milligrams per liter. See also salinity."@en;
  skos:inScheme :ca-dwr-g;
  skos:topConceptOf :ca-dwr-g;
  skosxl:prefLabel :xl_en_f0f8f3fb .

:xl_en_f0f8f3fb a skosxl:Label;
  skosxl:literalForm "total dissolved solids "@en .

:c_5d9abd67 a :Terms, skos:Concept;
  skos:broader :Water_Use;
  skos:definition "This represents the total amount of industrial activity (e.g., employment, productivity, industrial land use) that occurs in a given study area. This factor is a driver of (and indicator for) industrial water use."@en;
  skos:inScheme :ca-dwr-g;
  skos:topConceptOf :ca-dwr-g;
  skosxl:prefLabel :xl_en_7e0185a2 .

:xl_en_7e0185a2 a skosxl:Label;
  skosxl:literalForm "total industrial activity "@en .

:c_d97c237e a :Terms, skos:Concept;
  skos:broader :Water_Use;
  skos:definition "This represents the total area of irrigated crops planted in a planning area during a given year. This number includes multiple cropping."@en;
  skos:inScheme :ca-dwr-g;
  skos:topConceptOf :ca-dwr-g;
  skosxl:prefLabel :xl_en_42338579 .

:xl_en_42338579 a skosxl:Label;
  skosxl:literalForm "total irrigated crop area "@en .

:c_2debc15c a :Terms, skos:Concept;
  skos:broader :Water_Quality;
  skos:definition "An evaluation of the condition of an impaired surface water that appears on the federal Clean Water Act Section 303(d) list, which establishes limitations on the amount of pollution that water can be exposed to without adversely affecting its beneficial uses and allocates proportions of the total limitation among dischargers to the impaired surface water."@en;
  skos:inScheme :ca-dwr-g;
  skos:topConceptOf :ca-dwr-g;
  skosxl:altLabel :xl_en_b0a87491;
  skosxl:prefLabel :xl_en_89cd07a6 .

:xl_en_89cd07a6 a skosxl:Label;
  skosxl:literalForm "total maximum daily load "@en .

:xl_en_b0a87491 a skosxl:Label;
  skosxl:literalForm "TMDL"@en .

:c_b09b9d1a a :Terms, skos:Concept;
  skos:broader :Data_;
  skos:definition "This represents the statewide total population projection regardless of geographical distribution."@en;
  skos:inScheme :ca-dwr-g;
  skos:topConceptOf :ca-dwr-g;
  skosxl:prefLabel :xl_en_eba779ab .

:xl_en_eba779ab a skosxl:Label;
  skosxl:literalForm "total population "@en .

:c_63915526 a :Terms, skos:Concept;
  skos:definition "California Native American Tribes' traditional practices for land stewardship consider the need for sustainability and regeneration for future generations. As with many other first peoples, these traditional practices and knowledge have been maintained and passed down through generations and make up the basis of what is termed traditional (or tribal) ecological knowledge."@en;
  skos:inScheme :ca-dwr-g;
  skos:topConceptOf :ca-dwr-g;
  skosxl:prefLabel :xl_en_a382f6cd .

:xl_en_a382f6cd a skosxl:Label;
  skosxl:literalForm "traditional (or tribal) ecological knowledge (TEK) "@en .

:c_755997be a :Terms, skos:Concept;
  skos:broader :Legal_and_Regulatory, :Utilities;
  skos:definition "A public water system that is not a community water system or a nontransient-noncommunity water system (California Code of Regulations, Title 22, Section 64401.85). Transient-noncommunity water systems provide water to 25 or more people for at least 60 days/year, but not to the same people and not on a regular basis (e.g., those using campgrounds, parks, ski resorts, rest stops, gas stations, and motels)."@en;
  skos:inScheme :ca-dwr-g;
  skos:topConceptOf :ca-dwr-g;
  skosxl:prefLabel :xl_en_e598d2e1 .

:xl_en_e598d2e1 a skosxl:Label;
  skosxl:literalForm "transient-noncommunity water system "@en .

:c_35b15093 a :Terms, skos:Concept;
  skos:broader :Hydrology;
  skos:definition "An essential physiological process in which plant tissues give off water vapor to the atmosphere."@en;
  skos:inScheme :ca-dwr-g;
  skos:topConceptOf :ca-dwr-g;
  skosxl:prefLabel :xl_en_1fbd4fe5 .

:xl_en_1fbd4fe5 a skosxl:Label;
  skosxl:literalForm "transpiration "@en .

:c_573f27ba a :Terms, skos:Concept;
  skos:broader :Hydrology;
  skos:definition "Tsunami flooding occurs as a result of high-speed ocean waves triggered by mass movement that displaces a large volume of water. Earthquakes and underwater landslides may cause a tsunami, and the impact on land depends on wave height and inundation area."@en;
  skos:inScheme :ca-dwr-g;
  skos:topConceptOf :ca-dwr-g;
  skosxl:prefLabel :xl_en_47df327f .

:xl_en_47df327f a skosxl:Label;
  skosxl:literalForm "tsunami flooding "@en .

:c_bc33cf3a a :Terms, skos:Concept;
  skos:definition "Uncertainty is what we do not know about the system. For example, engineers do not know the foundation conditions under all California levees. Uncertainty can be reduced by reducing data gaps to increase knowledge."@en;
  skos:inScheme :ca-dwr-g;
  skos:topConceptOf :ca-dwr-g;
  skosxl:prefLabel :xl_en_98736c35 .

:xl_en_98736c35 a skosxl:Label;
  skosxl:literalForm "uncertainty "@en .

:c_0e60ce7b a :Terms, skos:Concept;
  skos:broader :Hydrology;
  skos:definition "An aquifer that is not bounded on top by an aquitard. The upper surface of an unconfined aquifer is the water table. See also artesian aquifer, confined aquifer, and semi-confined aquifer."@en;
  skos:inScheme :ca-dwr-g;
  skos:topConceptOf :ca-dwr-g;
  skosxl:prefLabel :xl_en_059e5706 .

:xl_en_059e5706 a skosxl:Label;
  skosxl:literalForm "unconfined aquifer "@en .

:c_811be5a6 a :Terms, skos:Concept;
  skos:broader :Hydrology;
  skos:definition "See subterranean stream. "@en;
  skos:inScheme :ca-dwr-g;
  skos:topConceptOf :ca-dwr-g;
  skosxl:prefLabel :xl_en_76a7cbfd .

:xl_en_76a7cbfd a skosxl:Label;
  skosxl:literalForm "underground stream "@en .

:c_011a16f7 a :Terms, skos:Concept;
  skos:broader :Water_Use;
  skos:definition "The quantity of water applied to a specific crop per unit area (sometimes expressed in inches of depth)."@en;
  skos:inScheme :ca-dwr-g;
  skos:topConceptOf :ca-dwr-g;
  skosxl:prefLabel :xl_en_605f5379 .

:xl_en_605f5379 a skosxl:Label;
  skosxl:literalForm "unit applied water "@en .

:c_07f3279e a :Terms, skos:Concept;
  skos:broader :Water_Use;
  skos:definition "Reuse of treated wastewater effluent by a second party that occurs after disposal by an unrelated first party. See also indirect reuse."@en;
  skos:inScheme :ca-dwr-g;
  skos:topConceptOf :ca-dwr-g;
  skosxl:prefLabel :xl_en_55bbaf55 .

:xl_en_55bbaf55 a skosxl:Label;
  skosxl:literalForm "unplanned reuse "@en .

:c_742e0c19 a :Terms, skos:Concept;
  skos:broader :Hydrology;
  skos:definition "The portion of the subsurface that lies between the bottom of the land surface and the water table that defines the upper boundary of the groundwater system (also known as vadose zone). It includes the root zone, which is the top layer of the unsaturated portion of the subsurface designated by the depth of the plant roots that draw moisture from the soil. The thickness of the unsaturated zone varies seasonally. The variation in thickness may be caused by groundwater pumping, water management practices, or climatic conditions. In areas with shallow groundwater conditions, the groundwater system may connect directly to the land surface, thus eliminating the unsaturated zone, allowing direct uptake of groundwater by plants, and potentially causing groundwater to discharge directly to the land surface through seeps, wetlands, or springs."@en;
  skos:inScheme :ca-dwr-g;
  skos:topConceptOf :ca-dwr-g;
  skosxl:prefLabel :xl_en_eaa20e1f .

:xl_en_eaa20e1f a skosxl:Label;
  skosxl:literalForm "unsaturated zone "@en .

:c_ab924cc4 a :Terms, skos:Concept;
  skos:broader :Water_Use;
  skos:definition "The amount of water used by light industry and non-manufacturing business establishments, including retail services, office buildings, restaurants, dry cleaners, and other consumer-oriented services or businesses. This also includes employee uses and recreational facilities (temporary lodging) and may include institutional or governmental use, as well."@en;
  skos:inScheme :ca-dwr-g;
  skos:topConceptOf :ca-dwr-g;
  skosxl:prefLabel :xl_en_b64c5990 .

:xl_en_b64c5990 a skosxl:Label;
  skosxl:literalForm "urban commercial use "@en .

:c_fc0bb98b a :Terms, skos:Concept;
  skos:broader :Water_Use;
  skos:definition "The amount of water needed for hydroelectric or thermoelectric power generation."@en;
  skos:inScheme :ca-dwr-g;
  skos:topConceptOf :ca-dwr-g;
  skosxl:prefLabel :xl_en_a458822c .

:xl_en_a458822c a skosxl:Label;
  skosxl:literalForm "urban energy production "@en .

:c_13eae583 a :Terms, skos:Concept;
  skos:broader :Water_Use;
  skos:definition "Water use in water-intensive manufacturing for processing, manufacturing, and other industrial plant uses (e.g., canneries, mills, other large, complex users of supply), as defined by the North American Industry Classification System (NAICS). This water can be used as cooling water or for rinsing, washing, diluting, and other sanitation operations. Also included are employee uses and landscape irrigation."@en;
  skos:inScheme :ca-dwr-g;
  skos:topConceptOf :ca-dwr-g;
  skosxl:prefLabel :xl_en_a85ee513 .

:xl_en_a85ee513 a skosxl:Label;
  skosxl:literalForm "urban industrial use "@en .

:c_64c6788f a :Terms, skos:Concept;
  skos:broader :Infrastructure;
  skos:definition "Planning for the housing and economic development needs of a growing population, while providing for the efficient use of water and other resources."@en;
  skos:inScheme :ca-dwr-g;
  skos:topConceptOf :ca-dwr-g;
  skosxl:prefLabel :xl_en_c8260077 .

:xl_en_c8260077 a skosxl:Label;
  skosxl:literalForm "urban land use management "@en .

:c_bef60696 a :Terms, skos:Concept;
  skos:broader :Water_Use;
  skos:definition "The amount of water used to irrigate recreational and large landscape areas, such as golf courses, parks, play fields, highway medians, and cemeteries."@en;
  skos:inScheme :ca-dwr-g;
  skos:topConceptOf :ca-dwr-g;
  skosxl:prefLabel :xl_en_6cdf95d0 .

:xl_en_6cdf95d0 a skosxl:Label;
  skosxl:literalForm "urban large landscape use "@en .

:c_d142c2c8 a :Terms, skos:Concept;
  skos:broader :Water_Use;
  skos:definition "The amount of water used outside a multi-family residential housing unit. Examples include landscape irrigation, swimming pools, car washing, sidewalk cleaning, and the watering of domestic animals."@en;
  skos:inScheme :ca-dwr-g;
  skos:topConceptOf :ca-dwr-g;
  skosxl:prefLabel :xl_en_b129cd5d .

:xl_en_b129cd5d a skosxl:Label;
  skosxl:literalForm "urban residential use - multi-family-exterior "@en .

:c_29c4800c a :Terms, skos:Concept;
  skos:broader :Water_Use;
  skos:definition "The amount of water used within a residential, multi-family housing unit (with two or more units), which houses two or more households (such as duplexes, apartments, or condominiums). Uses include personal hygiene, cooking, drinking, and laundry."@en;
  skos:inScheme :ca-dwr-g;
  skos:topConceptOf :ca-dwr-g;
  skosxl:prefLabel :xl_en_18f3fede .

:xl_en_18f3fede a skosxl:Label;
  skosxl:literalForm "urban residential use - multi-family-interior "@en .

:c_0b21d527 a :Terms, skos:Concept;
  skos:broader :Water_Use;
  skos:definition "The amount of water used outside a single-family residential housing unit. Examples include landscape irrigation, swimming pools, car washing, sidewalk cleaning, and the watering of domestic animals."@en;
  skos:inScheme :ca-dwr-g;
  skos:topConceptOf :ca-dwr-g;
  skosxl:prefLabel :xl_en_e55c1258 .

:xl_en_e55c1258 a skosxl:Label;
  skosxl:literalForm "urban residential use - single-family-exterior "@en .

:c_d664dfce a :Terms, skos:Concept;
  skos:broader :Water_Use;
  skos:definition "The amount of water used within a single-family, detached housing unit for such uses as personal hygiene, cooking, drinking, and laundry. "@en;
  skos:inScheme :ca-dwr-g;
  skos:topConceptOf :ca-dwr-g;
  skosxl:prefLabel :xl_en_da0d5285 .

:xl_en_da0d5285 a skosxl:Label;
  skosxl:literalForm "urban residential use - single-family-interior "@en .

:c_8a0c518d a :Terms, skos:Concept;
  skos:broader :Infrastructure, :Legal_and_Regulatory, :Utilities, :Water_Quality;
  skos:definition "A broad series of activities to manage both urban stormwater and dry-weather runoff that carry pollutants."@en;
  skos:inScheme :ca-dwr-g;
  skos:topConceptOf :ca-dwr-g;
  skosxl:prefLabel :xl_en_41eb7668 .

:xl_en_41eb7668 a skosxl:Label;
  skosxl:literalForm "urban runoff management "@en .

:c_5e33be66 a :Terms, skos:Concept;
  skos:broader :Utilities, :Water_Use;
  skos:definition "The flow from urban areas into urban wastewater treatment plants and septic tanks."@en;
  skos:inScheme :ca-dwr-g;
  skos:topConceptOf :ca-dwr-g;
  skosxl:prefLabel :xl_en_28453162 .

:xl_en_28453162 a skosxl:Label;
  skosxl:literalForm "urban wastewater produced "@en .

:c_5848fc8f a :Terms, skos:Concept;
  skos:broader :Legal_and_Regulatory, :Utilities;
  skos:definition "California Water Code Sections 10610 through 10657. The act requires urban water suppliers to prepare urban water management plans that describe and evaluate sources of water supplies, efficient uses of water, demand management measures, implementation strategies and schedules, and other relevant information and programs within their water service areas. Urban water suppliers (California Water Code Section 10617) are either publicly or privately owned and provide water for municipal purposes, either directly or indirectly, to more than 3,000 customers or supply more than 3,000 acre-feet of water annually."@en;
  skos:inScheme :ca-dwr-g;
  skos:topConceptOf :ca-dwr-g;
  skosxl:prefLabel :xl_en_0773a639 .

:xl_en_0773a639 a skosxl:Label;
  skosxl:literalForm "Urban Water Management Planning Act "@en .

:c_aa0adb16 a :Terms, skos:Concept;
  skos:broader :Water_Use;
  skos:definition "The use of potable and non-potable water for urban purposes, including residential, commercial, industrial, recreation, energy production, and large landscape. These are types of uses rather than places of use. "@en;
  skos:inScheme :ca-dwr-g;
  skos:topConceptOf :ca-dwr-g;
  skosxl:prefLabel :xl_en_fa072fc1 .

:xl_en_fa072fc1 a skosxl:Label;
  skosxl:literalForm "urban water use "@en .

:c_3c6c4680 a :Terms, skos:Concept;
  skos:broader :Water_Use;
  skos:definition "Methods or technologies resulting in the same beneficial residential, commercial, industrial, and institutional uses with less water or increased beneficial uses from existing water quantities."@en;
  skos:inScheme :ca-dwr-g;
  skos:topConceptOf :ca-dwr-g;
  skosxl:prefLabel :xl_en_f99bd19d .

:xl_en_f99bd19d a skosxl:Label;
  skosxl:literalForm "urban water use efficiency "@en .

:c_13b63802 a :Terms, skos:Concept;
  skos:broader :Hydrology, :Water_Use;
  skos:definition "The quantity of groundwater of acceptable quality that can be economically withdrawn from storage."@en;
  skos:inScheme :ca-dwr-g;
  skos:topConceptOf :ca-dwr-g;
  skosxl:prefLabel :xl_en_0f5cb6bf .

:xl_en_0f5cb6bf a skosxl:Label;
  skosxl:literalForm "usable storage capacity "@en .

:c_b030f0a1 a :Terms, skos:Concept;
  skos:definition "Use values are based on water taken up and utilized in the environment. Non-use values are not associated with actual use of, or even an option to use, an ecosystem or its service."@en;
  skos:inScheme :ca-dwr-g;
  skos:topConceptOf :ca-dwr-g;
  skosxl:prefLabel :xl_en_c78a53e4 .

:xl_en_c78a53e4 a skosxl:Label;
  skosxl:literalForm "use values "@en .

:c_8ada818a a :Terms, skos:Concept;
  skos:broader :Water_Quality;
  skos:definition "Fluoridation at levels up to the optimal level, which depends on many factors, including time of year, water demand, and the use of sources that may not have fluoridation treatment facilities. Variable fluoridation is most often the result of a water system receiving fluoridated water from a wholesale provider, while also using local unfluoridated water sources."@en;
  skos:inScheme :ca-dwr-g;
  skos:topConceptOf :ca-dwr-g;
  skosxl:prefLabel :xl_en_3c9bb6ab .

:xl_en_3c9bb6ab a skosxl:Label;
  skosxl:literalForm "variable fluoridation "@en .

:c_dc04118e a :Terms, skos:Concept;
  skos:broader :Hydrology;
  skos:definition "Vernal pools are a type of temporary wetlands. They are depressions in areas where low-permeability soils (e.g., clay or hardpan) prevent rainwater from draining downward into the subsoils. When rain fills the pools in the winter and spring, the water collects and remains in the depressions. In the springtime, the water gradually evaporates away, until the pools become completely dry in the summer and fall."@en;
  skos:inScheme :ca-dwr-g;
  skos:topConceptOf :ca-dwr-g;
  skosxl:prefLabel :xl_en_2a20f7e1 .

:xl_en_2a20f7e1 a skosxl:Label;
  skosxl:literalForm "vernal pools "@en .

:c_ce055e10 a :Terms, skos:Concept;
  skos:broader :Legal_and_Regulatory;
  skos:definition "The California Water Plan's vision statement describes the desired future for California water resources and management. It serves as a foundation for water and flood planning during the planning horizon."@en;
  skos:inScheme :ca-dwr-g;
  skos:topConceptOf :ca-dwr-g;
  skosxl:prefLabel :xl_en_37b1a2fb .

:xl_en_37b1a2fb a skosxl:Label;
  skosxl:literalForm "vision statement "@en .

:c_8fd58862 a :Terms, skos:Concept;
  skos:broader :Water_Quality;
  skos:definition "A human-made organic compound that readily vaporizes in the atmosphere. These compounds are often highly mobile in the groundwater system and are generally associated with industrial activities. VOCs are referred to as hydrocarbons."@en;
  skos:inScheme :ca-dwr-g;
  skos:topConceptOf :ca-dwr-g;
  skosxl:altLabel :xl_en_ccc67600;
  skosxl:prefLabel :xl_en_35a98e19 .

:xl_en_35a98e19 a skosxl:Label;
  skosxl:literalForm "volatile organic compound "@en .

:xl_en_ccc67600 a skosxl:Label;
  skosxl:literalForm "VOC"@en .

:c_8d9d52f3 a :Terms, skos:Concept;
  skos:broader :Legal_and_Regulatory;
  skos:definition "A community highly susceptible to the impacts of flood and drought, as well as those lacking the resources needed to effectively manage for water resource sustainability."@en;
  skos:inScheme :ca-dwr-g;
  skos:topConceptOf :ca-dwr-g;
  skosxl:prefLabel :xl_en_f43542ae .

:xl_en_f43542ae a skosxl:Label;
  skosxl:literalForm "vulnerable community "@en .

:c_7c177147 a :Terms, skos:Concept;
  skos:broader :Water_Use;
  skos:definition "Water reclamation, or wastewater reclamation, can have two meanings: (1) the process of treating wastewater for beneficial use, then storing and distributing it as recycled water; and (2) the actual use of recycled water. The latter definition is the more common of the two; that is, although the usage depends on the context, water reclamation is most often understood to mean the treatment of water of impaired quality to produce a water of suitable quality for intended use. See also water recycling and water reuse."@en;
  skos:inScheme :ca-dwr-g;
  skos:topConceptOf :ca-dwr-g;
  skosxl:prefLabel :xl_en_45ce0f24 .

:xl_en_45ce0f24 a skosxl:Label;
  skosxl:literalForm "wastewater reclamation "@en .

:c_94ec32bf a :Terms, skos:Concept;
  skos:broader :Water_Use;
  skos:definition "Diverting water in areas that have unallocated fresh water supplies, storing the water in large inflatable bladders, and towing them to an alternate coastal region."@en;
  skos:inScheme :ca-dwr-g;
  skos:topConceptOf :ca-dwr-g;
  skosxl:prefLabel :xl_en_00563624 .

:xl_en_00563624 a skosxl:Label;
  skosxl:literalForm "water bag transport/storage technology "@en .

:c_99cbcf4e a :Terms, skos:Concept;
  skos:broader :Hydrology, :Water_Use;
  skos:definition "Analyses of the total developed and dedicated supplies, uses, and operational characteristics for a region; the analyses show what water was applied to uses so that use equals supply. See also water portfolio."@en;
  skos:inScheme :ca-dwr-g;
  skos:topConceptOf :ca-dwr-g;
  skosxl:prefLabel :xl_en_8cc04de1 .

:xl_en_8cc04de1 a skosxl:Label;
  skosxl:literalForm "water balances "@en .

:c_2090e0a0 a :Terms, skos:Concept;
  skos:broader :Water_Use;
  skos:definition "The desired quantity of water that would be used if the water were available and if a number of other factors, such as price, did not change. Demand is not static. "@en;
  skos:inScheme :ca-dwr-g;
  skos:topConceptOf :ca-dwr-g;
  skosxl:prefLabel :xl_en_2c4413de .

:xl_en_2c4413de a skosxl:Label;
  skosxl:literalForm "water demand "@en .

:c_a129e2e6 a :Terms, skos:Concept;
  skos:broader :Water_Use;
  skos:definition "A phrase describing that the desire to use water is based on a number of factors, such as the intended use for the water, the price of water, and the cost of alternative ways to meet the intended use."@en;
  skos:inScheme :ca-dwr-g;
  skos:topConceptOf :ca-dwr-g;
  skosxl:prefLabel :xl_en_7795b9a1 .

:xl_en_7795b9a1 a skosxl:Label;
  skosxl:literalForm "water demand elasticity "@en .

:c_4e2199a4 a :Terms, skos:Concept;
  skos:broader :Legal_and_Regulatory, :Water_Use;
  skos:definition "The adaptation and implementation of a strategy by a water institution or consumer to influence the water demand and usage of water to meet any of these objectives: economic efficiency, social development, social equity, environmental protection, sustainability of water supply and services, and political acceptability."@en;
  skos:inScheme :ca-dwr-g;
  skos:topConceptOf :ca-dwr-g;
  skosxl:prefLabel :xl_en_78a74e54 .

:xl_en_78a74e54 a skosxl:Label;
  skosxl:literalForm "water demand management"@en .

:c_c74079c5 a :Terms, skos:Concept;
  skos:broader :Hydrology, :Water_Use;
  skos:definition "The amount of net water use minus water that can be recovered later, such as deep percolation and return flow to the developed supply."@en;
  skos:inScheme :ca-dwr-g;
  skos:topConceptOf :ca-dwr-g;
  skosxl:prefLabel :xl_en_a0f38c4a .

:xl_en_a0f38c4a a skosxl:Label;
  skosxl:literalForm "water depletion "@en .

:c_067feb81 a :Terms, skos:Concept;
  skos:broader :Legal_and_Regulatory, :Water_Use;
  skos:definition "Typically, water delivered by one water user to another water user; the receiving water user will return the water at a specified time or when the conditions of the parties' agreement are met. See also water transfers."@en;
  skos:inScheme :ca-dwr-g;
  skos:topConceptOf :ca-dwr-g;
  skosxl:prefLabel :xl_en_7d00a6d4 .

:xl_en_7d00a6d4 a skosxl:Label;
  skosxl:literalForm "water exchanges "@en .

:c_612484f6 a :Terms, skos:Concept;
  skos:broader :Water_Use;
  skos:definition "The amount of water produced as a byproduct of the oil or gas refining process."@en;
  skos:inScheme :ca-dwr-g;
  skos:topConceptOf :ca-dwr-g;
  skosxl:prefLabel :xl_en_eecd2c07 .

:xl_en_eecd2c07 a skosxl:Label;
  skosxl:literalForm "water from refineries "@en .

:c_776a5572 a :Terms, skos:Concept;
  skos:broader :Environment_and_Ecology, :Water_Use;
  skos:definition "Consumptive and nonconsumptive use of water, not including agricultural and urban uses. Defined by the Sustainability Roundtable as a measure of the water remaining in the environment after withdrawals and consumption."@en;
  skos:inScheme :ca-dwr-g;
  skos:topConceptOf :ca-dwr-g;
  skosxl:prefLabel :xl_en_18661215 .

:xl_en_18661215 a skosxl:Label;
  skosxl:literalForm "water in the environment "@en .

:c_4fe522af a :Terms, skos:Concept;
  skos:broader :Data_, :Legal_and_Regulatory;
  skos:definition "The California Department of Water Resources envisioned building an online information exchange system called Water PIE to share water-related information among state, regional, and local agencies and governments, universities, and the public. The goal was to support regional partnerships by providing a common way of developing and sharing information. A broader state agency process initiated through the passage of Assembly Bill 1755 - The Open and Transparent Water Data Act in 2016 - has superseded the need for developing the Water PIE. See also AB 1755."@en;
  skos:inScheme :ca-dwr-g;
  skos:topConceptOf :ca-dwr-g;
  skosxl:altLabel :xl_en_fb2cf7ab;
  skosxl:prefLabel :xl_en_59ca789e .

:xl_en_59ca789e a skosxl:Label;
  skosxl:literalForm "Water Planning Information Exchange "@en .

:xl_en_fb2cf7ab a skosxl:Label;
  skosxl:literalForm "Water PIE"@en .

:c_0c9af948 a :Terms, skos:Concept;
  skos:broader :Hydrology, :Water_Use;
  skos:definition "An accounting of water uses and supplies for a given year statewide or by hydrologic region, subject to availability of data, including flow diagrams, flow diagram tables, water balances, summary tables, and information."@en;
  skos:inScheme :ca-dwr-g;
  skos:topConceptOf :ca-dwr-g;
  skosxl:prefLabel :xl_en_d07bdb5c .

:xl_en_d07bdb5c a skosxl:Label;
  skosxl:literalForm "water portfolio "@en .

:c_26d1b24c a :Terms, skos:Concept;
  skos:broader :Water_Quality;
  skos:definition "A description of the chemical, physical, and biological characteristics of water, usually with regard to its suitability for a particular purpose or use. See also groundwater quality."@en;
  skos:inScheme :ca-dwr-g;
  skos:topConceptOf :ca-dwr-g;
  skosxl:prefLabel :xl_en_52633475 .

:xl_en_52633475 a skosxl:Label;
  skosxl:literalForm "water quality "@en .

:c_c79028e5 a :Terms, skos:Concept;
  skos:broader :Legal_and_Regulatory, :Water_Quality;
  skos:definition "Each regional water quality control board establishes the beneficial uses of the waters within its region. The basin plan contains numeric and/or narrative water quality objectives and spells out a program by which the objectives can be achieved within their boundaries."@en;
  skos:inScheme :ca-dwr-g;
  skos:topConceptOf :ca-dwr-g;
  skosxl:prefLabel :xl_en_c45efe95 .

:xl_en_c45efe95 a skosxl:Label;
  skosxl:literalForm "water quality control plan (basin plan) "@en .

:c_201e9665 a :Terms, skos:Concept;
  skos:broader :Legal_and_Regulatory, :Water_Quality;
  skos:definition "State-adopted and U.S. Environmental Protection Agency-approved ambient standards for water bodies. The standards prescribe the use of the water body and establish the water quality criteria that must be met to protect designated uses."@en;
  skos:inScheme :ca-dwr-g;
  skos:topConceptOf :ca-dwr-g;
  skosxl:prefLabel :xl_en_00da2cd9 .

:xl_en_00da2cd9 a skosxl:Label;
  skosxl:literalForm "water quality standards "@en .

:c_5bacec3a a :Terms, skos:Concept;
  skos:broader :Water_Use;
  skos:definition "(1) The process of treating wastewater for beneficial use, storing and distributing recycled water, and the actual use of recycled water; (2) the reuse or recirculation of water through the same series of processes, pipes, or vessels more than once by one user, often without treatment between uses, such as in cooling towers or cascading uses within an industry where the wastewater from one process is the source water for another process. See also recycled water and water reuse."@en;
  skos:inScheme :ca-dwr-g;
  skos:topConceptOf :ca-dwr-g;
  skosxl:prefLabel :xl_en_deaf2495 .

:xl_en_deaf2495 a skosxl:Label;
  skosxl:literalForm "water recycling "@en .

:c_8e25cca4 a :Terms, skos:Concept;
  skos:broader :Data_, :Water_Use;
  skos:definition "This is reported as the percentage of years in which water supply meets most of the water demand (e.g., 95 percent). Different reliability thresholds were defined for the urban and agricultural sectors to reflect different historical levels of delivery. For instream flows and other environmental objectives, water supply reliability is reported as the percentage of months in which water supply meets most of the water requirement (e.g., 95 percent)."@en;
  skos:inScheme :ca-dwr-g;
  skos:topConceptOf :ca-dwr-g;
  skosxl:prefLabel :xl_en_50007393 .

:xl_en_50007393 a skosxl:Label;
  skosxl:literalForm "water reliability "@en .

:c_aaf07f67 a :Terms, skos:Concept;
  skos:broader :Data_, :Hydrology;
  skos:definition "Formally named CALSIM, WRIMS is a generalized water-resources modeling system for evaluating operational alternatives of large, complex river basins. WRIMS integrates a simulation language for flexible operational criteria specification, a linear programming solver for efficient water allocation decisions, and graphics capabilities for ease of use. These combined capabilities provide a comprehensive and powerful modeling tool for water resource systems simulation. See also CALSIM."@en;
  skos:inScheme :ca-dwr-g;
  skos:topConceptOf :ca-dwr-g;
  skosxl:altLabel :xl_en_5ec800b2;
  skosxl:prefLabel :xl_en_f4653da9 .

:xl_en_f4653da9 a skosxl:Label;
  skosxl:literalForm "Water Resource Integrated Modeling System"@en .

:xl_en_5ec800b2 a skosxl:Label;
  skosxl:literalForm "WRIMS"@en .

:c_9ea5b9fa a :Terms, skos:Concept;
  skos:broader :Water_Use;
  skos:definition "The additional use of previously used water, with or without treatment. This term often takes on the more encompassing meaning in the first definition of wastewater reclamation, above. Direct reuse is the use of recycled water that has been transported from a wastewater treatment plant to a reuse site without passing through a natural body of either surface or groundwater. This is also called pipe-to-pipe reuse, where the recycled water is conveyed in a distribution system after treatment. Indirect reuse is the use of recycled water indirectly after it has passed through a natural body of water after discharge from a wastewater treatment plant. Groundwater recharge is an example. Another is the reuse of Sacramento's wastewater after discharge by downstream users. Planned reuse is the deliberate direct or indirect use of recycled water without relinquishing control over the water during its delivery. Direct reuse is always considered planned because it involves delivery in a distribution system leading from the wastewater treatment plant to the point of reuse. Unplanned reuse or incidental reuse is the unplanned use of wastewater after disposal. The reuse of Sacramento's effluent by downstream users is considered unplanned; there is no planned intent by Sacramento to have the State Water Project pump a portion of its effluent to Southern California. See wastewater reclamation."@en;
  skos:inScheme :ca-dwr-g;
  skos:topConceptOf :ca-dwr-g;
  skosxl:prefLabel :xl_en_66191c40 .

:xl_en_66191c40 a skosxl:Label;
  skosxl:literalForm "water reuse "@en .

:c_d34efe8c a :Terms, skos:Concept;
  skos:broader :Legal_and_Regulatory, :Water_Use;
  skos:definition "In water law, the right of a user to use water from a water source (i.e., a lake, river, stream, creek, pond, or source of groundwater)."@en;
  skos:inScheme :ca-dwr-g;
  skos:topConceptOf :ca-dwr-g;
  skosxl:prefLabel :xl_en_6e5a8e31 .

:xl_en_6e5a8e31 a skosxl:Label;
  skosxl:literalForm "water rights "@en .

:c_f7131b7e a :Terms, skos:Concept;
  skos:broader :Utilities, :Water_Use;
  skos:definition "A geographic area in which a water agency is the designated water service provider."@en;
  skos:inScheme :ca-dwr-g;
  skos:topConceptOf :ca-dwr-g;
  skosxl:prefLabel :xl_en_5d3919d0 .

:xl_en_5d3919d0 a skosxl:Label;
  skosxl:literalForm "water service area "@en .

:c_4c3e3fc4 a :Terms, skos:Concept;
  skos:broader :Water_Use;
  skos:definition "This represents where the water came from each year to meet the water uses. See also applied water use and dedicated and developed water supplies."@en;
  skos:inScheme :ca-dwr-g;
  skos:topConceptOf :ca-dwr-g;
  skosxl:prefLabel :xl_en_b4caaab8 .

:xl_en_b4caaab8 a skosxl:Label;
  skosxl:literalForm "water supply "@en .

:c_45a607f1 a :Terms, skos:Concept;
  skos:broader :Water_Use;
  skos:definition "The amount of water that a region transfers to another to meet needs."@en;
  skos:inScheme :ca-dwr-g;
  skos:topConceptOf :ca-dwr-g;
  skosxl:prefLabel :xl_en_f9099079 .

:xl_en_f9099079 a skosxl:Label;
  skosxl:literalForm "water supply exports "@en .

:c_98d55d23 a :Terms, skos:Concept;
  skos:broader :Water_Use;
  skos:definition "The amount of water brought in from other regions to meet needs. See water transfer."@en;
  skos:inScheme :ca-dwr-g;
  skos:topConceptOf :ca-dwr-g;
  skosxl:prefLabel :xl_en_cab0e5f7 .

:xl_en_cab0e5f7 a skosxl:Label;
  skosxl:literalForm "water supply imports "@en .

:c_db15abe8 a :Terms, skos:Concept;
  skos:broader :Water_Use;
  skos:definition "Percentage of the time water supplies meet demands."@en;
  skos:inScheme :ca-dwr-g;
  skos:topConceptOf :ca-dwr-g;
  skosxl:prefLabel :xl_en_47ab50d6 .

:xl_en_47ab50d6 a skosxl:Label;
  skosxl:literalForm "water supply reliability "@en .

:c_273ff2ea a :Terms, skos:Concept;
  skos:broader :Hydrology;
  skos:definition "See groundwater table."@en;
  skos:inScheme :ca-dwr-g;
  skos:topConceptOf :ca-dwr-g;
  skosxl:prefLabel :xl_en_8c84b599 .

:xl_en_8c84b599 a skosxl:Label;
  skosxl:literalForm "water table "@en .

:c_81c6c67e a :Terms, skos:Concept;
  skos:broader :Legal_and_Regulatory, :Water_Use;
  skos:definition "A water transfer is defined in the California Water Code as a temporary or long-term change in the point of diversion, place of use, or purpose of use due to a transfer or exchange of water or water rights. A temporary water transfer has a duration of one year or less (California Water Code Section 1728), and a long-term water transfer has a duration of more than one year (California Water Code Section 1735). Many transfers, such as those among contractors of the State Water Project or Central Valley Project, do not fit this definition. A more general definition is that water transfers are a voluntary change in the way water is usually distributed among water users in response to water scarcity. Compare this with water exchanges, which are typically water delivered by one water user to another water user; the receiving water user will return the water at a specified time or when the conditions of the parties to the agreement are met."@en;
  skos:inScheme :ca-dwr-g;
  skos:topConceptOf :ca-dwr-g;
  skosxl:prefLabel :xl_en_d63d72bc .

:xl_en_d63d72bc a skosxl:Label;
  skosxl:literalForm "water transfer "@en .

:c_7466b4ef a :Terms, skos:Concept;
  skos:broader :Legal_and_Regulatory, :Water_Use;
  skos:definition "The amount of water transferred across hydrologic region boundaries from one agency to another. Transfer requires approval from the State Water Resources Control Board for a change in place of use."@en;
  skos:inScheme :ca-dwr-g;
  skos:topConceptOf :ca-dwr-g;
  skosxl:prefLabel :xl_en_4b1c251b .

:xl_en_4b1c251b a skosxl:Label;
  skosxl:literalForm "water transfers - imported "@en .

:c_208194d7 a :Terms, skos:Concept;
  skos:broader :Legal_and_Regulatory, :Water_Use;
  skos:definition "The amount of water transferred within a hydrologic region from one agency to another. Transfer requires approval from the State Water Resources Control Board for a change in place of use."@en;
  skos:inScheme :ca-dwr-g;
  skos:topConceptOf :ca-dwr-g;
  skosxl:prefLabel :xl_en_b2d3b39c .

:xl_en_b2d3b39c a skosxl:Label;
  skosxl:literalForm "water transfers - regional "@en .

:c_047981ea a :Terms, skos:Concept;
  skos:broader :Legal_and_Regulatory, :Water_Quality;
  skos:definition "Any method, technique, or process designed to remove solids and/or pollutants from water or wastewater. For drinking water, treatment is defined by Title 22, Section 64401.90, of the California Code of Regulations as any physical, biological, or chemical processes, including blending, designed to affect water quality parameters to render the water acceptable for domestic use."@en;
  skos:inScheme :ca-dwr-g;
  skos:topConceptOf :ca-dwr-g;
  skosxl:prefLabel :xl_en_7656904b .

:xl_en_7656904b a skosxl:Label;
  skosxl:literalForm "water treatment "@en .

:c_9f7b2cdf a :Terms, skos:Concept;
  skos:broader :Hydrology, :Legal_and_Regulatory;
  skos:definition "A continuous 12-month period for which hydrologic records are compiled and summarized. Different agencies may use different calendar periods for their water years. For the California Department of Water Resources, a water year is October 1 through September 30."@en;
  skos:inScheme :ca-dwr-g;
  skos:topConceptOf :ca-dwr-g;
  skosxl:prefLabel :xl_en_64c26cae .

:xl_en_64c26cae a skosxl:Label;
  skosxl:literalForm "water year "@en .

:c_698eed7f a :Terms, skos:Concept;
  skos:broader :Hydrology;
  skos:definition "The land area from which water drains into a stream, river, or reservoir. The watershed for a major river may encompass a number of smaller watersheds that ultimately combine at a common point."@en;
  skos:inScheme :ca-dwr-g;
  skos:topConceptOf :ca-dwr-g;
  skosxl:prefLabel :xl_en_2f322543 .

:xl_en_2f322543 a skosxl:Label;
  skosxl:literalForm "watershed "@en .

:c_a4f19db6 a :Terms, skos:Concept;
  skos:broader :Legal_and_Regulatory;
  skos:definition "The process of evaluating, planning, managing, restoring, and organizing land and other resource use within an area that has a single common drainage point."@en;
  skos:inScheme :ca-dwr-g;
  skos:topConceptOf :ca-dwr-g;
  skosxl:prefLabel :xl_en_e9f6bb5c .

:xl_en_e9f6bb5c a skosxl:Label;
  skosxl:literalForm "watershed management "@en .

:c_b0015750 a :Terms, skos:Concept;
  skos:broader :Legal_and_Regulatory;
  skos:definition "A WMA is a geographically defined watershed area where the regional water quality control board will implement the watershed approach. See also Watershed Management Initiative. "@en;
  skos:inScheme :ca-dwr-g;
  skos:topConceptOf :ca-dwr-g;
  skosxl:altLabel :xl_en_9c8157e2;
  skosxl:prefLabel :xl_en_d27454fd .

:xl_en_d27454fd a skosxl:Label;
  skosxl:literalForm "watershed management area "@en .

:xl_en_9c8157e2 a skosxl:Label;
  skosxl:literalForm "WMA"@en .

:c_9a73fa48 a :Terms, skos:Concept;
  skos:broader :Legal_and_Regulatory;
  skos:definition "The WMI is part of the State Water Resources Control Board's (SWRCB's) and the nine regional water quality control boards' (RWQCBs') strategic plan and establishes a broad framework overlying the numerous federally mandated and State-mandated priorities. As such, the WMI helps the SWRCB and RWQCBs achieve water resource protection, enhancement, and restoration while balancing economic and environmental impacts. See also watershed management areas."@en;
  skos:inScheme :ca-dwr-g;
  skos:topConceptOf :ca-dwr-g;
  skosxl:altLabel :xl_en_3f2b1af7;
  skosxl:prefLabel :xl_en_5dd3e776 .

:xl_en_5dd3e776 a skosxl:Label;
  skosxl:literalForm "Watershed Management Initiative "@en .

:xl_en_3f2b1af7 a skosxl:Label;
  skosxl:literalForm "WMI"@en .

:c_791f1d59 a :Terms, skos:Concept;
  skos:broader :Infrastructure, :Utilities;
  skos:definition "A protected surface and subsurface zone, which surrounds a well or well field that supplies a public water system, intended to keep contaminants from reaching the well water."@en;
  skos:inScheme :ca-dwr-g;
  skos:topConceptOf :ca-dwr-g;
  skosxl:prefLabel :xl_en_b1d9e4b5 .

:xl_en_b1d9e4b5 a skosxl:Label;
  skosxl:literalForm "wellhead protection area "@en .

:c_4ea25fc4 a :Terms, skos:Concept;
  skos:broader :Hydrology;
  skos:definition "The period of time on an annual cycle in which the majority of rainfall occurs. In California, that period is from late October through March."@en;
  skos:inScheme :ca-dwr-g;
  skos:topConceptOf :ca-dwr-g;
  skosxl:prefLabel :xl_en_e4fbaca2 .

:xl_en_e4fbaca2 a skosxl:Label;
  skosxl:literalForm "wet season "@en .

:c_e0549647 a :Terms, skos:Concept;
  skos:broader :Legal_and_Regulatory;
  skos:definition "Formally designated and State-designated river systems under the 1968 National Wild and Scenic Rivers Act and the 1972 California Wild and Scenic Rivers Act. Many rivers and river reaches in California, including many forks and tributaries - more than 2,000 miles of river - are designated wild, scenic, or recreational."@en;
  skos:inScheme :ca-dwr-g;
  skos:topConceptOf :ca-dwr-g;
  skosxl:prefLabel :xl_en_fd45bb28 .

:xl_en_fd45bb28 a skosxl:Label;
  skosxl:literalForm "Wild and Scenic rivers"@en .

:c_2c6b8654 a :Terms, skos:Concept;
  skos:broader :Legal_and_Regulatory, :Water_Use;
  skos:definition "The annual volume of natural flows from the designated State and federal Wild and Scenic Rivers systems."@en;
  skos:inScheme :ca-dwr-g;
  skos:topConceptOf :ca-dwr-g;
  skosxl:prefLabel :xl_en_48f227c6 .

:xl_en_48f227c6 a skosxl:Label;
  skosxl:literalForm "wild and scenic rivers water "@en .

:c_6b743d49 a :Terms, skos:Concept;
  skos:broader :Data_, :Environment_and_Ecology;
  skos:definition "A comparable concept to willingness to pay is called willingness to accept or willingness to receive, which measures how much an individual would accept or receive as payment if he or she could be induced to forego a good or service. See also willingness to pay."@en;
  skos:inScheme :ca-dwr-g;
  skos:topConceptOf :ca-dwr-g;
  skosxl:prefLabel :xl_en_3ef0b3ee .

:xl_en_3ef0b3ee a skosxl:Label;
  skosxl:literalForm "willingness to accept "@en .

:c_3a189415 a :Terms, skos:Concept;
  skos:broader :Data_;
  skos:definition "The economic value of a good or service to a person, measured by the maximum amount (in dollar terms) that he or she is willing to give up in order to acquire that good or service. See also willingness to accept."@en;
  skos:inScheme :ca-dwr-g;
  skos:topConceptOf :ca-dwr-g;
  skosxl:prefLabel :xl_en_f9f6c062 .

:xl_en_f9f6c062 a skosxl:Label;
  skosxl:literalForm "willingness to pay "@en .

:c_43eb1b10 a :Terms, skos:Concept;
  skos:inScheme :ca-dwr-g .

:c_d508285a dct:modified "2019-10-02T15:48:30.220Z"^^xsd:dateTime;
  skos:related :c_57905db2, :c_62cd83cf, :c_b1adfc02, :c_f56468de .

:Data_Sources a :Themes;
  dct:modified "2019-10-02T15:51:23.624Z"^^xsd:dateTime .

:Geospatial a :Themes;
  dct:modified "2019-10-02T15:51:30.451Z"^^xsd:dateTime .

:Units a :Themes;
  dct:modified "2019-10-02T15:51:36.710Z"^^xsd:dateTime .

:Variables a :Themes;
  dct:modified "2019-10-02T15:51:43.121Z"^^xsd:dateTime .

:CA-DWR dct:modified "2019-10-02T15:54:37.568Z"^^xsd:dateTime .

:c_86ddc733 dct:modified "2019-10-02T16:03:17.784Z"^^xsd:dateTime;
  skos:exactMatch :c_32d84bc0 .

:c_4f8328ff dct:modified "2019-10-02T16:06:06.781Z"^^xsd:dateTime;
  skos:exactMatch :c_80dd6550 .

:c_e3620d23 dct:modified "2019-10-02T16:08:06.857Z"^^xsd:dateTime;
  skos:exactMatch :c_a26b32ac .

:c_5cc31c7e dct:modified "2019-10-02T16:38:48.206Z"^^xsd:dateTime .

:usgs-wut dct:modified "2019-10-02T16:52:35.999Z"^^xsd:dateTime .
